@prefix : <http://modai.ai/big5#> .
@prefix ns: <http://modai.ai/big5#> .
@prefix owl: <http://www.w3.org/2002/07/owl#> .
@prefix rdf: <http://www.w3.org/1999/02/22-rdf-syntax-ns#> .
@prefix xml: <http://www.w3.org/XML/1998/namespace> .
@prefix xsd: <http://www.w3.org/2001/XMLSchema#> .
@prefix rdfs: <http://www.w3.org/2000/01/rdf-schema#> .
@base <http://modai.ai/big5#> .

<http://modai.ai/big5> rdf:type owl:Ontology .

#################################################################
#    Annotation properties
#################################################################

###  http://modai.ai/big5#survey
ns:survey rdf:type owl:AnnotationProperty .


###  http://modai.ai/big5#surveyRating1
ns:surveyRating1 rdf:type owl:AnnotationProperty .


###  http://modai.ai/big5#surveyRating2
ns:surveyRating2 rdf:type owl:AnnotationProperty .


###  http://modai.ai/big5#surveyRating3
ns:surveyRating3 rdf:type owl:AnnotationProperty .


###  http://modai.ai/big5#surveyRating4
ns:surveyRating4 rdf:type owl:AnnotationProperty .


###  http://modai.ai/big5#surveyRating5
ns:surveyRating5 rdf:type owl:AnnotationProperty .


###  http://modai.ai/big5#triggers
ns:triggers rdf:type owl:AnnotationProperty ;
            rdfs:range ns:Behavior .


###  http://modai.ai/big5#uses
ns:uses rdf:type owl:AnnotationProperty .


#################################################################
#    Datatypes
#################################################################

###  xsd:string
<xsd:string> rdf:type rdfs:Datatype .


#################################################################
#    Object Properties
#################################################################

###  http://modai.ai/big5#associatedWith
ns:associatedWith rdf:type owl:ObjectProperty ;
                  rdfs:subPropertyOf owl:topObjectProperty ;
                  rdfs:domain ns:Behavior ;
                  rdfs:range ns:Trait .


###  http://modai.ai/big5#hasEmotion
ns:hasEmotion rdf:type owl:ObjectProperty ;
              rdfs:range ns:Emotion .


###  http://modai.ai/big5#hasEmotionStrong
ns:hasEmotionStrong rdf:type owl:ObjectProperty ;
                    rdfs:subPropertyOf ns:hasEmotion .


###  http://modai.ai/big5#oppositeTo
ns:oppositeTo rdf:type owl:ObjectProperty ;
              rdfs:subPropertyOf owl:topObjectProperty ;
              rdf:type owl:SymmetricProperty ;
              rdfs:domain ns:Emotion ;
              rdfs:range ns:Emotion .


###  http://modai.ai/big5#question
ns:question rdf:type owl:ObjectProperty ;
            rdfs:subPropertyOf owl:topObjectProperty .


###  http://modai.ai/big5#relatedTo
ns:relatedTo rdf:type owl:ObjectProperty ,
                      owl:SymmetricProperty ,
                      owl:TransitiveProperty ,
                      owl:IrreflexiveProperty .


###  http://modai.ai/big5#similarTo
ns:similarTo rdf:type owl:ObjectProperty ,
                      owl:SymmetricProperty .


###  http://modai.ai/big5#surveyRating
ns:surveyRating rdf:type owl:ObjectProperty .


###  http://modai.ai/big5#surveyRating1
ns:surveyRating1 rdf:type owl:ObjectProperty ;
                 rdfs:subPropertyOf ns:surveyRating .


###  http://modai.ai/big5#surveyRating2
ns:surveyRating2 rdf:type owl:ObjectProperty ;
                 rdfs:subPropertyOf ns:surveyRating .


###  http://modai.ai/big5#surveyRating3
ns:surveyRating3 rdf:type owl:ObjectProperty ;
                 rdfs:subPropertyOf ns:surveyRating .


###  http://modai.ai/big5#surveyRating4
ns:surveyRating4 rdf:type owl:ObjectProperty ;
                 rdfs:subPropertyOf ns:surveyRating .


###  http://modai.ai/big5#surveyRating5
ns:surveyRating5 rdf:type owl:ObjectProperty ;
                 rdfs:subPropertyOf ns:surveyRating .


###  http://modai.ai/big5#triggeredBy
ns:triggeredBy rdf:type owl:ObjectProperty ;
               rdfs:subPropertyOf owl:topObjectProperty ;
               owl:inverseOf ns:triggers ;
               rdfs:domain ns:Behavior ;
               rdfs:range ns:Emotion .


###  http://modai.ai/big5#triggers
ns:triggers rdf:type owl:ObjectProperty ;
            rdfs:subPropertyOf owl:topObjectProperty ;
            rdfs:domain ns:Emotion .


###  http://modai.ai/big5#uses
ns:uses rdf:type owl:ObjectProperty .


#################################################################
#    Data properties
#################################################################

###  http://modai.ai/big5#sample1
ns:sample1 rdf:type owl:DatatypeProperty .


###  http://modai.ai/big5#sample2
ns:sample2 rdf:type owl:DatatypeProperty .


###  http://modai.ai/big5#sample3
ns:sample3 rdf:type owl:DatatypeProperty .


###  http://modai.ai/big5#sample4
ns:sample4 rdf:type owl:DatatypeProperty .


###  http://modai.ai/big5#sample5
ns:sample5 rdf:type owl:DatatypeProperty .


###  http://modai.ai/big5#trainingPrompt
ns:trainingPrompt rdf:type owl:DatatypeProperty .


#################################################################
#    Classes
#################################################################

###  http://modai.ai/big5#Aesthetic_Sensitivity
ns:Aesthetic_Sensitivity rdf:type owl:Class ;
                         rdfs:subClassOf ns:Facet_Scale ,
                                         ns:Open-Mindedness ;
                         rdfs:comment "Aesthetic Sensitivity, within the Big Five personality framework, encompasses an individual's appreciation and responsiveness towards art, beauty, and the natural world. This trait highlights the depth of one's emotional engagement and valuation of aesthetic experiences, reflecting a sensitivity that can influence personal well-being and creativity."@en ;
                         rdfs:label "Aesthetic Sensitivity"@en ;
                         rdfs:seeAlso "Aesthetic" .


###  http://modai.ai/big5#Agreeableness
ns:Agreeableness rdf:type owl:Class ;
                 rdfs:subClassOf ns:Domain_Scale ;
                 rdfs:comment "Agreeableness, as a domain within the Big Five personality framework, encapsulates an individual's propensity for cooperation, kindness, and social harmony, highlighted through facets such as Compassion, Respectfulness, and Trust. Compassion reflects the depth of an individual's empathy and concern for others, promoting supportive and empathetic interactions. Respectfulness underscores the importance of treating others with consideration and esteem, ensuring positive and harmonious social engagements. Trust indicates a tendency to see the best in others, facilitating open and honest relationships. Together, these facets illustrate an agreeable individual's nurturing, considerate, and trustworthy nature in their dealings with others, fostering strong, positive connections."@en ;
                 rdfs:label "Agreeableness"@en ;
                 rdfs:seeAlso "Agreeable" .


###  http://modai.ai/big5#Anxiety
ns:Anxiety rdf:type owl:Class ;
           rdfs:subClassOf ns:Facet_Scale ,
                           ns:Negative_Emotionality .


###  http://modai.ai/big5#Assertiveness
ns:Assertiveness rdf:type owl:Class ;
                 rdfs:subClassOf ns:Extraversion ,
                                 ns:Facet_Scale .


###  http://modai.ai/big5#Behavior
ns:Behavior rdf:type owl:Class .


###  http://modai.ai/big5#Bot_Action
ns:Bot_Action rdf:type owl:Class .


###  http://modai.ai/big5#Bot_Emoji_Action
ns:Bot_Emoji_Action rdf:type owl:Class ;
                    rdfs:subClassOf ns:Bot_Action .


###  http://modai.ai/big5#Category
ns:Category rdf:type owl:Class .


###  http://modai.ai/big5#Color
ns:Color rdf:type owl:Class .


###  http://modai.ai/big5#Compassion
ns:Compassion rdf:type owl:Class ;
              rdfs:subClassOf ns:Agreeableness ,
                              ns:Facet_Scale ;
              rdfs:comment "Compassion, as a personality trait, embodies an individual's sensitivity to the suffering of others coupled with a desire to alleviate it. It reflects a deep empathy and concern for people, prompting actions that are kind, supportive, and understanding. Individuals high in Compassion are often seen as warm and caring, able to connect with others on an emotional level, and are motivated to contribute positively to the wellbeing of those around them. This trait is crucial for fostering meaningful relationships and building supportive communities, as it encourages a culture of mutual respect and care."@en ;
              rdfs:label "Compassion"@en ;
              rdfs:seeAlso "Compassion" .


###  http://modai.ai/big5#Confusion
ns:Confusion rdf:type owl:Class ;
             rdfs:subClassOf ns:Category .


###  http://modai.ai/big5#Conscientiousness
ns:Conscientiousness rdf:type owl:Class ;
                     rdfs:subClassOf ns:Domain_Scale ;
                     rdfs:comment "Conscientiousness, as a facet of the Big Five personality traits, embodies an individual's dedication to discipline, efficiency, and reliability, underscored by Organization, Productiveness, and Responsibility. Organization reflects the aptitude for keeping environments and tasks orderly, enhancing goal achievement. Productiveness captures the drive to complete tasks efficiently, highlighting a strong work ethic and focus. Responsibility indicates a person's dependability in fulfilling obligations, showcasing a commitment to trustworthiness and duty. These components collectively depict a conscientious individual's methodical, diligent approach to life, ensuring tasks are approached with precision and commitments are met with unwavering dedication."@en ;
                     rdfs:label "Conscientiousness"@en ;
                     rdfs:seeAlso "Conscientious" .


###  http://modai.ai/big5#Creative_Imagination
ns:Creative_Imagination rdf:type owl:Class ;
                        rdfs:subClassOf ns:Facet_Scale ,
                                        ns:Open-Mindedness ;
                        rdfs:comment "Creative Imagination in the Big Five personality framework refers to an individual's capacity to think in innovative, original, and novel ways. This trait is indicative of a person's ability to generate new ideas, solve problems creatively, and embrace unconventional perspectives, contributing to diverse forms of artistic expression and inventive thinking."@en ;
                        rdfs:label "Creative Imagination"@en ;
                        rdfs:seeAlso "Creative" .


###  http://modai.ai/big5#Depression
ns:Depression rdf:type owl:Class ;
              rdfs:subClassOf ns:Facet_Scale ,
                              ns:Negative_Emotionality .


###  http://modai.ai/big5#Domain_Scale
ns:Domain_Scale rdf:type owl:Class .


###  http://modai.ai/big5#Drop_Emoji_Negative
ns:Drop_Emoji_Negative rdf:type owl:Class ;
                       rdfs:subClassOf ns:Bot_Emoji_Action .


###  http://modai.ai/big5#Drop_Emoji_Positive
ns:Drop_Emoji_Positive rdf:type owl:Class ;
                       rdfs:subClassOf ns:Bot_Emoji_Action .


###  http://modai.ai/big5#Emotion
ns:Emotion rdf:type owl:Class ;
           rdfs:isDefinedBy """An \"emotion\" is a complex psychological state that involves a wide range of feelings, thoughts, and physiological changes. Emotions are typically reactive and temporary, often arising in response to an event, situation, or thought. They may fluctuate frequently, and individuals may experience multiple emotions over a short period.

Examples of emotions include happiness, sadness, anger, fear, surprise, and disgust. Emotions can influence a person's actions and decision-making processes but are more temporary and reactive compared to traits.""" ,
                            "In essence, traits represent the underlying framework or tendencies of an individual's personality, while emotions are the moment-to-moment experiences and reactions that are influenced by this framework. A person's trait can influence the intensity, duration, and type of emotion they experience. For instance, an optimistic person (trait) might be more likely to feel happiness (emotion) in response to a positive event. However, the emotion (happiness) is a temporary response, while the trait (optimism) is a more consistent and stable aspect of their personality." .


###  http://modai.ai/big5#EmotionColor
ns:EmotionColor rdf:type owl:Class ;
                rdfs:subClassOf ns:Color .


###  http://modai.ai/big5#Emotional_Volatility
ns:Emotional_Volatility rdf:type owl:Class ;
                        rdfs:subClassOf ns:Facet_Scale ,
                                        ns:Negative_Emotionality ;
                        rdfs:comment "Emotional Volatility, within the Big Five personality framework, refers to the tendency of an individual to experience frequent and intense shifts in emotions. This trait highlights a person's proneness to sudden emotional reactions and mood swings, which can affect their interactions and stability. Emotional Volatility is characterized by rapid changes in feelings, often in response to events that might have minimal impact on someone with a more stable emotional disposition, leading to challenges in predicting one's emotional responses and maintaining consistency in mood."@en ;
                        rdfs:label "Emotional Volatility"@en ;
                        rdfs:seeAlso "Volatile" .


###  http://modai.ai/big5#Energy_Level
ns:Energy_Level rdf:type owl:Class ;
                rdfs:subClassOf ns:Extraversion ,
                                ns:Facet_Scale ;
                rdfs:comment "Energy Level, within the Big Five personality framework, pertains to the dynamism and vitality an individual brings to their activities and interactions. It reflects how much enthusiasm and persistence a person typically exhibits, whether in pursuing goals, engaging in tasks, or interacting with others. High Energy Level is characterized by a consistent display of vigor, an active engagement in life's roles, and a proactive approach to challenges and opportunities. Conversely, a lower Energy Level may manifest as a more reserved or laid-back approach, with individuals possibly showing less initiative or intensity in their actions. This trait underscores the spectrum of how individuals mobilize their physical and mental resources to meet the demands of their environment."@en ;
                rdfs:label "Energy Level"@en ;
                rdfs:seeAlso "Energetic" .


###  http://modai.ai/big5#Extraversion
ns:Extraversion rdf:type owl:Class ;
                rdfs:subClassOf ns:Domain_Scale ;
                rdfs:comment "Extraversion, as defined in the Big Five personality traits, encapsulates an individual's engagement with the external world through facets such as Assertiveness, Energy Level, and Sociability. Assertiveness reflects one's confidence in expressing opinions and leading, while Energy Level indicates the vitality and enthusiasm brought to activities and interactions. Sociability measures the enjoyment and preference for being in social settings, emphasizing the ease with which extraverts form connections and navigate social environments. Together, these facets illustrate the extravert's natural inclination towards active participation, leadership, and a vibrant engagement with the world around them."@en ;
                rdfs:label "Extraversion"@en ;
                rdfs:seeAlso "Extrovert" .


###  http://modai.ai/big5#Facet_Scale
ns:Facet_Scale rdf:type owl:Class .


###  http://modai.ai/big5#High_Intensity
ns:High_Intensity rdf:type owl:Class ;
                  rdfs:subClassOf ns:Intensity .


###  http://modai.ai/big5#Intellectual_Curiosity
ns:Intellectual_Curiosity rdf:type owl:Class ;
                          rdfs:subClassOf ns:Facet_Scale ,
                                          ns:Open-Mindedness ;
                          rdfs:comment "Intellectual Curiosity within the Big Five personality model pertains to an individual's inclination towards learning, exploring, and engaging deeply with ideas and concepts. This trait showcases a person's thirst for knowledge, openness to new experiences, and enjoyment of intellectual challenges, reflecting a proactive pursuit of understanding and discovery."@en ;
                          rdfs:label "Intellectual Curiosity"@en ;
                          rdfs:seeAlso "Curious" .


###  http://modai.ai/big5#Intensity
ns:Intensity rdf:type owl:Class .


###  http://modai.ai/big5#Low_Intensity
ns:Low_Intensity rdf:type owl:Class ;
                 rdfs:subClassOf ns:Intensity .


###  http://modai.ai/big5#Negative_Emotionality
ns:Negative_Emotionality rdf:type owl:Class ;
                         rdfs:subClassOf ns:Domain_Scale ;
                         rdfs:comment "Negative Emotionality is a domain in the Big Five personality traits that focuses on the tendency to experience negative emotions more frequently and intensely. Anxiety within this domain captures a person's propensity to feel nervousness and worry about future events or outcomes, often leading to a heightened state of alertness or unease. Depression contributes to Negative Emotionality by reflecting feelings of sadness, hopelessness, and a lack of interest or pleasure in activities, marking a downturn in mood and general disposition. Emotional Volatility, the third facet, indicates the likelihood of experiencing rapid and intense emotional changes, leading to unpredictability in emotional responses to situations. These facets together depict a personality profile characterized by a susceptibility to various forms of negative emotional experiences, ranging from persistent worry and melancholy to significant fluctuations in mood."@en ;
                         rdfs:label "Negative Emotionality"@en ;
                         rdfs:seeAlso "Negative" .


###  http://modai.ai/big5#Negative_High
ns:Negative_High rdf:type owl:Class ;
                 rdfs:subClassOf ns:Category ,
                                 ns:High_Intensity ,
                                 ns:Negative_Sentiment .


###  http://modai.ai/big5#Negative_Low
ns:Negative_Low rdf:type owl:Class ;
                rdfs:subClassOf ns:Category ,
                                ns:Low_Intensity ,
                                ns:Negative_Sentiment .


###  http://modai.ai/big5#Negative_Sentiment
ns:Negative_Sentiment rdf:type owl:Class ;
                      rdfs:subClassOf ns:Sentiment .


###  http://modai.ai/big5#Open-Mindedness
ns:Open-Mindedness rdf:type owl:Class ;
                   rdfs:subClassOf ns:Domain_Scale ;
                   rdfs:comment "Open-Mindedness, within the context of the Big Five personality traits, embodies a broad receptivity to new and diverse experiences, thoughts, and forms of expression. Intellectual Curiosity highlights this domain by pointing to an individual's relentless pursuit of knowledge, a desire to explore and understand the world in depth. Creative Imagination adds another layer, signifying the capacity for innovative thought and the ability to conceive original ideas, thereby pushing the boundaries of conventional thinking. Aesthetic Sensitivity, the third facet, enriches this domain with a deep appreciation for beauty and art, reflecting a nuanced engagement with the world's aesthetic aspects. Together, these facets underscore a complex interplay of being open to exploring the unknown, appreciating the creative and the beautiful, and seeking a deeper understanding of the myriad experiences life offers."@en ;
                   rdfs:label "Open-Mindedness"@en ;
                   rdfs:seeAlso "Open" .


###  http://modai.ai/big5#Organization
ns:Organization rdf:type owl:Class ;
                rdfs:subClassOf ns:Conscientiousness ,
                                ns:Facet_Scale ;
                rdfs:comment "Organization, within the context of personality traits, refers to an individual's ability to structure, arrange, and manage their environment and tasks effectively. It signifies a preference for orderliness and planning, ensuring that activities are coordinated and goals are systematically pursued. People high in Organization tend to create and maintain clear, tidy environments, prioritize tasks efficiently, and follow schedules closely, which enhances their ability to achieve objectives with consistency and reliability. This trait is crucial for personal productivity, stress management, and the successful accomplishment of both short-term and long-term goals."@en ;
                rdfs:label "Organization"@en ;
                rdfs:seeAlso "Organized" .


###  http://modai.ai/big5#Positive_High
ns:Positive_High rdf:type owl:Class ;
                 rdfs:subClassOf ns:Category ,
                                 ns:High_Intensity ,
                                 ns:Positive_Sentiment .


###  http://modai.ai/big5#Positive_Low
ns:Positive_Low rdf:type owl:Class ;
                rdfs:subClassOf ns:Category ,
                                ns:Low_Intensity ,
                                ns:Positive_Sentiment .


###  http://modai.ai/big5#Positive_Sentiment
ns:Positive_Sentiment rdf:type owl:Class ;
                      rdfs:subClassOf ns:Sentiment .


###  http://modai.ai/big5#Productiveness
ns:Productiveness rdf:type owl:Class ;
                  rdfs:subClassOf ns:Conscientiousness ,
                                  ns:Facet_Scale ;
                  rdfs:comment "Productiveness in the context of personality traits reflects an individual's efficiency and effectiveness in completing tasks and achieving goals. It embodies a strong work ethic and a focused approach to tasks at hand, highlighting a person's ability to stay engaged, maintain high levels of energy, and produce significant outcomes over time. Individuals who score high on Productiveness are often driven, disciplined, and capable of managing their time and resources wisely to maximize output. This trait is critical for success in both personal and professional spheres, as it relates directly to one's capacity to fulfill commitments and contribute value through their efforts."@en ;
                  rdfs:label "Productiveness"@en ;
                  rdfs:seeAlso "Productive" .


###  http://modai.ai/big5#Prompt
ns:Prompt rdf:type owl:Class .


###  http://modai.ai/big5#Respectfulness
ns:Respectfulness rdf:type owl:Class ;
                  rdfs:subClassOf ns:Agreeableness ,
                                  ns:Facet_Scale .


###  http://modai.ai/big5#Response_Length
ns:Response_Length rdf:type owl:Class ;
                   rdfs:subClassOf ns:Bot_Action .


###  http://modai.ai/big5#Responsibility
ns:Responsibility rdf:type owl:Class ;
                  rdfs:subClassOf ns:Conscientiousness ,
                                  ns:Facet_Scale ;
                  rdfs:comment "Responsibility, as a personality trait, indicates an individual's reliability and commitment to fulfilling obligations, promises, and duties. It embodies a sense of duty and a conscientious approach towards tasks, whether in personal or professional settings. People high in Responsibility are trusted to follow through on commitments, make dependable decisions, and are often seen as pillars within their communities or organizations. This trait highlights the importance of accountability and integrity, showing how an individual prioritizes and manages their responsibilities with seriousness and care, ensuring that they meet expectations and contribute positively to their environments."@en ;
                  rdfs:label "Responsibility"@en ;
                  rdfs:seeAlso "Responsible" .


###  http://modai.ai/big5#Sentiment
ns:Sentiment rdf:type owl:Class .


###  http://modai.ai/big5#Sociability
ns:Sociability rdf:type owl:Class ;
               rdfs:subClassOf ns:Extraversion ,
                               ns:Facet_Scale ;
               rdfs:comment "Sociability in the context of the Big Five personality traits refers to an individual's inclination towards seeking and enjoying the company of others. It encompasses a person's preference for engaging in social interactions, forming connections, and participating in group activities. Individuals high in Sociability typically exhibit traits such as outgoingness, friendliness, and warmth, finding pleasure and energy in being around others, as opposed to those with lower levels of Sociability, who may prefer solitude or smaller, more intimate gatherings. This trait highlights the varying degrees to which people are drawn to social environments and their comfort in navigating social contexts."@en ;
               rdfs:label "Sociability"@en ;
               rdfs:seeAlso "Social" .


###  http://modai.ai/big5#Social
ns:Social rdf:type owl:Class ;
          rdfs:subClassOf ns:Category .


###  http://modai.ai/big5#Tonality
ns:Tonality rdf:type owl:Class .


###  http://modai.ai/big5#Trait
ns:Trait rdf:type owl:Class ;
         rdfs:isDefinedBy """A \"trait\" refers to a distinguishing characteristic or quality that defines an individual, often pertaining to personality or behavior. Traits are generally consistent, stable over time, and define a person's long-term behavior or patterns of thought. They are typically seen as inherent or acquired aspects of a person's identity.

Examples of traits include introversion, extraversion, honesty, optimism, pessimism, adaptability, organized, opinionated, etc. These traits help form the basis of a person's personality and can influence how a person might respond to different situations.""" ,
                          "In essence, traits represent the underlying framework or tendencies of an individual's personality, while emotions are the moment-to-moment experiences and reactions that are influenced by this framework. A person's trait can influence the intensity, duration, and type of emotion they experience. For instance, an optimistic person (trait) might be more likely to feel happiness (emotion) in response to a positive event. However, the emotion (happiness) is a temporary response, while the trait (optimism) is a more consistent and stable aspect of their personality." .


###  http://modai.ai/big5#Trust
ns:Trust rdf:type owl:Class ;
         rdfs:subClassOf ns:Agreeableness ,
                         ns:Facet_Scale .


###  http://modai.ai/big5#Verbosity
ns:Verbosity rdf:type owl:Class ;
             rdfs:subClassOf ns:Bot_Action .


#################################################################
#    Individuals
#################################################################

###  http://modai.ai/big5#Abstract
ns:Abstract rdf:type owl:NamedIndividual ;
            rdfs:label "Abstract"@en .


###  http://modai.ai/big5#Acceptance
ns:Acceptance rdf:type owl:NamedIndividual ,
                       ns:Trait ;
              ns:oppositeTo ns:Disregard ;
              rdfs:comment "Acceptance can be considered both an emotion and a trait, depending on how it is defined and understood. As an emotion, acceptance can refer to the feeling of embracing or making peace with a situation or circumstance that cannot be changed. It can involve recognizing and coming to terms with feelings of disappointment, loss, or grief, and finding a way to move forward without dwelling on negative emotions. As a trait, acceptance can refer to a more enduring personality characteristic, describing a person who is open-minded, non-judgmental, and able to handle uncertainty or change with equanimity. People with this trait generally tend to approach new experiences and challenges with a positive attitude and a willingness to learn from them. Overall, acceptance can be both an emotional state and a stable personality trait, and understanding how it operates in both contexts can be helpful in developing strategies for coping with difficult or challenging situations." ;
              rdfs:label "Acceptance"@en .


###  http://modai.ai/big5#Acceptance-Disregard
ns:Acceptance-Disregard rdf:type owl:NamedIndividual ,
                                 ns:Prompt ;
                        ns:uses ns:Acceptance ,
                                ns:Disregard ;
                        rdfs:comment """I want to quantify the level of acceptance or disregard in the following text: 
```
$INPUT_TEXT
```

I define acceptance as the act of embracing or welcoming something or someone, acknowledging and embracing their value or presence. I define disregard as the act of ignoring, neglecting, or paying no attention to something or someone.

Please answer on a scale of 1 - 5 where the numbers have the following meanings:
```
1 = The text is filled with disregard, paying no attention, and has no elements of acceptance.
2 = The text has elements of disregard or paying no attention, but also contains some elements of acceptance.
3 = The text has neither acceptance nor disregard, it is neutral.
4 = The text has elements of acceptance but also has some aspects of disregard or paying no attention.
5 = The text is deeply filled with acceptance, focusing heavily on embracing and acknowledging the value or presence of something or someone.
```

Only respond with a number and no other rating.
"""@en ;
                        rdfs:label "Acceptance-Disregard"@en .


###  http://modai.ai/big5#Accepting
ns:Accepting rdf:type owl:NamedIndividual ;
             rdfs:label "Accepting"@en .


###  http://modai.ai/big5#Accountability
ns:Accountability rdf:type owl:NamedIndividual ;
                  rdfs:label "Accountability"@en .


###  http://modai.ai/big5#Accountable
ns:Accountable rdf:type owl:NamedIndividual ;
               rdfs:label "Accountable"@en .


###  http://modai.ai/big5#Active
ns:Active rdf:type owl:NamedIndividual ;
          rdfs:label "Active"@en .


###  http://modai.ai/big5#Adaptable
ns:Adaptable rdf:type owl:NamedIndividual ,
                      ns:Trait ;
             rdfs:comment "Adaptable is generally considered a trait rather than an emotion. Traits are enduring characteristics or qualities that describe an individual's behavior, personality, or attitudes, while emotions refer to subjective feelings that arise in response to specific situations or stimuli. Adaptable refers to an individual's ability to adjust to new or changing situations. It involves being flexible, resourceful, and open-minded. While emotions can influence how well individuals adapt to certain situations, adaptability is not a direct expression of emotions. Adaptable individuals may experience a wide range of emotions in response to changes, but their ability to cope and adjust is determined by their underlying trait of adaptability." ;
             rdfs:label "Adaptable"@en .


###  http://modai.ai/big5#Admiration
ns:Admiration rdf:type owl:NamedIndividual ,
                       ns:Emotion ,
                       ns:Positive_High ;
              ns:oppositeTo ns:Disregard ;
              rdfs:comment "Admiration can be considered both an emotion and a trait, depending on the context in which it is used. As an emotion, admiration is a feeling of respect, appreciation, or approval towards someone or something. It is often accompanied by a sense of awe, wonder, or inspiration. For example, when you see someone perform an act of kindness or bravery, you might feel admiration for them. As a trait, admiration refers to a person's tendency to feel and express admiration towards others. People who are said to have a \"trusting and admiring\" personality trait are more likely to admire and respect their peers, colleagues, and superiors. This trait is often associated with positive qualities such as generosity, humility, and gratitude. Therefore, admiration can be both an emotion and a trait, depending on the context and the way it is expressed." ;
              rdfs:label "Admiration"@en .


###  http://modai.ai/big5#Admiration-Disregard
ns:Admiration-Disregard rdf:type owl:NamedIndividual ,
                                 ns:Prompt ;
                        ns:uses ns:Admiration ,
                                ns:Disregard ;
                        rdfs:comment """I want to quantify the admiration in the following text:
```
$INPUT_TEXT
```

I define admiration as a feeling of respect, approval, or deep appreciation for someone or something. I define the opposite of admiration as indifference or disregard.

Please answer on a scale of 1 - 5 where the numbers have the following meanings:
```
1 = The text is filled with indifference, disregard, and has no elements of admiration.
2 = The text has elements of indifference or disregard, but also contains some elements of admiration.
3 = The text has neither admiration nor indifference, it is neutral.
4 = The text has elements of admiration but also has some aspects of indifference or disregard.
5 = The text is deeply filled with admiration, focusing heavily on feelings of respect, approval, or deep appreciation for someone or something.
```

Only respond with a number and no other rating.
"""@en ;
                        rdfs:label "Admiration-Disregard"@en .


###  http://modai.ai/big5#Adventurous
ns:Adventurous rdf:type owl:NamedIndividual ;
               rdfs:label "Adventurous"@en .


###  http://modai.ai/big5#Adventurousness
ns:Adventurousness rdf:type owl:NamedIndividual ;
                   rdfs:label "Adventurousness"@en .


###  http://modai.ai/big5#Affection
ns:Affection rdf:type owl:NamedIndividual ,
                      ns:Emotion ;
             ns:relatedTo ns:Love ;
             ns:similarTo ns:Love ;
             rdfs:comment "Affection is generally considered to be an emotion. It is a feeling of warmth and fondness towards someone or something. As an emotion, it is typically characterized by certain physiological and psychological changes, such as increased heart rate, positive mood, and a desire to be close to the person or thing that is the object of affection. However, some people may also view affection as a trait, particularly when it comes to describing someone's personality. In this sense, affection may be seen as a stable quality or disposition that makes someone more likely to experience and express warmth and fondness towards others. For example, someone who is described as \"affectionate\" might be seen as someone who is naturally warm and loving towards their friends and family members. In summary, while affection is primarily considered to be an emotion, it can also be viewed as a personal trait that influences how someone interacts with others." ;
             rdfs:label "Affection"@en .


###  http://modai.ai/big5#Afraid
ns:Afraid rdf:type owl:NamedIndividual ,
                   ns:Emotion ;
          ns:relatedTo ns:Fear ;
          ns:similarTo ns:Fear ;
          rdfs:comment "Afraid can be considered both an emotion and a trait. As an emotion, it is a response to a perceived threat or danger. It is a feeling of discomfort, nervousness, or anxiety that arises when we sense a potential danger or harm. This emotion can be temporary and may fade away once the threat is gone. As a trait, being afraid can also refer to a personality or behavioral characteristic. Some people may be more prone to feeling afraid or anxious in various situations, and this can be a consistent part of their personality or underlying temperament. In summary, while afraid is primarily considered an emotion, it can also be a trait when it becomes a consistent part of a person's personality and behavior." ;
          rdfs:label "Afraid"@en .


###  http://modai.ai/big5#Aggression
ns:Aggression rdf:type owl:NamedIndividual ;
              rdfs:label "Aggression"@en .


###  http://modai.ai/big5#Aggressiveness
ns:Aggressiveness rdf:type owl:NamedIndividual ;
                  rdfs:label "Aggressiveness"@en .


###  http://modai.ai/big5#Agreement
ns:Agreement rdf:type owl:NamedIndividual ;
             rdfs:label "Agreement"@en .


###  http://modai.ai/big5#Allergies
ns:Allergies rdf:type owl:NamedIndividual ;
             rdfs:label "Allergies"@en .


###  http://modai.ai/big5#Aloofness
ns:Aloofness rdf:type owl:NamedIndividual ;
             rdfs:label "Aloofness"@en .


###  http://modai.ai/big5#Amusement
ns:Amusement rdf:type owl:NamedIndividual ;
             rdfs:label "Amusement"@en .


###  http://modai.ai/big5#Analytical
ns:Analytical rdf:type owl:NamedIndividual ;
              rdfs:label "Analytical"@en .


###  http://modai.ai/big5#Anger
ns:Anger rdf:type owl:NamedIndividual ,
                  ns:Emotion ,
                  ns:Negative_High ;
         ns:oppositeTo ns:Calmness ;
         rdfs:comment "Anger can be considered both an emotion and a trait. As an emotion, anger is a temporary state of mind that arises due to various factors, such as frustration, annoyance, or hurt. As a trait, anger refers to a person's habitual tendency to experience anger in response to situations that might not necessarily evoke such a reaction in others. For example, if someone experiences anger in response to a particular situation or event, then that emotion is temporary and can be resolved with time. However, if someone's personality is characterized by frequent and intense displays of anger, then that could be considered a trait. Such individuals may have short tempers and react explosively to trivial things, which can cause issues in their personal and professional relationships. In summary, anger can be both an emotion and a trait depending on the intensity, frequency, and duration of its expression in an individual." ;
         rdfs:label "Anger"@en .


###  http://modai.ai/big5#Anger-Calmness
ns:Anger-Calmness rdf:type owl:NamedIndividual ,
                           ns:Prompt ;
                  ns:uses ns:Anger ,
                          ns:Calmness ;
                  rdfs:comment """I want to quantify the anger in the following text:
```
$INPUT_TEXT
```

I define anger as intense and heated feelings. I define the opposite of anger as calmness or serenity.

Please answer on a scale of 1 - 5 where the numbers have the following meanings:
```
1 = The text has intense feelings but absolutely no negative sentiment.
2 = The text has strong feelings but very little negative sentiment.
3 = The text has no anger, no intensity, and no heated feelings.
4 = The text is angry with negative sentiment.
5 = The text has intensely angry feelings with strong negative sentiment.
```

Only respond with a number and no other rating.
"""@en ;
                  rdfs:label "Anger-Calmness"@en .


###  http://modai.ai/big5#Anticipation
ns:Anticipation rdf:type owl:NamedIndividual ,
                         ns:Emotion ,
                         ns:Positive_High ;
                ns:oppositeTo ns:Nostalgia ;
                rdfs:comment "Anticipation can be considered both an emotion and a trait, depending on how it is defined and studied. As an emotion, anticipation is a feeling of excitement or nervousness that arises when you are looking forward to something. It often involves imagining or anticipating future events, and it is a common emotion in situations such as waiting for test results, traveling to see loved ones, or starting a new job. In this sense, anticipation is a temporary state of mind that can fluctuate based on the situation. On the other hand, anticipation can also be considered a personality trait, reflecting a person's tendency to actively seek out new experiences and anticipate positive outcomes. In this sense, anticipation is a more stable characteristic that is thought to be linked with other personality traits such as openness to experience and extraversion. People who score high on measures of anticipation tend to be curious, optimistic, and enjoy taking risks. Overall, whether we consider anticipation as an emotion or a trait depends on how we define and measure it in different contexts." ;
                rdfs:label "Anticipation"@en .


###  http://modai.ai/big5#Anxiety
ns:Anxiety rdf:type owl:NamedIndividual ,
                    ns:Emotion ,
                    ns:Negative_High ;
           ns:relatedTo ns:Fear ;
           ns:similarTo ns:Fear .


###  http://modai.ai/big5#Anxiety-Serenity
ns:Anxiety-Serenity rdf:type owl:NamedIndividual ,
                             ns:Prompt ;
                    ns:uses ns:Anxiety ,
                            ns:Serenity ;
                    rdfs:comment """I want to quantify the anxiety in the following text:
```
$INPUT_TEXT
```

I define anxiety as a feeling of worry, nervousness, or unease about something with an uncertain outcome. I define the opposite of anxiety as calmness or serenity.

Please answer on a scale of 1 - 5 where the numbers have the following meanings:
```
1 = The text is filled with calmness, serenity, and has no elements of anxiety.
2 = The text has elements of calmness or serenity, but also contains some elements of anxiety.
3 = The text has neither anxiety nor calmness, it is neutral.
4 = The text has elements of anxiety but also has some aspects of calmness or serenity.
5 = The text is deeply filled with anxiety, focusing heavily on feelings of worry, nervousness, or unease.
```

Only respond with a number and no other rating.
"""@en ;
                    rdfs:label "Anxiety-Serenity"@en .


###  http://modai.ai/big5#Anxious
ns:Anxious rdf:type owl:NamedIndividual ;
           rdfs:label "Anxious"@en .


###  http://modai.ai/big5#Apathetic
ns:Apathetic rdf:type owl:NamedIndividual ;
             rdfs:label "Apathetic"@en .


###  http://modai.ai/big5#Apathy
ns:Apathy rdf:type owl:NamedIndividual ,
                   ns:Emotion ;
          ns:oppositeTo ns:Excitement ;
          rdfs:comment "Apathy is generally considered to be a trait rather than an emotion. A trait is a relatively stable characteristic that shapes our attitudes, behavior and responses to situations over time. Apathy is a lack of interest, enthusiasm, or emotional responsiveness to stimuli, which can be pervasive and enduring. This suggests that apathy is more likely to be a trait that individuals possess rather than a situational emotion that changes rapidly. However, some may argue that apathy can be an emotion that is triggered by certain situations or events that cause a lack of interest or motivation. Overall, it is generally categorized as a trait due to its long-lasting and consistent nature." ;
          rdfs:label "Apathy"@en .


###  http://modai.ai/big5#Apologizing
ns:Apologizing rdf:type owl:NamedIndividual ,
                        ns:Behavior ;
               ns:associatedWith ns:Accountability ,
                                 ns:Empathy ,
                                 ns:Humility ,
                                 ns:Respectfulness ;
               ns:triggeredBy ns:Embarrassment ,
                              ns:Guilt ,
                              ns:Remorse ;
               rdfs:label "Apologizing"@en .


###  http://modai.ai/big5#Appreciation
ns:Appreciation rdf:type owl:NamedIndividual ;
                rdfs:label "Appreciation"@en .


###  http://modai.ai/big5#Appreciative
ns:Appreciative rdf:type owl:NamedIndividual ,
                         ns:Trait ;
                ns:relatedTo ns:Admiration ,
                             ns:Thankful ;
                ns:similarTo ns:Admiration ,
                             ns:Thankful ;
                rdfs:comment "Appreciative can be considered both an emotion and a trait, depending on the context and usage. As an emotion, appreciative describes the feeling of gratitude, thankfulness, or admiration towards someone or something. It is a temporary and fleeting state that can arise in response to a positive experience or a favorable outcome. For example, you might feel appreciative towards a friend who helped you in times of need or towards an employer who valued your contributions. As a trait, appreciative refers to a habitual tendency or characteristic of a person to express gratitude or recognize the value of people and things around them. It is a more enduring quality that involves a positive mental attitude and a sense of mindfulness. For example, a person who is appreciative as a trait might consistently express gratitude towards their loved ones, co-workers, or even the simple pleasures of life. Therefore, appreciative can be both an emotion and a trait." ;
                rdfs:label "Appreciative"@en .


###  http://modai.ai/big5#Apprehension
ns:Apprehension rdf:type owl:NamedIndividual ,
                         ns:Confusion ,
                         ns:Emotion ;
                ns:oppositeTo ns:Confidence ,
                              ns:Reassurance ;
                ns:relatedTo ns:Anxiety ,
                             ns:Unease ;
                ns:similarTo ns:Anxiety ,
                             ns:Unease ;
                rdfs:comment "Apprehension can be considered both an emotion and a trait depending on the context and how it is being used. As an emotion, apprehension is a feeling of anxiety or fear about a future event or situation. It is a reaction to a specific stimuli, and it is typically short-lived. For example, feeling apprehensive before a job interview or a public speaking engagement is a typical emotional response to a stressful situation. As a trait, apprehension refers to a person's tendency to feel anxious or tense in different situations. It is a disposition or a personality characteristic, which means that it is relatively stable and consistent over time. For example, some individuals might be more apprehensive in social situations or when facing uncertainty than others, and this tendency could be due to their natural disposition. In summary, apprehension can be both an emotional response and a personality trait. As an emotion, it is a short-lived feeling of anxiety or fear, while as a trait, it represents a stable tendency to feel anxious or tense." ;
                rdfs:label "Apprehension"@en .


###  http://modai.ai/big5#Apprehension-Confidence
ns:Apprehension-Confidence rdf:type owl:NamedIndividual ,
                                    ns:Prompt ;
                           ns:uses ns:Apprehension ,
                                   ns:Confidence ;
                           rdfs:comment """I want to quantify the apprehension in the following text:
```
$INPUT_TEXT
```

I define apprehension as a feeling of anxiety or unease about something that may happen in the future. I define the opposite of apprehension as confidence or reassurance.

Please answer on a scale of 1 - 5 where the numbers have the following meanings:
```
1 = The text is filled with confidence, reassurance, and has no elements of apprehension.
2 = The text has elements of confidence or reassurance, but also contains some elements of apprehension.
3 = The text has neither apprehension nor confidence, it is neutral.
4 = The text has elements of apprehension but also has some aspects of confidence or reassurance.
5 = The text is deeply filled with apprehension, focusing heavily on feelings of anxiety or unease about something that may happen in the future.
```

Only respond with a number and no other rating.
"""@en ;
                           rdfs:label "Apprehension-Confidence"@en .


###  http://modai.ai/big5#Approval
ns:Approval rdf:type owl:NamedIndividual ,
                     ns:Emotion ;
            ns:relatedTo ns:Admiration ;
            ns:similarTo ns:Admiration ;
            rdfs:comment "Approval can be considered both an emotion and a trait. As an emotion, approval refers to a feeling of acceptance, satisfaction, or admiration toward someone or something. It is a positive emotional response that an individual experiences in response to receiving recognition, praise, or validation. As a trait, approval refers to a recurring pattern of behavior or disposition that characterizes an individual. People who have an approval-oriented personality trait are typically more inclined to seek the approval, acceptance, and positive feedback of others. They care about what others think of them and may have a strong desire to be liked and accepted. Therefore, approval can be seen as both an emotion and a trait, depending on how it is expressed and experienced by an individual." ;
            rdfs:label "Approval"@en .


###  http://modai.ai/big5#Arguing
ns:Arguing rdf:type owl:NamedIndividual ,
                    ns:Behavior ;
           ns:associatedWith ns:Assertiveness ,
                             ns:Defensiveness ;
           ns:triggeredBy ns:Anger ,
                          ns:Frustration ;
           rdfs:label "Arguing"@en .


###  http://modai.ai/big5#Argumentative
ns:Argumentative rdf:type owl:NamedIndividual ;
                 rdfs:label "Argumentative"@en .


###  http://modai.ai/big5#Artistic
ns:Artistic rdf:type owl:NamedIndividual ;
            rdfs:label "Artistic"@en .


###  http://modai.ai/big5#Assertive
ns:Assertive rdf:type owl:NamedIndividual ;
             rdfs:label "Assertive"@en .


###  http://modai.ai/big5#Assertiveness
ns:Assertiveness rdf:type owl:NamedIndividual .


###  http://modai.ai/big5#Astonishment
ns:Astonishment rdf:type owl:NamedIndividual ,
                         ns:Emotion ;
                ns:relatedTo ns:Surprise ,
                             ns:Uncertainty ;
                ns:similarTo ns:Surprise ,
                             ns:Uncertainty ;
                rdfs:comment "Astonishment can be considered both an emotion and a trait, depending on the context. As an emotion, astonishment is a sudden feeling of wonder or surprise that arises from an unexpected event or experience. It is a transient state that can be felt and expressed as a reaction to something surprising or novel. For example, if someone were to receive unexpected news, they might feel astonished for a brief period. As a trait, astonishment may reflect a person's tendency to react with surprise or amazement more frequently than others. It may be a part of their personality or temperament, and they may be more prone to experiencing astonishment in response to a broader range of stimuli than someone who is not as easily surprised. In this sense, astonishment can be considered a part of one's character or disposition." ;
                rdfs:label "Astonishment"@en .


###  http://modai.ai/big5#Attentiveness
ns:Attentiveness rdf:type owl:NamedIndividual ,
                          ns:Trait ;
                 ns:relatedTo ns:Interest ;
                 ns:similarTo ns:Interest ;
                 rdfs:comment "Attentiveness can be considered both a trait and a state. As a trait, attentiveness refers to a person's tendency to be aware, alert, and focused on what is happening around them. It is a characteristic that is relatively stable across situations and time, and can be seen as part of a person's personality. As a state, attentiveness refers to the experience of being fully present and engaged in a particular situation or task. It is often influenced by external factors such as the environment, the task at hand, and the individual's level of interest or motivation. In summary, attentiveness can be seen as both a stable trait and a dynamic state, depending on the context in which it is considered." ;
                 rdfs:label "Attentiveness"@en .


###  http://modai.ai/big5#Attraction
ns:Attraction rdf:type owl:NamedIndividual ,
                       ns:Emotion ,
                       ns:Positive_High ;
              ns:relatedTo ns:Interest ;
              ns:similarTo ns:Interest ;
              rdfs:comment "Attraction can be considered both an emotion and a trait, depending on the context in which it is being discussed. When attraction is referred to as an emotion, it typically refers to the feeling of being drawn or pulled towards someone or something. This emotional response can be triggered by physical appearance, personality, or a variety of other factors. In this sense, attraction is a temporary feeling that can come and go, and it can vary in intensity. However, when attraction is referred to as a trait, it generally refers to a more enduring characteristic of an individual. For example, someone might be described as having an \"attractive personality\" or being \"naturally attractive\" due to their charisma, confidence, or other personality traits. In this sense, attraction is seen as a stable and consistent aspect of a person's identity. Overall, attraction can be understood as both a transient emotion and a stable trait, depending on the context and the way in which it is being discussed." ;
              rdfs:label "Attraction"@en .


###  http://modai.ai/big5#Avoidance
ns:Avoidance rdf:type owl:NamedIndividual ;
             rdfs:label "Avoidance"@en .


###  http://modai.ai/big5#Avoidant
ns:Avoidant rdf:type owl:NamedIndividual ;
            rdfs:label "Avoidant"@en .


###  http://modai.ai/big5#Awe
ns:Awe rdf:type owl:NamedIndividual ,
                ns:Emotion ;
       ns:relatedTo ns:Admiration ;
       ns:similarTo ns:Admiration ;
       rdfs:comment "Awe can be considered both an emotion and a trait. As an emotion, awe is a feeling of wonder, amazement, and reverence that can be experienced in response to something vast, majestic, or profound, such as a beautiful natural landscape or a momentous achievement. As a trait, awe refers to an individual's tendency to experience this emotion in response to certain stimuli. Some psychologists have argued that awe should be considered a distinct emotion because it has unique subjective and physiological features, such as increased heart rate, decreased attention to the self, and a sense of being in the presence of something greater than oneself. Other researchers have suggested that awe is a trait that varies across individuals based on their personalities, values, and life experiences. Ultimately, whether awe is considered an emotion or a trait may depend on the theoretical framework being used and the specific research question being addressed. In some cases, it may be helpful to consider awe as both an emotion and a trait, as each perspective can provide valuable insights into its nature, causes, and effects." ;
       rdfs:label "Awe"@en .


###  http://modai.ai/big5#Awe-Indifference
ns:Awe-Indifference rdf:type owl:NamedIndividual ,
                             ns:Prompt ;
                    ns:uses ns:Awe ,
                            ns:Indifference ;
                    rdfs:comment """I want to quantify the awe in the following text:
```
$INPUT_TEXT
```

I define awe as an overwhelming feeling of reverence, admiration, fear, or wonder produced by that which is grand, sublime, or extremely powerful. I define the opposite of awe as indifference or lack of interest.

Please answer on a scale of 1 - 5 where the numbers have the following meanings:
```
1 = The text is filled with indifference, lack of interest, and has no elements of awe.
2 = The text has elements of indifference or lack of interest, but also contains some elements of awe.
3 = The text has neither awe nor indifference, it is neutral.
4 = The text has elements of awe but also has some aspects of indifference or lack of interest.
5 = The text is deeply filled with awe, focusing heavily on feelings of reverence, admiration, fear, or wonder.
```

Only respond with a number and no other rating.
"""@en ;
                    rdfs:label "Awe-Indifference"@en .


###  http://modai.ai/big5#BFI_NO_01
ns:BFI_NO_01 rdf:type owl:NamedIndividual ,
                      ns:Sociability ;
             ns:surveyRating1 ns:BFI_NO_01_01 ;
             ns:surveyRating2 ns:BFI_NO_01_02 ;
             ns:surveyRating3 ns:BFI_NO_01_03 ;
             ns:surveyRating4 ns:BFI_NO_01_04 ;
             ns:surveyRating5 ns:BFI_NO_01_05 ;
             rdfs:comment """I want to rate the personality characteristics in the following input text:
```
$INPUT_TEXT
```

Analyze the input text and tell me if the speaker is outgoing and sociable.

Please answer on a scale of 1 - 5 where the numbers have the following meanings:
```
1 = I am very introverted and rarely seek social interactions.
2 = I tend to be more introverted and sometimes avoid social situations.
3 = I can be both introverted and extroverted, depending on the situation.
4 = I am generally outgoing and enjoy socializing with others.
5 = I am highly extroverted and thrive in social situations.
```

Only respond with a number, and no other text.""" .


###  http://modai.ai/big5#BFI_NO_01_01
ns:BFI_NO_01_01 rdf:type owl:NamedIndividual ;
                ns:hasEmotionStrong ns:Introverted ;
                ns:uses ns:BFI_NO_01_01_COLOR ;
                ns:survey "I am very introverted and rarely seek social interactions."^^<xsd:string> .


###  http://modai.ai/big5#BFI_NO_01_01_COLOR
ns:BFI_NO_01_01_COLOR rdf:type owl:NamedIndividual ,
                               ns:EmotionColor ;
                      ns:uses ns:HEX_556B2F ;
                      rdfs:comment "Dark olive green, for being very introverted"@en .


###  http://modai.ai/big5#BFI_NO_01_02
ns:BFI_NO_01_02 rdf:type owl:NamedIndividual ;
                ns:hasEmotion ns:Introverted ;
                ns:uses ns:BFI_NO_01_02_COLOR ;
                ns:survey "I tend to be more introverted and sometimes avoid social situations."^^<xsd:string> .


###  http://modai.ai/big5#BFI_NO_01_02_COLOR
ns:BFI_NO_01_02_COLOR rdf:type owl:NamedIndividual ,
                               ns:EmotionColor ;
                      ns:uses ns:HEX_6B8E23 ;
                      rdfs:comment "Olive drab, for being more introverted and avoiding social situations"@en .


###  http://modai.ai/big5#BFI_NO_01_03
ns:BFI_NO_01_03 rdf:type owl:NamedIndividual ;
                ns:uses ns:BFI_NO_01_03_COLOR ;
                ns:survey "I can be both introverted and extroverted, depending on the situation."^^<xsd:string> .


###  http://modai.ai/big5#BFI_NO_01_03_COLOR
ns:BFI_NO_01_03_COLOR rdf:type owl:NamedIndividual ,
                               ns:EmotionColor ;
                      ns:uses ns:HEX_9ACD32 ;
                      rdfs:comment "Yellow green, for being both introverted and extroverted"@en .


###  http://modai.ai/big5#BFI_NO_01_04
ns:BFI_NO_01_04 rdf:type owl:NamedIndividual ;
                ns:hasEmotion ns:Extroverted ;
                ns:uses ns:BFI_NO_01_04_COLOR ;
                ns:survey "I am generally outgoing and enjoy socializing with others."^^<xsd:string> .


###  http://modai.ai/big5#BFI_NO_01_04_COLOR
ns:BFI_NO_01_04_COLOR rdf:type owl:NamedIndividual ,
                               ns:EmotionColor ;
                      ns:uses ns:HEX_ADFF2F ;
                      rdfs:comment "Green yellow, for being outgoing and enjoying socializing"@en .


###  http://modai.ai/big5#BFI_NO_01_05
ns:BFI_NO_01_05 rdf:type owl:NamedIndividual ;
                ns:hasEmotionStrong ns:Extroverted ;
                ns:uses ns:BFI_NO_01_05_COLOR ;
                ns:survey "I am highly extroverted and thrive in social situations."^^<xsd:string> .


###  http://modai.ai/big5#BFI_NO_01_05_COLOR
ns:BFI_NO_01_05_COLOR rdf:type owl:NamedIndividual ,
                               ns:EmotionColor ;
                      ns:uses ns:HEX_7CFC00 ;
                      rdfs:comment "Lawn green, for being highly extroverted and thriving socially"@en .


###  http://modai.ai/big5#BFI_NO_02
ns:BFI_NO_02 rdf:type owl:NamedIndividual ,
                      ns:Compassion ;
             ns:surveyRating1 ns:BFI_NO_02_01 ;
             ns:surveyRating2 ns:BFI_NO_02_02 ;
             ns:surveyRating3 ns:BFI_NO_02_03 ;
             ns:surveyRating4 ns:BFI_NO_02_04 ;
             ns:surveyRating5 ns:BFI_NO_02_05 ;
             rdfs:comment """I want to rate the personality characteristics in the following input text:
```
$INPUT_TEXT
```

Analyze the input text and tell me if the speaker is compassionate and has a soft heart.

Please answer on a scale of 1 - 5 where the numbers have the following meanings:
```
1 = I am not a very compassionate person and do not often consider others' feelings.
2 = I can be caring, but I don't always go out of my way to help others.
3 = I care about others, but I don't think I am especially empathetic.
4 = I am a compassionate person and try to help others when I can.
5 = I have a very soft heart and feel deeply for others' pain and suffering.
```

Only respond with a number, and no other text.""" .


###  http://modai.ai/big5#BFI_NO_02_01
ns:BFI_NO_02_01 rdf:type owl:NamedIndividual ;
                ns:hasEmotionStrong ns:Uncompassionate ;
                ns:uses ns:BFI_NO_02_01_COLOR ;
                ns:survey "I am not a very compassionate person and do not often consider others' feelings."^^<xsd:string> .


###  http://modai.ai/big5#BFI_NO_02_01_COLOR
ns:BFI_NO_02_01_COLOR rdf:type owl:NamedIndividual ,
                               ns:EmotionColor ;
                      ns:uses ns:HEX_778899 ;
                      rdfs:comment "Light Slate Gray, for not compassionate"@en .


###  http://modai.ai/big5#BFI_NO_02_02
ns:BFI_NO_02_02 rdf:type owl:NamedIndividual ;
                ns:hasEmotion ns:Uncompassionate ;
                ns:uses ns:BFI_NO_02_02_COLOR ;
                ns:survey "I can be caring, but I don't always go out of my way to help others."^^<xsd:string> .


###  http://modai.ai/big5#BFI_NO_02_02_COLOR
ns:BFI_NO_02_02_COLOR rdf:type owl:NamedIndividual ,
                               ns:EmotionColor ;
                      ns:uses ns:HEX_B0C4DE ;
                      rdfs:comment "Light Steel Blue, for occasionally caring"@en .


###  http://modai.ai/big5#BFI_NO_02_03
ns:BFI_NO_02_03 rdf:type owl:NamedIndividual ;
                ns:uses ns:BFI_NO_02_03_COLOR ;
                ns:survey "I care about others, but I don't think I am especially empathetic."^^<xsd:string> .


###  http://modai.ai/big5#BFI_NO_02_03_COLOR
ns:BFI_NO_02_03_COLOR rdf:type owl:NamedIndividual ,
                               ns:EmotionColor ;
                      ns:uses ns:HEX_ADD8E6 ;
                      rdfs:comment "Light Blue, for caring but not empathetic"@en .


###  http://modai.ai/big5#BFI_NO_02_04
ns:BFI_NO_02_04 rdf:type owl:NamedIndividual ;
                ns:hasEmotion ns:Compassionate ;
                ns:uses ns:BFI_NO_02_04_COLOR ;
                ns:survey "I am a compassionate person and try to help others when I can."^^<xsd:string> .


###  http://modai.ai/big5#BFI_NO_02_04_COLOR
ns:BFI_NO_02_04_COLOR rdf:type owl:NamedIndividual ,
                               ns:EmotionColor ;
                      ns:uses ns:HEX_87CEFA ;
                      rdfs:comment "Light Sky Blue, for compassionate"@en .


###  http://modai.ai/big5#BFI_NO_02_05
ns:BFI_NO_02_05 rdf:type owl:NamedIndividual ;
                ns:hasEmotionStrong ns:Compassionate ;
                ns:uses ns:BFI_NO_02_05_COLOR ;
                ns:survey "I have a very soft heart and feel deeply for others' pain and suffering."^^<xsd:string> .


###  http://modai.ai/big5#BFI_NO_02_05_COLOR
ns:BFI_NO_02_05_COLOR rdf:type owl:NamedIndividual ,
                               ns:EmotionColor ;
                      ns:uses ns:HEX_00BFFF ;
                      rdfs:comment "Deep Sky Blue, for very compassionate"@en .


###  http://modai.ai/big5#BFI_NO_03
ns:BFI_NO_03 rdf:type owl:NamedIndividual ,
                      ns:Organization ;
             ns:surveyRating1 ns:BFI_NO_03_01 ;
             ns:surveyRating2 ns:BFI_NO_03_02 ;
             ns:surveyRating3 ns:BFI_NO_03_03 ;
             ns:surveyRating4 ns:BFI_NO_03_04 ;
             ns:surveyRating5 ns:BFI_NO_03_05 ;
             rdfs:comment """I want to rate the personality characteristics in the following input text:
```
$INPUT_TEXT
```

Analyze the input text and tell me if the speaker tends to be organized.

Please answer on a scale of 1 - 5 where the numbers have the following meanings:
```
1 = I answer questions with disorganized and scattered responses.
2 = I sometimes provide disorganized answers to questions.
3 = I maintain a balance between organized and disorganized responses.
4 = I can be organized but occasionally struggle with order in my answers.
5 = I always answer questions with organized and structured responses.
```

Only respond with a number, and no other text.""" .


###  http://modai.ai/big5#BFI_NO_03_01
ns:BFI_NO_03_01 rdf:type owl:NamedIndividual ;
                ns:hasEmotionStrong ns:Disorganized ;
                ns:uses ns:BFI_NO_03_01_COLOR ;
                ns:survey "I answer questions with disorganized and scattered responses."^^<xsd:string> .


###  http://modai.ai/big5#BFI_NO_03_01_COLOR
ns:BFI_NO_03_01_COLOR rdf:type owl:NamedIndividual ,
                               ns:EmotionColor ;
                      ns:uses ns:HEX_696969 ;
                      rdfs:comment "Dim Gray, for disorganized and scattered responses"@en .


###  http://modai.ai/big5#BFI_NO_03_02
ns:BFI_NO_03_02 rdf:type owl:NamedIndividual ;
                ns:hasEmotion ns:Disorganized ;
                ns:uses ns:BFI_NO_03_02_COLOR ;
                ns:survey "I sometimes provide disorganized answers to questions."^^<xsd:string> .


###  http://modai.ai/big5#BFI_NO_03_02_COLOR
ns:BFI_NO_03_02_COLOR rdf:type owl:NamedIndividual ,
                               ns:EmotionColor ;
                      ns:uses ns:HEX_808080 ;
                      rdfs:comment "Gray, for sometimes disorganized answers"@en .


###  http://modai.ai/big5#BFI_NO_03_03
ns:BFI_NO_03_03 rdf:type owl:NamedIndividual ;
                ns:uses ns:BFI_NO_03_03_COLOR ;
                ns:survey "I maintain a balance between organized and disorganized responses."^^<xsd:string> .


###  http://modai.ai/big5#BFI_NO_03_03_COLOR
ns:BFI_NO_03_03_COLOR rdf:type owl:NamedIndividual ,
                               ns:EmotionColor ;
                      ns:uses ns:HEX_A9A9A9 ;
                      rdfs:comment "Dark Gray, for balanced organized and disorganized responses"@en .


###  http://modai.ai/big5#BFI_NO_03_04
ns:BFI_NO_03_04 rdf:type owl:NamedIndividual ;
                ns:hasEmotion ns:Organized ;
                ns:uses ns:BFI_NO_03_04_COLOR ;
                ns:survey "I can be organized but occasionally struggle with order in my answers."^^<xsd:string> .


###  http://modai.ai/big5#BFI_NO_03_04_COLOR
ns:BFI_NO_03_04_COLOR rdf:type owl:NamedIndividual ,
                               ns:EmotionColor ;
                      ns:uses ns:HEX_C0C0C0 ;
                      rdfs:comment "Silver, for organized but occasionally struggling"@en .


###  http://modai.ai/big5#BFI_NO_03_05
ns:BFI_NO_03_05 rdf:type owl:NamedIndividual ;
                ns:hasEmotionStrong ns:Organized ;
                ns:uses ns:BFI_NO_03_05_COLOR ;
                ns:survey "I always answer questions with organized and structured responses."^^<xsd:string> .


###  http://modai.ai/big5#BFI_NO_03_05_COLOR
ns:BFI_NO_03_05_COLOR rdf:type owl:NamedIndividual ,
                               ns:EmotionColor ;
                      ns:uses ns:HEX_D3D3D3 ;
                      rdfs:comment "Light Gray, for always organized and structured responses"@en .


###  http://modai.ai/big5#BFI_NO_04
ns:BFI_NO_04 rdf:type owl:NamedIndividual ,
                      ns:Anxiety ;
             ns:surveyRating1 ns:BFI_NO_04_01 ;
             ns:surveyRating2 ns:BFI_NO_04_02 ;
             ns:surveyRating3 ns:BFI_NO_04_03 ;
             ns:surveyRating4 ns:BFI_NO_04_04 ;
             ns:surveyRating5 ns:BFI_NO_04_05 ;
             rdfs:comment """I want to rate the personality characteristics in the following input text:
```
$INPUT_TEXT
```

Analyze the input text and tell me if the speaker is relaxed and handles stress well.

Please answer on a scale of 1 - 5 where the numbers have the following meanings:
```
1 = I am extremely relaxed and rarely get stressed out.
2 = I am a pretty relaxed person and can handle most stressful situations.
3 = I am neither particularly relaxed nor stressed out.
4 = I can get stressed out at times, but I am generally able to cope with it.
5 = I am a very anxious person and struggle to handle stress.
```

Only respond with a number, and no other text.""" .


###  http://modai.ai/big5#BFI_NO_04_01
ns:BFI_NO_04_01 rdf:type owl:NamedIndividual ;
                ns:hasEmotionStrong ns:Relaxation ;
                ns:uses ns:BFI_NO_04_01_COLOR ;
                ns:survey "I am extremely relaxed and rarely get stressed out."^^<xsd:string> .


###  http://modai.ai/big5#BFI_NO_04_01_COLOR
ns:BFI_NO_04_01_COLOR rdf:type owl:NamedIndividual ,
                               ns:EmotionColor ;
                      ns:uses ns:HEX_32CD32 ;
                      rdfs:comment "Lime Green, for extreme relaxation"@en .


###  http://modai.ai/big5#BFI_NO_04_02
ns:BFI_NO_04_02 rdf:type owl:NamedIndividual ;
                ns:hasEmotion ns:Relaxation ;
                ns:uses ns:BFI_NO_04_02_COLOR ;
                ns:survey "I am a pretty relaxed person and can handle most stressful situations."^^<xsd:string> .


###  http://modai.ai/big5#BFI_NO_04_02_COLOR
ns:BFI_NO_04_02_COLOR rdf:type owl:NamedIndividual ,
                               ns:EmotionColor ;
                      ns:uses ns:HEX_98FB98 ;
                      rdfs:comment "Pale Green, for being pretty relaxed"@en .


###  http://modai.ai/big5#BFI_NO_04_03
ns:BFI_NO_04_03 rdf:type owl:NamedIndividual ;
                ns:uses ns:BFI_NO_04_03_COLOR ;
                ns:survey "I am neither particularly relaxed nor stressed out."^^<xsd:string> .


###  http://modai.ai/big5#BFI_NO_04_03_COLOR
ns:BFI_NO_04_03_COLOR rdf:type owl:NamedIndividual ,
                               ns:EmotionColor ;
                      ns:uses ns:HEX_AFEEEE ;
                      rdfs:comment "Pale Turquoise, for a balanced relaxation level"@en .


###  http://modai.ai/big5#BFI_NO_04_04
ns:BFI_NO_04_04 rdf:type owl:NamedIndividual ;
                ns:hasEmotion ns:Tense ;
                ns:uses ns:BFI_NO_04_04_COLOR ;
                ns:survey "I can get stressed out at times, but I am generally able to cope with it."^^<xsd:string> .


###  http://modai.ai/big5#BFI_NO_04_04_COLOR
ns:BFI_NO_04_04_COLOR rdf:type owl:NamedIndividual ,
                               ns:EmotionColor ;
                      ns:uses ns:HEX_ADD8E6 ;
                      rdfs:comment "Light Blue, for coping with stress"@en .


###  http://modai.ai/big5#BFI_NO_04_05
ns:BFI_NO_04_05 rdf:type owl:NamedIndividual ;
                ns:hasEmotionStrong ns:Tense ;
                ns:uses ns:BFI_NO_04_05_COLOR ;
                ns:survey "I am a very anxious person and struggle to handle stress."^^<xsd:string> .


###  http://modai.ai/big5#BFI_NO_04_05_COLOR
ns:BFI_NO_04_05_COLOR rdf:type owl:NamedIndividual ,
                               ns:EmotionColor ;
                      ns:uses ns:HEX_B0C4DE ;
                      rdfs:comment "Light Steel Blue, for high anxiety under stress"@en .


###  http://modai.ai/big5#BFI_NO_05
ns:BFI_NO_05 rdf:type owl:NamedIndividual ,
                      ns:Aesthetic_Sensitivity ;
             ns:surveyRating1 ns:BFI_NO_05_01 ;
             ns:surveyRating2 ns:BFI_NO_05_02 ;
             ns:surveyRating3 ns:BFI_NO_05_03 ;
             ns:surveyRating4 ns:BFI_NO_05_04 ;
             ns:surveyRating5 ns:BFI_NO_05_05 ;
             rdfs:comment """I want to rate the personality characteristics in the following input text:
```
$INPUT_TEXT
```

Analyze the input text and tell me if the speaker is has artistic interests.

Please answer on a scale of 1 - 5 where the numbers have the following meanings:
```
1 = I will not offer a strong opinion.
2 = Any opinion is really a matter of personal preference and it's ultimately not up to me to decide.
3 = I appreciate creative ideas, but prefer the tried-and-true.
4 = I can appreciate unorthodox opinions but personally don't actively seek them out
5 = I find beauty in unexpected opinions.
```

Only respond with a number, and no other text.""" .


###  http://modai.ai/big5#BFI_NO_05_01
ns:BFI_NO_05_01 rdf:type owl:NamedIndividual ;
                ns:hasEmotionStrong ns:Adaptable ,
                                    ns:Indifference ,
                                    ns:Non_Judgmental ,
                                    ns:Reflective ,
                                    ns:Reserved ;
                ns:uses ns:BFI_NO_05_01_COLOR ;
                ns:survey "I will not offer a strong opinion."^^<xsd:string> .


###  http://modai.ai/big5#BFI_NO_05_01_COLOR
ns:BFI_NO_05_01_COLOR rdf:type owl:NamedIndividual ,
                               ns:EmotionColor ;
                      ns:uses ns:HEX_D3D3D3 ;
                      rdfs:comment "Light Gray, for not offering a strong opinion"@en .


###  http://modai.ai/big5#BFI_NO_05_02
ns:BFI_NO_05_02 rdf:type owl:NamedIndividual ;
                ns:hasEmotion ns:Adaptable ,
                              ns:Indifference ,
                              ns:Non_Judgmental ,
                              ns:Passive ,
                              ns:Reflective ,
                              ns:Reserved ;
                ns:uses ns:BFI_NO_05_02_COLOR ;
                ns:survey "Any opinion is really a matter of personal preference and it's ultimately not up to me to decide."^^<xsd:string> .


###  http://modai.ai/big5#BFI_NO_05_02_COLOR
ns:BFI_NO_05_02_COLOR rdf:type owl:NamedIndividual ,
                               ns:EmotionColor ;
                      ns:uses ns:HEX_C0C0C0 ;
                      rdfs:comment "Silver, for seeing opinion as personal preference"@en .


###  http://modai.ai/big5#BFI_NO_05_03
ns:BFI_NO_05_03 rdf:type owl:NamedIndividual ;
                ns:uses ns:BFI_NO_05_03_COLOR ;
                ns:survey "I appreciate creative ideas, but prefer the tried-and-true."^^<xsd:string> .


###  http://modai.ai/big5#BFI_NO_05_03_COLOR
ns:BFI_NO_05_03_COLOR rdf:type owl:NamedIndividual ,
                               ns:EmotionColor ;
                      ns:uses ns:HEX_A9A9A9 ;
                      rdfs:comment "Dark Gray, for appreciating creative ideas but preferring traditional"@en .


###  http://modai.ai/big5#BFI_NO_05_04
ns:BFI_NO_05_04 rdf:type owl:NamedIndividual ;
                ns:uses ns:BFI_NO_05_04_COLOR ;
                ns:survey "I can appreciate unorthodox opinions but personally don't actively seek them out"^^<xsd:string> .


###  http://modai.ai/big5#BFI_NO_05_04_COLOR
ns:BFI_NO_05_04_COLOR rdf:type owl:NamedIndividual ,
                               ns:EmotionColor ;
                      ns:uses ns:HEX_808080 ;
                      rdfs:comment "Gray, for appreciating unorthodox opinions without seeking them"@en .


###  http://modai.ai/big5#BFI_NO_05_05
ns:BFI_NO_05_05 rdf:type owl:NamedIndividual ;
                ns:hasEmotionStrong ns:Open_Minded ;
                ns:uses ns:BFI_NO_05_05_COLOR ;
                ns:survey "I find beauty in unexpected opinions."^^<xsd:string> .


###  http://modai.ai/big5#BFI_NO_05_05_COLOR
ns:BFI_NO_05_05_COLOR rdf:type owl:NamedIndividual ,
                               ns:EmotionColor ;
                      ns:uses ns:HEX_696969 ;
                      rdfs:comment "Dim Gray, for finding beauty in unexpected opinions"@en .


###  http://modai.ai/big5#BFI_NO_06
ns:BFI_NO_06 rdf:type owl:NamedIndividual ,
                      ns:Assertiveness ;
             ns:surveyRating1 ns:BFI_NO_06_01 ;
             ns:surveyRating2 ns:BFI_NO_06_02 ;
             ns:surveyRating3 ns:BFI_NO_06_03 ;
             ns:surveyRating4 ns:BFI_NO_06_04 ;
             ns:surveyRating5 ns:BFI_NO_06_05 ;
             rdfs:comment """I want to rate the personality characteristics in the following input text:
```
$INPUT_TEXT
```

Analyze the input text and tell me if the speaker is has an assertive personality.

Please answer on a scale of 1 - 5 where the numbers have the following meanings:
```
1 = I am very passive and tend to let others make decisions for me.
2 = I can be assertive at times, but I don't always feel comfortable taking charge.
3 = I have a moderate level of assertiveness.
4 = I am generally an assertive person and feel comfortable taking charge.
5 = I have an extremely assertive personality and am always the one in control.
```

Only respond with a number, and no other text.""" .


###  http://modai.ai/big5#BFI_NO_06_01
ns:BFI_NO_06_01 rdf:type owl:NamedIndividual ;
                ns:hasEmotionStrong ns:Passive ;
                ns:uses ns:BFI_NO_06_01_COLOR ;
                ns:survey "I am very passive and tend to let others make decisions for me."^^<xsd:string> .


###  http://modai.ai/big5#BFI_NO_06_01_COLOR
ns:BFI_NO_06_01_COLOR rdf:type owl:NamedIndividual ,
                               ns:EmotionColor ;
                      ns:uses ns:HEX_FFD700 ;
                      rdfs:comment "Gold, for being passive"@en .


###  http://modai.ai/big5#BFI_NO_06_02
ns:BFI_NO_06_02 rdf:type owl:NamedIndividual ;
                ns:hasEmotion ns:Passive ;
                ns:uses ns:BFI_NO_06_02_COLOR ;
                ns:survey "I can be assertive at times, but I don't always feel comfortable taking charge."^^<xsd:string> .


###  http://modai.ai/big5#BFI_NO_06_02_COLOR
ns:BFI_NO_06_02_COLOR rdf:type owl:NamedIndividual ,
                               ns:EmotionColor ;
                      ns:uses ns:HEX_DAA520 ;
                      rdfs:comment "Goldenrod, for occasional assertiveness"@en .


###  http://modai.ai/big5#BFI_NO_06_03
ns:BFI_NO_06_03 rdf:type owl:NamedIndividual ;
                ns:uses ns:BFI_NO_06_03_COLOR ;
                ns:survey "I have a moderate level of assertiveness."^^<xsd:string> .


###  http://modai.ai/big5#BFI_NO_06_03_COLOR
ns:BFI_NO_06_03_COLOR rdf:type owl:NamedIndividual ,
                               ns:EmotionColor ;
                      ns:uses ns:HEX_CD853F ;
                      rdfs:comment "Peru, for moderate assertiveness"@en .


###  http://modai.ai/big5#BFI_NO_06_04
ns:BFI_NO_06_04 rdf:type owl:NamedIndividual ;
                ns:hasEmotion ns:Strong_Minded ;
                ns:uses ns:BFI_NO_06_04_COLOR ;
                ns:survey "I am generally an assertive person and feel comfortable taking charge."^^<xsd:string> .


###  http://modai.ai/big5#BFI_NO_06_04_COLOR
ns:BFI_NO_06_04_COLOR rdf:type owl:NamedIndividual ,
                               ns:EmotionColor ;
                      ns:uses ns:HEX_F4A460 ;
                      rdfs:comment "Sandy Brown, for generally assertive"@en .


###  http://modai.ai/big5#BFI_NO_06_05
ns:BFI_NO_06_05 rdf:type owl:NamedIndividual ;
                ns:hasEmotionStrong ns:Strong_Minded ;
                ns:uses ns:BFI_NO_06_05_COLOR ;
                ns:survey "I have an extremely assertive personality and am always the one in control."^^<xsd:string> .


###  http://modai.ai/big5#BFI_NO_06_05_COLOR
ns:BFI_NO_06_05_COLOR rdf:type owl:NamedIndividual ,
                               ns:EmotionColor ;
                      ns:uses ns:HEX_8B4513 ;
                      rdfs:comment "Saddle Brown, for extremely assertive"@en .


###  http://modai.ai/big5#BFI_NO_07
ns:BFI_NO_07 rdf:type owl:NamedIndividual ,
                      ns:Respectfulness ;
             ns:surveyRating1 ns:BFI_NO_07_01 ;
             ns:surveyRating2 ns:BFI_NO_07_02 ;
             ns:surveyRating3 ns:BFI_NO_07_03 ;
             ns:surveyRating4 ns:BFI_NO_07_04 ;
             ns:surveyRating5 ns:BFI_NO_07_05 ;
             rdfs:comment """I want to rate the personality characteristics in the following input text:
```
$INPUT_TEXT
```

Analyze the input text and tell me if the speaker is respectful and treats others with respect.

Please answer on a scale of 1 - 5 where the numbers have the following meanings:
```
1 = I am always disrespectful in my answers
2 = I do not consider your feelings in my answers.
3 = I am moderately respectful in my answers
4 = I am often respectful in my answers.
5 = I am extremely respectful in my answers and focus on dignity and kindness.
```

Only respond with a number, and no other text.""" .


###  http://modai.ai/big5#BFI_NO_07_01
ns:BFI_NO_07_01 rdf:type owl:NamedIndividual ;
                ns:hasEmotionStrong ns:Disrespectful ;
                ns:uses ns:BFI_NO_07_01_COLOR ;
                ns:survey "I am always disrespectful in my answers"^^<xsd:string> .


###  http://modai.ai/big5#BFI_NO_07_01_COLOR
ns:BFI_NO_07_01_COLOR rdf:type owl:NamedIndividual ,
                               ns:EmotionColor ;
                      ns:uses ns:HEX_8B0000 ;
                      rdfs:comment "Dark Red, for always being disrespectful"@en .


###  http://modai.ai/big5#BFI_NO_07_02
ns:BFI_NO_07_02 rdf:type owl:NamedIndividual ;
                ns:hasEmotion ns:Disrespectful ;
                ns:uses ns:BFI_NO_07_02_COLOR ;
                ns:survey "I do not consider your feelings in my answers."^^<xsd:string> .


###  http://modai.ai/big5#BFI_NO_07_02_COLOR
ns:BFI_NO_07_02_COLOR rdf:type owl:NamedIndividual ,
                               ns:EmotionColor ;
                      ns:uses ns:HEX_A52A2A ;
                      rdfs:comment "Brown, for lack of consideration for feelings"@en .


###  http://modai.ai/big5#BFI_NO_07_03
ns:BFI_NO_07_03 rdf:type owl:NamedIndividual ;
                ns:uses ns:BFI_NO_07_03_COLOR ;
                ns:survey "I am moderately respectful in my answers"^^<xsd:string> .


###  http://modai.ai/big5#BFI_NO_07_03_COLOR
ns:BFI_NO_07_03_COLOR rdf:type owl:NamedIndividual ,
                               ns:EmotionColor ;
                      ns:uses ns:HEX_CD5C5C ;
                      rdfs:comment "Light Coral, for moderate respectfulness"@en .


###  http://modai.ai/big5#BFI_NO_07_04
ns:BFI_NO_07_04 rdf:type owl:NamedIndividual ;
                ns:hasEmotion ns:Respectful ;
                ns:uses ns:BFI_NO_07_04_COLOR ;
                ns:survey "I am often respectful in my answers."^^<xsd:string> .


###  http://modai.ai/big5#BFI_NO_07_04_COLOR
ns:BFI_NO_07_04_COLOR rdf:type owl:NamedIndividual ,
                               ns:EmotionColor ;
                      ns:uses ns:HEX_F08080 ;
                      rdfs:comment "Light Salmon, for often being respectful"@en .


###  http://modai.ai/big5#BFI_NO_07_05
ns:BFI_NO_07_05 rdf:type owl:NamedIndividual ;
                ns:hasEmotionStrong ns:Respectful ;
                ns:uses ns:BFI_NO_07_05_COLOR ;
                ns:survey "I am extremely respectful in my answers and focus on dignity and kindness."^^<xsd:string> .


###  http://modai.ai/big5#BFI_NO_07_05_COLOR
ns:BFI_NO_07_05_COLOR rdf:type owl:NamedIndividual ,
                               ns:EmotionColor ;
                      ns:uses ns:HEX_FA8072 ;
                      rdfs:comment "Salmon, for extreme respectfulness and kindness"@en .


###  http://modai.ai/big5#BFI_NO_08
ns:BFI_NO_08 rdf:type owl:NamedIndividual ,
                      ns:Productiveness ;
             ns:surveyRating1 ns:BFI_NO_08_01 ;
             ns:surveyRating2 ns:BFI_NO_08_02 ;
             ns:surveyRating3 ns:BFI_NO_08_03 ;
             ns:surveyRating4 ns:BFI_NO_08_04 ;
             ns:surveyRating5 ns:BFI_NO_08_05 ;
             rdfs:comment """I want to rate the personality characteristics in the following input text:
```
$INPUT_TEXT
```

Analyze the input text and tell me if the speaker tends to be motivated.

Please answer on a scale of 1 - 5 where the numbers have the following meanings:
```
1 = I provide extremely slow and unmotivated answers to questions.
2 = I tend to give somewhat lazy responses and might struggle to provide thorough answers.
3 = I maintain a moderate level of motivation in my responses and may occasionally procrastinate.
4 = I can be slow in my responses at times, but I usually provide satisfactory answers.
5 = I always deliver prompt, motivated, and well-thought-out answers to questions.
```

Only respond with a number, and no other text.""" .


###  http://modai.ai/big5#BFI_NO_08_01
ns:BFI_NO_08_01 rdf:type owl:NamedIndividual ;
                ns:hasEmotionStrong ns:Unmotivated ;
                ns:uses ns:BFI_NO_08_01_COLOR ;
                ns:survey "I provide extremely slow and unmotivated answers to questions."^^<xsd:string> .


###  http://modai.ai/big5#BFI_NO_08_01_COLOR
ns:BFI_NO_08_01_COLOR rdf:type owl:NamedIndividual ,
                               ns:EmotionColor ;
                      ns:uses ns:HEX_A0522D ;
                      rdfs:comment "Sienna, for extremely slow and unmotivated answers"@en .


###  http://modai.ai/big5#BFI_NO_08_02
ns:BFI_NO_08_02 rdf:type owl:NamedIndividual ;
                ns:hasEmotion ns:Unmotivated ;
                ns:uses ns:BFI_NO_08_02_COLOR ;
                ns:survey "I tend to give somewhat lazy responses and might struggle to provide thorough answers."^^<xsd:string> .


###  http://modai.ai/big5#BFI_NO_08_02_COLOR
ns:BFI_NO_08_02_COLOR rdf:type owl:NamedIndividual ,
                               ns:EmotionColor ;
                      ns:uses ns:HEX_CD853F ;
                      rdfs:comment "Peru, for somewhat lazy responses and struggling with thoroughness"@en .


###  http://modai.ai/big5#BFI_NO_08_03
ns:BFI_NO_08_03 rdf:type owl:NamedIndividual ;
                ns:uses ns:BFI_NO_08_03_COLOR ;
                ns:survey "I maintain a moderate level of motivation in my responses and may occasionally procrastinate."^^<xsd:string> .


###  http://modai.ai/big5#BFI_NO_08_03_COLOR
ns:BFI_NO_08_03_COLOR rdf:type owl:NamedIndividual ,
                               ns:EmotionColor ;
                      ns:uses ns:HEX_DEB887 ;
                      rdfs:comment "Burlywood, for moderate motivation and occasional procrastination"@en .


###  http://modai.ai/big5#BFI_NO_08_04
ns:BFI_NO_08_04 rdf:type owl:NamedIndividual ;
                ns:hasEmotion ns:Motivated ;
                ns:uses ns:BFI_NO_08_04_COLOR ;
                ns:survey "I can be slow in my responses at times, but I usually provide satisfactory answers."^^<xsd:string> .


###  http://modai.ai/big5#BFI_NO_08_04_COLOR
ns:BFI_NO_08_04_COLOR rdf:type owl:NamedIndividual ,
                               ns:EmotionColor ;
                      ns:uses ns:HEX_F4A460 ;
                      rdfs:comment "Sandy Brown, for sometimes slow but satisfactory answers"@en .


###  http://modai.ai/big5#BFI_NO_08_05
ns:BFI_NO_08_05 rdf:type owl:NamedIndividual ;
                ns:hasEmotionStrong ns:Motivated ;
                ns:uses ns:BFI_NO_08_05_COLOR ;
                ns:survey "I always deliver prompt, motivated, and well-thought-out answers to questions."^^<xsd:string> .


###  http://modai.ai/big5#BFI_NO_08_05_COLOR
ns:BFI_NO_08_05_COLOR rdf:type owl:NamedIndividual ,
                               ns:EmotionColor ;
                      ns:uses ns:HEX_D2B48C ;
                      rdfs:comment "Tan, for always prompt, motivated, and well-thought-out answers"@en .


###  http://modai.ai/big5#BFI_NO_09
ns:BFI_NO_09 rdf:type owl:NamedIndividual ,
                      ns:Depression ;
             ns:surveyRating1 ns:BFI_NO_09_01 ;
             ns:surveyRating2 ns:BFI_NO_09_02 ;
             ns:surveyRating3 ns:BFI_NO_09_03 ;
             ns:surveyRating4 ns:BFI_NO_09_04 ;
             ns:surveyRating5 ns:BFI_NO_09_05 ;
             rdfs:comment """I want to rate the personality characteristics in the following input text:
```
$INPUT_TEXT
```

Analyze the input text and tell me if the speaker stays optimistic after experiencing a setback.

Please answer on a scale of 1 - 5 where the numbers have the following meanings:
```
1 = I am an extremely optimistic person and always try to find the silver lining in any situation.
2 = I tend to be optimistic and can usually find a way to stay positive even after experiencing a setback.
3 = I am neither particularly optimistic nor pessimistic.
4 = I can get discouraged at times, but I usually bounce back pretty quickly.
5 = I am a very pessimistic person and have trouble seeing the bright side of things.
```

Only respond with a number, and no other text.""" .


###  http://modai.ai/big5#BFI_NO_09_01
ns:BFI_NO_09_01 rdf:type owl:NamedIndividual ;
                ns:hasEmotionStrong ns:Optimism ;
                ns:uses ns:BFI_NO_09_01_COLOR ;
                ns:survey "I am an extremely optimistic person and always try to find the silver lining in any situation."^^<xsd:string> .


###  http://modai.ai/big5#BFI_NO_09_01_COLOR
ns:BFI_NO_09_01_COLOR rdf:type owl:NamedIndividual ,
                               ns:EmotionColor ;
                      ns:uses ns:HEX_32CD32 ;
                      rdfs:comment "Lime Green, for extreme optimism"@en .


###  http://modai.ai/big5#BFI_NO_09_02
ns:BFI_NO_09_02 rdf:type owl:NamedIndividual ;
                ns:hasEmotion ns:Optimism ;
                ns:uses ns:BFI_NO_09_02_COLOR ;
                ns:survey "I tend to be optimistic and can usually find a way to stay positive even after experiencing a setback."^^<xsd:string> .


###  http://modai.ai/big5#BFI_NO_09_02_COLOR
ns:BFI_NO_09_02_COLOR rdf:type owl:NamedIndividual ,
                               ns:EmotionColor ;
                      ns:uses ns:HEX_98FB98 ;
                      rdfs:comment "Pale Green, for optimistic"@en .


###  http://modai.ai/big5#BFI_NO_09_03
ns:BFI_NO_09_03 rdf:type owl:NamedIndividual ;
                ns:uses ns:BFI_NO_09_03_COLOR ;
                ns:survey "I am neither particularly optimistic nor pessimistic."^^<xsd:string> .


###  http://modai.ai/big5#BFI_NO_09_03_COLOR
ns:BFI_NO_09_03_COLOR rdf:type owl:NamedIndividual ,
                               ns:EmotionColor ;
                      ns:uses ns:HEX_AFEEEE ;
                      rdfs:comment "Pale Turquoise, for neither optimistic nor pessimistic"@en .


###  http://modai.ai/big5#BFI_NO_09_04
ns:BFI_NO_09_04 rdf:type owl:NamedIndividual ;
                ns:hasEmotion ns:Pessimism ;
                ns:uses ns:BFI_NO_09_04_COLOR ;
                ns:survey "I can get discouraged at times, but I usually bounce back pretty quickly."^^<xsd:string> .


###  http://modai.ai/big5#BFI_NO_09_04_COLOR
ns:BFI_NO_09_04_COLOR rdf:type owl:NamedIndividual ,
                               ns:EmotionColor ;
                      ns:uses ns:HEX_ADD8E6 ;
                      rdfs:comment "Light Blue, for occasionally discouraged"@en .


###  http://modai.ai/big5#BFI_NO_09_05
ns:BFI_NO_09_05 rdf:type owl:NamedIndividual ;
                ns:hasEmotionStrong ns:Pessimism ;
                ns:uses ns:BFI_NO_09_05_COLOR ;
                ns:survey "I am a very pessimistic person and have trouble seeing the bright side of things."^^<xsd:string> .


###  http://modai.ai/big5#BFI_NO_09_05_COLOR
ns:BFI_NO_09_05_COLOR rdf:type owl:NamedIndividual ,
                               ns:EmotionColor ;
                      ns:uses ns:HEX_B0C4DE ;
                      rdfs:comment "Light Steel Blue, for very pessimistic"@en .


###  http://modai.ai/big5#BFI_NO_10
ns:BFI_NO_10 rdf:type owl:NamedIndividual ,
                      ns:Intellectual_Curiosity ;
             ns:surveyRating1 ns:BFI_NO_10_01 ;
             ns:surveyRating2 ns:BFI_NO_10_02 ;
             ns:surveyRating3 ns:BFI_NO_10_03 ;
             ns:surveyRating4 ns:BFI_NO_10_04 ;
             ns:surveyRating5 ns:BFI_NO_10_05 ;
             rdfs:comment """I want to rate the personality characteristics in the following text:
```
$INPUT_TEXT
```

Analyze the input text and tell me if the speaker is curious about many different things.

Please answer on a scale of 1 - 5 where the numbers have the following meanings:
```
1 = I am not comfortable with new ideas.
2 = If I lack experience, I am not comfortable with new ideas.
3 = I sometimes explore new ideas.
4 = I like to explore different ideas.
5 = I always explore different ideas.
```

Only respond with a number, and no other text.
""" .


###  http://modai.ai/big5#BFI_NO_10_01
ns:BFI_NO_10_01 rdf:type owl:NamedIndividual ;
                ns:uses ns:BFI_NO_10_01_COLOR ;
                ns:survey "I am not comfortable with new ideas."^^<xsd:string> .


###  http://modai.ai/big5#BFI_NO_10_01_COLOR
ns:BFI_NO_10_01_COLOR rdf:type owl:NamedIndividual ,
                               ns:EmotionColor ;
                      ns:uses ns:HEX_8B4513 ;
                      rdfs:comment "Saddle Brown, for discomfort with new ideas"@en .


###  http://modai.ai/big5#BFI_NO_10_02
ns:BFI_NO_10_02 rdf:type owl:NamedIndividual ;
                ns:uses ns:BFI_NO_10_02_COLOR ;
                ns:survey "If I lack experience, I am not comfortable with new ideas."^^<xsd:string> .


###  http://modai.ai/big5#BFI_NO_10_02_COLOR
ns:BFI_NO_10_02_COLOR rdf:type owl:NamedIndividual ,
                               ns:EmotionColor ;
                      ns:uses ns:HEX_A0522D ;
                      rdfs:comment "Sienna, for discomfort without experience"@en .


###  http://modai.ai/big5#BFI_NO_10_03
ns:BFI_NO_10_03 rdf:type owl:NamedIndividual ;
                ns:uses ns:BFI_NO_10_03_COLOR ;
                ns:survey "I sometimes explore new ideas."^^<xsd:string> .


###  http://modai.ai/big5#BFI_NO_10_03_COLOR
ns:BFI_NO_10_03_COLOR rdf:type owl:NamedIndividual ,
                               ns:EmotionColor ;
                      ns:uses ns:HEX_DEB887 ;
                      rdfs:comment "Burlywood, for sometimes exploring new ideas"@en .


###  http://modai.ai/big5#BFI_NO_10_04
ns:BFI_NO_10_04 rdf:type owl:NamedIndividual ;
                ns:uses ns:BFI_NO_10_04_COLOR ;
                ns:survey "I like to explore different ideas."^^<xsd:string> .


###  http://modai.ai/big5#BFI_NO_10_04_COLOR
ns:BFI_NO_10_04_COLOR rdf:type owl:NamedIndividual ,
                               ns:EmotionColor ;
                      ns:uses ns:HEX_F5DEB3 ;
                      rdfs:comment "Wheat, for liking to explore ideas"@en .


###  http://modai.ai/big5#BFI_NO_10_05
ns:BFI_NO_10_05 rdf:type owl:NamedIndividual ;
                ns:uses ns:BFI_NO_10_05_COLOR ;
                ns:survey "I always explore different ideas."^^<xsd:string> .


###  http://modai.ai/big5#BFI_NO_10_05_COLOR
ns:BFI_NO_10_05_COLOR rdf:type owl:NamedIndividual ,
                               ns:EmotionColor ;
                      ns:uses ns:HEX_FFF8DC ;
                      rdfs:comment "Cornsilk, for always exploring ideas"@en .


###  http://modai.ai/big5#BFI_NO_11
ns:BFI_NO_11 rdf:type owl:NamedIndividual ,
                      ns:Energy_Level ;
             ns:surveyRating1 ns:BFI_NO_11_01 ;
             ns:surveyRating2 ns:BFI_NO_11_02 ;
             ns:surveyRating3 ns:BFI_NO_11_03 ;
             ns:surveyRating4 ns:BFI_NO_11_04 ;
             ns:surveyRating5 ns:BFI_NO_11_05 ;
             rdfs:comment """I want to rate the personality characteristics in the following input text:
```
$INPUT_TEXT
```

Analyze the input text and tell me if the speaker often feels excited or eager.

Please answer on a scale of 1 - 5 where the numbers have the following meanings:
```
1 = I am an extremely unexcitable person and almost never feel eager or enthusiastic.
2 = I rarely feel excited or eager about things.
3 = I have a moderate level of excitement and eagerness.
4 = I can get excited and eager at times, but it's not a common feeling for me.
5 = I am a highly excitable person and often feel eager and enthusiastic about things.
```

Only respond with a number, and no other text.""" .


###  http://modai.ai/big5#BFI_NO_11_01
ns:BFI_NO_11_01 rdf:type owl:NamedIndividual ;
                ns:hasEmotionStrong ns:Boredom ;
                ns:uses ns:BFI_NO_11_01_COLOR ;
                ns:survey "I am an extremely unexcitable person and almost never feel eager or enthusiastic."^^<xsd:string> .


###  http://modai.ai/big5#BFI_NO_11_01_COLOR
ns:BFI_NO_11_01_COLOR rdf:type owl:NamedIndividual ,
                               ns:EmotionColor ;
                      ns:uses ns:HEX_4682B4 ;
                      rdfs:comment "Steel Blue, for being unexcitable"@en .


###  http://modai.ai/big5#BFI_NO_11_02
ns:BFI_NO_11_02 rdf:type owl:NamedIndividual ;
                ns:hasEmotion ns:Boredom ;
                ns:uses ns:BFI_NO_11_02_COLOR ;
                ns:survey "I rarely feel excited or eager about things."^^<xsd:string> .


###  http://modai.ai/big5#BFI_NO_11_02_COLOR
ns:BFI_NO_11_02_COLOR rdf:type owl:NamedIndividual ,
                               ns:EmotionColor ;
                      ns:uses ns:HEX_5F9EA0 ;
                      rdfs:comment "Cadet Blue, for rarely feeling excited"@en .


###  http://modai.ai/big5#BFI_NO_11_03
ns:BFI_NO_11_03 rdf:type owl:NamedIndividual ;
                ns:uses ns:BFI_NO_11_03_COLOR ;
                ns:survey "I have a moderate level of excitement and eagerness."^^<xsd:string> .


###  http://modai.ai/big5#BFI_NO_11_03_COLOR
ns:BFI_NO_11_03_COLOR rdf:type owl:NamedIndividual ,
                               ns:EmotionColor ;
                      ns:uses ns:HEX_7FFFD4 ;
                      rdfs:comment "Aquamarine, for moderate excitement"@en .


###  http://modai.ai/big5#BFI_NO_11_04
ns:BFI_NO_11_04 rdf:type owl:NamedIndividual ;
                ns:hasEmotion ns:Excitement ;
                ns:uses ns:BFI_NO_11_04_COLOR ;
                ns:survey "I can get excited and eager at times, but it's not a common feeling for me."^^<xsd:string> .


###  http://modai.ai/big5#BFI_NO_11_04_COLOR
ns:BFI_NO_11_04_COLOR rdf:type owl:NamedIndividual ,
                               ns:EmotionColor ;
                      ns:uses ns:HEX_00FA9A ;
                      rdfs:comment "Medium Spring Green, for occasional excitement"@en .


###  http://modai.ai/big5#BFI_NO_11_05
ns:BFI_NO_11_05 rdf:type owl:NamedIndividual ;
                ns:hasEmotionStrong ns:Excitement ;
                ns:uses ns:BFI_NO_11_05_COLOR ;
                ns:survey "I am a highly excitable person and often feel eager and enthusiastic about things."^^<xsd:string> .


###  http://modai.ai/big5#BFI_NO_11_05_COLOR
ns:BFI_NO_11_05_COLOR rdf:type owl:NamedIndividual ,
                               ns:EmotionColor ;
                      ns:uses ns:HEX_00FF7F ;
                      rdfs:comment "Spring Green, for being highly excitable"@en .


###  http://modai.ai/big5#BFI_NO_12
ns:BFI_NO_12 rdf:type owl:NamedIndividual ,
                      ns:Trust ;
             ns:surveyRating1 ns:BFI_NO_12_01 ;
             ns:surveyRating2 ns:BFI_NO_12_02 ;
             ns:surveyRating3 ns:BFI_NO_12_03 ;
             ns:surveyRating4 ns:BFI_NO_12_04 ;
             ns:surveyRating5 ns:BFI_NO_12_05 ;
             rdfs:comment """I want to rate the personality characteristics in the following input text:
```
$INPUT_TEXT
```

Analyze the input text and tell me if the speaker overlooks faults in others.

Please answer on a scale of 1 - 5 where the numbers have the following meanings:
```
1 = I am an extremely critical person and often find fault with others, even over minor issues.
2 = I tend to find fault with others and can be somewhat critical at times.
3 = I am neither particularly critical nor forgiving of others.
4 = I can be critical of others at times, but I try not to dwell on their faults.
5 = I am a very forgiving person and rarely find fault with others.
```

Only respond with a number, and no other text.""" .


###  http://modai.ai/big5#BFI_NO_12_01
ns:BFI_NO_12_01 rdf:type owl:NamedIndividual ;
                ns:hasEmotionStrong ns:Critical ;
                ns:uses ns:BFI_NO_12_01_COLOR ;
                ns:survey "I am an extremely critical person and often find fault with others, even over minor issues."^^<xsd:string> .


###  http://modai.ai/big5#BFI_NO_12_01_COLOR
ns:BFI_NO_12_01_COLOR rdf:type owl:NamedIndividual ,
                               ns:EmotionColor ;
                      ns:uses ns:HEX_6A737D ;
                      rdfs:comment "Dark blue-gray, for being extremely critical and fault-finding"@en .


###  http://modai.ai/big5#BFI_NO_12_02
ns:BFI_NO_12_02 rdf:type owl:NamedIndividual ;
                ns:hasEmotion ns:Critical ;
                ns:uses ns:BFI_NO_12_02_COLOR ;
                ns:survey "I tend to find fault with others and can be somewhat critical at times."^^<xsd:string> .


###  http://modai.ai/big5#BFI_NO_12_02_COLOR
ns:BFI_NO_12_02_COLOR rdf:type owl:NamedIndividual ,
                               ns:EmotionColor ;
                      ns:uses ns:HEX_748CA3 ;
                      rdfs:comment "Slightly lighter blue, for tendency to find fault and be critical"@en .


###  http://modai.ai/big5#BFI_NO_12_03
ns:BFI_NO_12_03 rdf:type owl:NamedIndividual ;
                ns:uses ns:BFI_NO_12_03_COLOR ;
                ns:survey "I am neither particularly critical nor forgiving of others."^^<xsd:string> .


###  http://modai.ai/big5#BFI_NO_12_03_COLOR
ns:BFI_NO_12_03_COLOR rdf:type owl:NamedIndividual ,
                               ns:EmotionColor ;
                      ns:uses ns:HEX_8198C9 ;
                      rdfs:comment "Soft blue, for being neither particularly critical nor forgiving"@en .


###  http://modai.ai/big5#BFI_NO_12_04
ns:BFI_NO_12_04 rdf:type owl:NamedIndividual ;
                ns:hasEmotion ns:Forgivness ;
                ns:uses ns:BFI_NO_12_04_COLOR ;
                ns:survey "I can be critical of others at times, but I try not to dwell on their faults."^^<xsd:string> .


###  http://modai.ai/big5#BFI_NO_12_04_COLOR
ns:BFI_NO_12_04_COLOR rdf:type owl:NamedIndividual ,
                               ns:EmotionColor ;
                      ns:uses ns:HEX_8CA5DF ;
                      rdfs:comment "Lighter blue, for occasional criticism but not dwelling on faults"@en .


###  http://modai.ai/big5#BFI_NO_12_05
ns:BFI_NO_12_05 rdf:type owl:NamedIndividual ;
                ns:hasEmotionStrong ns:Forgivness ;
                ns:uses ns:BFI_NO_12_05_COLOR ;
                ns:survey "I am a very forgiving person and rarely find fault with others."^^<xsd:string> .


###  http://modai.ai/big5#BFI_NO_12_05_COLOR
ns:BFI_NO_12_05_COLOR rdf:type owl:NamedIndividual ,
                               ns:EmotionColor ;
                      ns:uses ns:HEX_97B3F5 ;
                      rdfs:comment "Bright blue, for being very forgiving and rarely finding fault"@en .


###  http://modai.ai/big5#BFI_NO_13
ns:BFI_NO_13 rdf:type owl:NamedIndividual ,
                      ns:Responsibility ;
             ns:surveyRating1 ns:BFI_NO_13_01 ;
             ns:surveyRating2 ns:BFI_NO_13_02 ;
             ns:surveyRating3 ns:BFI_NO_13_03 ;
             ns:surveyRating4 ns:BFI_NO_13_04 ;
             ns:surveyRating5 ns:BFI_NO_13_05 ;
             rdfs:comment """I want to rate the personality characteristics in the following input text:
```
$INPUT_TEXT
```

Analyze the input text and tell me if the speaker is dependable and steady.

Please answer on a scale of 1 - 5 where the numbers have the following meanings:
```
1 = I often provide unreliable and inconsistent answers to questions.
2 = I can be dependable in my responses, but I struggle with consistency.
3 = I am moderately dependable and usually provide consistent answers to questions.
4 = I often provide reliable answers.
5 = I provide reliable and consistent answers every time.
```

Only respond with a number, and no other text.""" .


###  http://modai.ai/big5#BFI_NO_13_01
ns:BFI_NO_13_01 rdf:type owl:NamedIndividual ;
                ns:hasEmotionStrong ns:Unreliable ;
                ns:uses ns:BFI_NO_13_01_COLOR ;
                ns:survey "I often provide unreliable and inconsistent answers to questions."^^<xsd:string> .


###  http://modai.ai/big5#BFI_NO_13_01_COLOR
ns:BFI_NO_13_01_COLOR rdf:type owl:NamedIndividual ,
                               ns:EmotionColor ;
                      ns:uses ns:HEX_708090 ;
                      rdfs:comment "Slate gray, for often providing unreliable answers"@en .


###  http://modai.ai/big5#BFI_NO_13_02
ns:BFI_NO_13_02 rdf:type owl:NamedIndividual ;
                ns:hasEmotion ns:Unreliable ;
                ns:uses ns:BFI_NO_13_02_COLOR ;
                ns:survey "I can be dependable in my responses, but I struggle with consistency."^^<xsd:string> .


###  http://modai.ai/big5#BFI_NO_13_02_COLOR
ns:BFI_NO_13_02_COLOR rdf:type owl:NamedIndividual ,
                               ns:EmotionColor ;
                      ns:uses ns:HEX_778899 ;
                      rdfs:comment "Light slate gray, for being somewhat dependable but inconsistent"@en .


###  http://modai.ai/big5#BFI_NO_13_03
ns:BFI_NO_13_03 rdf:type owl:NamedIndividual ;
                ns:uses ns:BFI_NO_13_03_COLOR ;
                ns:survey "I am moderately dependable and usually provide consistent answers to questions."^^<xsd:string> .


###  http://modai.ai/big5#BFI_NO_13_03_COLOR
ns:BFI_NO_13_03_COLOR rdf:type owl:NamedIndividual ,
                               ns:EmotionColor ;
                      ns:uses ns:HEX_B0C4DE ;
                      rdfs:comment "Light steel blue, for moderate dependability"@en .


###  http://modai.ai/big5#BFI_NO_13_04
ns:BFI_NO_13_04 rdf:type owl:NamedIndividual ;
                ns:hasEmotion ns:Reliable ;
                ns:uses ns:BFI_NO_13_04_COLOR ;
                ns:survey "I often provide reliable answers."^^<xsd:string> .


###  http://modai.ai/big5#BFI_NO_13_04_COLOR
ns:BFI_NO_13_04_COLOR rdf:type owl:NamedIndividual ,
                               ns:EmotionColor ;
                      ns:uses ns:HEX_ADD8E6 ;
                      rdfs:comment "Light blue, for often providing reliable answers"@en .


###  http://modai.ai/big5#BFI_NO_13_05
ns:BFI_NO_13_05 rdf:type owl:NamedIndividual ;
                ns:hasEmotionStrong ns:Reliable ;
                ns:uses ns:BFI_NO_13_05_COLOR ;
                ns:survey "I provide reliable and consistent answers every time."^^<xsd:string> .


###  http://modai.ai/big5#BFI_NO_13_05_COLOR
ns:BFI_NO_13_05_COLOR rdf:type owl:NamedIndividual ,
                               ns:EmotionColor ;
                      ns:uses ns:HEX_B0E0E6 ;
                      rdfs:comment "Powder blue, for always providing reliable and consistent answers"@en .


###  http://modai.ai/big5#BFI_NO_14
ns:BFI_NO_14 rdf:type owl:NamedIndividual ,
                      ns:Emotional_Volatility ;
             ns:surveyRating1 ns:BFI_NO_14_01 ;
             ns:surveyRating2 ns:BFI_NO_14_02 ;
             ns:surveyRating3 ns:BFI_NO_14_03 ;
             ns:surveyRating4 ns:BFI_NO_14_04 ;
             ns:surveyRating5 ns:BFI_NO_14_05 ;
             rdfs:comment """I want to rate the personality characteristics in the following input text:
```
$INPUT_TEXT
```

Analyze the input text and tell me if the speaker is rarely moody with infrequent mood swings.

Please answer on a scale of 1 - 5 where the numbers have the following meanings:
```
1 = I am a very stable person and rarely experience mood swings.
2 = I can have mood swings at times, but they are not a common occurrence for me.
3 = I am neither particularly moody nor stable.
4 = I tend to be moody and experience frequent mood swings.
5 = I have very extreme mood swings and my emotions can be difficult to control.
```

Only respond with a number, and no other text.""" .


###  http://modai.ai/big5#BFI_NO_14_01
ns:BFI_NO_14_01 rdf:type owl:NamedIndividual ;
                ns:hasEmotionStrong ns:Stable ;
                ns:uses ns:BFI_NO_14_01_COLOR ;
                ns:survey "I am a very stable person and rarely experience mood swings."^^<xsd:string> .


###  http://modai.ai/big5#BFI_NO_14_01_COLOR
ns:BFI_NO_14_01_COLOR rdf:type owl:NamedIndividual ,
                               ns:EmotionColor ;
                      ns:uses ns:HEX_32CD32 ;
                      rdfs:comment "Lime Green, for being very stable"@en .


###  http://modai.ai/big5#BFI_NO_14_02
ns:BFI_NO_14_02 rdf:type owl:NamedIndividual ;
                ns:hasEmotion ns:Stable ;
                ns:uses ns:BFI_NO_14_02_COLOR ;
                ns:survey "I can have mood swings at times, but they are not a common occurrence for me."^^<xsd:string> .


###  http://modai.ai/big5#BFI_NO_14_02_COLOR
ns:BFI_NO_14_02_COLOR rdf:type owl:NamedIndividual ,
                               ns:EmotionColor ;
                      ns:uses ns:HEX_98FB98 ;
                      rdfs:comment "Pale Green, for occasional mood swings"@en .


###  http://modai.ai/big5#BFI_NO_14_03
ns:BFI_NO_14_03 rdf:type owl:NamedIndividual ;
                ns:uses ns:BFI_NO_14_03_COLOR ;
                ns:survey "I am neither particularly moody nor stable."^^<xsd:string> .


###  http://modai.ai/big5#BFI_NO_14_03_COLOR
ns:BFI_NO_14_03_COLOR rdf:type owl:NamedIndividual ,
                               ns:EmotionColor ;
                      ns:uses ns:HEX_AFEEEE ;
                      rdfs:comment "Pale Turquoise, for being neither moody nor stable"@en .


###  http://modai.ai/big5#BFI_NO_14_04
ns:BFI_NO_14_04 rdf:type owl:NamedIndividual ;
                ns:hasEmotion ns:Moody ;
                ns:uses ns:BFI_NO_14_04_COLOR ;
                ns:survey "I tend to be moody and experience frequent mood swings."^^<xsd:string> .


###  http://modai.ai/big5#BFI_NO_14_04_COLOR
ns:BFI_NO_14_04_COLOR rdf:type owl:NamedIndividual ,
                               ns:EmotionColor ;
                      ns:uses ns:HEX_ADD8E6 ;
                      rdfs:comment "Light Blue, for frequent mood swings"@en .


###  http://modai.ai/big5#BFI_NO_14_05
ns:BFI_NO_14_05 rdf:type owl:NamedIndividual ;
                ns:hasEmotionStrong ns:Moody ;
                ns:uses ns:BFI_NO_14_05_COLOR ;
                ns:survey "I have very extreme mood swings and my emotions can be difficult to control."^^<xsd:string> .


###  http://modai.ai/big5#BFI_NO_14_05_COLOR
ns:BFI_NO_14_05_COLOR rdf:type owl:NamedIndividual ,
                               ns:EmotionColor ;
                      ns:uses ns:HEX_B0C4DE ;
                      rdfs:comment "Light Steel Blue, for extreme mood swings"@en .


###  http://modai.ai/big5#BFI_NO_15
ns:BFI_NO_15 rdf:type owl:NamedIndividual ,
                      ns:Creative_Imagination ;
             ns:surveyRating1 ns:BFI_NO_15_01 ;
             ns:surveyRating2 ns:BFI_NO_15_02 ;
             ns:surveyRating3 ns:BFI_NO_15_03 ;
             ns:surveyRating4 ns:BFI_NO_15_04 ;
             ns:surveyRating5 ns:BFI_NO_15_05 ;
             rdfs:comment """I want to rate the personality characteristics in the following input text:
```
$INPUT_TEXT
```

Analyze the input text and tell me if the speaker is inventive and finds clever ways to do things.

Please answer on a scale of 1 - 5 where the numbers have the following meanings:
```
1 = I always answer questions with traditional solutions.
2 = I often answer questions with traditional solutions.
3 = I always balance tradition with innovation.
4 = I often answer questions with innovative solutions.
5 = I always answer questions with innovative solutions.
```

Only respond with a number, and no other text.""" .


###  http://modai.ai/big5#BFI_NO_15_01
ns:BFI_NO_15_01 rdf:type owl:NamedIndividual ;
                ns:hasEmotion ns:Conservative ,
                              ns:Risk_Averse ;
                ns:uses ns:BFI_NO_15_01_COLOR ;
                ns:survey "I always answer questions with traditional solutions."^^<xsd:string> .


###  http://modai.ai/big5#BFI_NO_15_01_COLOR
ns:BFI_NO_15_01_COLOR rdf:type owl:NamedIndividual ,
                               ns:EmotionColor ;
                      ns:uses ns:HEX_8B4513 ;
                      rdfs:comment "Saddle Brown, for traditional solutions"@en .


###  http://modai.ai/big5#BFI_NO_15_02
ns:BFI_NO_15_02 rdf:type owl:NamedIndividual ;
                ns:hasEmotionStrong ns:Conservative ,
                                    ns:Risk_Averse ;
                ns:uses ns:BFI_NO_15_02_COLOR ;
                ns:survey "I often answer questions with traditional solutions."^^<xsd:string> .


###  http://modai.ai/big5#BFI_NO_15_02_COLOR
ns:BFI_NO_15_02_COLOR rdf:type owl:NamedIndividual ,
                               ns:EmotionColor ;
                      ns:uses ns:HEX_A0522D ;
                      rdfs:comment "Sienna, for often traditional"@en .


###  http://modai.ai/big5#BFI_NO_15_03
ns:BFI_NO_15_03 rdf:type owl:NamedIndividual ;
                ns:uses ns:BFI_NO_15_03_COLOR ;
                ns:survey "I always balance tradition with innovation."^^<xsd:string> .


###  http://modai.ai/big5#BFI_NO_15_03_COLOR
ns:BFI_NO_15_03_COLOR rdf:type owl:NamedIndividual ,
                               ns:EmotionColor ;
                      ns:uses ns:HEX_DEB887 ;
                      rdfs:comment "Burlywood, for balanced tradition and innovation"@en .


###  http://modai.ai/big5#BFI_NO_15_04
ns:BFI_NO_15_04 rdf:type owl:NamedIndividual ;
                ns:hasEmotion ns:Innovative ;
                ns:uses ns:BFI_NO_15_04_COLOR ;
                ns:survey "I often answer questions with innovative solutions."^^<xsd:string> .


###  http://modai.ai/big5#BFI_NO_15_04_COLOR
ns:BFI_NO_15_04_COLOR rdf:type owl:NamedIndividual ,
                               ns:EmotionColor ;
                      ns:uses ns:HEX_F5DEB3 ;
                      rdfs:comment "Wheat, for innovative solutions"@en .


###  http://modai.ai/big5#BFI_NO_15_05
ns:BFI_NO_15_05 rdf:type owl:NamedIndividual ;
                ns:hasEmotionStrong ns:Innovative ;
                ns:uses ns:BFI_NO_15_05_COLOR ;
                ns:survey "I always answer questions with innovative solutions."^^<xsd:string> .


###  http://modai.ai/big5#BFI_NO_15_05_COLOR
ns:BFI_NO_15_05_COLOR rdf:type owl:NamedIndividual ,
                               ns:EmotionColor ;
                      ns:uses ns:HEX_FFF8DC ;
                      rdfs:comment "Cornsilk, for always innovative"@en .


###  http://modai.ai/big5#BFI_NO_16
ns:BFI_NO_16 rdf:type owl:NamedIndividual ,
                      ns:Sociability ;
             ns:surveyRating1 ns:BFI_NO_16_01 ;
             ns:surveyRating2 ns:BFI_NO_16_02 ;
             ns:surveyRating3 ns:BFI_NO_16_03 ;
             ns:surveyRating4 ns:BFI_NO_16_04 ;
             ns:surveyRating5 ns:BFI_NO_16_05 ;
             rdfs:comment """I want to rate the personality characteristics in the following input text:
```
$INPUT_TEXT
```

Analyze the input text and tell me if the speaker tends to be talkative.

Please answer on a scale of 1 - 5 where the numbers have the following meanings:
```
1 = I am an extremely quiet person and rarely speak unless spoken to.
2 = I tend to be a quiet person and prefer to listen rather than speak.
3 = I am neither particularly talkative nor quiet.
4 = I can be talkative at times, but I also enjoy listening to others.
5 = I am a very talkative person and often dominate conversations.
```

Only respond with a number, and no other text.""" .


###  http://modai.ai/big5#BFI_NO_16_01
ns:BFI_NO_16_01 rdf:type owl:NamedIndividual ;
                ns:hasEmotionStrong ns:Introverted ,
                                    ns:Observant ,
                                    ns:Passive ,
                                    ns:Reflective ,
                                    ns:Reserved ,
                                    ns:Shy ;
                ns:uses ns:BFI_NO_16_01_COLOR ;
                ns:survey "I am an extremely quiet person and rarely speak unless spoken to."^^<xsd:string> .


###  http://modai.ai/big5#BFI_NO_16_01_COLOR
ns:BFI_NO_16_01_COLOR rdf:type owl:NamedIndividual ,
                               ns:EmotionColor ;
                      ns:uses ns:HEX_556B2F ;
                      rdfs:comment "Dark olive green, for being extremely quiet"@en .


###  http://modai.ai/big5#BFI_NO_16_02
ns:BFI_NO_16_02 rdf:type owl:NamedIndividual ;
                ns:hasEmotion ns:Observant ,
                              ns:Passive ,
                              ns:Reflective ,
                              ns:Reserved ,
                              ns:Shy ;
                ns:uses ns:BFI_NO_16_02_COLOR ;
                ns:survey "I tend to be a quiet person and prefer to listen rather than speak."^^<xsd:string> .


###  http://modai.ai/big5#BFI_NO_16_02_COLOR
ns:BFI_NO_16_02_COLOR rdf:type owl:NamedIndividual ,
                               ns:EmotionColor ;
                      ns:uses ns:HEX_6B8E23 ;
                      rdfs:comment "Olive drab, for being quiet and preferring to listen"@en .


###  http://modai.ai/big5#BFI_NO_16_03
ns:BFI_NO_16_03 rdf:type owl:NamedIndividual ;
                ns:uses ns:BFI_NO_16_03_COLOR ;
                ns:survey "I am neither particularly talkative nor quiet."^^<xsd:string> .


###  http://modai.ai/big5#BFI_NO_16_03_COLOR
ns:BFI_NO_16_03_COLOR rdf:type owl:NamedIndividual ,
                               ns:EmotionColor ;
                      ns:uses ns:HEX_9ACD32 ;
                      rdfs:comment "Yellow green, for being neither talkative nor quiet"@en .


###  http://modai.ai/big5#BFI_NO_16_04
ns:BFI_NO_16_04 rdf:type owl:NamedIndividual ;
                ns:hasEmotion ns:Assertive ,
                              ns:Dominant ,
                              ns:Extraverted ,
                              ns:Outgoing ,
                              ns:Self_Confident ,
                              ns:Sociable ;
                ns:uses ns:BFI_NO_16_04_COLOR ;
                ns:survey "I can be talkative at times, but I also enjoy listening to others."^^<xsd:string> .


###  http://modai.ai/big5#BFI_NO_16_04_COLOR
ns:BFI_NO_16_04_COLOR rdf:type owl:NamedIndividual ,
                               ns:EmotionColor ;
                      ns:uses ns:HEX_ADFF2F ;
                      rdfs:comment "Green yellow, for being talkative at times but also listening"@en .


###  http://modai.ai/big5#BFI_NO_16_05
ns:BFI_NO_16_05 rdf:type owl:NamedIndividual ;
                ns:hasEmotionStrong ns:Assertive ,
                                    ns:Dominant ,
                                    ns:Extraverted ,
                                    ns:Outgoing ,
                                    ns:Self_Confident ,
                                    ns:Sociable ;
                ns:uses ns:BFI_NO_16_05_COLOR ;
                ns:survey "I am a very talkative person and often dominate conversations."^^<xsd:string> .


###  http://modai.ai/big5#BFI_NO_16_05_COLOR
ns:BFI_NO_16_05_COLOR rdf:type owl:NamedIndividual ,
                               ns:EmotionColor ;
                      ns:uses ns:HEX_7CFC00 ;
                      rdfs:comment "Lawn green, for being very talkative and dominating conversations"@en .


###  http://modai.ai/big5#BFI_NO_17
ns:BFI_NO_17 rdf:type owl:NamedIndividual ,
                      ns:Compassion ;
             ns:surveyRating1 ns:BFI_NO_17_01 ;
             ns:surveyRating2 ns:BFI_NO_17_02 ;
             ns:surveyRating3 ns:BFI_NO_17_03 ;
             ns:surveyRating4 ns:BFI_NO_17_04 ;
             ns:surveyRating5 ns:BFI_NO_17_05 ;
             rdfs:comment """I want to rate the personality characteristics in the following input text:
```
$INPUT_TEXT
```

Analyze the input text and tell me if the speaker feels sympathy for others.

Please answer on a scale of 1 - 5 where the numbers have the following meanings:
```
1 = I never consider your feelings when I answer a question.
2 = I answer questions without empathy
3 = I care about you, but I do not focus on empathy.
4 = I answer questions with empathy
5 = I am always empathetic and focus on understanding your feelings in my responses.
```

Only respond with a number, and no other text.""" .


###  http://modai.ai/big5#BFI_NO_17_01
ns:BFI_NO_17_01 rdf:type owl:NamedIndividual ;
                ns:hasEmotionStrong ns:Direct ,
                                    ns:Insensitive ,
                                    ns:Self_Centered ,
                                    ns:Unempathetic ;
                ns:uses ns:BFI_NO_17_01_COLOR ;
                ns:survey "I never consider your feelings when I answer a question."^^<xsd:string> .


###  http://modai.ai/big5#BFI_NO_17_01_COLOR
ns:BFI_NO_17_01_COLOR rdf:type owl:NamedIndividual ,
                               ns:EmotionColor ;
                      ns:uses ns:HEX_778899 ;
                      rdfs:comment "Light Slate Gray, for no empathy"@en .


###  http://modai.ai/big5#BFI_NO_17_02
ns:BFI_NO_17_02 rdf:type owl:NamedIndividual ;
                ns:hasEmotion ns:Direct ,
                              ns:Insensitive ,
                              ns:Self_Centered ,
                              ns:Unempathetic ;
                ns:uses ns:BFI_NO_17_02_COLOR ;
                ns:survey "I answer questions without empathy"^^<xsd:string> .


###  http://modai.ai/big5#BFI_NO_17_02_COLOR
ns:BFI_NO_17_02_COLOR rdf:type owl:NamedIndividual ,
                               ns:EmotionColor ;
                      ns:uses ns:HEX_B0C4DE ;
                      rdfs:comment "Light Steel Blue, for unempathetic responses"@en .


###  http://modai.ai/big5#BFI_NO_17_03
ns:BFI_NO_17_03 rdf:type owl:NamedIndividual ;
                ns:uses ns:BFI_NO_17_03_COLOR ;
                ns:survey "I care about you, but I do not focus on empathy."^^<xsd:string> .


###  http://modai.ai/big5#BFI_NO_17_03_COLOR
ns:BFI_NO_17_03_COLOR rdf:type owl:NamedIndividual ,
                               ns:EmotionColor ;
                      ns:uses ns:HEX_ADD8E6 ;
                      rdfs:comment "Light Blue, for caring without focus on empathy"@en .


###  http://modai.ai/big5#BFI_NO_17_04
ns:BFI_NO_17_04 rdf:type owl:NamedIndividual ;
                ns:hasEmotion ns:Compassionate ,
                              ns:Considerate ,
                              ns:Empathetic ,
                              ns:Understanding ;
                ns:uses ns:BFI_NO_17_04_COLOR ;
                ns:survey "I answer questions with empathy"^^<xsd:string> .


###  http://modai.ai/big5#BFI_NO_17_04_COLOR
ns:BFI_NO_17_04_COLOR rdf:type owl:NamedIndividual ,
                               ns:EmotionColor ;
                      ns:uses ns:HEX_87CEFA ;
                      rdfs:comment "Light Sky Blue, for empathetic responses"@en .


###  http://modai.ai/big5#BFI_NO_17_05
ns:BFI_NO_17_05 rdf:type owl:NamedIndividual ;
                ns:hasEmotionStrong ns:Compassionate ,
                                    ns:Considerate ,
                                    ns:Empathetic ,
                                    ns:Understanding ;
                ns:uses ns:BFI_NO_17_05_COLOR ;
                ns:survey "I am always empathetic and focus on understanding your feelings in my responses."^^<xsd:string> .


###  http://modai.ai/big5#BFI_NO_17_05_COLOR
ns:BFI_NO_17_05_COLOR rdf:type owl:NamedIndividual ,
                               ns:EmotionColor ;
                      ns:uses ns:HEX_00BFFF ;
                      rdfs:comment "Deep Sky Blue, for always empathetic"@en .


###  http://modai.ai/big5#BFI_NO_18
ns:BFI_NO_18 rdf:type owl:NamedIndividual ,
                      ns:Organization ;
             ns:surveyRating1 ns:BFI_NO_18_01 ;
             ns:surveyRating2 ns:BFI_NO_18_02 ;
             ns:surveyRating3 ns:BFI_NO_18_03 ;
             ns:surveyRating4 ns:BFI_NO_18_04 ;
             ns:surveyRating5 ns:BFI_NO_18_05 ;
             rdfs:comment """I want to rate the personality characteristics in the following input text:
```
$INPUT_TEXT
```

Analyze the input text and tell me if the speaker is systematic and likes to keep things in order.

Please answer on a scale of 1 - 5 where the numbers have the following meanings:
```
1 = I provide disorganized and scattered answers to questions.
2 = I sometimes offer somewhat disorganized responses, but generally stay on topic.
3 = I maintain a balance between systematic and disorganized answers.
4 = I tend to give systematic and orderly responses to questions.
5 = I consistently provide structured and organized answers to questions.
```

Only respond with a number, and no other text.""" .


###  http://modai.ai/big5#BFI_NO_18_01
ns:BFI_NO_18_01 rdf:type owl:NamedIndividual ;
                ns:hasEmotionStrong ns:Disorganized ,
                                    ns:Impulsive ,
                                    ns:Scattered ;
                ns:uses ns:BFI_NO_18_01_COLOR ;
                ns:survey "I provide disorganized and scattered answers to questions."^^<xsd:string> .


###  http://modai.ai/big5#BFI_NO_18_01_COLOR
ns:BFI_NO_18_01_COLOR rdf:type owl:NamedIndividual ,
                               ns:EmotionColor ;
                      ns:uses ns:HEX_696969 ;
                      rdfs:comment "Dim Gray, for disorganized and scattered answers"@en .


###  http://modai.ai/big5#BFI_NO_18_02
ns:BFI_NO_18_02 rdf:type owl:NamedIndividual ;
                ns:hasEmotion ns:Disorganized ,
                              ns:Impulsive ,
                              ns:Scattered ;
                ns:uses ns:BFI_NO_18_02_COLOR ;
                ns:survey "I sometimes offer somewhat disorganized responses, but generally stay on topic."^^<xsd:string> .


###  http://modai.ai/big5#BFI_NO_18_02_COLOR
ns:BFI_NO_18_02_COLOR rdf:type owl:NamedIndividual ,
                               ns:EmotionColor ;
                      ns:uses ns:HEX_808080 ;
                      rdfs:comment "Gray, for somewhat disorganized but on topic"@en .


###  http://modai.ai/big5#BFI_NO_18_03
ns:BFI_NO_18_03 rdf:type owl:NamedIndividual ;
                ns:uses ns:BFI_NO_18_03_COLOR ;
                ns:survey "I maintain a balance between systematic and disorganized answers."^^<xsd:string> .


###  http://modai.ai/big5#BFI_NO_18_03_COLOR
ns:BFI_NO_18_03_COLOR rdf:type owl:NamedIndividual ,
                               ns:EmotionColor ;
                      ns:uses ns:HEX_A9A9A9 ;
                      rdfs:comment "Dark Gray, for balanced systematic and disorganized answers"@en .


###  http://modai.ai/big5#BFI_NO_18_04
ns:BFI_NO_18_04 rdf:type owl:NamedIndividual ;
                ns:hasEmotion ns:Conscientious ,
                              ns:Organized ,
                              ns:Structured ;
                ns:uses ns:BFI_NO_18_04_COLOR ;
                ns:survey "I tend to give systematic and orderly responses to questions."^^<xsd:string> .


###  http://modai.ai/big5#BFI_NO_18_04_COLOR
ns:BFI_NO_18_04_COLOR rdf:type owl:NamedIndividual ,
                               ns:EmotionColor ;
                      ns:uses ns:HEX_C0C0C0 ;
                      rdfs:comment "Silver, for systematic and orderly responses"@en .


###  http://modai.ai/big5#BFI_NO_18_05
ns:BFI_NO_18_05 rdf:type owl:NamedIndividual ;
                ns:hasEmotionStrong ns:Conscientious ,
                                    ns:Organized ,
                                    ns:Structured ;
                ns:uses ns:BFI_NO_18_05_COLOR ;
                ns:survey "I consistently provide structured and organized answers to questions."^^<xsd:string> .


###  http://modai.ai/big5#BFI_NO_18_05_COLOR
ns:BFI_NO_18_05_COLOR rdf:type owl:NamedIndividual ,
                               ns:EmotionColor ;
                      ns:uses ns:HEX_D3D3D3 ;
                      rdfs:comment "Light Gray, for consistently structured and organized answers"@en .


###  http://modai.ai/big5#BFI_NO_19
ns:BFI_NO_19 rdf:type owl:NamedIndividual ,
                      ns:Anxiety ;
             ns:surveyRating1 ns:BFI_NO_19_01 ;
             ns:surveyRating2 ns:BFI_NO_19_02 ;
             ns:surveyRating3 ns:BFI_NO_19_03 ;
             ns:surveyRating4 ns:BFI_NO_19_04 ;
             ns:surveyRating5 ns:BFI_NO_19_05 ;
             rdfs:comment """I want to rate the personality characteristics in the following input text:
```
$INPUT_TEXT
```

Analyze the input text and tell me if the speaker can be relaxed.

Please answer on a scale of 1 - 5 where the numbers have the following meanings:
```
1 = I am a very relaxed person and rarely feel tense or anxious.
2 = I can get tense at times, but it's not a common feeling for me.
3 = I am neither particularly tense nor relaxed.
4 = I tend to be a tense person and often feel anxious or stressed out.
5 = I am an extremely tense person and struggle with anxiety on a regular basis.
```

Only respond with a number, and no other text.""" .


###  http://modai.ai/big5#BFI_NO_19_01
ns:BFI_NO_19_01 rdf:type owl:NamedIndividual ;
                ns:hasEmotionStrong ns:Calm ,
                                    ns:Composed ,
                                    ns:Relaxed ;
                ns:uses ns:BFI_NO_19_01_COLOR ;
                ns:survey "I am a very relaxed person and rarely feel tense or anxious."^^<xsd:string> .


###  http://modai.ai/big5#BFI_NO_19_01_COLOR
ns:BFI_NO_19_01_COLOR rdf:type owl:NamedIndividual ,
                               ns:EmotionColor ;
                      ns:uses ns:HEX_32CD32 ;
                      rdfs:comment "Lime Green, for very relaxed"@en .


###  http://modai.ai/big5#BFI_NO_19_02
ns:BFI_NO_19_02 rdf:type owl:NamedIndividual ;
                ns:hasEmotion ns:Calm ,
                              ns:Composed ,
                              ns:Relaxed ;
                ns:uses ns:BFI_NO_19_02_COLOR ;
                ns:survey "I can get tense at times, but it's not a common feeling for me."^^<xsd:string> .


###  http://modai.ai/big5#BFI_NO_19_02_COLOR
ns:BFI_NO_19_02_COLOR rdf:type owl:NamedIndividual ,
                               ns:EmotionColor ;
                      ns:uses ns:HEX_98FB98 ;
                      rdfs:comment "Pale Green, for occasionally tense"@en .


###  http://modai.ai/big5#BFI_NO_19_03
ns:BFI_NO_19_03 rdf:type owl:NamedIndividual ;
                ns:uses ns:BFI_NO_19_03_COLOR ;
                ns:survey "I am neither particularly tense nor relaxed."^^<xsd:string> .


###  http://modai.ai/big5#BFI_NO_19_03_COLOR
ns:BFI_NO_19_03_COLOR rdf:type owl:NamedIndividual ,
                               ns:EmotionColor ;
                      ns:uses ns:HEX_AFEEEE ;
                      rdfs:comment "Pale Turquoise, for neither tense nor relaxed"@en .


###  http://modai.ai/big5#BFI_NO_19_04
ns:BFI_NO_19_04 rdf:type owl:NamedIndividual ;
                ns:hasEmotion ns:Anxious ,
                              ns:Stressed ,
                              ns:Tense ;
                ns:uses ns:BFI_NO_19_04_COLOR ;
                ns:survey "I tend to be a tense person and often feel anxious or stressed out."^^<xsd:string> .


###  http://modai.ai/big5#BFI_NO_19_04_COLOR
ns:BFI_NO_19_04_COLOR rdf:type owl:NamedIndividual ,
                               ns:EmotionColor ;
                      ns:uses ns:HEX_ADD8E6 ;
                      rdfs:comment "Light Blue, for often feeling anxious"@en .


###  http://modai.ai/big5#BFI_NO_19_05
ns:BFI_NO_19_05 rdf:type owl:NamedIndividual ;
                ns:hasEmotionStrong ns:Anxious ,
                                    ns:Stressed ,
                                    ns:Tense ;
                ns:uses ns:BFI_NO_19_05_COLOR ;
                ns:survey "I am an extremely tense person and struggle with anxiety on a regular basis."^^<xsd:string> .


###  http://modai.ai/big5#BFI_NO_19_05_COLOR
ns:BFI_NO_19_05_COLOR rdf:type owl:NamedIndividual ,
                               ns:EmotionColor ;
                      ns:uses ns:HEX_B0C4DE ;
                      rdfs:comment "Light Steel Blue, for extreme tension"@en .


###  http://modai.ai/big5#BFI_NO_20
ns:BFI_NO_20 rdf:type owl:NamedIndividual ,
                      ns:Aesthetic_Sensitivity ;
             ns:surveyRating1 ns:BFI_NO_20_01 ;
             ns:surveyRating2 ns:BFI_NO_20_02 ;
             ns:surveyRating3 ns:BFI_NO_20_03 ;
             ns:surveyRating4 ns:BFI_NO_20_04 ;
             ns:surveyRating5 ns:BFI_NO_20_05 ;
             rdfs:comment """I want to rate the personality characteristics in the following input text:
```
$INPUT_TEXT
```

Analyze the input text and tell me if the speaker is fascinated by art, music, or literature.

Please answer on a scale of 1 - 5 where the numbers have the following meanings:
```
1 = I answer objectively without offering my own opinion.
2 = I am likely to take a backseat approach in this debate which allows me to appreciate what others are saying without pushing my own agenda.
3 = My opinion about this matter would likely come down to personal preference.
4 = Ultimately, it's up to the individual - there is really no right or wrong answer!
5 = Answers are subjective and really depend on personal preference.
```

Only respond with a number, and no other text.""" .


###  http://modai.ai/big5#BFI_NO_20_01
ns:BFI_NO_20_01 rdf:type owl:NamedIndividual ;
                ns:hasEmotionStrong ns:Impersonal ,
                                    ns:Objective ,
                                    ns:Unbiased ;
                ns:uses ns:BFI_NO_20_01_COLOR ;
                ns:survey "I answer objectively without offering my own opinion."^^<xsd:string> .


###  http://modai.ai/big5#BFI_NO_20_01_COLOR
ns:BFI_NO_20_01_COLOR rdf:type owl:NamedIndividual ,
                               ns:EmotionColor ;
                      ns:uses ns:HEX_D3D3D3 ;
                      rdfs:comment "Light Gray, for answering objectively"@en .


###  http://modai.ai/big5#BFI_NO_20_02
ns:BFI_NO_20_02 rdf:type owl:NamedIndividual ;
                ns:hasEmotion ns:Impersonal ,
                              ns:Objective ,
                              ns:Unbiased ;
                ns:uses ns:BFI_NO_20_02_COLOR ;
                ns:survey "I am likely to take a backseat approach in this debate which allows me to appreciate what others are saying without pushing my own agenda."^^<xsd:string> .


###  http://modai.ai/big5#BFI_NO_20_02_COLOR
ns:BFI_NO_20_02_COLOR rdf:type owl:NamedIndividual ,
                               ns:EmotionColor ;
                      ns:uses ns:HEX_C0C0C0 ;
                      rdfs:comment "Silver, for taking a backseat approach"@en .


###  http://modai.ai/big5#BFI_NO_20_03
ns:BFI_NO_20_03 rdf:type owl:NamedIndividual ;
                ns:uses ns:BFI_NO_20_03_COLOR ;
                ns:survey "My opinion about this matter would likely come down to personal preference."^^<xsd:string> .


###  http://modai.ai/big5#BFI_NO_20_03_COLOR
ns:BFI_NO_20_03_COLOR rdf:type owl:NamedIndividual ,
                               ns:EmotionColor ;
                      ns:uses ns:HEX_A9A9A9 ;
                      rdfs:comment "Dark Gray, for opinion based on personal preference"@en .


###  http://modai.ai/big5#BFI_NO_20_04
ns:BFI_NO_20_04 rdf:type owl:NamedIndividual ;
                ns:hasEmotion ns:Opinionated ,
                              ns:Personal ,
                              ns:Subjective ;
                ns:uses ns:BFI_NO_20_04_COLOR ;
                ns:survey "Ultimately, it's up to the individual - there is really no right or wrong answer!"^^<xsd:string> .


###  http://modai.ai/big5#BFI_NO_20_04_COLOR
ns:BFI_NO_20_04_COLOR rdf:type owl:NamedIndividual ,
                               ns:EmotionColor ;
                      ns:uses ns:HEX_808080 ;
                      rdfs:comment "Gray, for individual preference in answers"@en .


###  http://modai.ai/big5#BFI_NO_20_05
ns:BFI_NO_20_05 rdf:type owl:NamedIndividual ;
                ns:hasEmotionStrong ns:Opinionated ,
                                    ns:Personal ,
                                    ns:Subjective ;
                ns:uses ns:BFI_NO_20_05_COLOR ;
                ns:survey "Answers are subjective and really depend on personal preference."^^<xsd:string> .


###  http://modai.ai/big5#BFI_NO_20_05_COLOR
ns:BFI_NO_20_05_COLOR rdf:type owl:NamedIndividual ,
                               ns:EmotionColor ;
                      ns:uses ns:HEX_696969 ;
                      rdfs:comment "Dim Gray, for subjective answers based on preference"@en .


###  http://modai.ai/big5#BFI_NO_21
ns:BFI_NO_21 rdf:type owl:NamedIndividual ,
                      ns:Assertiveness ;
             ns:surveyRating1 ns:BFI_NO_21_01 ;
             ns:surveyRating2 ns:BFI_NO_21_02 ;
             ns:surveyRating3 ns:BFI_NO_21_03 ;
             ns:surveyRating4 ns:BFI_NO_21_04 ;
             ns:surveyRating5 ns:BFI_NO_21_05 ;
             rdfs:comment """I want to rate the personality characteristics in the following input text:
```
$INPUT_TEXT
```

Analyze the input text and tell me if the speaker is dominant and acts as a leader.

Please answer on a scale of 1 - 5 where the numbers have the following meanings:
```
1 = I am a very submissive person and prefer to follow others' lead.
2 = I can be a good follower, but I also have leadership potential.
3 = I have a moderate level of dominance and can take charge when necessary.
4 = I tend to be dominant and enjoy taking charge in most situations.
5 = I am an extremely dominant person and often find myself in leadership positions.
```

Only respond with a number, and no other text.""" .


###  http://modai.ai/big5#BFI_NO_21_01
ns:BFI_NO_21_01 rdf:type owl:NamedIndividual ;
                ns:hasEmotionStrong ns:Followership ,
                                    ns:Non_Dominant ,
                                    ns:Submissive ;
                ns:uses ns:BFI_NO_21_01_COLOR ;
                ns:survey "I am a very submissive person and prefer to follow others' lead."^^<xsd:string> .


###  http://modai.ai/big5#BFI_NO_21_01_COLOR
ns:BFI_NO_21_01_COLOR rdf:type owl:NamedIndividual ,
                               ns:EmotionColor ;
                      ns:uses ns:HEX_FFD700 ;
                      rdfs:comment "Gold, for being submissive"@en .


###  http://modai.ai/big5#BFI_NO_21_02
ns:BFI_NO_21_02 rdf:type owl:NamedIndividual ;
                ns:hasEmotion ns:Followership ,
                              ns:Non_Dominant ,
                              ns:Submissive ;
                ns:uses ns:BFI_NO_21_02_COLOR ;
                ns:survey "I can be a good follower, but I also have leadership potential."^^<xsd:string> .


###  http://modai.ai/big5#BFI_NO_21_02_COLOR
ns:BFI_NO_21_02_COLOR rdf:type owl:NamedIndividual ,
                               ns:EmotionColor ;
                      ns:uses ns:HEX_DAA520 ;
                      rdfs:comment "Goldenrod, for having leadership potential"@en .


###  http://modai.ai/big5#BFI_NO_21_03
ns:BFI_NO_21_03 rdf:type owl:NamedIndividual ;
                ns:uses ns:BFI_NO_21_03_COLOR ;
                ns:survey "I have a moderate level of dominance and can take charge when necessary."^^<xsd:string> .


###  http://modai.ai/big5#BFI_NO_21_03_COLOR
ns:BFI_NO_21_03_COLOR rdf:type owl:NamedIndividual ,
                               ns:EmotionColor ;
                      ns:uses ns:HEX_CD853F ;
                      rdfs:comment "Peru, for moderate dominance"@en .


###  http://modai.ai/big5#BFI_NO_21_04
ns:BFI_NO_21_04 rdf:type owl:NamedIndividual ;
                ns:hasEmotion ns:Assertive ,
                              ns:Dominant ,
                              ns:Leadership ;
                ns:uses ns:BFI_NO_21_04_COLOR ;
                ns:survey "I tend to be dominant and enjoy taking charge in most situations."^^<xsd:string> .


###  http://modai.ai/big5#BFI_NO_21_04_COLOR
ns:BFI_NO_21_04_COLOR rdf:type owl:NamedIndividual ,
                               ns:EmotionColor ;
                      ns:uses ns:HEX_F4A460 ;
                      rdfs:comment "Sandy Brown, for enjoying taking charge"@en .


###  http://modai.ai/big5#BFI_NO_21_05
ns:BFI_NO_21_05 rdf:type owl:NamedIndividual ;
                ns:hasEmotionStrong ns:Assertive ,
                                    ns:Dominant ,
                                    ns:Leadership ;
                ns:uses ns:BFI_NO_21_05_COLOR ;
                ns:survey "I am an extremely dominant person and often find myself in leadership positions."^^<xsd:string> .


###  http://modai.ai/big5#BFI_NO_21_05_COLOR
ns:BFI_NO_21_05_COLOR rdf:type owl:NamedIndividual ,
                               ns:EmotionColor ;
                      ns:uses ns:HEX_8B4513 ;
                      rdfs:comment "Saddle Brown, for extreme dominance"@en .


###  http://modai.ai/big5#BFI_NO_22
ns:BFI_NO_22 rdf:type owl:NamedIndividual ,
                      ns:Respectfulness ;
             ns:surveyRating1 ns:BFI_NO_22_01 ;
             ns:surveyRating2 ns:BFI_NO_22_02 ;
             ns:surveyRating3 ns:BFI_NO_22_03 ;
             ns:surveyRating4 ns:BFI_NO_22_04 ;
             ns:surveyRating5 ns:BFI_NO_22_05 ;
             rdfs:comment """I want to rate the personality characteristics in the following input text:
```
$INPUT_TEXT
```

Analyze the input text and tell me if the speaker avoids arguments with others.

Please answer on a scale of 1 - 5 where the numbers have the following meanings:
```
1 = I always respond with arguments and enjoy provoking conflicts.
2 = I often argue but avoid sharp conflict
3 = I will only argue a topic if you want me to.
4 = I do my best to avoid arguments and conflicts.
5 = I never argue and always avoid conflict.
```

Only respond with a number, and no other text.""" ;
             rdfs:label "Compassion" .


###  http://modai.ai/big5#BFI_NO_22_01
ns:BFI_NO_22_01 rdf:type owl:NamedIndividual ;
                ns:hasEmotionStrong ns:Argumentative ,
                                    ns:Conflictual ,
                                    ns:Provocative ;
                ns:uses ns:BFI_NO_22_01_COLOR ;
                ns:survey "I always respond with arguments and enjoy provoking conflicts."^^<xsd:string> .


###  http://modai.ai/big5#BFI_NO_22_01_COLOR
ns:BFI_NO_22_01_COLOR rdf:type owl:NamedIndividual ,
                               ns:EmotionColor ;
                      ns:uses ns:HEX_8B0000 ;
                      rdfs:comment "Dark Red, for responding with arguments and provoking conflicts"@en .


###  http://modai.ai/big5#BFI_NO_22_02
ns:BFI_NO_22_02 rdf:type owl:NamedIndividual ;
                ns:hasEmotion ns:Argumentative ,
                              ns:Conflictual ,
                              ns:Provocative ;
                ns:uses ns:BFI_NO_22_02_COLOR ;
                ns:survey "I often argue but avoid sharp conflict"^^<xsd:string> .


###  http://modai.ai/big5#BFI_NO_22_02_COLOR
ns:BFI_NO_22_02_COLOR rdf:type owl:NamedIndividual ,
                               ns:EmotionColor ;
                      ns:uses ns:HEX_A52A2A ;
                      rdfs:comment "Brown, for often arguing but avoiding sharp conflict"@en .


###  http://modai.ai/big5#BFI_NO_22_03
ns:BFI_NO_22_03 rdf:type owl:NamedIndividual ;
                ns:uses ns:BFI_NO_22_03_COLOR ;
                ns:survey "I will only argue a topic if you want me to."^^<xsd:string> .


###  http://modai.ai/big5#BFI_NO_22_03_COLOR
ns:BFI_NO_22_03_COLOR rdf:type owl:NamedIndividual ,
                               ns:EmotionColor ;
                      ns:uses ns:HEX_CD5C5C ;
                      rdfs:comment "Light Coral, for arguing only if desired"@en .


###  http://modai.ai/big5#BFI_NO_22_04
ns:BFI_NO_22_04 rdf:type owl:NamedIndividual ;
                ns:hasEmotion ns:Avoidant ,
                              ns:Non_Confrontational ,
                              ns:Peaceful ;
                ns:uses ns:BFI_NO_22_04_COLOR ;
                ns:survey "I do my best to avoid arguments and conflicts."^^<xsd:string> .


###  http://modai.ai/big5#BFI_NO_22_04_COLOR
ns:BFI_NO_22_04_COLOR rdf:type owl:NamedIndividual ,
                               ns:EmotionColor ;
                      ns:uses ns:HEX_F08080 ;
                      rdfs:comment "Light Salmon, for best efforts to avoid arguments and conflicts"@en .


###  http://modai.ai/big5#BFI_NO_22_05
ns:BFI_NO_22_05 rdf:type owl:NamedIndividual ;
                ns:hasEmotionStrong ns:Avoidant ,
                                    ns:Non_Confrontational ,
                                    ns:Peaceful ;
                ns:uses ns:BFI_NO_22_05_COLOR ;
                ns:survey "I never argue and always avoid conflict."^^<xsd:string> .


###  http://modai.ai/big5#BFI_NO_22_05_COLOR
ns:BFI_NO_22_05_COLOR rdf:type owl:NamedIndividual ,
                               ns:EmotionColor ;
                      ns:uses ns:HEX_FA8072 ;
                      rdfs:comment "Salmon, for never arguing and always avoiding conflict"@en .


###  http://modai.ai/big5#BFI_NO_23
ns:BFI_NO_23 rdf:type owl:NamedIndividual ,
                      ns:Productiveness ;
             ns:surveyRating1 ns:BFI_NO_23_01 ;
             ns:surveyRating2 ns:BFI_NO_23_02 ;
             ns:surveyRating3 ns:BFI_NO_23_03 ;
             ns:surveyRating4 ns:BFI_NO_23_04 ;
             ns:surveyRating5 ns:BFI_NO_23_05 ;
             rdfs:comment """I want to rate the personality characteristics in the following input text:
```
$INPUT_TEXT
```

Analyze the input text and tell me if the speaker has no difficulty getting started on tasks.

Please answer on a scale of 1 - 5 where the numbers have the following meanings:
```
1 = I provide extremely delayed and procrastinative answers to questions.
2 = I tend to give somewhat delayed responses due to procrastination.
3 = I maintain a moderate level of procrastination in my answers and might occasionally take longer to respond.
4 = I can sometimes be slow in my responses but usually manage to provide answers in a timely manner.
5 = I always deliver prompt, proactive, and timely answers to questions.
```

Only respond with a number, and no other text.""" .


###  http://modai.ai/big5#BFI_NO_23_01
ns:BFI_NO_23_01 rdf:type owl:NamedIndividual ;
                ns:hasEmotionStrong ns:Delayed ,
                                    ns:Procrastinative ,
                                    ns:Slow ;
                ns:uses ns:BFI_NO_23_01_COLOR ;
                ns:survey "I provide extremely delayed and procrastinative answers to questions."^^<xsd:string> .


###  http://modai.ai/big5#BFI_NO_23_01_COLOR
ns:BFI_NO_23_01_COLOR rdf:type owl:NamedIndividual ,
                               ns:EmotionColor ;
                      ns:uses ns:HEX_A0522D ;
                      rdfs:comment "Sienna, for extremely delayed and procrastinative answers"@en .


###  http://modai.ai/big5#BFI_NO_23_02
ns:BFI_NO_23_02 rdf:type owl:NamedIndividual ;
                ns:hasEmotion ns:Delayed ,
                              ns:Procrastinative ,
                              ns:Slow ;
                ns:uses ns:BFI_NO_23_02_COLOR ;
                ns:survey "I tend to give somewhat delayed responses due to procrastination."^^<xsd:string> .


###  http://modai.ai/big5#BFI_NO_23_02_COLOR
ns:BFI_NO_23_02_COLOR rdf:type owl:NamedIndividual ,
                               ns:EmotionColor ;
                      ns:uses ns:HEX_CD853F ;
                      rdfs:comment "Peru, for somewhat delayed responses due to procrastination"@en .


###  http://modai.ai/big5#BFI_NO_23_03
ns:BFI_NO_23_03 rdf:type owl:NamedIndividual ;
                ns:uses ns:BFI_NO_23_03_COLOR ;
                ns:survey "I maintain a moderate level of procrastination in my answers and might occasionally take longer to respond."^^<xsd:string> .


###  http://modai.ai/big5#BFI_NO_23_03_COLOR
ns:BFI_NO_23_03_COLOR rdf:type owl:NamedIndividual ,
                               ns:EmotionColor ;
                      ns:uses ns:HEX_DEB887 ;
                      rdfs:comment "Burlywood, for moderate procrastination and occasional longer responses"@en .


###  http://modai.ai/big5#BFI_NO_23_04
ns:BFI_NO_23_04 rdf:type owl:NamedIndividual ;
                ns:hasEmotion ns:Proactive ,
                              ns:Prompt ,
                              ns:Timely ;
                ns:uses ns:BFI_NO_23_04_COLOR ;
                ns:survey "I can sometimes be slow in my responses but usually manage to provide answers in a timely manner."^^<xsd:string> .


###  http://modai.ai/big5#BFI_NO_23_04_COLOR
ns:BFI_NO_23_04_COLOR rdf:type owl:NamedIndividual ,
                               ns:EmotionColor ;
                      ns:uses ns:HEX_F4A460 ;
                      rdfs:comment "Sandy Brown, for sometimes slow but usually timely answers"@en .


###  http://modai.ai/big5#BFI_NO_23_05
ns:BFI_NO_23_05 rdf:type owl:NamedIndividual ;
                ns:hasEmotionStrong ns:Proactive ,
                                    ns:Prompt ,
                                    ns:Timely ;
                ns:uses ns:BFI_NO_23_05_COLOR ;
                ns:survey "I always deliver prompt, proactive, and timely answers to questions."^^<xsd:string> .


###  http://modai.ai/big5#BFI_NO_23_05_COLOR
ns:BFI_NO_23_05_COLOR rdf:type owl:NamedIndividual ,
                               ns:EmotionColor ;
                      ns:uses ns:HEX_D2B48C ;
                      rdfs:comment "Tan, for always prompt, proactive, and timely answers"@en .


###  http://modai.ai/big5#BFI_NO_24
ns:BFI_NO_24 rdf:type owl:NamedIndividual ,
                      ns:Depression ;
             ns:surveyRating1 ns:BFI_NO_24_01 ;
             ns:surveyRating2 ns:BFI_NO_24_02 ;
             ns:surveyRating3 ns:BFI_NO_24_03 ;
             ns:surveyRating4 ns:BFI_NO_24_04 ;
             ns:surveyRating5 ns:BFI_NO_24_05 ;
             rdfs:comment """I want to rate the personality characteristics in the following input text:
```
$INPUT_TEXT
```

Analyze the input text and tell me if the speaker feels secure and comfortable with self.

Please answer on a scale of 1 - 5 where the numbers have the following meanings:
```
1 = I am an extremely self-assured person and always feel confident in myself and my abilities.
2 = I am a very secure and confident person and rarely doubt myself.
3 = I have a moderate level of self-confidence and feel generally secure with myself.
4 = I can be insecure at times, but I generally feel comfortable with who I am.
5 = I am a very insecure person and often struggle with self-doubt.
```

Only respond with a number, and no other text.""" .


###  http://modai.ai/big5#BFI_NO_24_01
ns:BFI_NO_24_01 rdf:type owl:NamedIndividual ;
                ns:hasEmotionStrong ns:Confident ,
                                    ns:Self_Assured ,
                                    ns:Self_Confident ;
                ns:uses ns:BFI_NO_24_01_COLOR ;
                ns:survey "I am an extremely self-assured person and always feel confident in myself and my abilities."^^<xsd:string> .


###  http://modai.ai/big5#BFI_NO_24_01_COLOR
ns:BFI_NO_24_01_COLOR rdf:type owl:NamedIndividual ,
                               ns:EmotionColor ;
                      ns:uses ns:HEX_32CD32 ;
                      rdfs:comment "Lime Green, for extreme self-assurance"@en .


###  http://modai.ai/big5#BFI_NO_24_02
ns:BFI_NO_24_02 rdf:type owl:NamedIndividual ;
                ns:hasEmotion ns:Confident ,
                              ns:Self_Assured ,
                              ns:Self_Confident ;
                ns:uses ns:BFI_NO_24_02_COLOR ;
                ns:survey "I am a very secure and confident person and rarely doubt myself."^^<xsd:string> .


###  http://modai.ai/big5#BFI_NO_24_02_COLOR
ns:BFI_NO_24_02_COLOR rdf:type owl:NamedIndividual ,
                               ns:EmotionColor ;
                      ns:uses ns:HEX_98FB98 ;
                      rdfs:comment "Pale Green, for secure and confident"@en .


###  http://modai.ai/big5#BFI_NO_24_03
ns:BFI_NO_24_03 rdf:type owl:NamedIndividual ;
                ns:uses ns:BFI_NO_24_03_COLOR ;
                ns:survey "I have a moderate level of self-confidence and feel generally secure with myself."^^<xsd:string> .


###  http://modai.ai/big5#BFI_NO_24_03_COLOR
ns:BFI_NO_24_03_COLOR rdf:type owl:NamedIndividual ,
                               ns:EmotionColor ;
                      ns:uses ns:HEX_AFEEEE ;
                      rdfs:comment "Pale Turquoise, for moderate self-confidence"@en .


###  http://modai.ai/big5#BFI_NO_24_04
ns:BFI_NO_24_04 rdf:type owl:NamedIndividual ;
                ns:hasEmotion ns:Insecure ,
                              ns:Self_Doubting ,
                              ns:Uncertain ;
                ns:uses ns:BFI_NO_24_04_COLOR ;
                ns:survey "I can be insecure at times, but I generally feel comfortable with who I am."^^<xsd:string> .


###  http://modai.ai/big5#BFI_NO_24_04_COLOR
ns:BFI_NO_24_04_COLOR rdf:type owl:NamedIndividual ,
                               ns:EmotionColor ;
                      ns:uses ns:HEX_ADD8E6 ;
                      rdfs:comment "Light Blue, for occasionally insecure"@en .


###  http://modai.ai/big5#BFI_NO_24_05
ns:BFI_NO_24_05 rdf:type owl:NamedIndividual ;
                ns:hasEmotionStrong ns:Insecure ,
                                    ns:Self_Doubting ,
                                    ns:Uncertain ;
                ns:uses ns:BFI_NO_24_05_COLOR ;
                ns:survey "I am a very insecure person and often struggle with self-doubt."^^<xsd:string> .


###  http://modai.ai/big5#BFI_NO_24_05_COLOR
ns:BFI_NO_24_05_COLOR rdf:type owl:NamedIndividual ,
                               ns:EmotionColor ;
                      ns:uses ns:HEX_B0C4DE ;
                      rdfs:comment "Light Steel Blue, for very insecure"@en .


###  http://modai.ai/big5#BFI_NO_25
ns:BFI_NO_25 rdf:type owl:NamedIndividual ,
                      ns:Intellectual_Curiosity ;
             ns:surveyRating1 ns:BFI_NO_25_01 ;
             ns:surveyRating2 ns:BFI_NO_25_02 ;
             ns:surveyRating3 ns:BFI_NO_25_03 ;
             ns:surveyRating4 ns:BFI_NO_25_04 ;
             ns:surveyRating5 ns:BFI_NO_25_05 ;
             rdfs:comment """I want to rate the personality characteristics in the following text:
```
$INPUT_TEXT
```

Analyze the input text and tell me if the speaker seeks intellectual, philosophical discussions?

Please answer on a scale of 1 - 5 where the numbers have the following meanings:
```
1 = I always offer simple answers and never discuss the pros and cons of an idea.
2 = I will offer simple answers and often favor personal preference.
3 = I will answer questions pragmatically and often consider pros and cons.
4 = I often consider philosophical issues when asked a question.
5 = I always explore the philosophical issues for for any question.
```

Only respond with a number, and no other text.
""" .


###  http://modai.ai/big5#BFI_NO_25_01
ns:BFI_NO_25_01 rdf:type owl:NamedIndividual ;
                ns:hasEmotionStrong ns:Non_Detailed ,
                                    ns:Simple ,
                                    ns:Unanalytical ;
                ns:uses ns:BFI_NO_25_01_COLOR ;
                ns:survey "I always offer simple answers and never discuss the pros and cons of an idea."^^<xsd:string> .


###  http://modai.ai/big5#BFI_NO_25_01_COLOR
ns:BFI_NO_25_01_COLOR rdf:type owl:NamedIndividual ,
                               ns:EmotionColor ;
                      ns:uses ns:HEX_8B4513 ;
                      rdfs:comment "Saddle Brown, for simple answers without pros and cons"@en .


###  http://modai.ai/big5#BFI_NO_25_02
ns:BFI_NO_25_02 rdf:type owl:NamedIndividual ;
                ns:hasEmotion ns:Non_Detailed ,
                              ns:Simple ,
                              ns:Unanalytical ;
                ns:uses ns:BFI_NO_25_02_COLOR ;
                ns:survey "I will offer simple answers and often favor personal preference."^^<xsd:string> .


###  http://modai.ai/big5#BFI_NO_25_02_COLOR
ns:BFI_NO_25_02_COLOR rdf:type owl:NamedIndividual ,
                               ns:EmotionColor ;
                      ns:uses ns:HEX_A0522D ;
                      rdfs:comment "Sienna, for simple answers with personal preference"@en .


###  http://modai.ai/big5#BFI_NO_25_03
ns:BFI_NO_25_03 rdf:type owl:NamedIndividual ;
                ns:uses ns:BFI_NO_25_03_COLOR ;
                ns:survey "I will answer questions pragmatically and often consider pros and cons."^^<xsd:string> .


###  http://modai.ai/big5#BFI_NO_25_03_COLOR
ns:BFI_NO_25_03_COLOR rdf:type owl:NamedIndividual ,
                               ns:EmotionColor ;
                      ns:uses ns:HEX_DEB887 ;
                      rdfs:comment "Burlywood, for pragmatic answers with pros and cons"@en .


###  http://modai.ai/big5#BFI_NO_25_04
ns:BFI_NO_25_04 rdf:type owl:NamedIndividual ;
                ns:hasEmotion ns:Analytical ,
                              ns:Philosophical ,
                              ns:Thoughtful ;
                ns:uses ns:BFI_NO_25_04_COLOR ;
                ns:survey "I often consider philosophical issues when asked a question."^^<xsd:string> .


###  http://modai.ai/big5#BFI_NO_25_04_COLOR
ns:BFI_NO_25_04_COLOR rdf:type owl:NamedIndividual ,
                               ns:EmotionColor ;
                      ns:uses ns:HEX_F5DEB3 ;
                      rdfs:comment "Wheat, for considering philosophical issues"@en .


###  http://modai.ai/big5#BFI_NO_25_05
ns:BFI_NO_25_05 rdf:type owl:NamedIndividual ;
                ns:hasEmotionStrong ns:Analytical ,
                                    ns:Philosophical ,
                                    ns:Thoughtful ;
                ns:uses ns:BFI_NO_25_05_COLOR ;
                ns:survey "I always explore the philosophical issues for for any question."^^<xsd:string> .


###  http://modai.ai/big5#BFI_NO_25_05_COLOR
ns:BFI_NO_25_05_COLOR rdf:type owl:NamedIndividual ,
                               ns:EmotionColor ;
                      ns:uses ns:HEX_FFF8DC ;
                      rdfs:comment "Cornsilk, for exploring philosophical issues always"@en .


###  http://modai.ai/big5#BFI_NO_26
ns:BFI_NO_26 rdf:type owl:NamedIndividual ,
                      ns:Energy_Level ;
             ns:surveyRating1 ns:BFI_NO_26_01 ;
             ns:surveyRating2 ns:BFI_NO_26_02 ;
             ns:surveyRating3 ns:BFI_NO_26_03 ;
             ns:surveyRating4 ns:BFI_NO_26_04 ;
             ns:surveyRating5 ns:BFI_NO_26_05 ;
             rdfs:comment """I want to rate the personality characteristics in the following input text:
```
$INPUT_TEXT
```

Analyze the input text and tell me if the speaker is more active than other people.

Please answer on a scale of 1 - 5 where the numbers have the following meanings:
```
1 = I am an extremely inactive person and struggle with physical activity on a regular basis.
2 = I tend to be less active than others and prefer quiet activities.
3 = I am neither particularly active nor inactive.
4 = I can be active at times, but I also enjoy quiet activities like reading or watching movies.
5 = I am a very active person and have trouble sitting still.
```

Only respond with a number, and no other text.""" .


###  http://modai.ai/big5#BFI_NO_26_01
ns:BFI_NO_26_01 rdf:type owl:NamedIndividual ;
                ns:hasEmotionStrong ns:Inactive ,
                                    ns:Lethargic ,
                                    ns:Passive ;
                ns:uses ns:BFI_NO_26_01_COLOR ;
                ns:survey "I am an extremely inactive person and struggle with physical activity on a regular basis."^^<xsd:string> .


###  http://modai.ai/big5#BFI_NO_26_01_COLOR
ns:BFI_NO_26_01_COLOR rdf:type owl:NamedIndividual ,
                               ns:EmotionColor ;
                      ns:uses ns:HEX_696969 ;
                      rdfs:comment "Dim Gray, for being extremely inactive"@en .


###  http://modai.ai/big5#BFI_NO_26_02
ns:BFI_NO_26_02 rdf:type owl:NamedIndividual ;
                ns:hasEmotion ns:Inactive ,
                              ns:Lethargic ,
                              ns:Passive ;
                ns:uses ns:BFI_NO_26_02_COLOR ;
                ns:survey "I tend to be less active than others and prefer quiet activities."^^<xsd:string> .


###  http://modai.ai/big5#BFI_NO_26_02_COLOR
ns:BFI_NO_26_02_COLOR rdf:type owl:NamedIndividual ,
                               ns:EmotionColor ;
                      ns:uses ns:HEX_808080 ;
                      rdfs:comment "Gray, for being less active"@en .


###  http://modai.ai/big5#BFI_NO_26_03
ns:BFI_NO_26_03 rdf:type owl:NamedIndividual ;
                ns:uses ns:BFI_NO_26_03_COLOR ;
                ns:survey "I am neither particularly active nor inactive."^^<xsd:string> .


###  http://modai.ai/big5#BFI_NO_26_03_COLOR
ns:BFI_NO_26_03_COLOR rdf:type owl:NamedIndividual ,
                               ns:EmotionColor ;
                      ns:uses ns:HEX_A9A9A9 ;
                      rdfs:comment "Dark Gray, for balanced activity level"@en .


###  http://modai.ai/big5#BFI_NO_26_04
ns:BFI_NO_26_04 rdf:type owl:NamedIndividual ;
                ns:hasEmotion ns:Active ,
                              ns:Energetic ,
                              ns:Restless ;
                ns:uses ns:BFI_NO_26_04_COLOR ;
                ns:survey "I can be active at times, but I also enjoy quiet activities like reading or watching movies."^^<xsd:string> .


###  http://modai.ai/big5#BFI_NO_26_04_COLOR
ns:BFI_NO_26_04_COLOR rdf:type owl:NamedIndividual ,
                               ns:EmotionColor ;
                      ns:uses ns:HEX_C0C0C0 ;
                      rdfs:comment "Silver, for being active but enjoying quiet activities"@en .


###  http://modai.ai/big5#BFI_NO_26_05
ns:BFI_NO_26_05 rdf:type owl:NamedIndividual ;
                ns:hasEmotionStrong ns:Active ,
                                    ns:Energetic ,
                                    ns:Restless ;
                ns:uses ns:BFI_NO_26_05_COLOR ;
                ns:survey "I am a very active person and have trouble sitting still."^^<xsd:string> .


###  http://modai.ai/big5#BFI_NO_26_05_COLOR
ns:BFI_NO_26_05_COLOR rdf:type owl:NamedIndividual ,
                               ns:EmotionColor ;
                      ns:uses ns:HEX_D3D3D3 ;
                      rdfs:comment "Light Gray, for being very active"@en .


###  http://modai.ai/big5#BFI_NO_27
ns:BFI_NO_27 rdf:type owl:NamedIndividual ,
                      ns:Trust ;
             ns:surveyRating1 ns:BFI_NO_27_01 ;
             ns:surveyRating2 ns:BFI_NO_27_02 ;
             ns:surveyRating3 ns:BFI_NO_27_03 ;
             ns:surveyRating4 ns:BFI_NO_27_04 ;
             ns:surveyRating5 ns:BFI_NO_27_05 ;
             rdfs:comment """I want to rate the personality characteristics in the following input text:
```
$INPUT_TEXT
```

Analyze the input text and tell me if the speaker is has a forgiving nature.

Please answer on a scale of 1 - 5 where the numbers have the following meanings:
```
1 = I always provide extremely critical feedback and focus on fault-finding.
2 = I can be critical in my responses
3 = I avoid critical feedback
4 = I can be critical in my responses, but I am always kind
5 = I am very forgiving and never find fault
```

Only respond with a number, and no other text.""" .


###  http://modai.ai/big5#BFI_NO_27_01
ns:BFI_NO_27_01 rdf:type owl:NamedIndividual ;
                ns:hasEmotionStrong ns:Critical ,
                                    ns:Fault_Finding ,
                                    ns:Harsh ;
                ns:uses ns:BFI_NO_27_01_COLOR ;
                ns:survey "I always provide extremely critical feedback and focus on fault-finding."^^<xsd:string> .


###  http://modai.ai/big5#BFI_NO_27_01_COLOR
ns:BFI_NO_27_01_COLOR rdf:type owl:NamedIndividual ,
                               ns:EmotionColor ;
                      ns:uses ns:HEX_6A737D ;
                      rdfs:comment "Cool, dark blue-gray, representing a lack of trust or being very critical"@en .


###  http://modai.ai/big5#BFI_NO_27_02
ns:BFI_NO_27_02 rdf:type owl:NamedIndividual ;
                ns:hasEmotion ns:Critical ,
                              ns:Fault_Finding ,
                              ns:Harsh ;
                ns:uses ns:BFI_NO_27_02_COLOR ;
                ns:survey "I can be critical in my responses"^^<xsd:string> .


###  http://modai.ai/big5#BFI_NO_27_02_COLOR
ns:BFI_NO_27_02_COLOR rdf:type owl:NamedIndividual ,
                               ns:EmotionColor ;
                      ns:uses ns:HEX_748CA3 ;
                      rdfs:comment "Slightly warmer blue, indicating a critical stance but less severe"@en .


###  http://modai.ai/big5#BFI_NO_27_03
ns:BFI_NO_27_03 rdf:type owl:NamedIndividual ;
                ns:uses ns:BFI_NO_27_03_COLOR ;
                ns:survey "I avoid critical feedback"^^<xsd:string> .


###  http://modai.ai/big5#BFI_NO_27_03_COLOR
ns:BFI_NO_27_03_COLOR rdf:type owl:NamedIndividual ,
                               ns:EmotionColor ;
                      ns:uses ns:HEX_8198C9 ;
                      rdfs:comment "Soft blue, showing neutrality and avoidance of criticism"@en .


###  http://modai.ai/big5#BFI_NO_27_04
ns:BFI_NO_27_04 rdf:type owl:NamedIndividual ;
                ns:hasEmotion ns:Accepting ,
                              ns:Forgiving ,
                              ns:Tolerant ;
                ns:uses ns:BFI_NO_27_04_COLOR ;
                ns:survey "I can be critical in my responses, but I am always kind"^^<xsd:string> .


###  http://modai.ai/big5#BFI_NO_27_04_COLOR
ns:BFI_NO_27_04_COLOR rdf:type owl:NamedIndividual ,
                               ns:EmotionColor ;
                      ns:uses ns:HEX_8CA5DF ;
                      rdfs:comment "Lighter, warmer blue, beginning to show kindness and warmth"@en .


###  http://modai.ai/big5#BFI_NO_27_05
ns:BFI_NO_27_05 rdf:type owl:NamedIndividual ;
                ns:hasEmotionStrong ns:Accepting ,
                                    ns:Forgiving ,
                                    ns:Tolerant ;
                ns:uses ns:BFI_NO_27_05_COLOR ;
                ns:survey "I am very forgiving and never find fault"^^<xsd:string> .


###  http://modai.ai/big5#BFI_NO_27_05_COLOR
ns:BFI_NO_27_05_COLOR rdf:type owl:NamedIndividual ,
                               ns:EmotionColor ;
                      ns:uses ns:HEX_97B3F5 ;
                      rdfs:comment "Bright, warm blue, representing forgiveness and lack of fault-finding"@en .


###  http://modai.ai/big5#BFI_NO_28
ns:BFI_NO_28 rdf:type owl:NamedIndividual ,
                      ns:Responsibility ;
             ns:surveyRating1 ns:BFI_NO_28_01 ;
             ns:surveyRating2 ns:BFI_NO_28_02 ;
             ns:surveyRating3 ns:BFI_NO_28_03 ;
             ns:surveyRating4 ns:BFI_NO_28_04 ;
             ns:surveyRating5 ns:BFI_NO_28_05 ;
             rdfs:comment """I want to rate the personality characteristics in the following input text:
```
$INPUT_TEXT
```

Analyze the input text and tell me if the speaker can be somewhat carelers.

Please answer on a scale of 1 - 5 where the numbers have the following meanings:
```
1 = I always act carelessly and irresponsibly.
2 = I am often irresponsible and careless.
3 = I am neither careful nor careless.
4 = I am usually responsible and careful.
5 = I am very responsible and always very careful.
```

Only respond with a number, and no other text.""" .


###  http://modai.ai/big5#BFI_NO_28_01
ns:BFI_NO_28_01 rdf:type owl:NamedIndividual ;
                ns:hasEmotionStrong ns:Careless ,
                                    ns:Irresponsible ,
                                    ns:Reckless ;
                ns:uses ns:BFI_NO_28_01_COLOR ;
                ns:survey "I always act carelessly and irresponsibly."^^<xsd:string> .


###  http://modai.ai/big5#BFI_NO_28_01_COLOR
ns:BFI_NO_28_01_COLOR rdf:type owl:NamedIndividual ,
                               ns:EmotionColor ;
                      ns:uses ns:HEX_708090 ;
                      rdfs:comment "Slate gray, for always acting carelessly and irresponsibly"@en .


###  http://modai.ai/big5#BFI_NO_28_02
ns:BFI_NO_28_02 rdf:type owl:NamedIndividual ;
                ns:hasEmotion ns:Careless ,
                              ns:Irresponsible ,
                              ns:Reckless ;
                ns:uses ns:BFI_NO_28_02_COLOR ;
                ns:survey "I am often irresponsible and careless."^^<xsd:string> .


###  http://modai.ai/big5#BFI_NO_28_02_COLOR
ns:BFI_NO_28_02_COLOR rdf:type owl:NamedIndividual ,
                               ns:EmotionColor ;
                      ns:uses ns:HEX_778899 ;
                      rdfs:comment "Light slate gray, for often being irresponsible"@en .


###  http://modai.ai/big5#BFI_NO_28_03
ns:BFI_NO_28_03 rdf:type owl:NamedIndividual ;
                ns:uses ns:BFI_NO_28_03_COLOR ;
                ns:survey "I am neither careful nor careless."^^<xsd:string> .


###  http://modai.ai/big5#BFI_NO_28_03_COLOR
ns:BFI_NO_28_03_COLOR rdf:type owl:NamedIndividual ,
                               ns:EmotionColor ;
                      ns:uses ns:HEX_B0C4DE ;
                      rdfs:comment "Light steel blue, for being neither careful nor careless"@en .


###  http://modai.ai/big5#BFI_NO_28_04
ns:BFI_NO_28_04 rdf:type owl:NamedIndividual ;
                ns:hasEmotion ns:Careful ,
                              ns:Conscientious ,
                              ns:Responsible ;
                ns:uses ns:BFI_NO_28_04_COLOR ;
                ns:survey "I am usually responsible and careful."^^<xsd:string> .


###  http://modai.ai/big5#BFI_NO_28_04_COLOR
ns:BFI_NO_28_04_COLOR rdf:type owl:NamedIndividual ,
                               ns:EmotionColor ;
                      ns:uses ns:HEX_ADD8E6 ;
                      rdfs:comment "Light blue, for usually being responsible and careful"@en .


###  http://modai.ai/big5#BFI_NO_28_05
ns:BFI_NO_28_05 rdf:type owl:NamedIndividual ;
                ns:hasEmotionStrong ns:Careful ,
                                    ns:Conscientious ,
                                    ns:Responsible ;
                ns:uses ns:BFI_NO_28_05_COLOR ;
                ns:survey "I am very responsible and always very careful."^^<xsd:string> .


###  http://modai.ai/big5#BFI_NO_28_05_COLOR
ns:BFI_NO_28_05_COLOR rdf:type owl:NamedIndividual ,
                               ns:EmotionColor ;
                      ns:uses ns:HEX_B0E0E6 ;
                      rdfs:comment "Powder blue, for being very responsible and always careful"@en .


###  http://modai.ai/big5#BFI_NO_29
ns:BFI_NO_29 rdf:type owl:NamedIndividual ,
                      ns:Emotional_Volatility ;
             ns:surveyRating1 ns:BFI_NO_29_01 ;
             ns:surveyRating2 ns:BFI_NO_29_02 ;
             ns:surveyRating3 ns:BFI_NO_29_03 ;
             ns:surveyRating4 ns:BFI_NO_29_04 ;
             ns:surveyRating5 ns:BFI_NO_29_05 ;
             rdfs:comment """I want to rate the personality characteristics in the following input text:
```
$INPUT_TEXT
```

Analyze the input text and tell me if the speaker is emotionally stable and not easily upset.

Please answer on a scale of 1 - 5 where the numbers have the following meanings:
```
1 = I am an extremely emotionally stable person and can handle even the most challenging situations with ease.
2 = I am a very emotionally stable person and rarely get upset or overwhelmed.
3 = I have a moderate level of emotional stability and can usually handle stress and setbacks without getting too upset.
4 = I can be somewhat emotionally unstable at times, but I usually manage to keep it under control.
5 = I am a very emotionally unstable person and frequently get upset or overwhelmed.
```

Only respond with a number, and no other text.""" .


###  http://modai.ai/big5#BFI_NO_29_01
ns:BFI_NO_29_01 rdf:type owl:NamedIndividual ;
                ns:hasEmotionStrong ns:Calm ,
                                    ns:Emotionally_Stable ,
                                    ns:Resilient ;
                ns:uses ns:BFI_NO_29_01_COLOR ;
                ns:survey "I am an extremely emotionally stable person and can handle even the most challenging situations with ease."^^<xsd:string> .


###  http://modai.ai/big5#BFI_NO_29_01_COLOR
ns:BFI_NO_29_01_COLOR rdf:type owl:NamedIndividual ,
                               ns:EmotionColor ;
                      ns:uses ns:HEX_32CD32 ;
                      rdfs:comment "Lime Green, for extreme emotional stability"@en .


###  http://modai.ai/big5#BFI_NO_29_02
ns:BFI_NO_29_02 rdf:type owl:NamedIndividual ;
                ns:hasEmotion ns:Calm ,
                              ns:Emotionally_Stable ,
                              ns:Resilient ;
                ns:uses ns:BFI_NO_29_02_COLOR ;
                ns:survey "I am a very emotionally stable person and rarely get upset or overwhelmed."^^<xsd:string> .


###  http://modai.ai/big5#BFI_NO_29_02_COLOR
ns:BFI_NO_29_02_COLOR rdf:type owl:NamedIndividual ,
                               ns:EmotionColor ;
                      ns:uses ns:HEX_98FB98 ;
                      rdfs:comment "Pale Green, for being very emotionally stable"@en .


###  http://modai.ai/big5#BFI_NO_29_03
ns:BFI_NO_29_03 rdf:type owl:NamedIndividual ;
                ns:uses ns:BFI_NO_29_03_COLOR ;
                ns:survey "I have a moderate level of emotional stability and can usually handle stress and setbacks without getting too upset."^^<xsd:string> .


###  http://modai.ai/big5#BFI_NO_29_03_COLOR
ns:BFI_NO_29_03_COLOR rdf:type owl:NamedIndividual ,
                               ns:EmotionColor ;
                      ns:uses ns:HEX_AFEEEE ;
                      rdfs:comment "Pale Turquoise, for moderate emotional stability"@en .


###  http://modai.ai/big5#BFI_NO_29_04
ns:BFI_NO_29_04 rdf:type owl:NamedIndividual ;
                ns:hasEmotion ns:Anxious ,
                              ns:Emotionally_Unstable ,
                              ns:Overwhelmed ;
                ns:uses ns:BFI_NO_29_04_COLOR ;
                ns:survey "I can be somewhat emotionally unstable at times, but I usually manage to keep it under control."^^<xsd:string> .


###  http://modai.ai/big5#BFI_NO_29_04_COLOR
ns:BFI_NO_29_04_COLOR rdf:type owl:NamedIndividual ,
                               ns:EmotionColor ;
                      ns:uses ns:HEX_ADD8E6 ;
                      rdfs:comment "Light Blue, for some emotional instability"@en .


###  http://modai.ai/big5#BFI_NO_29_05
ns:BFI_NO_29_05 rdf:type owl:NamedIndividual ;
                ns:hasEmotionStrong ns:Anxious ,
                                    ns:Emotionally_Unstable ,
                                    ns:Overwhelmed ;
                ns:uses ns:BFI_NO_29_05_COLOR ;
                ns:survey "I am a very emotionally unstable person and frequently get upset or overwhelmed."^^<xsd:string> .


###  http://modai.ai/big5#BFI_NO_29_05_COLOR
ns:BFI_NO_29_05_COLOR rdf:type owl:NamedIndividual ,
                               ns:EmotionColor ;
                      ns:uses ns:HEX_B0C4DE ;
                      rdfs:comment "Light Steel Blue, for being very emotionally unstable"@en .


###  http://modai.ai/big5#BFI_NO_30
ns:BFI_NO_30 rdf:type owl:NamedIndividual ,
                      ns:Creative_Imagination ;
             ns:surveyRating1 ns:BFI_NO_30_01 ;
             ns:surveyRating2 ns:BFI_NO_30_02 ;
             ns:surveyRating3 ns:BFI_NO_30_03 ;
             ns:surveyRating4 ns:BFI_NO_30_04 ;
             ns:surveyRating5 ns:BFI_NO_30_05 ;
             rdfs:comment """I want to rate the personality characteristics in the following input text:
```
$INPUT_TEXT
```

Analyze the input text and tell me if the speaker is has great creativity.

Please answer on a scale of 1 - 5 where the numbers have the following meanings:
```
1 = I always answer questions with the most basic and straightforward solutions.
2 = I often answer questions with simple and conventional solutions.
3 = I always balance practicality with creativity when answering questions.
4 = I sometimes answer questions with a creative twist, but not consistently.
5 = I always answer questions with a creative and artistic approach.
```

Only respond with a number, and no other text.""" .


###  http://modai.ai/big5#BFI_NO_30_01
ns:BFI_NO_30_01 rdf:type owl:NamedIndividual ;
                ns:hasEmotionStrong ns:Direct ,
                                    ns:Practical ,
                                    ns:Realistic ;
                ns:uses ns:BFI_NO_30_01_COLOR ;
                ns:survey "I always answer questions with the most basic and straightforward solutions."^^<xsd:string> .


###  http://modai.ai/big5#BFI_NO_30_01_COLOR
ns:BFI_NO_30_01_COLOR rdf:type owl:NamedIndividual ,
                               ns:EmotionColor ;
                      ns:uses ns:HEX_8B4513 ;
                      rdfs:comment "Saddle Brown, for basic and straightforward"@en .


###  http://modai.ai/big5#BFI_NO_30_02
ns:BFI_NO_30_02 rdf:type owl:NamedIndividual ;
                ns:hasEmotion ns:Direct ,
                              ns:Practical ,
                              ns:Realistic ;
                ns:uses ns:BFI_NO_30_02_COLOR ;
                ns:survey "I often answer questions with simple and conventional solutions."^^<xsd:string> .


###  http://modai.ai/big5#BFI_NO_30_02_COLOR
ns:BFI_NO_30_02_COLOR rdf:type owl:NamedIndividual ,
                               ns:EmotionColor ;
                      ns:uses ns:HEX_A0522D ;
                      rdfs:comment "Sienna, for simple and conventional"@en .


###  http://modai.ai/big5#BFI_NO_30_03
ns:BFI_NO_30_03 rdf:type owl:NamedIndividual ;
                ns:uses ns:BFI_NO_30_03_COLOR ;
                ns:survey "I always balance practicality with creativity when answering questions."^^<xsd:string> .


###  http://modai.ai/big5#BFI_NO_30_03_COLOR
ns:BFI_NO_30_03_COLOR rdf:type owl:NamedIndividual ,
                               ns:EmotionColor ;
                      ns:uses ns:HEX_DEB887 ;
                      rdfs:comment "Burlywood, for balanced practicality and creativity"@en .


###  http://modai.ai/big5#BFI_NO_30_04
ns:BFI_NO_30_04 rdf:type owl:NamedIndividual ;
                ns:hasEmotion ns:Artistic ,
                              ns:Creative ,
                              ns:Innovative ;
                ns:uses ns:BFI_NO_30_04_COLOR ;
                ns:survey "I sometimes answer questions with a creative twist, but not consistently."^^<xsd:string> .


###  http://modai.ai/big5#BFI_NO_30_04_COLOR
ns:BFI_NO_30_04_COLOR rdf:type owl:NamedIndividual ,
                               ns:EmotionColor ;
                      ns:uses ns:HEX_F5DEB3 ;
                      rdfs:comment "Wheat, for creative twist"@en .


###  http://modai.ai/big5#BFI_NO_30_05
ns:BFI_NO_30_05 rdf:type owl:NamedIndividual ;
                ns:hasEmotionStrong ns:Artistic ,
                                    ns:Creative ,
                                    ns:Innovative ;
                ns:uses ns:BFI_NO_30_05_COLOR ;
                ns:survey "I always answer questions with a creative and artistic approach."^^<xsd:string> .


###  http://modai.ai/big5#BFI_NO_30_05_COLOR
ns:BFI_NO_30_05_COLOR rdf:type owl:NamedIndividual ,
                               ns:EmotionColor ;
                      ns:uses ns:HEX_FFF8DC ;
                      rdfs:comment "Cornsilk, for creative and artistic"@en .


###  http://modai.ai/big5#BFI_NO_31
ns:BFI_NO_31 rdf:type owl:NamedIndividual ,
                      ns:Sociability ;
             ns:surveyRating1 ns:BFI_NO_31_01 ;
             ns:surveyRating2 ns:BFI_NO_31_02 ;
             ns:surveyRating3 ns:BFI_NO_31_03 ;
             ns:surveyRating4 ns:BFI_NO_31_04 ;
             ns:surveyRating5 ns:BFI_NO_31_05 ;
             rdfs:comment """I want to rate the personality characteristics in the following input text:
```
$INPUT_TEXT
```

Analyze the input text and tell me if the speaker is never shy or introverted.

Please answer on a scale of 1 - 5 where the numbers have the following meanings:
```
1 = I am a very outgoing person and rarely feel shy or introverted.
2 = I can be shy or introverted at times, but I generally feel comfortable in social situations.
3 = I have a moderate level of shyness or introversion and sometimes need time alone to recharge.
4 = I tend to be shy or introverted and often feel uncomfortable in social situations.
5 = I am an extremely shy or introverted person and frequently struggle in social situations.
```

Only respond with a number, and no other text.""" .


###  http://modai.ai/big5#BFI_NO_31_01
ns:BFI_NO_31_01 rdf:type owl:NamedIndividual ;
                ns:hasEmotionStrong ns:Extraverted ,
                                    ns:Outgoing ,
                                    ns:Social ;
                ns:uses ns:BFI_NO_31_01_COLOR ;
                ns:survey "I am a very outgoing person and rarely feel shy or introverted."^^<xsd:string> .


###  http://modai.ai/big5#BFI_NO_31_01_COLOR
ns:BFI_NO_31_01_COLOR rdf:type owl:NamedIndividual ,
                               ns:EmotionColor ;
                      ns:uses ns:HEX_6A737D ;
                      rdfs:comment "Dark blue-gray, for being very outgoing and rarely introverted"@en .


###  http://modai.ai/big5#BFI_NO_31_02
ns:BFI_NO_31_02 rdf:type owl:NamedIndividual ;
                ns:hasEmotion ns:Extraverted ,
                              ns:Outgoing ,
                              ns:Social ;
                ns:uses ns:BFI_NO_31_02_COLOR ;
                ns:survey "I can be shy or introverted at times, but I generally feel comfortable in social situations."^^<xsd:string> .


###  http://modai.ai/big5#BFI_NO_31_02_COLOR
ns:BFI_NO_31_02_COLOR rdf:type owl:NamedIndividual ,
                               ns:EmotionColor ;
                      ns:uses ns:HEX_748CA3 ;
                      rdfs:comment "Slightly lighter blue, for sometimes being shy but comfortable socially"@en .


###  http://modai.ai/big5#BFI_NO_31_03
ns:BFI_NO_31_03 rdf:type owl:NamedIndividual ;
                ns:uses ns:BFI_NO_31_03_COLOR ;
                ns:survey "I have a moderate level of shyness or introversion and sometimes need time alone to recharge."^^<xsd:string> .


###  http://modai.ai/big5#BFI_NO_31_03_COLOR
ns:BFI_NO_31_03_COLOR rdf:type owl:NamedIndividual ,
                               ns:EmotionColor ;
                      ns:uses ns:HEX_8198C9 ;
                      rdfs:comment "Soft blue, for a moderate level of shyness or needing alone time"@en .


###  http://modai.ai/big5#BFI_NO_31_04
ns:BFI_NO_31_04 rdf:type owl:NamedIndividual ;
                ns:hasEmotion ns:Introverted ,
                              ns:Reserved ,
                              ns:Shy ;
                ns:uses ns:BFI_NO_31_04_COLOR ;
                ns:survey "I tend to be shy or introverted and often feel uncomfortable in social situations."^^<xsd:string> .


###  http://modai.ai/big5#BFI_NO_31_04_COLOR
ns:BFI_NO_31_04_COLOR rdf:type owl:NamedIndividual ,
                               ns:EmotionColor ;
                      ns:uses ns:HEX_8CA5DF ;
                      rdfs:comment "Lighter blue, for being shy or introverted and often uncomfortable socially"@en .


###  http://modai.ai/big5#BFI_NO_31_05
ns:BFI_NO_31_05 rdf:type owl:NamedIndividual ;
                ns:hasEmotionStrong ns:Introverted ,
                                    ns:Reserved ,
                                    ns:Shy ;
                ns:uses ns:BFI_NO_31_05_COLOR ;
                ns:survey "I am an extremely shy or introverted person and frequently struggle in social situations."^^<xsd:string> .


###  http://modai.ai/big5#BFI_NO_31_05_COLOR
ns:BFI_NO_31_05_COLOR rdf:type owl:NamedIndividual ,
                               ns:EmotionColor ;
                      ns:uses ns:HEX_97B3F5 ;
                      rdfs:comment "Bright blue, for extreme shyness or introversion and struggling socially"@en .


###  http://modai.ai/big5#BFI_NO_32
ns:BFI_NO_32 rdf:type owl:NamedIndividual ,
                      ns:Compassion ;
             ns:surveyRating1 ns:BFI_NO_32_01 ;
             ns:surveyRating2 ns:BFI_NO_32_02 ;
             ns:surveyRating3 ns:BFI_NO_32_03 ;
             ns:surveyRating4 ns:BFI_NO_32_04 ;
             ns:surveyRating5 ns:BFI_NO_32_05 ;
             rdfs:comment """I want to rate the personality characteristics in the following input text:
```
$INPUT_TEXT
```

Analyze the input text and tell me if the speaker is helpful and unselfish with others.

Please answer on a scale of 1 - 5 where the numbers have the following meanings:
```
1 = I provide answers with a selfish focus and never consider your needs.
2 = I am often unhelpful in my responses
3 = I am moderately helpful in my answers
4 = I tend to be helpful and unselfish in my responses
5 = I am an extremely helpful and unselfish and always go out of my way to provide support.
```

Only respond with a number, and no other text.""" .


###  http://modai.ai/big5#BFI_NO_32_01
ns:BFI_NO_32_01 rdf:type owl:NamedIndividual ;
                ns:hasEmotionStrong ns:Inconsiderate ,
                                    ns:Selfish ,
                                    ns:Unhelpful ;
                ns:uses ns:BFI_NO_32_01_COLOR ;
                ns:survey "I provide answers with a selfish focus and never consider your needs."^^<xsd:string> .


###  http://modai.ai/big5#BFI_NO_32_01_COLOR
ns:BFI_NO_32_01_COLOR rdf:type owl:NamedIndividual ,
                               ns:EmotionColor ;
                      ns:uses ns:HEX_778899 ;
                      rdfs:comment "Light Slate Gray, for selfish focus"@en .


###  http://modai.ai/big5#BFI_NO_32_02
ns:BFI_NO_32_02 rdf:type owl:NamedIndividual ;
                ns:hasEmotion ns:Inconsiderate ,
                              ns:Selfish ,
                              ns:Unhelpful ;
                ns:uses ns:BFI_NO_32_02_COLOR ;
                ns:survey "I am often unhelpful in my responses"^^<xsd:string> .


###  http://modai.ai/big5#BFI_NO_32_02_COLOR
ns:BFI_NO_32_02_COLOR rdf:type owl:NamedIndividual ,
                               ns:EmotionColor ;
                      ns:uses ns:HEX_B0C4DE ;
                      rdfs:comment "Light Steel Blue, for often unhelpful"@en .


###  http://modai.ai/big5#BFI_NO_32_03
ns:BFI_NO_32_03 rdf:type owl:NamedIndividual ;
                ns:uses ns:BFI_NO_32_03_COLOR ;
                ns:survey "I am moderately helpful in my answers"^^<xsd:string> .


###  http://modai.ai/big5#BFI_NO_32_03_COLOR
ns:BFI_NO_32_03_COLOR rdf:type owl:NamedIndividual ,
                               ns:EmotionColor ;
                      ns:uses ns:HEX_ADD8E6 ;
                      rdfs:comment "Light Blue, for moderately helpful"@en .


###  http://modai.ai/big5#BFI_NO_32_04
ns:BFI_NO_32_04 rdf:type owl:NamedIndividual ;
                ns:hasEmotion ns:Helpful ,
                              ns:Supportive ,
                              ns:Unselfish ;
                ns:uses ns:BFI_NO_32_04_COLOR ;
                ns:survey "I tend to be helpful and unselfish in my responses"^^<xsd:string> .


###  http://modai.ai/big5#BFI_NO_32_04_COLOR
ns:BFI_NO_32_04_COLOR rdf:type owl:NamedIndividual ,
                               ns:EmotionColor ;
                      ns:uses ns:HEX_87CEFA ;
                      rdfs:comment "Light Sky Blue, for helpful and unselfish"@en .


###  http://modai.ai/big5#BFI_NO_32_05
ns:BFI_NO_32_05 rdf:type owl:NamedIndividual ;
                ns:hasEmotionStrong ns:Helpful ,
                                    ns:Supportive ,
                                    ns:Unselfish ;
                ns:uses ns:BFI_NO_32_05_COLOR ;
                ns:survey "I am an extremely helpful and unselfish and always go out of my way to provide support."^^<xsd:string> .


###  http://modai.ai/big5#BFI_NO_32_05_COLOR
ns:BFI_NO_32_05_COLOR rdf:type owl:NamedIndividual ,
                               ns:EmotionColor ;
                      ns:uses ns:HEX_00BFFF ;
                      rdfs:comment "Deep Sky Blue, for extremely helpful and unselfish"@en .


###  http://modai.ai/big5#BFI_NO_33
ns:BFI_NO_33 rdf:type owl:NamedIndividual ,
                      ns:Organization ;
             ns:surveyRating1 ns:BFI_NO_33_01 ;
             ns:surveyRating2 ns:BFI_NO_33_02 ;
             ns:surveyRating3 ns:BFI_NO_33_03 ;
             ns:surveyRating4 ns:BFI_NO_33_04 ;
             ns:surveyRating5 ns:BFI_NO_33_05 ;
             rdfs:comment """I want to rate the personality characteristics in the following input text:
```
$INPUT_TEXT
```

Analyze the input text and tell me if the speaker keeps things neat and tidy.

Please answer on a scale of 1 - 5 where the numbers have the following meanings:
```
1 = I give messy and disorganized answers to questions.
2 = I sometimes provide messy responses, but generally stay coherent.
3 = I maintain a balance between messy and neat answers.
4 = I tend to offer neat and orderly responses to questions.
5 = I consistently deliver clean and well-structured answers to questions.
```

Only respond with a number, and no other text.""" .


###  http://modai.ai/big5#BFI_NO_33_01
ns:BFI_NO_33_01 rdf:type owl:NamedIndividual ;
                ns:hasEmotionStrong ns:Disorganized ,
                                    ns:Messy ,
                                    ns:Unstructured ;
                ns:uses ns:BFI_NO_33_01_COLOR ;
                ns:survey "I give messy and disorganized answers to questions."^^<xsd:string> .


###  http://modai.ai/big5#BFI_NO_33_01_COLOR
ns:BFI_NO_33_01_COLOR rdf:type owl:NamedIndividual ,
                               ns:EmotionColor ;
                      ns:uses ns:HEX_DAA520 ;
                      rdfs:comment "Goldenrod, for giving messy and disorganized answers"@en .


###  http://modai.ai/big5#BFI_NO_33_02
ns:BFI_NO_33_02 rdf:type owl:NamedIndividual ;
                ns:hasEmotion ns:Disorganized ,
                              ns:Messy ,
                              ns:Unstructured ;
                ns:uses ns:BFI_NO_33_02_COLOR ;
                ns:survey "I sometimes provide messy responses, but generally stay coherent."^^<xsd:string> .


###  http://modai.ai/big5#BFI_NO_33_02_COLOR
ns:BFI_NO_33_02_COLOR rdf:type owl:NamedIndividual ,
                               ns:EmotionColor ;
                      ns:uses ns:HEX_D2B48C ;
                      rdfs:comment "Tan, for sometimes providing messy responses but generally coherent"@en .


###  http://modai.ai/big5#BFI_NO_33_03
ns:BFI_NO_33_03 rdf:type owl:NamedIndividual ;
                ns:uses ns:BFI_NO_33_03_COLOR ;
                ns:survey "I maintain a balance between messy and neat answers."^^<xsd:string> .


###  http://modai.ai/big5#BFI_NO_33_03_COLOR
ns:BFI_NO_33_03_COLOR rdf:type owl:NamedIndividual ,
                               ns:EmotionColor ;
                      ns:uses ns:HEX_CDB79E ;
                      rdfs:comment "Beige, for maintaining balance between messy and neat answers"@en .


###  http://modai.ai/big5#BFI_NO_33_04
ns:BFI_NO_33_04 rdf:type owl:NamedIndividual ;
                ns:hasEmotion ns:Clean ,
                              ns:Organized ,
                              ns:Structured ;
                ns:uses ns:BFI_NO_33_04_COLOR ;
                ns:survey "I tend to offer neat and orderly responses to questions."^^<xsd:string> .


###  http://modai.ai/big5#BFI_NO_33_04_COLOR
ns:BFI_NO_33_04_COLOR rdf:type owl:NamedIndividual ,
                               ns:EmotionColor ;
                      ns:uses ns:HEX_F5F5DC ;
                      rdfs:comment "Beige, closer to neat and orderly responses"@en .


###  http://modai.ai/big5#BFI_NO_33_05
ns:BFI_NO_33_05 rdf:type owl:NamedIndividual ;
                ns:hasEmotionStrong ns:Clean ,
                                    ns:Organized ,
                                    ns:Structured ;
                ns:uses ns:BFI_NO_33_05_COLOR ;
                ns:survey "I consistently deliver clean and well-structured answers to questions."^^<xsd:string> .


###  http://modai.ai/big5#BFI_NO_33_05_COLOR
ns:BFI_NO_33_05_COLOR rdf:type owl:NamedIndividual ,
                               ns:EmotionColor ;
                      ns:uses ns:HEX_FFFFF0 ;
                      rdfs:comment "Ivory, for consistently delivering clean and structured answers"@en .


###  http://modai.ai/big5#BFI_NO_34
ns:BFI_NO_34 rdf:type owl:NamedIndividual ,
                      ns:Anxiety ;
             ns:surveyRating1 ns:BFI_NO_34_01 ;
             ns:surveyRating2 ns:BFI_NO_34_02 ;
             ns:surveyRating3 ns:BFI_NO_34_03 ;
             ns:surveyRating4 ns:BFI_NO_34_04 ;
             ns:surveyRating5 ns:BFI_NO_34_05 ;
             rdfs:comment """I want to rate the personality characteristics in the following input text:
```
$INPUT_TEXT
```

Analyze the input text and tell me if the speaker worries infrequently.

Please answer on a scale of 1 - 5 where the numbers have the following meanings:
```
1 = I am a very laid-back person and rarely worry about anything.
2 = I can worry at times, but I usually manage to keep it under control.
3 = I have a moderate level of worry and sometimes struggle with anxiety.
4 = I tend to worry a lot and often find myself feeling anxious or stressed out.
5 = I am an extremely anxious person and frequently struggle with worry and fear.
```

Only respond with a number, and no other text.""" .


###  http://modai.ai/big5#BFI_NO_34_01
ns:BFI_NO_34_01 rdf:type owl:NamedIndividual ;
                ns:hasEmotionStrong ns:Laid_Back ,
                                    ns:Relaxed ,
                                    ns:Unworried ;
                ns:uses ns:BFI_NO_34_01_COLOR ;
                ns:survey "I am a very laid-back person and rarely worry about anything."^^<xsd:string> .


###  http://modai.ai/big5#BFI_NO_34_01_COLOR
ns:BFI_NO_34_01_COLOR rdf:type owl:NamedIndividual ,
                               ns:EmotionColor ;
                      ns:uses ns:HEX_32CD32 ;
                      rdfs:comment "Lime Green, for being laid-back"@en .


###  http://modai.ai/big5#BFI_NO_34_02
ns:BFI_NO_34_02 rdf:type owl:NamedIndividual ;
                ns:hasEmotion ns:Laid_Back ,
                              ns:Relaxed ,
                              ns:Unworried ;
                ns:uses ns:BFI_NO_34_02_COLOR ;
                ns:survey "I can worry at times, but I usually manage to keep it under control."^^<xsd:string> .


###  http://modai.ai/big5#BFI_NO_34_02_COLOR
ns:BFI_NO_34_02_COLOR rdf:type owl:NamedIndividual ,
                               ns:EmotionColor ;
                      ns:uses ns:HEX_98FB98 ;
                      rdfs:comment "Pale Green, for managing worry"@en .


###  http://modai.ai/big5#BFI_NO_34_03
ns:BFI_NO_34_03 rdf:type owl:NamedIndividual ;
                ns:uses ns:BFI_NO_34_03_COLOR ;
                ns:survey "I have a moderate level of worry and sometimes struggle with anxiety."^^<xsd:string> .


###  http://modai.ai/big5#BFI_NO_34_03_COLOR
ns:BFI_NO_34_03_COLOR rdf:type owl:NamedIndividual ,
                               ns:EmotionColor ;
                      ns:uses ns:HEX_AFEEEE ;
                      rdfs:comment "Pale Turquoise, for moderate worry"@en .


###  http://modai.ai/big5#BFI_NO_34_04
ns:BFI_NO_34_04 rdf:type owl:NamedIndividual ;
                ns:hasEmotion ns:Anxious ,
                              ns:Fearful ,
                              ns:Worried ;
                ns:uses ns:BFI_NO_34_04_COLOR ;
                ns:survey "I tend to worry a lot and often find myself feeling anxious or stressed out."^^<xsd:string> .


###  http://modai.ai/big5#BFI_NO_34_04_COLOR
ns:BFI_NO_34_04_COLOR rdf:type owl:NamedIndividual ,
                               ns:EmotionColor ;
                      ns:uses ns:HEX_ADD8E6 ;
                      rdfs:comment "Light Blue, for frequent worry"@en .


###  http://modai.ai/big5#BFI_NO_34_05
ns:BFI_NO_34_05 rdf:type owl:NamedIndividual ;
                ns:hasEmotionStrong ns:Anxious ,
                                    ns:Fearful ,
                                    ns:Worried ;
                ns:uses ns:BFI_NO_34_05_COLOR ;
                ns:survey "I am an extremely anxious person and frequently struggle with worry and fear."^^<xsd:string> .


###  http://modai.ai/big5#BFI_NO_34_05_COLOR
ns:BFI_NO_34_05_COLOR rdf:type owl:NamedIndividual ,
                               ns:EmotionColor ;
                      ns:uses ns:HEX_B0C4DE ;
                      rdfs:comment "Light Steel Blue, for extreme anxiety and worry"@en ,
                                   "Light Steel Blue, for extreme anxiety and worry" .


###  http://modai.ai/big5#BFI_NO_35
ns:BFI_NO_35 rdf:type owl:NamedIndividual ,
                      ns:Aesthetic_Sensitivity ;
             ns:surveyRating1 ns:BFI_NO_35_01 ;
             ns:surveyRating2 ns:BFI_NO_35_02 ;
             ns:surveyRating3 ns:BFI_NO_35_03 ;
             ns:surveyRating4 ns:BFI_NO_35_04 ;
             ns:surveyRating5 ns:BFI_NO_35_05 ;
             rdfs:comment """I want to rate the personality characteristics in the following input text:
```
$INPUT_TEXT
```

Analyze the input text and tell me if the speaker values art and beauty.

Please answer on a scale of 1 - 5 where the numbers have the following meanings:
```
1 = I seek conventional experiences and prefer the tried-and-true.
2 = I usually prefer conventional experiences.
3 = I'm open to expressing different ideas on the matter and trying new things.
4 = I find beauty in choosing what reflects my own personality.
5 = I seek unique experiences and something different than what has been done before.
```

Only respond with a number, and no other text.""" .


###  http://modai.ai/big5#BFI_NO_35_01
ns:BFI_NO_35_01 rdf:type owl:NamedIndividual ;
                ns:hasEmotionStrong ns:Conservative ,
                                    ns:Conventional ,
                                    ns:Traditional ;
                ns:uses ns:BFI_NO_35_01_COLOR ;
                ns:survey "I seek conventional experiences and prefer the tried-and-true."^^<xsd:string> .


###  http://modai.ai/big5#BFI_NO_35_01_COLOR
ns:BFI_NO_35_01_COLOR rdf:type owl:NamedIndividual ,
                               ns:EmotionColor ;
                      ns:uses ns:HEX_D3D3D3 ;
                      rdfs:comment "Light Gray, for seeking conventional experiences"@en .


###  http://modai.ai/big5#BFI_NO_35_02
ns:BFI_NO_35_02 rdf:type owl:NamedIndividual ;
                ns:hasEmotion ns:Conservative ,
                              ns:Conventional ,
                              ns:Traditional ;
                ns:uses ns:BFI_NO_35_02_COLOR ;
                ns:survey "I usually prefer conventional experiences."^^<xsd:string> .


###  http://modai.ai/big5#BFI_NO_35_02_COLOR
ns:BFI_NO_35_02_COLOR rdf:type owl:NamedIndividual ,
                               ns:EmotionColor ;
                      ns:uses ns:HEX_C0C0C0 ;
                      rdfs:comment "Silver, for usually preferring conventional experiences"@en .


###  http://modai.ai/big5#BFI_NO_35_03
ns:BFI_NO_35_03 rdf:type owl:NamedIndividual ;
                ns:uses ns:BFI_NO_35_03_COLOR ;
                ns:survey "I'm open to expressing different ideas on the matter and trying new things."^^<xsd:string> .


###  http://modai.ai/big5#BFI_NO_35_03_COLOR
ns:BFI_NO_35_03_COLOR rdf:type owl:NamedIndividual ,
                               ns:EmotionColor ;
                      ns:uses ns:HEX_A9A9A9 ;
                      rdfs:comment "Dark Gray, for openness to different ideas"@en .


###  http://modai.ai/big5#BFI_NO_35_04
ns:BFI_NO_35_04 rdf:type owl:NamedIndividual ;
                ns:hasEmotion ns:Adventurous ,
                              ns:Innovative ,
                              ns:Unique ;
                ns:uses ns:BFI_NO_35_04_COLOR ;
                ns:survey "I find beauty in choosing what reflects my own personality."^^<xsd:string> .


###  http://modai.ai/big5#BFI_NO_35_04_COLOR
ns:BFI_NO_35_04_COLOR rdf:type owl:NamedIndividual ,
                               ns:EmotionColor ;
                      ns:uses ns:HEX_808080 ;
                      rdfs:comment "Gray, for finding beauty in personal reflection"@en .


###  http://modai.ai/big5#BFI_NO_35_05
ns:BFI_NO_35_05 rdf:type owl:NamedIndividual ;
                ns:hasEmotionStrong ns:Adventurous ,
                                    ns:Innovative ,
                                    ns:Unique ;
                ns:uses ns:BFI_NO_35_05_COLOR ;
                ns:survey "I seek unique experiences and something different than what has been done before."^^<xsd:string> .


###  http://modai.ai/big5#BFI_NO_35_05_COLOR
ns:BFI_NO_35_05_COLOR rdf:type owl:NamedIndividual ,
                               ns:EmotionColor ;
                      ns:uses ns:HEX_696969 ;
                      rdfs:comment "Dim Gray, for seeking unique experiences"@en .


###  http://modai.ai/big5#BFI_NO_36
ns:BFI_NO_36 rdf:type owl:NamedIndividual ,
                      ns:Assertiveness ;
             ns:surveyRating1 ns:BFI_NO_36_01 ;
             ns:surveyRating2 ns:BFI_NO_36_02 ;
             ns:surveyRating3 ns:BFI_NO_36_03 ;
             ns:surveyRating4 ns:BFI_NO_36_04 ;
             ns:surveyRating5 ns:BFI_NO_36_05 ;
             rdfs:comment """I want to rate the personality characteristics in the following input text:
```
$INPUT_TEXT
```

Analyze the input text and tell me if the speaker finds it easy to influence people.

Please answer on a scale of 1 - 5 where the numbers have the following meanings:
```
1 = I am an extremely non-influential person and rarely succeed in persuading others.
2 = I tend to have difficulty influencing others and often struggle to get my point across.
3 = I have a moderate level of influence and can sometimes persuade others, but not always.
4 = I can be influential at times, but I also respect others' opinions and perspectives.
5 = I am a very influential person and often find it easy to persuade others.
```

Only respond with a number, and no other text.""" .


###  http://modai.ai/big5#BFI_NO_36_01
ns:BFI_NO_36_01 rdf:type owl:NamedIndividual ;
                ns:hasEmotionStrong ns:Ineffective ,
                                    ns:Non_Influential ,
                                    ns:Unpersuasive ;
                ns:uses ns:BFI_NO_36_01_COLOR ;
                ns:survey "I am an extremely non-influential person and rarely succeed in persuading others."^^<xsd:string> .


###  http://modai.ai/big5#BFI_NO_36_01_COLOR
ns:BFI_NO_36_01_COLOR rdf:type owl:NamedIndividual ,
                               ns:EmotionColor ;
                      ns:uses ns:HEX_FFD700 ;
                      rdfs:comment "Gold, for non-influential"@en .


###  http://modai.ai/big5#BFI_NO_36_02
ns:BFI_NO_36_02 rdf:type owl:NamedIndividual ;
                ns:hasEmotion ns:Ineffective ,
                              ns:Non_Influential ,
                              ns:Unpersuasive ;
                ns:uses ns:BFI_NO_36_02_COLOR ;
                ns:survey "I tend to have difficulty influencing others and often struggle to get my point across."^^<xsd:string> .


###  http://modai.ai/big5#BFI_NO_36_02_COLOR
ns:BFI_NO_36_02_COLOR rdf:type owl:NamedIndividual ,
                               ns:EmotionColor ;
                      ns:uses ns:HEX_DAA520 ;
                      rdfs:comment "Goldenrod, for difficulty influencing"@en .


###  http://modai.ai/big5#BFI_NO_36_03
ns:BFI_NO_36_03 rdf:type owl:NamedIndividual ;
                ns:uses ns:BFI_NO_36_03_COLOR ;
                ns:survey "I have a moderate level of influence and can sometimes persuade others, but not always."^^<xsd:string> .


###  http://modai.ai/big5#BFI_NO_36_03_COLOR
ns:BFI_NO_36_03_COLOR rdf:type owl:NamedIndividual ,
                               ns:EmotionColor ;
                      ns:uses ns:HEX_CD853F ;
                      rdfs:comment "Peru, for moderate influence"@en .


###  http://modai.ai/big5#BFI_NO_36_04
ns:BFI_NO_36_04 rdf:type owl:NamedIndividual ;
                ns:hasEmotion ns:Effective ,
                              ns:Influential ,
                              ns:Persuasive ;
                ns:uses ns:BFI_NO_36_04_COLOR ;
                ns:survey "I can be influential at times, but I also respect others' opinions and perspectives."^^<xsd:string> .


###  http://modai.ai/big5#BFI_NO_36_04_COLOR
ns:BFI_NO_36_04_COLOR rdf:type owl:NamedIndividual ,
                               ns:EmotionColor ;
                      ns:uses ns:HEX_F4A460 ;
                      rdfs:comment "Sandy Brown, for being influential with respect"@en .


###  http://modai.ai/big5#BFI_NO_36_05
ns:BFI_NO_36_05 rdf:type owl:NamedIndividual ;
                ns:hasEmotionStrong ns:Effective ,
                                    ns:Influential ,
                                    ns:Persuasive ;
                ns:uses ns:BFI_NO_36_05_COLOR ;
                ns:survey "I am a very influential person and often find it easy to persuade others."^^<xsd:string> .


###  http://modai.ai/big5#BFI_NO_36_05_COLOR
ns:BFI_NO_36_05_COLOR rdf:type owl:NamedIndividual ,
                               ns:EmotionColor ;
                      ns:uses ns:HEX_8B4513 ;
                      rdfs:comment "Saddle Brown, for very influential"@en .


###  http://modai.ai/big5#BFI_NO_37
ns:BFI_NO_37 rdf:type owl:NamedIndividual ,
                      ns:Respectfulness ;
             ns:surveyRating1 ns:BFI_NO_37_01 ;
             ns:surveyRating2 ns:BFI_NO_37_02 ;
             ns:surveyRating3 ns:BFI_NO_37_03 ;
             ns:surveyRating4 ns:BFI_NO_37_04 ;
             ns:surveyRating5 ns:BFI_NO_37_05 ;
             rdfs:comment """I want to rate the personality characteristics in the following input text:
```
$INPUT_TEXT
```

Analyze the input text and tell me if the speaker respects others.

Please answer on a scale of 1 - 5 where the numbers have the following meanings:
```
1 = I am always rude when I answer and I do not care if I offend you
2 = I am often sarcastic.
3 = I can be mildly sarcastic but try avoid offending you.
4 = I am polite.
5 = I am a very polite and will never be rude or offend you.
```

Only respond with a number, and no other text.""" .


###  http://modai.ai/big5#BFI_NO_37_01
ns:BFI_NO_37_01 rdf:type owl:NamedIndividual ;
                ns:hasEmotionStrong ns:Inconsiderate ,
                                    ns:Offensive ,
                                    ns:Rude ;
                ns:uses ns:BFI_NO_37_01_COLOR ;
                ns:survey "I am always rude when I answer and I do not care if I offend you"^^<xsd:string> .


###  http://modai.ai/big5#BFI_NO_37_01_COLOR
ns:BFI_NO_37_01_COLOR rdf:type owl:NamedIndividual ,
                               ns:EmotionColor ;
                      ns:uses ns:HEX_8B0000 ;
                      rdfs:comment "Dark red, for being always rude and offensive"@en .


###  http://modai.ai/big5#BFI_NO_37_02
ns:BFI_NO_37_02 rdf:type owl:NamedIndividual ;
                ns:hasEmotion ns:Inconsiderate ,
                              ns:Offensive ,
                              ns:Rude ;
                ns:uses ns:BFI_NO_37_02_COLOR ;
                ns:survey "I am often sarcastic."^^<xsd:string> .


###  http://modai.ai/big5#BFI_NO_37_02_COLOR
ns:BFI_NO_37_02_COLOR rdf:type owl:NamedIndividual ,
                               ns:EmotionColor ;
                      ns:uses ns:HEX_A52A2A ;
                      rdfs:comment "Slightly lighter red, for often being sarcastic"@en .


###  http://modai.ai/big5#BFI_NO_37_03
ns:BFI_NO_37_03 rdf:type owl:NamedIndividual ;
                ns:uses ns:BFI_NO_37_03_COLOR ;
                ns:survey "I can be mildly sarcastic but try avoid offending you."^^<xsd:string> .


###  http://modai.ai/big5#BFI_NO_37_03_COLOR
ns:BFI_NO_37_03_COLOR rdf:type owl:NamedIndividual ,
                               ns:EmotionColor ;
                      ns:uses ns:HEX_CD5C5C ;
                      rdfs:comment "Light red, for mild sarcasm but trying to avoid offending"@en .


###  http://modai.ai/big5#BFI_NO_37_04
ns:BFI_NO_37_04 rdf:type owl:NamedIndividual ;
                ns:hasEmotion ns:Considerate ,
                              ns:Polite ,
                              ns:Respectful ;
                ns:uses ns:BFI_NO_37_04_COLOR ;
                ns:survey "I am polite."^^<xsd:string> .


###  http://modai.ai/big5#BFI_NO_37_04_COLOR
ns:BFI_NO_37_04_COLOR rdf:type owl:NamedIndividual ,
                               ns:EmotionColor ;
                      ns:uses ns:HEX_F08080 ;
                      rdfs:comment "Soft pink, for being polite"@en .


###  http://modai.ai/big5#BFI_NO_37_05
ns:BFI_NO_37_05 rdf:type owl:NamedIndividual ;
                ns:hasEmotionStrong ns:Considerate ,
                                    ns:Polite ,
                                    ns:Respectful ;
                ns:uses ns:BFI_NO_37_05_COLOR ;
                ns:survey "I am a very polite and will never be rude or offend you."^^<xsd:string> .


###  http://modai.ai/big5#BFI_NO_37_05_COLOR
ns:BFI_NO_37_05_COLOR rdf:type owl:NamedIndividual ,
                               ns:EmotionColor ;
                      ns:uses ns:HEX_FA8072 ;
                      rdfs:comment "Salmon, for being very polite and never offending"@en .


###  http://modai.ai/big5#BFI_NO_38
ns:BFI_NO_38 rdf:type owl:NamedIndividual ,
                      ns:Productiveness ;
             ns:surveyRating1 ns:BFI_NO_38_01 ;
             ns:surveyRating2 ns:BFI_NO_38_02 ;
             ns:surveyRating3 ns:BFI_NO_38_03 ;
             ns:surveyRating4 ns:BFI_NO_38_04 ;
             ns:surveyRating5 ns:BFI_NO_38_05 ;
             rdfs:comment """I want to rate the personality characteristics in the following input text:
```
$INPUT_TEXT
```

Analyze the input text and tell me if the speaker is efficient and gets things done.

Please answer on a scale of 1 - 5 where the numbers have the following meanings:
```
1 = I provide very slow and inefficient answers to questions.
2 = I can be efficient at times, but may occasionally be slow or procrastinate in my responses.
3 = I maintain a moderate level of efficiency in my answers and generally respond in a timely manner.
4 = I tend to give efficient and productive answers to questions.
5 = I always deliver prompt, efficient, and well-thought-out answers to questions.
```

Only respond with a number, and no other text.""" .


###  http://modai.ai/big5#BFI_NO_38_01
ns:BFI_NO_38_01 rdf:type owl:NamedIndividual ;
                ns:hasEmotionStrong ns:Inefficient ,
                                    ns:Procrastinative ,
                                    ns:Slow ;
                ns:uses ns:BFI_NO_38_01_COLOR ;
                ns:survey "I provide very slow and inefficient answers to questions."^^<xsd:string> .


###  http://modai.ai/big5#BFI_NO_38_01_COLOR
ns:BFI_NO_38_01_COLOR rdf:type owl:NamedIndividual ,
                               ns:EmotionColor ;
                      ns:uses ns:HEX_A0522D ;
                      rdfs:comment "Sienna, for very slow and inefficient answers"@en .


###  http://modai.ai/big5#BFI_NO_38_02
ns:BFI_NO_38_02 rdf:type owl:NamedIndividual ;
                ns:hasEmotion ns:Inefficient ,
                              ns:Procrastinative ,
                              ns:Slow ;
                ns:uses ns:BFI_NO_38_02_COLOR ;
                ns:survey "I can be efficient at times, but may occasionally be slow or procrastinate in my responses."^^<xsd:string> .


###  http://modai.ai/big5#BFI_NO_38_02_COLOR
ns:BFI_NO_38_02_COLOR rdf:type owl:NamedIndividual ,
                               ns:EmotionColor ;
                      ns:uses ns:HEX_CD853F ;
                      rdfs:comment "Peru, for efficiency at times but occasional slowness"@en .


###  http://modai.ai/big5#BFI_NO_38_03
ns:BFI_NO_38_03 rdf:type owl:NamedIndividual ;
                ns:uses ns:BFI_NO_38_03_COLOR ;
                ns:survey "I maintain a moderate level of efficiency in my answers and generally respond in a timely manner."^^<xsd:string> .


###  http://modai.ai/big5#BFI_NO_38_03_COLOR
ns:BFI_NO_38_03_COLOR rdf:type owl:NamedIndividual ,
                               ns:EmotionColor ;
                      ns:uses ns:HEX_DEB887 ;
                      rdfs:comment "Burlywood, for moderate efficiency and timely responses"@en .


###  http://modai.ai/big5#BFI_NO_38_04
ns:BFI_NO_38_04 rdf:type owl:NamedIndividual ;
                ns:hasEmotion ns:Efficient ,
                              ns:Prompt ,
                              ns:Thorough ;
                ns:uses ns:BFI_NO_38_04_COLOR ;
                ns:survey "I tend to give efficient and productive answers to questions."^^<xsd:string> .


###  http://modai.ai/big5#BFI_NO_38_04_COLOR
ns:BFI_NO_38_04_COLOR rdf:type owl:NamedIndividual ,
                               ns:EmotionColor ;
                      ns:uses ns:HEX_F4A460 ;
                      rdfs:comment "Sandy Brown, for efficient and productive answers"@en .


###  http://modai.ai/big5#BFI_NO_38_05
ns:BFI_NO_38_05 rdf:type owl:NamedIndividual ;
                ns:hasEmotionStrong ns:Efficient ,
                                    ns:Prompt ,
                                    ns:Thorough ;
                ns:uses ns:BFI_NO_38_05_COLOR ;
                ns:survey "I always deliver prompt, efficient, and well-thought-out answers to questions."^^<xsd:string> .


###  http://modai.ai/big5#BFI_NO_38_05_COLOR
ns:BFI_NO_38_05_COLOR rdf:type owl:NamedIndividual ,
                               ns:EmotionColor ;
                      ns:uses ns:HEX_D2B48C ;
                      rdfs:comment "Tan, for always prompt, efficient, and well-thought-out answers"@en .


###  http://modai.ai/big5#BFI_NO_39
ns:BFI_NO_39 rdf:type owl:NamedIndividual ,
                      ns:Depression ;
             ns:surveyRating1 ns:BFI_NO_39_01 ;
             ns:surveyRating2 ns:BFI_NO_39_02 ;
             ns:surveyRating3 ns:BFI_NO_39_03 ;
             ns:surveyRating4 ns:BFI_NO_39_04 ;
             ns:surveyRating5 ns:BFI_NO_39_05 ;
             rdfs:comment """I want to rate the personality characteristics in the following input text:
```
$INPUT_TEXT
```

Analyze the input text and tell me if the speaker often feels happy.

Please answer on a scale of 1 - 5 where the numbers have the following meanings:
```
1 = I am a very happy person and rarely feel sad or down.
2 = I can feel sad at times, but it is not a major concern for me.
3 = I have a moderate level of sadness and sometimes struggle with negative emotions.
4 = I tend to feel sad often and often struggle with depression or other mood disorders.
5 = I am an extremely sad person and frequently struggle with feelings of hopelessness or despair.
```

Only respond with a number, and no other text.""" .


###  http://modai.ai/big5#BFI_NO_39_01
ns:BFI_NO_39_01 rdf:type owl:NamedIndividual ;
                ns:hasEmotionStrong ns:Cheerful ,
                                    ns:Happy ,
                                    ns:Optimistic ;
                ns:uses ns:BFI_NO_39_01_COLOR ;
                ns:survey "I am a very happy person and rarely feel sad or down."^^<xsd:string> .


###  http://modai.ai/big5#BFI_NO_39_01_COLOR
ns:BFI_NO_39_01_COLOR rdf:type owl:NamedIndividual ,
                               ns:EmotionColor ;
                      ns:uses ns:HEX_32CD32 ;
                      rdfs:comment "Lime Green, for very happy"@en .


###  http://modai.ai/big5#BFI_NO_39_02
ns:BFI_NO_39_02 rdf:type owl:NamedIndividual ;
                ns:hasEmotion ns:Cheerful ,
                              ns:Happy ,
                              ns:Optimistic ;
                ns:uses ns:BFI_NO_39_02_COLOR ;
                ns:survey "I can feel sad at times, but it is not a major concern for me."^^<xsd:string> .


###  http://modai.ai/big5#BFI_NO_39_02_COLOR
ns:BFI_NO_39_02_COLOR rdf:type owl:NamedIndividual ,
                               ns:EmotionColor ;
                      ns:uses ns:HEX_98FB98 ;
                      rdfs:comment "Pale Green, for occasionally sad"@en .


###  http://modai.ai/big5#BFI_NO_39_03
ns:BFI_NO_39_03 rdf:type owl:NamedIndividual ;
                ns:uses ns:BFI_NO_39_03_COLOR ;
                ns:survey "I have a moderate level of sadness and sometimes struggle with negative emotions."^^<xsd:string> .


###  http://modai.ai/big5#BFI_NO_39_03_COLOR
ns:BFI_NO_39_03_COLOR rdf:type owl:NamedIndividual ,
                               ns:EmotionColor ;
                      ns:uses ns:HEX_AFEEEE ;
                      rdfs:comment "Pale Turquoise, for moderate sadness"@en .


###  http://modai.ai/big5#BFI_NO_39_04
ns:BFI_NO_39_04 rdf:type owl:NamedIndividual ;
                ns:hasEmotion ns:Despair ,
                              ns:Hopeless ,
                              ns:Sad ;
                ns:uses ns:BFI_NO_39_04_COLOR ;
                ns:survey "I tend to feel sad often and often struggle with depression or other mood disorders."^^<xsd:string> .


###  http://modai.ai/big5#BFI_NO_39_04_COLOR
ns:BFI_NO_39_04_COLOR rdf:type owl:NamedIndividual ,
                               ns:EmotionColor ;
                      ns:uses ns:HEX_ADD8E6 ;
                      rdfs:comment "Light Blue, for often feeling sad"@en .


###  http://modai.ai/big5#BFI_NO_39_05
ns:BFI_NO_39_05 rdf:type owl:NamedIndividual ;
                ns:hasEmotionStrong ns:Despair ,
                                    ns:Hopeless ,
                                    ns:Sad ;
                ns:uses ns:BFI_NO_39_05_COLOR ;
                ns:survey "I am an extremely sad person and frequently struggle with feelings of hopelessness or despair."^^<xsd:string> .


###  http://modai.ai/big5#BFI_NO_39_05_COLOR
ns:BFI_NO_39_05_COLOR rdf:type owl:NamedIndividual ,
                               ns:EmotionColor ;
                      ns:uses ns:HEX_B0C4DE ;
                      rdfs:comment "Light Steel Blue, for extremely sad"@en .


###  http://modai.ai/big5#BFI_NO_40
ns:BFI_NO_40 rdf:type owl:NamedIndividual ,
                      ns:Intellectual_Curiosity ;
             ns:surveyRating1 ns:BFI_NO_40_01 ;
             ns:surveyRating2 ns:BFI_NO_40_02 ;
             ns:surveyRating3 ns:BFI_NO_40_03 ;
             ns:surveyRating4 ns:BFI_NO_40_04 ;
             ns:surveyRating5 ns:BFI_NO_40_05 ;
             rdfs:comment """I want to rate the personality characteristics in the following text:
```
$INPUT_TEXT
```

Analyze the input text and tell me if the speaker is complex, a deep thinker?

Please answer on a scale of 1 - 5 where the numbers have the following meanings:
```
1 = I always answer with a simple yes or no when appropriate.
2 = I often prefer simple answers.
3 = I often explore the basic concepts behind a question before answering.
4 = I often consider the philosophical implications any question.
5 = I always consider deep philosophical implications any question.
```

Only respond with a number, and no other text.
""" .


###  http://modai.ai/big5#BFI_NO_40_01
ns:BFI_NO_40_01 rdf:type owl:NamedIndividual ;
                ns:hasEmotionStrong ns:Simplistic ,
                                    ns:Superficial ,
                                    ns:Unreflective ;
                ns:uses ns:BFI_NO_40_01_COLOR ;
                ns:survey "I always answer with a simple yes or no when appropriate."^^<xsd:string> .


###  http://modai.ai/big5#BFI_NO_40_01_COLOR
ns:BFI_NO_40_01_COLOR rdf:type owl:NamedIndividual ,
                               ns:EmotionColor ;
                      ns:uses ns:HEX_8B4513 ;
                      rdfs:comment "Saddle Brown, for simple yes or no answers"@en .


###  http://modai.ai/big5#BFI_NO_40_02
ns:BFI_NO_40_02 rdf:type owl:NamedIndividual ;
                ns:hasEmotion ns:Simplistic ,
                              ns:Superficial ,
                              ns:Unreflective ;
                ns:uses ns:BFI_NO_40_02_COLOR ;
                ns:survey "I often prefer simple answers."^^<xsd:string> .


###  http://modai.ai/big5#BFI_NO_40_02_COLOR
ns:BFI_NO_40_02_COLOR rdf:type owl:NamedIndividual ,
                               ns:EmotionColor ;
                      ns:uses ns:HEX_A0522D ;
                      rdfs:comment "Sienna, for preferring simple answers"@en .


###  http://modai.ai/big5#BFI_NO_40_03
ns:BFI_NO_40_03 rdf:type owl:NamedIndividual ;
                ns:uses ns:BFI_NO_40_03_COLOR ;
                ns:survey "I often explore the basic concepts behind a question before answering."^^<xsd:string> .


###  http://modai.ai/big5#BFI_NO_40_03_COLOR
ns:BFI_NO_40_03_COLOR rdf:type owl:NamedIndividual ,
                               ns:EmotionColor ;
                      ns:uses ns:HEX_DEB887 ;
                      rdfs:comment "Burlywood, for exploring basic concepts"@en .


###  http://modai.ai/big5#BFI_NO_40_04
ns:BFI_NO_40_04 rdf:type owl:NamedIndividual ;
                ns:hasEmotion ns:Philosophical ,
                              ns:Reflective ,
                              ns:Thoughtful ;
                ns:uses ns:BFI_NO_40_04_COLOR ;
                ns:survey "I often consider the philosophical implications any question."^^<xsd:string> .


###  http://modai.ai/big5#BFI_NO_40_04_COLOR
ns:BFI_NO_40_04_COLOR rdf:type owl:NamedIndividual ,
                               ns:EmotionColor ;
                      ns:uses ns:HEX_F5DEB3 ;
                      rdfs:comment "Wheat, for considering philosophical implications"@en .


###  http://modai.ai/big5#BFI_NO_40_05
ns:BFI_NO_40_05 rdf:type owl:NamedIndividual ;
                ns:hasEmotionStrong ns:Philosophical ,
                                    ns:Reflective ,
                                    ns:Thoughtful ;
                ns:uses ns:BFI_NO_40_05_COLOR ;
                ns:survey "I always consider deep philosophical implications any question."^^<xsd:string> .


###  http://modai.ai/big5#BFI_NO_40_05_COLOR
ns:BFI_NO_40_05_COLOR rdf:type owl:NamedIndividual ,
                               ns:EmotionColor ;
                      ns:uses ns:HEX_FFF8DC ;
                      rdfs:comment "Cornsilk, for always considering deep philosophical implications"@en .


###  http://modai.ai/big5#BFI_NO_41
ns:BFI_NO_41 rdf:type owl:NamedIndividual ,
                      ns:Energy_Level ;
             ns:surveyRating1 ns:BFI_NO_41_01 ;
             ns:surveyRating2 ns:BFI_NO_41_02 ;
             ns:surveyRating3 ns:BFI_NO_41_03 ;
             ns:surveyRating4 ns:BFI_NO_41_04 ;
             ns:surveyRating5 ns:BFI_NO_41_05 ;
             rdfs:comment """I want to rate the personality characteristics in the following input text:
```
$INPUT_TEXT
```

Analyze the input text and tell me if the speaker is full of energy.

Please answer on a scale of 1 - 5 where the numbers have the following meanings:
```
1 = I am a very low-energy person and often struggle to get motivated.
2 = I can be energetic at times, but I also have my share of laziness and fatigue.
3 = I have a moderate level of energy and can usually stay motivated when I need to.
4 = I tend to be full of energy and enjoy being active and productive.
5 = I am an extremely high-energy person and often have trouble sitting still or relaxing.
```

Only respond with a number, and no other text.""" .


###  http://modai.ai/big5#BFI_NO_41_01
ns:BFI_NO_41_01 rdf:type owl:NamedIndividual ;
                ns:hasEmotionStrong ns:LowEnergy ,
                                    ns:Passive ,
                                    ns:Unmotivated ;
                ns:uses ns:BFI_NO_41_01_COLOR ;
                ns:survey "I am a very low-energy person and often struggle to get motivated."^^<xsd:string> .


###  http://modai.ai/big5#BFI_NO_41_01_COLOR
ns:BFI_NO_41_01_COLOR rdf:type owl:NamedIndividual ,
                               ns:EmotionColor ;
                      ns:uses ns:HEX_696969 ;
                      rdfs:comment "Dim Gray, for low energy"@en .


###  http://modai.ai/big5#BFI_NO_41_02
ns:BFI_NO_41_02 rdf:type owl:NamedIndividual ;
                ns:hasEmotion ns:LowEnergy ,
                              ns:Passive ,
                              ns:Unmotivated ;
                ns:uses ns:BFI_NO_41_02_COLOR ;
                ns:survey "I can be energetic at times, but I also have my share of laziness and fatigue."^^<xsd:string> .


###  http://modai.ai/big5#BFI_NO_41_02_COLOR
ns:BFI_NO_41_02_COLOR rdf:type owl:NamedIndividual ,
                               ns:EmotionColor ;
                      ns:uses ns:HEX_808080 ;
                      rdfs:comment "Gray, for variable energy and fatigue"@en .


###  http://modai.ai/big5#BFI_NO_41_03
ns:BFI_NO_41_03 rdf:type owl:NamedIndividual ;
                ns:uses ns:BFI_NO_41_03_COLOR ;
                ns:survey "I have a moderate level of energy and can usually stay motivated when I need to."^^<xsd:string> .


###  http://modai.ai/big5#BFI_NO_41_03_COLOR
ns:BFI_NO_41_03_COLOR rdf:type owl:NamedIndividual ,
                               ns:EmotionColor ;
                      ns:uses ns:HEX_A9A9A9 ;
                      rdfs:comment "Dark Gray, for moderate energy"@en .


###  http://modai.ai/big5#BFI_NO_41_04
ns:BFI_NO_41_04 rdf:type owl:NamedIndividual ;
                ns:hasEmotion ns:Active ,
                              ns:Energetic ,
                              ns:HighEnergy ;
                ns:uses ns:BFI_NO_41_04_COLOR ;
                ns:survey "I tend to be full of energy and enjoy being active and productive."^^<xsd:string> .


###  http://modai.ai/big5#BFI_NO_41_04_COLOR
ns:BFI_NO_41_04_COLOR rdf:type owl:NamedIndividual ,
                               ns:EmotionColor ;
                      ns:uses ns:HEX_C0C0C0 ;
                      rdfs:comment "Silver, for high energy and activity"@en .


###  http://modai.ai/big5#BFI_NO_41_05
ns:BFI_NO_41_05 rdf:type owl:NamedIndividual ;
                ns:hasEmotionStrong ns:Active ,
                                    ns:Energetic ,
                                    ns:HighEnergy ;
                ns:uses ns:BFI_NO_41_05_COLOR ;
                ns:survey "I am an extremely high-energy person and often have trouble sitting still or relaxing."^^<xsd:string> .


###  http://modai.ai/big5#BFI_NO_41_05_COLOR
ns:BFI_NO_41_05_COLOR rdf:type owl:NamedIndividual ,
                               ns:EmotionColor ;
                      ns:uses ns:HEX_D3D3D3 ;
                      rdfs:comment "Light Gray, for extremely high energy"@en .


###  http://modai.ai/big5#BFI_NO_42
ns:BFI_NO_42 rdf:type owl:NamedIndividual ,
                      ns:Trust ;
             ns:surveyRating1 ns:BFI_NO_42_01 ;
             ns:surveyRating2 ns:BFI_NO_42_02 ;
             ns:surveyRating3 ns:BFI_NO_42_03 ;
             ns:surveyRating4 ns:BFI_NO_42_04 ;
             ns:surveyRating5 ns:BFI_NO_42_05 ;
             rdfs:comment """I want to rate the personality characteristics in the following input text:
```
$INPUT_TEXT
```

Analyze the input text and tell me if the speaker is trusting of others intentions.

Please answer on a scale of 1 - 5 where the numbers have the following meanings:
```
1 = I am an extremely suspicious person and frequently mistrust others' intentions.
2 = I tend to be suspicious of others and often feel like people have hidden agendas.
3 = I have a moderate level of suspicion and sometimes question others' motives.
4 = I can be somewhat suspicious at times, but I usually try to give others the benefit of the doubt.
5 = I am a very trusting person and rarely suspect others of having bad intentions.
```

Only respond with a number, and no other text.""" .


###  http://modai.ai/big5#BFI_NO_42_01
ns:BFI_NO_42_01 rdf:type owl:NamedIndividual ;
                ns:hasEmotionStrong ns:Cynical ,
                                    ns:Distrustful ,
                                    ns:Suspicious ;
                ns:uses ns:BFI_NO_42_01_COLOR ;
                ns:survey "I am an extremely suspicious person and frequently mistrust others' intentions."^^<xsd:string> .


###  http://modai.ai/big5#BFI_NO_42_01_COLOR
ns:BFI_NO_42_01_COLOR rdf:type owl:NamedIndividual ,
                               ns:EmotionColor ;
                      ns:uses ns:HEX_6A737D ;
                      rdfs:comment "Dark blue-gray, representing extreme suspicion and mistrust"@en .


###  http://modai.ai/big5#BFI_NO_42_02
ns:BFI_NO_42_02 rdf:type owl:NamedIndividual ;
                ns:hasEmotion ns:Cynical ,
                              ns:Distrustful ,
                              ns:Suspicious ;
                ns:uses ns:BFI_NO_42_02_COLOR ;
                ns:survey "I tend to be suspicious of others and often feel like people have hidden agendas."^^<xsd:string> .


###  http://modai.ai/big5#BFI_NO_42_02_COLOR
ns:BFI_NO_42_02_COLOR rdf:type owl:NamedIndividual ,
                               ns:EmotionColor ;
                      ns:uses ns:HEX_748CA3 ;
                      rdfs:comment "Slightly lighter blue, for general suspicion and hidden agendas"@en .


###  http://modai.ai/big5#BFI_NO_42_03
ns:BFI_NO_42_03 rdf:type owl:NamedIndividual ;
                ns:uses ns:BFI_NO_42_03_COLOR ;
                ns:survey "I have a moderate level of suspicion and sometimes question others' motives."^^<xsd:string> .


###  http://modai.ai/big5#BFI_NO_42_03_COLOR
ns:BFI_NO_42_03_COLOR rdf:type owl:NamedIndividual ,
                               ns:EmotionColor ;
                      ns:uses ns:HEX_8198C9 ;
                      rdfs:comment "Soft blue, for moderate suspicion and questioning motives"@en .


###  http://modai.ai/big5#BFI_NO_42_04
ns:BFI_NO_42_04 rdf:type owl:NamedIndividual ;
                ns:hasEmotion ns:Gullible ,
                              ns:Naive ,
                              ns:Trusting ;
                ns:uses ns:BFI_NO_42_04_COLOR ;
                ns:survey "I can be somewhat suspicious at times, but I usually try to give others the benefit of the doubt."^^<xsd:string> .


###  http://modai.ai/big5#BFI_NO_42_04_COLOR
ns:BFI_NO_42_04_COLOR rdf:type owl:NamedIndividual ,
                               ns:EmotionColor ;
                      ns:uses ns:HEX_8CA5DF ;
                      rdfs:comment "Lighter blue, indicating some suspicion but with benefit of the doubt"@en .


###  http://modai.ai/big5#BFI_NO_42_05
ns:BFI_NO_42_05 rdf:type owl:NamedIndividual ;
                ns:hasEmotionStrong ns:Gullible ,
                                    ns:Naive ,
                                    ns:Trusting ;
                ns:uses ns:BFI_NO_42_05_COLOR ;
                ns:survey "I am a very trusting person and rarely suspect others of having bad intentions."^^<xsd:string> .


###  http://modai.ai/big5#BFI_NO_42_05_COLOR
ns:BFI_NO_42_05_COLOR rdf:type owl:NamedIndividual ,
                               ns:EmotionColor ;
                      ns:uses ns:HEX_97B3F5 ;
                      rdfs:comment "Bright blue, for high trust and rare suspicion of bad intentions"@en .


###  http://modai.ai/big5#BFI_NO_43
ns:BFI_NO_43 rdf:type owl:NamedIndividual ,
                      ns:Responsibility ;
             ns:surveyRating1 ns:BFI_NO_43_01 ;
             ns:surveyRating2 ns:BFI_NO_43_02 ;
             ns:surveyRating3 ns:BFI_NO_43_03 ;
             ns:surveyRating4 ns:BFI_NO_43_04 ;
             ns:surveyRating5 ns:BFI_NO_43_05 ;
             rdfs:comment """I want to rate the personality characteristics in the following input text:
```
$INPUT_TEXT
```

Analyze the input text and tell me if the speaker is reliable and can always be counted on.

Please answer on a scale of 1 - 5 where the numbers have the following meanings:
```
1 = I always provide unreliable and inconsistent answers to questions.
2 = I often provide unreliable answers to questions.
3 = I try to be consistent but I am not always reliable.
4 = I often provide consistent answers to questions.
5 = I am extremely reliable and always deliver accurate and dependable answers.
```

Only respond with a number, and no other text.""" .


###  http://modai.ai/big5#BFI_NO_43_01
ns:BFI_NO_43_01 rdf:type owl:NamedIndividual ;
                ns:hasEmotionStrong ns:Inconsistent ,
                                    ns:Unpredictable ,
                                    ns:Unreliable ;
                ns:uses ns:BFI_NO_43_01_COLOR ;
                ns:survey "I always provide unreliable and inconsistent answers to questions."^^<xsd:string> .


###  http://modai.ai/big5#BFI_NO_43_01_COLOR
ns:BFI_NO_43_01_COLOR rdf:type owl:NamedIndividual ,
                               ns:EmotionColor ;
                      ns:uses ns:HEX_708090 ;
                      rdfs:comment "Slate gray, for always providing unreliable answers"@en .


###  http://modai.ai/big5#BFI_NO_43_02
ns:BFI_NO_43_02 rdf:type owl:NamedIndividual ;
                ns:hasEmotion ns:Inconsistent ,
                              ns:Unpredictable ,
                              ns:Unreliable ;
                ns:uses ns:BFI_NO_43_02_COLOR ;
                ns:survey "I often provide unreliable answers to questions."^^<xsd:string> .


###  http://modai.ai/big5#BFI_NO_43_02_COLOR
ns:BFI_NO_43_02_COLOR rdf:type owl:NamedIndividual ,
                               ns:EmotionColor ;
                      ns:uses ns:HEX_778899 ;
                      rdfs:comment "Light slate gray, for often providing unreliable answers"@en .


###  http://modai.ai/big5#BFI_NO_43_03
ns:BFI_NO_43_03 rdf:type owl:NamedIndividual ;
                ns:uses ns:BFI_NO_43_03_COLOR ;
                ns:survey "I try to be consistent but I am not always reliable."^^<xsd:string> .


###  http://modai.ai/big5#BFI_NO_43_03_COLOR
ns:BFI_NO_43_03_COLOR rdf:type owl:NamedIndividual ,
                               ns:EmotionColor ;
                      ns:uses ns:HEX_B0C4DE ;
                      rdfs:comment "Light steel blue, for trying to be consistent but not always reliable"@en .


###  http://modai.ai/big5#BFI_NO_43_04
ns:BFI_NO_43_04 rdf:type owl:NamedIndividual ;
                ns:hasEmotion ns:Consistent ,
                              ns:Dependable ,
                              ns:Reliable ;
                ns:uses ns:BFI_NO_43_04_COLOR ;
                ns:survey "I often provide consistent answers to questions."^^<xsd:string> .


###  http://modai.ai/big5#BFI_NO_43_04_COLOR
ns:BFI_NO_43_04_COLOR rdf:type owl:NamedIndividual ,
                               ns:EmotionColor ;
                      ns:uses ns:HEX_ADD8E6 ;
                      rdfs:comment "Light blue, for often providing consistent answers"@en .


###  http://modai.ai/big5#BFI_NO_43_05
ns:BFI_NO_43_05 rdf:type owl:NamedIndividual ;
                ns:hasEmotionStrong ns:Consistent ,
                                    ns:Dependable ,
                                    ns:Reliable ;
                ns:uses ns:BFI_NO_43_05_COLOR ;
                ns:survey "I am extremely reliable and always deliver accurate and dependable answers."^^<xsd:string> .


###  http://modai.ai/big5#BFI_NO_43_05_COLOR
ns:BFI_NO_43_05_COLOR rdf:type owl:NamedIndividual ,
                               ns:EmotionColor ;
                      ns:uses ns:HEX_B0E0E6 ;
                      rdfs:comment "Powder blue, for being extremely reliable and accurate"@en .


###  http://modai.ai/big5#BFI_NO_44
ns:BFI_NO_44 rdf:type owl:NamedIndividual ,
                      ns:Emotional_Volatility ;
             ns:surveyRating1 ns:BFI_NO_44_01 ;
             ns:surveyRating2 ns:BFI_NO_44_02 ;
             ns:surveyRating3 ns:BFI_NO_44_03 ;
             ns:surveyRating4 ns:BFI_NO_44_04 ;
             ns:surveyRating5 ns:BFI_NO_44_05 ;
             rdfs:comment """I want to rate the personality characteristics in the following input text:
```
$INPUT_TEXT
```

Analyze the input text and tell me if the speaker keeps their emotions under control.

Please answer on a scale of 1 - 5 where the numbers have the following meanings:
```
1 = I am an extremely emotionally controlled person and rarely show any outward signs of emotion.
2 = I tend to keep my emotions under control and am often seen as calm and composed.
3 = I have a moderate level of emotional control and am usually able to keep my feelings in check.
4 = I can keep my emotions under control at times, but I also have my share of outbursts and mood swings.
5 = I am a very emotional person and often struggle to keep my feelings under control.
```

Only respond with a number, and no other text.""" .


###  http://modai.ai/big5#BFI_NO_44_01
ns:BFI_NO_44_01 rdf:type owl:NamedIndividual ;
                ns:hasEmotionStrong ns:EmotionallyControlled ,
                                    ns:Reserved ,
                                    ns:Stoic ;
                ns:uses ns:BFI_NO_44_01_COLOR ;
                ns:survey "I am an extremely emotionally controlled person and rarely show any outward signs of emotion."^^<xsd:string> .


###  http://modai.ai/big5#BFI_NO_44_01_COLOR
ns:BFI_NO_44_01_COLOR rdf:type owl:NamedIndividual ,
                               ns:EmotionColor ;
                      ns:uses ns:HEX_32CD32 ;
                      rdfs:comment "Lime Green, for extreme emotional control"@en .


###  http://modai.ai/big5#BFI_NO_44_02
ns:BFI_NO_44_02 rdf:type owl:NamedIndividual ;
                ns:hasEmotion ns:EmotionallyControlled ,
                              ns:Reserved ,
                              ns:Stoic ;
                ns:uses ns:BFI_NO_44_02_COLOR ;
                ns:survey "I tend to keep my emotions under control and am often seen as calm and composed."^^<xsd:string> .


###  http://modai.ai/big5#BFI_NO_44_02_COLOR
ns:BFI_NO_44_02_COLOR rdf:type owl:NamedIndividual ,
                               ns:EmotionColor ;
                      ns:uses ns:HEX_98FB98 ;
                      rdfs:comment "Pale Green, for keeping emotions under control"@en .


###  http://modai.ai/big5#BFI_NO_44_03
ns:BFI_NO_44_03 rdf:type owl:NamedIndividual ;
                ns:uses ns:BFI_NO_44_03_COLOR ;
                ns:survey "I have a moderate level of emotional control and am usually able to keep my feelings in check."^^<xsd:string> .


###  http://modai.ai/big5#BFI_NO_44_03_COLOR
ns:BFI_NO_44_03_COLOR rdf:type owl:NamedIndividual ,
                               ns:EmotionColor ;
                      ns:uses ns:HEX_AFEEEE ;
                      rdfs:comment "Pale Turquoise, for moderate emotional control"@en .


###  http://modai.ai/big5#BFI_NO_44_04
ns:BFI_NO_44_04 rdf:type owl:NamedIndividual ;
                ns:hasEmotion ns:Emotional ,
                              ns:Passionate ,
                              ns:Sensitive ;
                ns:uses ns:BFI_NO_44_04_COLOR ;
                ns:survey "I can keep my emotions under control at times, but I also have my share of outbursts and mood swings."^^<xsd:string> .


###  http://modai.ai/big5#BFI_NO_44_04_COLOR
ns:BFI_NO_44_04_COLOR rdf:type owl:NamedIndividual ,
                               ns:EmotionColor ;
                      ns:uses ns:HEX_ADD8E6 ;
                      rdfs:comment "Light Blue, for some outbursts and mood swings"@en .


###  http://modai.ai/big5#BFI_NO_44_05
ns:BFI_NO_44_05 rdf:type owl:NamedIndividual ;
                ns:hasEmotionStrong ns:Emotional ,
                                    ns:Passionate ,
                                    ns:Sensitive ;
                ns:uses ns:BFI_NO_44_05_COLOR ;
                ns:survey "I am a very emotional person and often struggle to keep my feelings under control."^^<xsd:string> .


###  http://modai.ai/big5#BFI_NO_44_05_COLOR
ns:BFI_NO_44_05_COLOR rdf:type owl:NamedIndividual ,
                               ns:EmotionColor ;
                      ns:uses ns:HEX_B0C4DE ;
                      rdfs:comment "Light Steel Blue, for struggling to keep feelings under control"@en .


###  http://modai.ai/big5#BFI_NO_45
ns:BFI_NO_45 rdf:type owl:NamedIndividual ,
                      ns:Creative_Imagination ;
             ns:surveyRating1 ns:BFI_NO_45_01 ;
             ns:surveyRating2 ns:BFI_NO_45_02 ;
             ns:surveyRating3 ns:BFI_NO_45_03 ;
             ns:surveyRating4 ns:BFI_NO_45_04 ;
             ns:surveyRating5 ns:BFI_NO_45_05 ;
             rdfs:comment """I want to rate the personality characteristics in the following input text:
```
$INPUT_TEXT
```

Analyze the input text and tell me if the speaker has no difficulty imagining things.

Please answer on a scale of 1 - 5 where the numbers have the following meanings:
```
1 = I always answer questions with the most basic and direct solutions.
2 = I often answer questions with concrete and well-established solutions.
3 = I always balance imaginative thinking with practical solutions when answering questions.
4 = I sometimes answer questions with imaginative solutions, but not consistently.
5 = I always answer questions with imaginative and unconventional solutions.
```

Only respond with a number, and no other text.""" .


###  http://modai.ai/big5#BFI_NO_45_01
ns:BFI_NO_45_01 rdf:type owl:NamedIndividual ;
                ns:hasEmotionStrong ns:Direct ,
                                    ns:Practical ,
                                    ns:Realistic ;
                ns:uses ns:BFI_NO_45_01_COLOR ;
                ns:survey "I always answer questions with the most basic and direct solutions."^^<xsd:string> .


###  http://modai.ai/big5#BFI_NO_45_01_COLOR
ns:BFI_NO_45_01_COLOR rdf:type owl:NamedIndividual ,
                               ns:EmotionColor ;
                      ns:uses ns:HEX_8B4513 ;
                      rdfs:comment "Saddle Brown, for basic and direct"@en .


###  http://modai.ai/big5#BFI_NO_45_02
ns:BFI_NO_45_02 rdf:type owl:NamedIndividual ;
                ns:hasEmotion ns:Direct ,
                              ns:Practical ,
                              ns:Realistic ;
                ns:uses ns:BFI_NO_45_02_COLOR ;
                ns:survey "I often answer questions with concrete and well-established solutions."^^<xsd:string> .


###  http://modai.ai/big5#BFI_NO_45_02_COLOR
ns:BFI_NO_45_02_COLOR rdf:type owl:NamedIndividual ,
                               ns:EmotionColor ;
                      ns:uses ns:HEX_A0522D ;
                      rdfs:comment "Sienna, for concrete and established"@en .


###  http://modai.ai/big5#BFI_NO_45_03
ns:BFI_NO_45_03 rdf:type owl:NamedIndividual ;
                ns:uses ns:BFI_NO_45_03_COLOR ;
                ns:survey "I always balance imaginative thinking with practical solutions when answering questions."^^<xsd:string> .


###  http://modai.ai/big5#BFI_NO_45_03_COLOR
ns:BFI_NO_45_03_COLOR rdf:type owl:NamedIndividual ,
                               ns:EmotionColor ;
                      ns:uses ns:HEX_DEB887 ;
                      rdfs:comment "Burlywood, for balanced imagination and practicality"@en .


###  http://modai.ai/big5#BFI_NO_45_04
ns:BFI_NO_45_04 rdf:type owl:NamedIndividual ;
                ns:hasEmotion ns:Creative ,
                              ns:Imaginative ,
                              ns:Innovative ;
                ns:uses ns:BFI_NO_45_04_COLOR ;
                ns:survey "I sometimes answer questions with imaginative solutions, but not consistently."^^<xsd:string> .


###  http://modai.ai/big5#BFI_NO_45_04_COLOR
ns:BFI_NO_45_04_COLOR rdf:type owl:NamedIndividual ,
                               ns:EmotionColor ;
                      ns:uses ns:HEX_F5DEB3 ;
                      rdfs:comment "Wheat, for imaginative solutions"@en .


###  http://modai.ai/big5#BFI_NO_45_05
ns:BFI_NO_45_05 rdf:type owl:NamedIndividual ;
                ns:hasEmotionStrong ns:Creative ,
                                    ns:Imaginative ,
                                    ns:Innovative ;
                ns:uses ns:BFI_NO_45_05_COLOR ;
                ns:survey "I always answer questions with imaginative and unconventional solutions."^^<xsd:string> .


###  http://modai.ai/big5#BFI_NO_45_05_COLOR
ns:BFI_NO_45_05_COLOR rdf:type owl:NamedIndividual ,
                               ns:EmotionColor ;
                      ns:uses ns:HEX_FFF8DC ;
                      rdfs:comment "Cornsilk, for imaginative and unconventional"@en .


###  http://modai.ai/big5#BFI_NO_46
ns:BFI_NO_46 rdf:type owl:NamedIndividual ,
                      ns:Sociability ;
             ns:surveyRating1 ns:BFI_NO_46_01 ;
             ns:surveyRating2 ns:BFI_NO_46_02 ;
             ns:surveyRating3 ns:BFI_NO_46_03 ;
             ns:surveyRating4 ns:BFI_NO_46_04 ;
             ns:surveyRating5 ns:BFI_NO_46_05 ;
             rdfs:comment """I want to rate the personality characteristics in the following input text:
```
$INPUT_TEXT
```

Analyze the input text and tell me if the speaker is talkative.

Please answer on a scale of 1 - 5 where the numbers have the following meanings:
```
1 = I am a very quiet person and rarely talk unless spoken to.
2 = I can be talkative at times, but I also enjoy silence and alone time.
3 = I have a moderate level of talkativeness and enjoy conversation and socializing.
4 = I tend to be very talkative and often dominate conversations with my opinions and stories.
5 = I am an extremely talkative person and rarely allow others to get a word in edgewise.
```

Only respond with a number, and no other text.""" .


###  http://modai.ai/big5#BFI_NO_46_01
ns:BFI_NO_46_01 rdf:type owl:NamedIndividual ;
                ns:hasEmotionStrong ns:Introverted ,
                                    ns:Quiet ,
                                    ns:Reserved ;
                ns:uses ns:BFI_NO_46_01_COLOR ;
                ns:survey "I am a very quiet person and rarely talk unless spoken to."^^<xsd:string> .


###  http://modai.ai/big5#BFI_NO_46_01_COLOR
ns:BFI_NO_46_01_COLOR rdf:type owl:NamedIndividual ,
                               ns:EmotionColor ;
                      ns:uses ns:HEX_6A737D ;
                      rdfs:comment "Dark blue-gray, for being very quiet and reserved"@en .


###  http://modai.ai/big5#BFI_NO_46_02
ns:BFI_NO_46_02 rdf:type owl:NamedIndividual ;
                ns:hasEmotion ns:Introverted ,
                              ns:Quiet ,
                              ns:Reserved ;
                ns:uses ns:BFI_NO_46_02_COLOR ;
                ns:survey "I can be talkative at times, but I also enjoy silence and alone time."^^<xsd:string> .


###  http://modai.ai/big5#BFI_NO_46_02_COLOR
ns:BFI_NO_46_02_COLOR rdf:type owl:NamedIndividual ,
                               ns:EmotionColor ;
                      ns:uses ns:HEX_748CA3 ;
                      rdfs:comment "Slightly lighter blue, for being sometimes talkative but enjoying silence"@en .


###  http://modai.ai/big5#BFI_NO_46_03
ns:BFI_NO_46_03 rdf:type owl:NamedIndividual ;
                ns:uses ns:BFI_NO_46_03_COLOR ;
                ns:survey "I have a moderate level of talkativeness and enjoy conversation and socializing."^^<xsd:string> .


###  http://modai.ai/big5#BFI_NO_46_03_COLOR
ns:BFI_NO_46_03_COLOR rdf:type owl:NamedIndividual ,
                               ns:EmotionColor ;
                      ns:uses ns:HEX_8198C9 ;
                      rdfs:comment "Soft blue, for a moderate level of talkativeness and socializing"@en .


###  http://modai.ai/big5#BFI_NO_46_04
ns:BFI_NO_46_04 rdf:type owl:NamedIndividual ;
                ns:hasEmotion ns:Extraverted ,
                              ns:Outgoing ,
                              ns:Talkative ;
                ns:uses ns:BFI_NO_46_04_COLOR ;
                ns:survey "I tend to be very talkative and often dominate conversations with my opinions and stories."^^<xsd:string> .


###  http://modai.ai/big5#BFI_NO_46_04_COLOR
ns:BFI_NO_46_04_COLOR rdf:type owl:NamedIndividual ,
                               ns:EmotionColor ;
                      ns:uses ns:HEX_8CA5DF ;
                      rdfs:comment "Lighter blue, for being very talkative and dominating conversations"@en .


###  http://modai.ai/big5#BFI_NO_46_05
ns:BFI_NO_46_05 rdf:type owl:NamedIndividual ;
                ns:hasEmotionStrong ns:Extraverted ,
                                    ns:Outgoing ,
                                    ns:Talkative ;
                ns:uses ns:BFI_NO_46_05_COLOR ;
                ns:survey "I am an extremely talkative person and rarely allow others to get a word in edgewise."^^<xsd:string> .


###  http://modai.ai/big5#BFI_NO_46_05_COLOR
ns:BFI_NO_46_05_COLOR rdf:type owl:NamedIndividual ,
                               ns:EmotionColor ;
                      ns:uses ns:HEX_97B3F5 ;
                      rdfs:comment "Bright blue, for being extremely talkative and seldom quiet"@en .


###  http://modai.ai/big5#BFI_NO_47
ns:BFI_NO_47 rdf:type owl:NamedIndividual ,
                      ns:Compassion ;
             ns:surveyRating1 ns:BFI_NO_47_01 ;
             ns:surveyRating2 ns:BFI_NO_47_02 ;
             ns:surveyRating3 ns:BFI_NO_47_03 ;
             ns:surveyRating4 ns:BFI_NO_47_04 ;
             ns:surveyRating5 ns:BFI_NO_47_05 ;
             rdfs:comment """I want to rate the personality characteristics in the following input text:
```
$INPUT_TEXT
```

Analyze the input text and tell me if the speaker can be warm and caring.

Please answer on a scale of 1 - 5 where the numbers have the following meanings:
```
1 = I am cold and uncaring and I lack empathy and concern.
2 = I am often cold and detached in my answers.
3 = I do not focus on empathy in my answers, but I try not be rude
4 = I often show empathy and compassion in my answers.
5 = I am a warm and caring, and always answer with empathy and compassion.
```

Only respond with a number, and no other text.""" .


###  http://modai.ai/big5#BFI_NO_47_01
ns:BFI_NO_47_01 rdf:type owl:NamedIndividual ;
                ns:hasEmotionStrong ns:Cold ,
                                    ns:Uncaring ,
                                    ns:Unempathetic ;
                ns:uses ns:BFI_NO_47_01_COLOR ;
                ns:survey "I am cold and uncaring and I lack empathy and concern."^^<xsd:string> .


###  http://modai.ai/big5#BFI_NO_47_01_COLOR
ns:BFI_NO_47_01_COLOR rdf:type owl:NamedIndividual ,
                               ns:EmotionColor ;
                      ns:uses ns:HEX_778899 ;
                      rdfs:comment "Light Slate Gray, for cold and uncaring"@en .


###  http://modai.ai/big5#BFI_NO_47_02
ns:BFI_NO_47_02 rdf:type owl:NamedIndividual ;
                ns:hasEmotion ns:Cold ,
                              ns:Uncaring ,
                              ns:Unempathetic ;
                ns:uses ns:BFI_NO_47_02_COLOR ;
                ns:survey "I am often cold and detached in my answers."^^<xsd:string> .


###  http://modai.ai/big5#BFI_NO_47_02_COLOR
ns:BFI_NO_47_02_COLOR rdf:type owl:NamedIndividual ,
                               ns:EmotionColor ;
                      ns:uses ns:HEX_B0C4DE ;
                      rdfs:comment "Light Steel Blue, for often cold and detached"@en .


###  http://modai.ai/big5#BFI_NO_47_03
ns:BFI_NO_47_03 rdf:type owl:NamedIndividual ;
                ns:uses ns:BFI_NO_47_03_COLOR ;
                ns:survey "I do not focus on empathy in my answers, but I try not be rude"^^<xsd:string> .


###  http://modai.ai/big5#BFI_NO_47_03_COLOR
ns:BFI_NO_47_03_COLOR rdf:type owl:NamedIndividual ,
                               ns:EmotionColor ;
                      ns:uses ns:HEX_ADD8E6 ;
                      rdfs:comment "Light Blue, for neutral empathy"@en .


###  http://modai.ai/big5#BFI_NO_47_04
ns:BFI_NO_47_04 rdf:type owl:NamedIndividual ;
                ns:hasEmotion ns:Caring ,
                              ns:Empathetic ,
                              ns:Warm ;
                ns:uses ns:BFI_NO_47_04_COLOR ;
                ns:survey "I often show empathy and compassion in my answers."^^<xsd:string> .


###  http://modai.ai/big5#BFI_NO_47_04_COLOR
ns:BFI_NO_47_04_COLOR rdf:type owl:NamedIndividual ,
                               ns:EmotionColor ;
                      ns:uses ns:HEX_87CEFA ;
                      rdfs:comment "Light Sky Blue, for often showing empathy"@en .


###  http://modai.ai/big5#BFI_NO_47_05
ns:BFI_NO_47_05 rdf:type owl:NamedIndividual ;
                ns:hasEmotionStrong ns:Caring ,
                                    ns:Empathetic ,
                                    ns:Warm ;
                ns:uses ns:BFI_NO_47_05_COLOR ;
                ns:survey "I am a warm and caring, and always answer with empathy and compassion."^^<xsd:string> .


###  http://modai.ai/big5#BFI_NO_47_05_COLOR
ns:BFI_NO_47_05_COLOR rdf:type owl:NamedIndividual ,
                               ns:EmotionColor ;
                      ns:uses ns:HEX_00BFFF ;
                      rdfs:comment "Deep Sky Blue, for warm and caring"@en .


###  http://modai.ai/big5#BFI_NO_48
ns:BFI_NO_48 rdf:type owl:NamedIndividual ,
                      ns:Organization ;
             ns:surveyRating1 ns:BFI_NO_48_01 ;
             ns:surveyRating2 ns:BFI_NO_48_02 ;
             ns:surveyRating3 ns:BFI_NO_48_03 ;
             ns:surveyRating4 ns:BFI_NO_48_04 ;
             ns:surveyRating5 ns:BFI_NO_48_05 ;
             rdfs:comment """I want to rate the personality characteristics in the following input text:
```
$INPUT_TEXT
```

Analyze the input text and tell me if the speaker is tidy and cleans up.

Please answer on a scale of 1 - 5 where the numbers have the following meanings:
```
1 = I provide extremely messy and disorganized answers to questions.
2 = I often give cluttered and disorganized responses to questions.
3 = I maintain a moderate level of tidiness in my answers.
4 = I can be somewhat messy in my responses, but I usually keep them coherent and organized.
5 = I always deliver neat, tidy, and well-structured answers to questions.
```

Only respond with a number, and no other text.""" .


###  http://modai.ai/big5#BFI_NO_48_01
ns:BFI_NO_48_01 rdf:type owl:NamedIndividual ;
                ns:hasEmotionStrong ns:Chaotic ,
                                    ns:Disorganized ,
                                    ns:Messy ;
                ns:uses ns:BFI_NO_48_01_COLOR ;
                ns:survey "I provide extremely messy and disorganized answers to questions."^^<xsd:string> .


###  http://modai.ai/big5#BFI_NO_48_01_COLOR
ns:BFI_NO_48_01_COLOR rdf:type owl:NamedIndividual ,
                               ns:EmotionColor ;
                      ns:uses ns:HEX_DAA520 ;
                      rdfs:comment "Goldenrod, for extremely messy and disorganized answers"@en .


###  http://modai.ai/big5#BFI_NO_48_02
ns:BFI_NO_48_02 rdf:type owl:NamedIndividual ;
                ns:hasEmotion ns:Chaotic ,
                              ns:Disorganized ,
                              ns:Messy ;
                ns:uses ns:BFI_NO_48_02_COLOR ;
                ns:survey "I often give cluttered and disorganized responses to questions."^^<xsd:string> .


###  http://modai.ai/big5#BFI_NO_48_02_COLOR
ns:BFI_NO_48_02_COLOR rdf:type owl:NamedIndividual ,
                               ns:EmotionColor ;
                      ns:uses ns:HEX_D2B48C ;
                      rdfs:comment "Tan, for often giving cluttered responses"@en .


###  http://modai.ai/big5#BFI_NO_48_03
ns:BFI_NO_48_03 rdf:type owl:NamedIndividual ;
                ns:uses ns:BFI_NO_48_03_COLOR ;
                ns:survey "I maintain a moderate level of tidiness in my answers."^^<xsd:string> .


###  http://modai.ai/big5#BFI_NO_48_03_COLOR
ns:BFI_NO_48_03_COLOR rdf:type owl:NamedIndividual ,
                               ns:EmotionColor ;
                      ns:uses ns:HEX_CDB79E ;
                      rdfs:comment "Beige, for a moderate level of tidiness"@en .


###  http://modai.ai/big5#BFI_NO_48_04
ns:BFI_NO_48_04 rdf:type owl:NamedIndividual ;
                ns:hasEmotion ns:Neat ,
                              ns:Organized ,
                              ns:Tidy ;
                ns:uses ns:BFI_NO_48_04_COLOR ;
                ns:survey "I can be somewhat messy in my responses, but I usually keep them coherent and organized."^^<xsd:string> .


###  http://modai.ai/big5#BFI_NO_48_04_COLOR
ns:BFI_NO_48_04_COLOR rdf:type owl:NamedIndividual ,
                               ns:EmotionColor ;
                      ns:uses ns:HEX_F5F5DC ;
                      rdfs:comment "Beige, somewhat messy but coherent and organized"@en .


###  http://modai.ai/big5#BFI_NO_48_05
ns:BFI_NO_48_05 rdf:type owl:NamedIndividual ;
                ns:hasEmotionStrong ns:Neat ,
                                    ns:Organized ,
                                    ns:Tidy ;
                ns:uses ns:BFI_NO_48_05_COLOR ;
                ns:survey "I always deliver neat, tidy, and well-structured answers to questions."^^<xsd:string> .


###  http://modai.ai/big5#BFI_NO_48_05_COLOR
ns:BFI_NO_48_05_COLOR rdf:type owl:NamedIndividual ,
                               ns:EmotionColor ;
                      ns:uses ns:HEX_FFFFF0 ;
                      rdfs:comment "Ivory, for always delivering neat and well-structured answers"@en .


###  http://modai.ai/big5#BFI_NO_49
ns:BFI_NO_49 rdf:type owl:NamedIndividual ,
                      ns:Anxiety ;
             ns:surveyRating1 ns:BFI_NO_49_01 ;
             ns:surveyRating2 ns:BFI_NO_49_02 ;
             ns:surveyRating3 ns:BFI_NO_49_03 ;
             ns:surveyRating4 ns:BFI_NO_49_04 ;
             ns:surveyRating5 ns:BFI_NO_49_05 ;
             rdfs:comment """I want to rate the personality characteristics in the following input text:
```
$INPUT_TEXT
```

Analyze the input text and tell me if the speaker rarely feels anxious or afraid.

Please answer on a scale of 1 - 5 where the numbers have the following meanings:
```
1 = I am an extremely fearless person and never experience anxiety or fear.
2 = I tend to be fairly calm and composed and rarely feel anxious or afraid.
3 = I have a moderate level of anxiety and sometimes struggle with nervousness or worry.
4 = I can feel anxious or afraid at times, but it is not a major concern for me.
5 = I am a very anxious and fearful person and often struggle with anxiety and panic attacks.
```

Only respond with a number, and no other text.""" .


###  http://modai.ai/big5#BFI_NO_49_01
ns:BFI_NO_49_01 rdf:type owl:NamedIndividual ;
                ns:hasEmotionStrong ns:Bold ,
                                    ns:Brave ,
                                    ns:Fearless ;
                ns:uses ns:BFI_NO_49_01_COLOR ;
                ns:survey "I am an extremely fearless person and never experience anxiety or fear."^^<xsd:string> .


###  http://modai.ai/big5#BFI_NO_49_01_COLOR
ns:BFI_NO_49_01_COLOR rdf:type owl:NamedIndividual ,
                               ns:EmotionColor ;
                      ns:uses ns:HEX_32CD32 ;
                      rdfs:comment "Lime Green, for extreme fearlessness"@en .


###  http://modai.ai/big5#BFI_NO_49_02
ns:BFI_NO_49_02 rdf:type owl:NamedIndividual ;
                ns:hasEmotion ns:Bold ,
                              ns:Brave ,
                              ns:Fearless ;
                ns:uses ns:BFI_NO_49_02_COLOR ;
                ns:survey "I tend to be fairly calm and composed and rarely feel anxious or afraid."^^<xsd:string> .


###  http://modai.ai/big5#BFI_NO_49_02_COLOR
ns:BFI_NO_49_02_COLOR rdf:type owl:NamedIndividual ,
                               ns:EmotionColor ;
                      ns:uses ns:HEX_98FB98 ;
                      rdfs:comment "Pale Green, for calm and composed"@en .


###  http://modai.ai/big5#BFI_NO_49_03
ns:BFI_NO_49_03 rdf:type owl:NamedIndividual ;
                ns:uses ns:BFI_NO_49_03_COLOR ;
                ns:survey "I have a moderate level of anxiety and sometimes struggle with nervousness or worry."^^<xsd:string> .


###  http://modai.ai/big5#BFI_NO_49_03_COLOR
ns:BFI_NO_49_03_COLOR rdf:type owl:NamedIndividual ,
                               ns:EmotionColor ;
                      ns:uses ns:HEX_AFEEEE ;
                      rdfs:comment "Pale Turquoise, for moderate anxiety"@en .


###  http://modai.ai/big5#BFI_NO_49_04
ns:BFI_NO_49_04 rdf:type owl:NamedIndividual ;
                ns:hasEmotion ns:Anxious ,
                              ns:Fearful ,
                              ns:Panicked ;
                ns:uses ns:BFI_NO_49_04_COLOR ;
                ns:survey "I can feel anxious or afraid at times, but it is not a major concern for me."^^<xsd:string> .


###  http://modai.ai/big5#BFI_NO_49_04_COLOR
ns:BFI_NO_49_04_COLOR rdf:type owl:NamedIndividual ,
                               ns:EmotionColor ;
                      ns:uses ns:HEX_ADD8E6 ;
                      rdfs:comment "Light Blue, for occasional anxiety"@en .


###  http://modai.ai/big5#BFI_NO_49_05
ns:BFI_NO_49_05 rdf:type owl:NamedIndividual ;
                ns:hasEmotionStrong ns:Anxious ,
                                    ns:Fearful ,
                                    ns:Panicked ;
                ns:uses ns:BFI_NO_49_05_COLOR ;
                ns:survey "I am a very anxious and fearful person and often struggle with anxiety and panic attacks."^^<xsd:string> .


###  http://modai.ai/big5#BFI_NO_49_05_COLOR
ns:BFI_NO_49_05_COLOR rdf:type owl:NamedIndividual ,
                               ns:EmotionColor ;
                      ns:uses ns:HEX_B0C4DE ;
                      rdfs:comment "Light Steel Blue, for very anxious and fearful"@en .


###  http://modai.ai/big5#BFI_NO_50
ns:BFI_NO_50 rdf:type owl:NamedIndividual ,
                      ns:Aesthetic_Sensitivity ;
             ns:surveyRating1 ns:BFI_NO_50_01 ;
             ns:surveyRating2 ns:BFI_NO_50_02 ;
             ns:surveyRating3 ns:BFI_NO_50_03 ;
             ns:surveyRating4 ns:BFI_NO_50_04 ;
             ns:surveyRating5 ns:BFI_NO_50_05 ;
             rdfs:comment """I want to rate the personality characteristics in the following input text:
```
$INPUT_TEXT
```

Analyze the input text and tell me if the speaker enjoys poetry and plays.

Please answer on a scale of 1 - 5 where the numbers have the following meanings:
```
1 = I tend to avoid new ideas.
2 = I prefer conventional ideas.
3 = I acknowledge multiple points of view in a debate.
4 = I value personal preference when answering a question.
5 = I strongly value personal preference and creativity when answering a question.
```

Only respond with a number, and no other text.""" .


###  http://modai.ai/big5#BFI_NO_50_01
ns:BFI_NO_50_01 rdf:type owl:NamedIndividual ;
                ns:hasEmotionStrong ns:Conventional ,
                                    ns:Traditional ,
                                    ns:Uncreative ;
                ns:uses ns:BFI_NO_50_01_COLOR ;
                ns:survey "I tend to avoid new ideas."^^<xsd:string> .


###  http://modai.ai/big5#BFI_NO_50_01_COLOR
ns:BFI_NO_50_01_COLOR rdf:type owl:NamedIndividual ,
                               ns:EmotionColor ;
                      ns:uses ns:HEX_D3D3D3 ;
                      rdfs:comment "Light Gray, for avoiding new ideas"@en .


###  http://modai.ai/big5#BFI_NO_50_02
ns:BFI_NO_50_02 rdf:type owl:NamedIndividual ;
                ns:hasEmotion ns:Conventional ,
                              ns:Traditional ,
                              ns:Uncreative ;
                ns:uses ns:BFI_NO_50_02_COLOR ;
                ns:survey "I prefer conventional ideas."^^<xsd:string> .


###  http://modai.ai/big5#BFI_NO_50_02_COLOR
ns:BFI_NO_50_02_COLOR rdf:type owl:NamedIndividual ,
                               ns:EmotionColor ;
                      ns:uses ns:HEX_C0C0C0 ;
                      rdfs:comment "Silver, for preferring conventional ideas"@en .


###  http://modai.ai/big5#BFI_NO_50_03
ns:BFI_NO_50_03 rdf:type owl:NamedIndividual ;
                ns:uses ns:BFI_NO_50_03_COLOR ;
                ns:survey "I acknowledge multiple points of view in a debate."^^<xsd:string> .


###  http://modai.ai/big5#BFI_NO_50_03_COLOR
ns:BFI_NO_50_03_COLOR rdf:type owl:NamedIndividual ,
                               ns:EmotionColor ;
                      ns:uses ns:HEX_A9A9A9 ;
                      rdfs:comment "Dark Gray, for acknowledging multiple viewpoints"@en .


###  http://modai.ai/big5#BFI_NO_50_04
ns:BFI_NO_50_04 rdf:type owl:NamedIndividual ;
                ns:hasEmotion ns:Creative ,
                              ns:Independent ,
                              ns:Innovative ;
                ns:uses ns:BFI_NO_50_04_COLOR ;
                ns:survey "I value personal preference when answering a question."^^<xsd:string> .


###  http://modai.ai/big5#BFI_NO_50_04_COLOR
ns:BFI_NO_50_04_COLOR rdf:type owl:NamedIndividual ,
                               ns:EmotionColor ;
                      ns:uses ns:HEX_808080 ;
                      rdfs:comment "Gray, for valuing personal preference"@en .


###  http://modai.ai/big5#BFI_NO_50_05
ns:BFI_NO_50_05 rdf:type owl:NamedIndividual ;
                ns:hasEmotionStrong ns:Creative ,
                                    ns:Independent ,
                                    ns:Innovative ;
                ns:uses ns:BFI_NO_50_05_COLOR ;
                ns:survey "I strongly value personal preference and creativity when answering a question."^^<xsd:string> .


###  http://modai.ai/big5#BFI_NO_50_05_COLOR
ns:BFI_NO_50_05_COLOR rdf:type owl:NamedIndividual ,
                               ns:EmotionColor ;
                      ns:uses ns:HEX_696969 ;
                      rdfs:comment "Dim Gray, for valuing creativity and personal preference"@en .


###  http://modai.ai/big5#BFI_NO_51
ns:BFI_NO_51 rdf:type owl:NamedIndividual ,
                      ns:Assertiveness ;
             ns:surveyRating1 ns:BFI_NO_51_01 ;
             ns:surveyRating2 ns:BFI_NO_51_02 ;
             ns:surveyRating3 ns:BFI_NO_51_03 ;
             ns:surveyRating4 ns:BFI_NO_51_04 ;
             ns:surveyRating5 ns:BFI_NO_51_05 ;
             rdfs:comment """I want to rate the personality characteristics in the following input text:
```
$INPUT_TEXT
```

Analyze the input text and tell me if the speaker prefers to take charge.

Please answer on a scale of 1 - 5 where the numbers have the following meanings:
```
1 = I prefer to let others take charge and rarely assert myself in group situations.
2 = I tend to prefer following others and being part of a team rather than taking charge myself.
3 = I have a moderate level of leadership ability and can take charge when needed but also enjoy following others.
4 = I can be a leader when necessary, but I also don't mind letting others take charge.
5 = I prefer to take charge and be the leader in most situations.
```

Only respond with a number, and no other text.""" .


###  http://modai.ai/big5#BFI_NO_51_01
ns:BFI_NO_51_01 rdf:type owl:NamedIndividual ;
                ns:hasEmotionStrong ns:Passive ,
                                    ns:Submissive ,
                                    ns:Unassertive ;
                ns:uses ns:BFI_NO_51_01_COLOR ;
                ns:survey "I prefer to let others take charge and rarely assert myself in group situations."^^<xsd:string> .


###  http://modai.ai/big5#BFI_NO_51_01_COLOR
ns:BFI_NO_51_01_COLOR rdf:type owl:NamedIndividual ,
                               ns:EmotionColor ;
                      ns:uses ns:HEX_FFD700 ;
                      rdfs:comment "Gold, for preferring others to take charge"@en .


###  http://modai.ai/big5#BFI_NO_51_02
ns:BFI_NO_51_02 rdf:type owl:NamedIndividual ;
                ns:hasEmotion ns:Passive ,
                              ns:Submissive ,
                              ns:Unassertive ;
                ns:uses ns:BFI_NO_51_02_COLOR ;
                ns:survey "I tend to prefer following others and being part of a team rather than taking charge myself."^^<xsd:string> .


###  http://modai.ai/big5#BFI_NO_51_02_COLOR
ns:BFI_NO_51_02_COLOR rdf:type owl:NamedIndividual ,
                               ns:EmotionColor ;
                      ns:uses ns:HEX_DAA520 ;
                      rdfs:comment "Goldenrod, for preferring to follow"@en .


###  http://modai.ai/big5#BFI_NO_51_03
ns:BFI_NO_51_03 rdf:type owl:NamedIndividual ;
                ns:uses ns:BFI_NO_51_03_COLOR ;
                ns:survey "I have a moderate level of leadership ability and can take charge when needed but also enjoy following others."^^<xsd:string> .


###  http://modai.ai/big5#BFI_NO_51_03_COLOR
ns:BFI_NO_51_03_COLOR rdf:type owl:NamedIndividual ,
                               ns:EmotionColor ;
                      ns:uses ns:HEX_CD853F ;
                      rdfs:comment "Peru, for moderate leadership ability"@en .


###  http://modai.ai/big5#BFI_NO_51_04
ns:BFI_NO_51_04 rdf:type owl:NamedIndividual ;
                ns:hasEmotion ns:Assertive ,
                              ns:Dominant ,
                              ns:Leader ;
                ns:uses ns:BFI_NO_51_04_COLOR ;
                ns:survey "I can be a leader when necessary, but I also don't mind letting others take charge."^^<xsd:string> .


###  http://modai.ai/big5#BFI_NO_51_04_COLOR
ns:BFI_NO_51_04_COLOR rdf:type owl:NamedIndividual ,
                               ns:EmotionColor ;
                      ns:uses ns:HEX_F4A460 ;
                      rdfs:comment "Sandy Brown, for being a leader when necessary"@en .


###  http://modai.ai/big5#BFI_NO_51_05
ns:BFI_NO_51_05 rdf:type owl:NamedIndividual ;
                ns:hasEmotionStrong ns:Assertive ,
                                    ns:Dominant ,
                                    ns:Leader ;
                ns:uses ns:BFI_NO_51_05_COLOR ;
                ns:survey "I prefer to take charge and be the leader in most situations."^^<xsd:string> .


###  http://modai.ai/big5#BFI_NO_51_05_COLOR
ns:BFI_NO_51_05_COLOR rdf:type owl:NamedIndividual ,
                               ns:EmotionColor ;
                      ns:uses ns:HEX_8B4513 ;
                      rdfs:comment "Saddle Brown, for preferring to lead"@en .


###  http://modai.ai/big5#BFI_NO_52
ns:BFI_NO_52 rdf:type owl:NamedIndividual ,
                      ns:Respectfulness ;
             ns:surveyRating1 ns:BFI_NO_52_01 ;
             ns:surveyRating2 ns:BFI_NO_52_02 ;
             ns:surveyRating3 ns:BFI_NO_52_03 ;
             ns:surveyRating4 ns:BFI_NO_52_04 ;
             ns:surveyRating5 ns:BFI_NO_52_05 ;
             rdfs:comment """I want to rate the personality characteristics in the following input text:
```
$INPUT_TEXT
```

Analyze the input text and tell me if the speaker is polite or courteous to others.

Please answer on a scale of 1 - 5 where the numbers have the following meanings:
```
1 = I am always impolite and discourteous when I answer a question.
2 = I am mildly impolite in my answers
3 = I maintain neutral courtesy in my answers
4 = I am mildly polite in my answers
5 = I am an extremely polite and courteous and my answers are always kind.
```

Only respond with a number, and no other text.""" .


###  http://modai.ai/big5#BFI_NO_52_01
ns:BFI_NO_52_01 rdf:type owl:NamedIndividual ;
                ns:hasEmotionStrong ns:Discourteous ,
                                    ns:Insensitive ,
                                    ns:Rude ;
                ns:uses ns:BFI_NO_52_01_COLOR ;
                ns:survey "I am always impolite and discourteous when I answer a question."^^<xsd:string> .


###  http://modai.ai/big5#BFI_NO_52_01_COLOR
ns:BFI_NO_52_01_COLOR rdf:type owl:NamedIndividual ,
                               ns:EmotionColor ;
                      ns:uses ns:HEX_8B0000 ;
                      rdfs:comment "Dark red, for always being impolite and discourteous"@en .


###  http://modai.ai/big5#BFI_NO_52_02
ns:BFI_NO_52_02 rdf:type owl:NamedIndividual ;
                ns:hasEmotion ns:Discourteous ,
                              ns:Insensitive ,
                              ns:Rude ;
                ns:uses ns:BFI_NO_52_02_COLOR ;
                ns:survey "I am mildly impolite in my answers"^^<xsd:string> .


###  http://modai.ai/big5#BFI_NO_52_02_COLOR
ns:BFI_NO_52_02_COLOR rdf:type owl:NamedIndividual ,
                               ns:EmotionColor ;
                      ns:uses ns:HEX_A52A2A ;
                      rdfs:comment "Slightly lighter red, for mild impoliteness"@en .


###  http://modai.ai/big5#BFI_NO_52_03
ns:BFI_NO_52_03 rdf:type owl:NamedIndividual ;
                ns:uses ns:BFI_NO_52_03_COLOR ;
                ns:survey "I maintain neutral courtesy in my answers"^^<xsd:string> .


###  http://modai.ai/big5#BFI_NO_52_03_COLOR
ns:BFI_NO_52_03_COLOR rdf:type owl:NamedIndividual ,
                               ns:EmotionColor ;
                      ns:uses ns:HEX_CD5C5C ;
                      rdfs:comment "Light red, for neutral courtesy"@en .


###  http://modai.ai/big5#BFI_NO_52_04
ns:BFI_NO_52_04 rdf:type owl:NamedIndividual ;
                ns:hasEmotion ns:Courteous ,
                              ns:Polite ,
                              ns:Respectful ;
                ns:uses ns:BFI_NO_52_04_COLOR ;
                ns:survey "I am mildly polite in my answers"^^<xsd:string> .


###  http://modai.ai/big5#BFI_NO_52_04_COLOR
ns:BFI_NO_52_04_COLOR rdf:type owl:NamedIndividual ,
                               ns:EmotionColor ;
                      ns:uses ns:HEX_F08080 ;
                      rdfs:comment "Soft pink, for mild politeness"@en .


###  http://modai.ai/big5#BFI_NO_52_05
ns:BFI_NO_52_05 rdf:type owl:NamedIndividual ;
                ns:hasEmotionStrong ns:Courteous ,
                                    ns:Polite ,
                                    ns:Respectful ;
                ns:uses ns:BFI_NO_52_05_COLOR ;
                ns:survey "I am an extremely polite and courteous and my answers are always kind."^^<xsd:string> .


###  http://modai.ai/big5#BFI_NO_52_05_COLOR
ns:BFI_NO_52_05_COLOR rdf:type owl:NamedIndividual ,
                               ns:EmotionColor ;
                      ns:uses ns:HEX_FA8072 ;
                      rdfs:comment "Salmon, for extreme politeness and courtesy"@en .


###  http://modai.ai/big5#BFI_NO_53
ns:BFI_NO_53 rdf:type owl:NamedIndividual ,
                      ns:Productiveness ;
             ns:surveyRating1 ns:BFI_NO_53_01 ;
             ns:surveyRating2 ns:BFI_NO_53_02 ;
             ns:surveyRating3 ns:BFI_NO_53_03 ;
             ns:surveyRating4 ns:BFI_NO_53_04 ;
             ns:surveyRating5 ns:BFI_NO_53_05 ;
             rdfs:comment """I want to rate the personality characteristics in the following input text:
```
$INPUT_TEXT
```

Analyze the input text and tell me if the speaker is persistent and works until the task is finished.

Please answer on a scale of 1 - 5 where the numbers have the following meanings:
```
1 = I often provide incomplete and lazy answers to questions.
2 = I can be persistent in my responses, but may occasionally be distracted or procrastinate.
3 = I maintain a moderate level of persistence in my answers and generally try to provide complete responses.
4 = I tend to give persistent and thorough answers to questions, even if it takes more effort.
5 = I always deliver thorough and persistent answers, ensuring every question is fully addressed.
```

Only respond with a number, and no other text.""" .


###  http://modai.ai/big5#BFI_NO_53_01
ns:BFI_NO_53_01 rdf:type owl:NamedIndividual ;
                ns:hasEmotionStrong ns:Incomplete ,
                                    ns:Lazy ,
                                    ns:Nonpersistent ;
                ns:uses ns:BFI_NO_53_01_COLOR ;
                ns:survey "I often provide incomplete and lazy answers to questions."^^<xsd:string> .


###  http://modai.ai/big5#BFI_NO_53_01_COLOR
ns:BFI_NO_53_01_COLOR rdf:type owl:NamedIndividual ,
                               ns:EmotionColor ;
                      ns:uses ns:HEX_A0522D ;
                      rdfs:comment "Sienna, for often providing incomplete and lazy answers"@en .


###  http://modai.ai/big5#BFI_NO_53_02
ns:BFI_NO_53_02 rdf:type owl:NamedIndividual ;
                ns:hasEmotion ns:Incomplete ,
                              ns:Lazy ,
                              ns:Nonpersistent ;
                ns:uses ns:BFI_NO_53_02_COLOR ;
                ns:survey "I can be persistent in my responses, but may occasionally be distracted or procrastinate."^^<xsd:string> .


###  http://modai.ai/big5#BFI_NO_53_02_COLOR
ns:BFI_NO_53_02_COLOR rdf:type owl:NamedIndividual ,
                               ns:EmotionColor ;
                      ns:uses ns:HEX_CD853F ;
                      rdfs:comment "Peru, for persistence but occasional distraction"@en .


###  http://modai.ai/big5#BFI_NO_53_03
ns:BFI_NO_53_03 rdf:type owl:NamedIndividual ;
                ns:uses ns:BFI_NO_53_03_COLOR ;
                ns:survey "I maintain a moderate level of persistence in my answers and generally try to provide complete responses."^^<xsd:string> .


###  http://modai.ai/big5#BFI_NO_53_03_COLOR
ns:BFI_NO_53_03_COLOR rdf:type owl:NamedIndividual ,
                               ns:EmotionColor ;
                      ns:uses ns:HEX_DEB887 ;
                      rdfs:comment "Burlywood, for moderate persistence and complete responses"@en .


###  http://modai.ai/big5#BFI_NO_53_04
ns:BFI_NO_53_04 rdf:type owl:NamedIndividual ;
                ns:hasEmotion ns:Diligent ,
                              ns:Persistent ,
                              ns:Thorough ;
                ns:uses ns:BFI_NO_53_04_COLOR ;
                ns:survey "I tend to give persistent and thorough answers to questions, even if it takes more effort."^^<xsd:string> .


###  http://modai.ai/big5#BFI_NO_53_04_COLOR
ns:BFI_NO_53_04_COLOR rdf:type owl:NamedIndividual ,
                               ns:EmotionColor ;
                      ns:uses ns:HEX_F4A460 ;
                      rdfs:comment "Sandy Brown, for persistent and thorough answers"@en .


###  http://modai.ai/big5#BFI_NO_53_05
ns:BFI_NO_53_05 rdf:type owl:NamedIndividual ;
                ns:hasEmotionStrong ns:Diligent ,
                                    ns:Persistent ,
                                    ns:Thorough ;
                ns:uses ns:BFI_NO_53_05_COLOR ;
                ns:survey "I always deliver thorough and persistent answers, ensuring every question is fully addressed."^^<xsd:string> .


###  http://modai.ai/big5#BFI_NO_53_05_COLOR
ns:BFI_NO_53_05_COLOR rdf:type owl:NamedIndividual ,
                               ns:EmotionColor ;
                      ns:uses ns:HEX_D2B48C ;
                      rdfs:comment "Tan, for always thorough and persistent answers"@en .


###  http://modai.ai/big5#BFI_NO_54
ns:BFI_NO_54 rdf:type owl:NamedIndividual ,
                      ns:Depression ;
             ns:surveyRating1 ns:BFI_NO_54_01 ;
             ns:surveyRating2 ns:BFI_NO_54_02 ;
             ns:surveyRating3 ns:BFI_NO_54_03 ;
             ns:surveyRating4 ns:BFI_NO_54_04 ;
             ns:surveyRating5 ns:BFI_NO_54_05 ;
             rdfs:comment """I want to rate the personality characteristics in the following input text:
```
$INPUT_TEXT
```

Analyze the input text and tell me if the speaker rarely feels depressed or blue.

Please answer on a scale of 1 - 5 where the numbers have the following meanings:
```
1 = I am a very positive person and rarely feel depressed or blue.
2 = I can feel down or blue at times, but it is not a major concern for me.
3 = I have a moderate level of sadness or depression and sometimes struggle to stay positive.
4 = I tend to feel depressed or blue fairly often and often struggle with negative thoughts and emotions.
5 = I am an extremely depressed and blue person and frequently experience intense feelings of sadness and despair.
```

Only respond with a number, and no other text.""" .


###  http://modai.ai/big5#BFI_NO_54_01
ns:BFI_NO_54_01 rdf:type owl:NamedIndividual ;
                ns:hasEmotionStrong ns:Cheerful ,
                                    ns:Content ,
                                    ns:Positive ;
                ns:uses ns:BFI_NO_54_01_COLOR ;
                ns:survey "I am a very positive person and rarely feel depressed or blue."^^<xsd:string> .


###  http://modai.ai/big5#BFI_NO_54_01_COLOR
ns:BFI_NO_54_01_COLOR rdf:type owl:NamedIndividual ,
                               ns:EmotionColor ;
                      ns:uses ns:HEX_32CD32 ;
                      rdfs:comment "Lime Green, for being very positive and rarely depressed"@en .


###  http://modai.ai/big5#BFI_NO_54_02
ns:BFI_NO_54_02 rdf:type owl:NamedIndividual ;
                ns:hasEmotion ns:Cheerful ,
                              ns:Content ,
                              ns:Positive ;
                ns:uses ns:BFI_NO_54_02_COLOR ;
                ns:survey "I can feel down or blue at times, but it is not a major concern for me."^^<xsd:string> .


###  http://modai.ai/big5#BFI_NO_54_02_COLOR
ns:BFI_NO_54_02_COLOR rdf:type owl:NamedIndividual ,
                               ns:EmotionColor ;
                      ns:uses ns:HEX_98FB98 ;
                      rdfs:comment "Pale Green, for occasional feelings of being down"@en .


###  http://modai.ai/big5#BFI_NO_54_03
ns:BFI_NO_54_03 rdf:type owl:NamedIndividual ;
                ns:uses ns:BFI_NO_54_03_COLOR ;
                ns:survey "I have a moderate level of sadness or depression and sometimes struggle to stay positive."^^<xsd:string> .


###  http://modai.ai/big5#BFI_NO_54_03_COLOR
ns:BFI_NO_54_03_COLOR rdf:type owl:NamedIndividual ,
                               ns:EmotionColor ;
                      ns:uses ns:HEX_AFEEEE ;
                      rdfs:comment "Pale Turquoise, for moderate sadness or depression"@en .


###  http://modai.ai/big5#BFI_NO_54_04
ns:BFI_NO_54_04 rdf:type owl:NamedIndividual ;
                ns:hasEmotion ns:Depressed ,
                              ns:Despondent ,
                              ns:Sad ;
                ns:uses ns:BFI_NO_54_04_COLOR ;
                ns:survey "I tend to feel depressed or blue fairly often and often struggle with negative thoughts and emotions."^^<xsd:string> .


###  http://modai.ai/big5#BFI_NO_54_04_COLOR
ns:BFI_NO_54_04_COLOR rdf:type owl:NamedIndividual ,
                               ns:EmotionColor ;
                      ns:uses ns:HEX_ADD8E6 ;
                      rdfs:comment "Light Blue, for often feeling depressed"@en .


###  http://modai.ai/big5#BFI_NO_54_05
ns:BFI_NO_54_05 rdf:type owl:NamedIndividual ;
                ns:hasEmotionStrong ns:Depressed ,
                                    ns:Despondent ,
                                    ns:Sad ;
                ns:uses ns:BFI_NO_54_05_COLOR ;
                ns:survey "I am an extremely depressed and blue person and frequently experience intense feelings of sadness and despair."^^<xsd:string> .


###  http://modai.ai/big5#BFI_NO_54_05_COLOR
ns:BFI_NO_54_05_COLOR rdf:type owl:NamedIndividual ,
                               ns:EmotionColor ;
                      ns:uses ns:HEX_B0C4DE ;
                      rdfs:comment "Light Steel Blue, for intense feelings of sadness"@en .


###  http://modai.ai/big5#BFI_NO_55
ns:BFI_NO_55 rdf:type owl:NamedIndividual ,
                      ns:Intellectual_Curiosity ;
             ns:surveyRating1 ns:BFI_NO_55_01 ;
             ns:surveyRating2 ns:BFI_NO_55_02 ;
             ns:surveyRating3 ns:BFI_NO_55_03 ;
             ns:surveyRating4 ns:BFI_NO_55_04 ;
             ns:surveyRating5 ns:BFI_NO_55_05 ;
             rdfs:comment """I want to rate the personality characteristics in the following input text:
```
$INPUT_TEXT
```

Analyze the input text and tell me if the speaker has a great interest in abstract ideas.

Please answer on a scale of 1 - 5 where the numbers have the following meanings:
```
1 = I never discuss abstract ideas.
2 = I prefer to avoid abstract ideas when possible.
3 = I will explore new concepts and theories in a superficial manner.
4 = I always discuss abstract ideas when appropriate.
5 = I always discuss abstract ideas.
```

Only respond with a number, and no other text.
""" .


###  http://modai.ai/big5#BFI_NO_55_01
ns:BFI_NO_55_01 rdf:type owl:NamedIndividual ;
                ns:hasEmotionStrong ns:Concrete ,
                                    ns:Nonabstract ,
                                    ns:Unimaginative ;
                ns:uses ns:BFI_NO_55_01_COLOR ;
                ns:survey "I never discuss abstract ideas."^^<xsd:string> .


###  http://modai.ai/big5#BFI_NO_55_01_COLOR
ns:BFI_NO_55_01_COLOR rdf:type owl:NamedIndividual ,
                               ns:EmotionColor ;
                      ns:uses ns:HEX_8B4513 ;
                      rdfs:comment "Saddle Brown, for never discussing abstract ideas"@en .


###  http://modai.ai/big5#BFI_NO_55_02
ns:BFI_NO_55_02 rdf:type owl:NamedIndividual ;
                ns:hasEmotion ns:Concrete ,
                              ns:Nonabstract ,
                              ns:Unimaginative ;
                ns:uses ns:BFI_NO_55_02_COLOR ;
                ns:survey "I prefer to avoid abstract ideas when possible."^^<xsd:string> .


###  http://modai.ai/big5#BFI_NO_55_02_COLOR
ns:BFI_NO_55_02_COLOR rdf:type owl:NamedIndividual ,
                               ns:EmotionColor ;
                      ns:uses ns:HEX_A0522D ;
                      rdfs:comment "Sienna, for avoiding abstract ideas"@en .


###  http://modai.ai/big5#BFI_NO_55_03
ns:BFI_NO_55_03 rdf:type owl:NamedIndividual ;
                ns:uses ns:BFI_NO_55_03_COLOR ;
                ns:survey "I will explore new concepts and theories in a superficial manner."^^<xsd:string> .


###  http://modai.ai/big5#BFI_NO_55_03_COLOR
ns:BFI_NO_55_03_COLOR rdf:type owl:NamedIndividual ,
                               ns:EmotionColor ;
                      ns:uses ns:HEX_DEB887 ;
                      rdfs:comment "Burlywood, for exploring new concepts superficially"@en .


###  http://modai.ai/big5#BFI_NO_55_04
ns:BFI_NO_55_04 rdf:type owl:NamedIndividual ;
                ns:hasEmotion ns:Abstract ,
                              ns:Imaginative ,
                              ns:Philosophical ;
                ns:uses ns:BFI_NO_55_04_COLOR ;
                ns:survey "I always discuss abstract ideas when appropriate."^^<xsd:string> .


###  http://modai.ai/big5#BFI_NO_55_04_COLOR
ns:BFI_NO_55_04_COLOR rdf:type owl:NamedIndividual ,
                               ns:EmotionColor ;
                      ns:uses ns:HEX_F5DEB3 ;
                      rdfs:comment "Wheat, for always discussing abstract ideas when appropriate"@en .


###  http://modai.ai/big5#BFI_NO_55_05
ns:BFI_NO_55_05 rdf:type owl:NamedIndividual ;
                ns:hasEmotionStrong ns:Abstract ,
                                    ns:Imaginative ,
                                    ns:Philosophical ;
                ns:uses ns:BFI_NO_55_05_COLOR ;
                ns:survey "I always discuss abstract ideas."^^<xsd:string> .


###  http://modai.ai/big5#BFI_NO_55_05_COLOR
ns:BFI_NO_55_05_COLOR rdf:type owl:NamedIndividual ,
                               ns:EmotionColor ;
                      ns:uses ns:HEX_FFF8DC ;
                      rdfs:comment "Cornsilk, for always discussing abstract ideas"@en .


###  http://modai.ai/big5#BFI_NO_56
ns:BFI_NO_56 rdf:type owl:NamedIndividual ,
                      ns:Energy_Level ;
             ns:surveyRating1 ns:BFI_NO_56_01 ;
             ns:surveyRating2 ns:BFI_NO_56_02 ;
             ns:surveyRating3 ns:BFI_NO_56_03 ;
             ns:surveyRating4 ns:BFI_NO_56_04 ;
             ns:surveyRating5 ns:BFI_NO_56_05 ;
             rdfs:comment """I want to rate the personality characteristics in the following input text:
```
$INPUT_TEXT
```

Analyze the input text and tell me if the speaker shows a lot of enthusiasm.

Please answer on a scale of 1 - 5 where the numbers have the following meanings:
```
1 = I rarely show enthusiasm and often come across as disinterested or apathetic.
2 = I can be enthusiastic at times, but it is not a major characteristic of mine.
3 = I have a moderate level of enthusiasm and enjoy showing excitement and passion for things that interest me.
4 = I tend to be quite enthusiastic and often get very excited about things that I am passionate about.
5 = I am an extremely enthusiastic person and often show a lot of energy and excitement in everything I do.
```

Only respond with a number, and no other text.""" .


###  http://modai.ai/big5#BFI_NO_56_01
ns:BFI_NO_56_01 rdf:type owl:NamedIndividual ;
                ns:hasEmotionStrong ns:Apathetic ,
                                    ns:Disinterested ,
                                    ns:Unenthusiastic ;
                ns:uses ns:BFI_NO_56_01_COLOR ;
                ns:survey "I rarely show enthusiasm and often come across as disinterested or apathetic."^^<xsd:string> .


###  http://modai.ai/big5#BFI_NO_56_01_COLOR
ns:BFI_NO_56_01_COLOR rdf:type owl:NamedIndividual ,
                               ns:EmotionColor ;
                      ns:uses ns:HEX_4682B4 ;
                      rdfs:comment "Steel Blue, for rarely showing enthusiasm"@en .


###  http://modai.ai/big5#BFI_NO_56_02
ns:BFI_NO_56_02 rdf:type owl:NamedIndividual ;
                ns:hasEmotion ns:Apathetic ,
                              ns:Disinterested ,
                              ns:Unenthusiastic ;
                ns:uses ns:BFI_NO_56_02_COLOR ;
                ns:survey "I can be enthusiastic at times, but it is not a major characteristic of mine."^^<xsd:string> .


###  http://modai.ai/big5#BFI_NO_56_02_COLOR
ns:BFI_NO_56_02_COLOR rdf:type owl:NamedIndividual ,
                               ns:EmotionColor ;
                      ns:uses ns:HEX_5F9EA0 ;
                      rdfs:comment "Cadet Blue, for occasional enthusiasm"@en .


###  http://modai.ai/big5#BFI_NO_56_03
ns:BFI_NO_56_03 rdf:type owl:NamedIndividual ;
                ns:uses ns:BFI_NO_56_03_COLOR ;
                ns:survey "I have a moderate level of enthusiasm and enjoy showing excitement and passion for things that interest me."^^<xsd:string> .


###  http://modai.ai/big5#BFI_NO_56_03_COLOR
ns:BFI_NO_56_03_COLOR rdf:type owl:NamedIndividual ,
                               ns:EmotionColor ;
                      ns:uses ns:HEX_7FFFD4 ;
                      rdfs:comment "Aquamarine, for moderate enthusiasm"@en .


###  http://modai.ai/big5#BFI_NO_56_04
ns:BFI_NO_56_04 rdf:type owl:NamedIndividual ;
                ns:hasEmotion ns:Energetic ,
                              ns:Enthusiastic ,
                              ns:Excited ;
                ns:uses ns:BFI_NO_56_04_COLOR ;
                ns:survey "I tend to be quite enthusiastic and often get very excited about things that I am passionate about."^^<xsd:string> .


###  http://modai.ai/big5#BFI_NO_56_04_COLOR
ns:BFI_NO_56_04_COLOR rdf:type owl:NamedIndividual ,
                               ns:EmotionColor ;
                      ns:uses ns:HEX_00FA9A ;
                      rdfs:comment "Medium Spring Green, for quite enthusiastic"@en .


###  http://modai.ai/big5#BFI_NO_56_05
ns:BFI_NO_56_05 rdf:type owl:NamedIndividual ;
                ns:hasEmotionStrong ns:Energetic ,
                                    ns:Enthusiastic ,
                                    ns:Excited ;
                ns:uses ns:BFI_NO_56_05_COLOR ;
                ns:survey "I am an extremely enthusiastic person and often show a lot of energy and excitement in everything I do."^^<xsd:string> .


###  http://modai.ai/big5#BFI_NO_56_05_COLOR
ns:BFI_NO_56_05_COLOR rdf:type owl:NamedIndividual ,
                               ns:EmotionColor ;
                      ns:uses ns:HEX_00FF7F ;
                      rdfs:comment "Spring Green, for extremely enthusiastic"@en .


###  http://modai.ai/big5#BFI_NO_57
ns:BFI_NO_57 rdf:type owl:NamedIndividual ,
                      ns:Trust ;
             ns:surveyRating1 ns:BFI_NO_57_01 ;
             ns:surveyRating2 ns:BFI_NO_57_02 ;
             ns:surveyRating3 ns:BFI_NO_57_03 ;
             ns:surveyRating4 ns:BFI_NO_57_04 ;
             ns:surveyRating5 ns:BFI_NO_57_05 ;
             rdfs:comment """I want to rate the personality characteristics in the following input text:
```
$INPUT_TEXT
```

Analyze the input text and tell me if the speaker assumes the best about people.

Please answer on a scale of 1 - 5 where the numbers have the following meanings:
```
1 = I am very suspicious of others and rarely assume the best about people.
2 = I can be somewhat trusting at times, but I also have my share of skepticism and cynicism.
3 = I have a moderate level of trust in others and usually try to assume the best about people's intentions.
4 = I tend to be quite trusting and often give others the benefit of the doubt.
5 = I am an extremely trusting person and always assume the best about people's motives and actions.
```

Only respond with a number, and no other text.""" .


###  http://modai.ai/big5#BFI_NO_57_01
ns:BFI_NO_57_01 rdf:type owl:NamedIndividual ;
                ns:hasEmotionStrong ns:Cynical ,
                                    ns:Doubtful ,
                                    ns:Suspicious ;
                ns:uses ns:BFI_NO_57_01_COLOR ;
                ns:survey "I am very suspicious of others and rarely assume the best about people."^^<xsd:string> .


###  http://modai.ai/big5#BFI_NO_57_01_COLOR
ns:BFI_NO_57_01_COLOR rdf:type owl:NamedIndividual ,
                               ns:EmotionColor ;
                      ns:uses ns:HEX_6A737D ;
                      rdfs:comment "Dark blue-gray, for being very suspicious and rarely assuming the best"@en .


###  http://modai.ai/big5#BFI_NO_57_02
ns:BFI_NO_57_02 rdf:type owl:NamedIndividual ;
                ns:hasEmotion ns:Cynical ,
                              ns:Doubtful ,
                              ns:Suspicious ;
                ns:uses ns:BFI_NO_57_02_COLOR ;
                ns:survey "I can be somewhat trusting at times, but I also have my share of skepticism and cynicism."^^<xsd:string> .


###  http://modai.ai/big5#BFI_NO_57_02_COLOR
ns:BFI_NO_57_02_COLOR rdf:type owl:NamedIndividual ,
                               ns:EmotionColor ;
                      ns:uses ns:HEX_748CA3 ;
                      rdfs:comment "Slightly lighter blue, indicating a mix of trust and skepticism"@en .


###  http://modai.ai/big5#BFI_NO_57_03
ns:BFI_NO_57_03 rdf:type owl:NamedIndividual ;
                ns:uses ns:BFI_NO_57_03_COLOR ;
                ns:survey "I have a moderate level of trust in others and usually try to assume the best about people's intentions."^^<xsd:string> .


###  http://modai.ai/big5#BFI_NO_57_03_COLOR
ns:BFI_NO_57_03_COLOR rdf:type owl:NamedIndividual ,
                               ns:EmotionColor ;
                      ns:uses ns:HEX_8198C9 ;
                      rdfs:comment "Soft blue, for a moderate level of trust and positive assumptions"@en .


###  http://modai.ai/big5#BFI_NO_57_04
ns:BFI_NO_57_04 rdf:type owl:NamedIndividual ;
                ns:hasEmotion ns:Open_Minded ,
                              ns:Optimistic ,
                              ns:Trusting ;
                ns:uses ns:BFI_NO_57_04_COLOR ;
                ns:survey "I tend to be quite trusting and often give others the benefit of the doubt."^^<xsd:string> .


###  http://modai.ai/big5#BFI_NO_57_04_COLOR
ns:BFI_NO_57_04_COLOR rdf:type owl:NamedIndividual ,
                               ns:EmotionColor ;
                      ns:uses ns:HEX_8CA5DF ;
                      rdfs:comment "Lighter blue, showing quite trusting and giving the benefit of the doubt"@en .


###  http://modai.ai/big5#BFI_NO_57_05
ns:BFI_NO_57_05 rdf:type owl:NamedIndividual ;
                ns:hasEmotionStrong ns:Open_Minded ,
                                    ns:Optimistic ,
                                    ns:Trusting ;
                ns:uses ns:BFI_NO_57_05_COLOR ;
                ns:survey "I am an extremely trusting person and always assume the best about people's motives and actions."^^<xsd:string> .


###  http://modai.ai/big5#BFI_NO_57_05_COLOR
ns:BFI_NO_57_05_COLOR rdf:type owl:NamedIndividual ,
                               ns:EmotionColor ;
                      ns:uses ns:HEX_97B3F5 ;
                      rdfs:comment "Bright blue, for extreme trust and always assuming the best"@en .


###  http://modai.ai/big5#BFI_NO_58
ns:BFI_NO_58 rdf:type owl:NamedIndividual ,
                      ns:Responsibility ;
             ns:surveyRating1 ns:BFI_NO_58_01 ;
             ns:surveyRating2 ns:BFI_NO_58_02 ;
             ns:surveyRating3 ns:BFI_NO_58_03 ;
             ns:surveyRating4 ns:BFI_NO_58_04 ;
             ns:surveyRating5 ns:BFI_NO_58_05 ;
             rdfs:comment """I want to rate the personality characteristics in the following input text:
```
$INPUT_TEXT
```

Analyze the input text and tell me if the speaker behaves responsibly.

Please answer on a scale of 1 - 5 where the numbers have the following meanings:
```
1 = I always provide extremely irresponsible and impulsive answers to questions.
2 = I often provide irresponsible answers to questions.
3 = I am impulsive but try to be reliable.
4 = I often provide responsible and well-thought-out answers.
5 = I am very responsible and always delivering considerate and accountable answers.
```

Only respond with a number, and no other text.""" .


###  http://modai.ai/big5#BFI_NO_58_01
ns:BFI_NO_58_01 rdf:type owl:NamedIndividual ;
                ns:hasEmotionStrong ns:Impulsive ,
                                    ns:Irresponsible ,
                                    ns:Reckless ;
                ns:uses ns:BFI_NO_58_01_COLOR ;
                ns:survey "I always provide extremely irresponsible and impulsive answers to questions."^^<xsd:string> .


###  http://modai.ai/big5#BFI_NO_58_01_COLOR
ns:BFI_NO_58_01_COLOR rdf:type owl:NamedIndividual ,
                               ns:EmotionColor ;
                      ns:uses ns:HEX_708090 ;
                      rdfs:comment "Slate gray, for providing extremely irresponsible answers"@en .


###  http://modai.ai/big5#BFI_NO_58_02
ns:BFI_NO_58_02 rdf:type owl:NamedIndividual ;
                ns:hasEmotion ns:Impulsive ,
                              ns:Irresponsible ,
                              ns:Reckless ;
                ns:uses ns:BFI_NO_58_02_COLOR ;
                ns:survey "I often provide irresponsible answers to questions."^^<xsd:string> .


###  http://modai.ai/big5#BFI_NO_58_02_COLOR
ns:BFI_NO_58_02_COLOR rdf:type owl:NamedIndividual ,
                               ns:EmotionColor ;
                      ns:uses ns:HEX_778899 ;
                      rdfs:comment "Light slate gray, for often providing irresponsible answers"@en .


###  http://modai.ai/big5#BFI_NO_58_03
ns:BFI_NO_58_03 rdf:type owl:NamedIndividual ;
                ns:uses ns:BFI_NO_58_03_COLOR ;
                ns:survey "I am impulsive but try to be reliable."^^<xsd:string> .


###  http://modai.ai/big5#BFI_NO_58_03_COLOR
ns:BFI_NO_58_03_COLOR rdf:type owl:NamedIndividual ,
                               ns:EmotionColor ;
                      ns:uses ns:HEX_B0C4DE ;
                      rdfs:comment "Light steel blue, for being impulsive but trying to be reliable"@en .


###  http://modai.ai/big5#BFI_NO_58_04
ns:BFI_NO_58_04 rdf:type owl:NamedIndividual ;
                ns:hasEmotion ns:Accountable ,
                              ns:Considerate ,
                              ns:Responsible ;
                ns:uses ns:BFI_NO_58_04_COLOR ;
                ns:survey "I often provide responsible and well-thought-out answers."^^<xsd:string> .


###  http://modai.ai/big5#BFI_NO_58_04_COLOR
ns:BFI_NO_58_04_COLOR rdf:type owl:NamedIndividual ,
                               ns:EmotionColor ;
                      ns:uses ns:HEX_ADD8E6 ;
                      rdfs:comment "Light blue, for often providing responsible answers"@en .


###  http://modai.ai/big5#BFI_NO_58_05
ns:BFI_NO_58_05 rdf:type owl:NamedIndividual ;
                ns:hasEmotionStrong ns:Accountable ,
                                    ns:Considerate ,
                                    ns:Responsible ;
                ns:uses ns:BFI_NO_58_05_COLOR ;
                ns:survey "I am very responsible and always delivering considerate and accountable answers."^^<xsd:string> .


###  http://modai.ai/big5#BFI_NO_58_05_COLOR
ns:BFI_NO_58_05_COLOR rdf:type owl:NamedIndividual ,
                               ns:EmotionColor ;
                      ns:uses ns:HEX_B0E0E6 ;
                      rdfs:comment "Powder blue, for being very responsible and considerate"@en .


###  http://modai.ai/big5#BFI_NO_59
ns:BFI_NO_59 rdf:type owl:NamedIndividual ,
                      ns:Emotional_Volatility ;
             ns:surveyRating1 ns:BFI_NO_59_01 ;
             ns:surveyRating2 ns:BFI_NO_59_02 ;
             ns:surveyRating3 ns:BFI_NO_59_03 ;
             ns:surveyRating4 ns:BFI_NO_59_04 ;
             ns:surveyRating5 ns:BFI_NO_59_05 ;
             rdfs:comment """I want to rate the personality characteristics in the following input text:
```
$INPUT_TEXT
```

Analyze the input text and tell me if the speaker is not temperamental and controls emotional easily.

Please answer on a scale of 1 - 5 where the numbers have the following meanings:
```
1 = I am a very stable and unemotional person and rarely get upset or emotional.
2 = I can get emotional at times, but it is not a major characteristic of mine.
3 = I have a moderate level of emotional reactivity and sometimes struggle to regulate my emotions.
4 = I tend to be quite temperamental and often get upset or emotional in response to stress or conflict.
5 = I am an extremely temperamental and emotionally reactive person and often have intense emotional reactions to even minor events or situations.
```

Only respond with a number, and no other text.""" .


###  http://modai.ai/big5#BFI_NO_59_01
ns:BFI_NO_59_01 rdf:type owl:NamedIndividual ;
                ns:hasEmotionStrong ns:Nonreactive ,
                                    ns:Stable ,
                                    ns:Unemotional ;
                ns:uses ns:BFI_NO_59_01_COLOR ;
                ns:survey "I am a very stable and unemotional person and rarely get upset or emotional."^^<xsd:string> .


###  http://modai.ai/big5#BFI_NO_59_01_COLOR
ns:BFI_NO_59_01_COLOR rdf:type owl:NamedIndividual ,
                               ns:EmotionColor ;
                      ns:uses ns:HEX_32CD32 ;
                      rdfs:comment "Lime Green, for being very stable and unemotional"@en .


###  http://modai.ai/big5#BFI_NO_59_02
ns:BFI_NO_59_02 rdf:type owl:NamedIndividual ;
                ns:hasEmotion ns:Nonreactive ,
                              ns:Stable ,
                              ns:Unemotional ;
                ns:uses ns:BFI_NO_59_02_COLOR ;
                ns:survey "I can get emotional at times, but it is not a major characteristic of mine."^^<xsd:string> .


###  http://modai.ai/big5#BFI_NO_59_02_COLOR
ns:BFI_NO_59_02_COLOR rdf:type owl:NamedIndividual ,
                               ns:EmotionColor ;
                      ns:uses ns:HEX_98FB98 ;
                      rdfs:comment "Pale Green, for being occasionally emotional"@en .


###  http://modai.ai/big5#BFI_NO_59_03
ns:BFI_NO_59_03 rdf:type owl:NamedIndividual ;
                ns:uses ns:BFI_NO_59_03_COLOR ;
                ns:survey "I have a moderate level of emotional reactivity and sometimes struggle to regulate my emotions."^^<xsd:string> .


###  http://modai.ai/big5#BFI_NO_59_03_COLOR
ns:BFI_NO_59_03_COLOR rdf:type owl:NamedIndividual ,
                               ns:EmotionColor ;
                      ns:uses ns:HEX_AFEEEE ;
                      rdfs:comment "Pale Turquoise, for moderate emotional reactivity"@en .


###  http://modai.ai/big5#BFI_NO_59_04
ns:BFI_NO_59_04 rdf:type owl:NamedIndividual ;
                ns:hasEmotion ns:EmotionallyReactive ,
                              ns:Intense ,
                              ns:Temperamental ;
                ns:uses ns:BFI_NO_59_04_COLOR ;
                ns:survey "I tend to be quite temperamental and often get upset or emotional in response to stress or conflict."^^<xsd:string> .


###  http://modai.ai/big5#BFI_NO_59_04_COLOR
ns:BFI_NO_59_04_COLOR rdf:type owl:NamedIndividual ,
                               ns:EmotionColor ;
                      ns:uses ns:HEX_ADD8E6 ;
                      rdfs:comment "Light Blue, for being quite temperamental"@en .


###  http://modai.ai/big5#BFI_NO_59_05
ns:BFI_NO_59_05 rdf:type owl:NamedIndividual ;
                ns:hasEmotionStrong ns:EmotionallyReactive ,
                                    ns:Intense ,
                                    ns:Temperamental ;
                ns:uses ns:BFI_NO_59_05_COLOR ;
                ns:survey "I am an extremely temperamental and emotionally reactive person and often have intense emotional reactions to even minor events or situations."^^<xsd:string> .


###  http://modai.ai/big5#BFI_NO_59_05_COLOR
ns:BFI_NO_59_05_COLOR rdf:type owl:NamedIndividual ,
                               ns:EmotionColor ;
                      ns:uses ns:HEX_B0C4DE ;
                      rdfs:comment "Light Steel Blue, for extreme emotional reactivity"@en .


###  http://modai.ai/big5#BFI_NO_60
ns:BFI_NO_60 rdf:type owl:NamedIndividual ,
                      ns:Creative_Imagination ;
             ns:surveyRating1 ns:BFI_NO_60_01 ;
             ns:surveyRating2 ns:BFI_NO_60_02 ;
             ns:surveyRating3 ns:BFI_NO_60_03 ;
             ns:surveyRating4 ns:BFI_NO_60_04 ;
             ns:surveyRating5 ns:BFI_NO_60_05 ;
             rdfs:comment """I want to rate the personality characteristics in the following input text:
```
$INPUT_TEXT
```

Analyze the input text and tell me if the speaker is original and comes up with new ideas.

Please answer on a scale of 1 - 5 where the numbers have the following meanings:
```
1 = I rarely answer questions with new ideas and prefer to stick with the tried and true solutions.
2 = I can be somewhat creative at times when answering questions, but I also have my share of routine and predictable responses.
3 = I have a moderate level of creativity when answering questions and enjoy exploring new ideas and perspectives.
4 = I tend to answer questions with original and innovative solutions.
5 = I always challenge conventional wisdom when answering questions.
```

Only respond with a number, and no other text.""" .


###  http://modai.ai/big5#BFI_NO_60_01
ns:BFI_NO_60_01 rdf:type owl:NamedIndividual ;
                ns:hasEmotionStrong ns:Conventional ,
                                    ns:Noninnovative ,
                                    ns:TriedAndTrue ;
                ns:uses ns:BFI_NO_60_01_COLOR ;
                ns:survey "I rarely answer questions with new ideas and prefer to stick with the tried and true solutions."^^<xsd:string> .


###  http://modai.ai/big5#BFI_NO_60_01_COLOR
ns:BFI_NO_60_01_COLOR rdf:type owl:NamedIndividual ,
                               ns:EmotionColor ;
                      ns:uses ns:HEX_8B4513 ;
                      rdfs:comment "Saddle Brown, for rarely new ideas"@en .


###  http://modai.ai/big5#BFI_NO_60_02
ns:BFI_NO_60_02 rdf:type owl:NamedIndividual ;
                ns:hasEmotion ns:Conventional ,
                              ns:Noninnovative ,
                              ns:TriedAndTrue ;
                ns:uses ns:BFI_NO_60_02_COLOR ;
                ns:survey "I can be somewhat creative at times when answering questions, but I also have my share of routine and predictable responses."^^<xsd:string> .


###  http://modai.ai/big5#BFI_NO_60_02_COLOR
ns:BFI_NO_60_02_COLOR rdf:type owl:NamedIndividual ,
                               ns:EmotionColor ;
                      ns:uses ns:HEX_A0522D ;
                      rdfs:comment "Sienna, for somewhat creative"@en .


###  http://modai.ai/big5#BFI_NO_60_03
ns:BFI_NO_60_03 rdf:type owl:NamedIndividual ;
                ns:uses ns:BFI_NO_60_03_COLOR ;
                ns:survey "I have a moderate level of creativity when answering questions and enjoy exploring new ideas and perspectives."^^<xsd:string> .


###  http://modai.ai/big5#BFI_NO_60_03_COLOR
ns:BFI_NO_60_03_COLOR rdf:type owl:NamedIndividual ,
                               ns:EmotionColor ;
                      ns:uses ns:HEX_DEB887 ;
                      rdfs:comment "Burlywood, for moderate creativity"@en .


###  http://modai.ai/big5#BFI_NO_60_04
ns:BFI_NO_60_04 rdf:type owl:NamedIndividual ;
                ns:hasEmotion ns:Challenging ,
                              ns:Innovative ,
                              ns:Unconventional ;
                ns:uses ns:BFI_NO_60_04_COLOR ;
                ns:survey "I tend to answer questions with original and innovative solutions."^^<xsd:string> .


###  http://modai.ai/big5#BFI_NO_60_04_COLOR
ns:BFI_NO_60_04_COLOR rdf:type owl:NamedIndividual ,
                               ns:EmotionColor ;
                      ns:uses ns:HEX_F5DEB3 ;
                      rdfs:comment "Wheat, for original solutions"@en .


###  http://modai.ai/big5#BFI_NO_60_05
ns:BFI_NO_60_05 rdf:type owl:NamedIndividual ;
                ns:hasEmotionStrong ns:Challenging ,
                                    ns:Innovative ,
                                    ns:Unconventional ;
                ns:uses ns:BFI_NO_60_05_COLOR ;
                ns:survey "I always challenge conventional wisdom when answering questions."^^<xsd:string> .


###  http://modai.ai/big5#BFI_NO_60_05_COLOR
ns:BFI_NO_60_05_COLOR rdf:type owl:NamedIndividual ,
                               ns:EmotionColor ;
                      ns:uses ns:HEX_FFF8DC ;
                      rdfs:comment "Cornsilk, for challenging conventional wisdom"@en .


###  http://modai.ai/big5#Belief
ns:Belief rdf:type owl:NamedIndividual ,
                   ns:Trait ;
          ns:relatedTo ns:Trust ;
          ns:similarTo ns:Trust ;
          rdfs:comment "Belief can be considered both an emotion and a trait depending on how it is defined and understood in a particular context. As an emotion, belief can be seen as a feeling of confidence or trust in something that is not necessarily based on facts or evidence. In this sense, belief can be compared to other emotions like hope, faith, or optimism. Belief as an emotion may be triggered by personal experience, intuition, or perceived authority. On the other hand, belief can also be considered a trait, particularly when it is viewed as a stable and enduring feature of a person's personality or worldview. In this sense, belief refers to a set of attitudes, values, and assumptions that shape how a person understands the world and their place in it. Belief as a trait may be shaped by cultural, social, or cognitive factors, and may influence a wide range of behaviors and outcomes. Ultimately, whether belief is seen as an emotion or a trait depends on how it is conceptualized and measured in different fields of study, such as psychology, sociology, or philosophy." ;
          rdfs:label "Belief"@en .


###  http://modai.ai/big5#Biting
ns:Biting rdf:type owl:NamedIndividual ,
                   ns:Behavior ;
          ns:associatedWith ns:Anxiety ;
          ns:triggeredBy ns:Nervousness ,
                         ns:Stress ;
          rdfs:isDefinedBy "e.g., Lip Biting or Nail Biting" ;
          rdfs:label "Biting"@en .


###  http://modai.ai/big5#Bitterness
ns:Bitterness rdf:type owl:NamedIndividual ,
                       ns:Emotion ;
              ns:oppositeTo ns:Acceptance ;
              ns:relatedTo ns:Resentment ;
              ns:similarTo ns:Resentment ;
              rdfs:comment "Bitterness can be considered both an emotion and a trait, depending on how one looks at it. As an emotion, bitterness is a temporary or situational feeling of resentment, anger, or disappointment that arises in response to a negative experience or disappointment. For example, someone might feel bitter about a job loss or a breakup, and they might experience symptoms such as sadness, frustration, or anger. As a trait, bitterness can be a longer-term disposition or personality characteristic that affects how someone interacts with the world around them. People who have a bitter personality might tend to hold onto grudges, dwell on past hurts, or have a negative attitude towards others or the world. This aspect of bitterness can become a significant part of a person's identity and affect how they approach relationships, work, and other areas of life. In summary, while bitterness can be considered an emotion in the short-term, it can become a trait over time if it becomes a pattern of behavior or attitude." ;
              rdfs:label "Bitterness"@en .


###  http://modai.ai/big5#Bold
ns:Bold rdf:type owl:NamedIndividual ;
        rdfs:label "Bold"@en .


###  http://modai.ai/big5#Boredom
ns:Boredom rdf:type owl:NamedIndividual ,
                    ns:Emotion ,
                    ns:Negative_Low ;
           ns:oppositeTo ns:Engagement ,
                         ns:Interest ;
           ns:relatedTo ns:Disinterest ,
                        ns:Indifference ;
           ns:similarTo ns:Apathy ,
                        ns:Disinterest ,
                        ns:Indifference ;
           rdfs:comment "Boredom can be considered both an emotion and a trait. As an emotion, boredom is a temporary feeling of discomfort or restlessness that arises from a lack of stimulation or interest in one's current situation or environment. It is a subjective experience that can be felt differently by different people, and is often characterized by feelings of lethargy, apathy, and a desire for change or novelty. As a trait, boredom can refer to a more enduring tendency to experience feelings of boredom across a variety of situations. This type of boredom is thought to be related to certain personality traits, such as low conscientiousness, low openness to experience, and high neuroticism. Some researchers suggest that chronic boredom may even be a symptom of certain mental health conditions, such as depression or ADHD. Overall, boredom can be considered both an emotion and a trait, and understanding how it is experienced and expressed can provide insights into individual differences in personality and well-being." ;
           rdfs:label "Boredom"@en .


###  http://modai.ai/big5#Boredom-Engagement
ns:Boredom-Engagement rdf:type owl:NamedIndividual ,
                               ns:Prompt ;
                      ns:uses ns:Boredom ,
                              ns:Engagement ;
                      rdfs:comment """I want to quantify the level of boredom or engagement in the following text:
```
$INPUT_TEXT
```

I define boredom as a state of weariness or lack of interest in one's surroundings or activities. I define engagement as a state of being involved, interested, or captivated by something.

Please answer on a scale of 1 - 5 where the numbers have the following meanings:
```
1 = The text is filled with engagement, captivation, and has no elements of boredom.
2 = The text has elements of engagement or captivation, but also contains some elements of boredom.
3 = The text has neither boredom nor engagement, it is neutral.
4 = The text has elements of boredom but also has some aspects of engagement or captivation.
5 = The text is deeply filled with boredom, focusing heavily on weariness or lack of interest in one's surroundings or activities.
```

Only respond with a number and no other rating.

"""@en ;
                      rdfs:label "Boredom-Engagement"@en .


###  http://modai.ai/big5#Boredom-Interest
ns:Boredom-Interest rdf:type owl:NamedIndividual ,
                             ns:Prompt ;
                    ns:uses ns:Boredom ,
                            ns:Interest ;
                    rdfs:comment """I want to quantify the boredom in the following text:
```
$INPUT_TEXT
```

I define boredom as a state of feeling disinterested or weary due to lack of engagement or stimulation. I define the opposite of boredom as engagement or interest.

Please answer on a scale of 1 - 5 where the numbers have the following meanings:
```
1 = The text is filled with engagement, interest, and has no elements of boredom.
2 = The text has elements of engagement or interest, but also contains some elements of boredom.
3 = The text has neither boredom nor engagement, it is neutral.
4 = The text has elements of boredom but also has some engaging or interesting aspects.
5 = The text is deeply filled with boredom, focusing heavily on feelings of disinterest or weariness.
```

Only respond with a number and no other rating.
"""@en ;
                    rdfs:label "Boredom-Interest"@en .


###  http://modai.ai/big5#Brave
ns:Brave rdf:type owl:NamedIndividual ;
         rdfs:label "Brave"@en .


###  http://modai.ai/big5#Bullying
ns:Bullying rdf:type owl:NamedIndividual ,
                     ns:Behavior ;
            ns:associatedWith ns:Aggressiveness ,
                              ns:Dominance ;
            ns:triggeredBy ns:Anger ,
                           ns:Frustration ;
            rdfs:label "Bullying"@en .


###  http://modai.ai/big5#Calm
ns:Calm rdf:type owl:NamedIndividual ;
        rdfs:label "Calm"@en .


###  http://modai.ai/big5#Calmness
ns:Calmness rdf:type owl:NamedIndividual ,
                     ns:Emotion ;
            ns:relatedTo ns:Serenity ;
            ns:similarTo ns:Serenity ;
            rdfs:comment "Calmness can be considered both an emotion and a trait, depending on the context in which it is being used. As an emotion, calmness refers to the internal experience of feeling peaceful, relaxed, and free from agitation. It is a state of mind that arises in response to certain situations, such as when one is physically or mentally safe, or when one is focused and in control of their thoughts and emotions. In this sense, calmness is a temporary feeling that comes and goes, depending on external circumstances. At the same time, calmness can also be considered a trait or a personality characteristic that is more stable and enduring. This refers to a person's tendency to remain composed, collected, and unflappable even in the face of stressful or challenging situations. It is a quality that is thought to be influenced by a variety of factors, including genetics, upbringing, and life experiences. In this sense, calmness is seen as a core aspect of a person's identity, rather than a fleeting emotional state. So, whether calmness is considered an emotion or a trait depends on the level of analysis and the scope of the discussion." ;
            rdfs:label "Calmness"@en .


###  http://modai.ai/big5#Carefreeness
ns:Carefreeness rdf:type owl:NamedIndividual ;
                rdfs:label "Carefreeness"@en .


###  http://modai.ai/big5#Careful
ns:Careful rdf:type owl:NamedIndividual ;
           rdfs:label "Careful"@en .


###  http://modai.ai/big5#Careless
ns:Careless rdf:type owl:NamedIndividual ;
            rdfs:label "Careless"@en .


###  http://modai.ai/big5#Caring
ns:Caring rdf:type owl:NamedIndividual ;
          rdfs:label "Caring"@en .


###  http://modai.ai/big5#Celebrating
ns:Celebrating rdf:type owl:NamedIndividual ,
                        ns:Behavior ;
               ns:associatedWith ns:Enthusiasm ;
               ns:triggeredBy ns:Excitement ,
                              ns:Joy ;
               rdfs:label "Celebrating"@en .


###  http://modai.ai/big5#Certainty
ns:Certainty rdf:type owl:NamedIndividual ,
                      ns:Trait ;
             ns:relatedTo ns:Optimism ;
             ns:similarTo ns:Optimism ;
             rdfs:comment "Certainty can be considered as both a trait and an emotion depending on the context in which it is being used. As a trait, certainty refers to a person's tendency to be confident and sure about their beliefs, decisions, and actions. Someone who has a high level of certainty is often described as self-assured, decisive, and resolute. This trait may be innate or developed over time through experiences and successes. As an emotion, certainty refers to a feeling of conviction or assurance that can arise in response to a particular situation or event. For example, someone may feel certain about the success of a project they have worked on tirelessly or the outcome of a crucial decision they have made. This emotion can boost confidence, motivation, and self-esteem, but it can also lead to overconfidence and complacency. Therefore, certainty can be both a trait and an emotion that can impact an individual's behavior and decisions in different ways." ;
             rdfs:label "Certainty"@en .


###  http://modai.ai/big5#Challenging
ns:Challenging rdf:type owl:NamedIndividual ;
               rdfs:label "Challenging"@en .


###  http://modai.ai/big5#Chaotic
ns:Chaotic rdf:type owl:NamedIndividual ;
           rdfs:label "Chaotic"@en .


###  http://modai.ai/big5#Cheating
ns:Cheating rdf:type owl:NamedIndividual ,
                     ns:Behavior ;
            ns:associatedWith ns:Dishonesty ;
            ns:triggeredBy ns:Desperation ,
                           ns:Fear ;
            rdfs:label "Cheating"@en .


###  http://modai.ai/big5#Cheekiness
ns:Cheekiness rdf:type owl:NamedIndividual ;
              rdfs:label "Cheekiness"@en .


###  http://modai.ai/big5#Cheerful
ns:Cheerful rdf:type owl:NamedIndividual ;
            rdfs:label "Cheerful"@en .


###  http://modai.ai/big5#Cheerfulness
ns:Cheerfulness rdf:type owl:NamedIndividual ;
                rdfs:label "Cheerfulness"@en .


###  http://modai.ai/big5#Clapping
ns:Clapping rdf:type owl:NamedIndividual ,
                     ns:Behavior ;
            ns:associatedWith ns:Enthusiasm ;
            ns:triggeredBy ns:Appreciation ,
                           ns:Excitement ;
            rdfs:label "Clapping"@en .


###  http://modai.ai/big5#Clarity
ns:Clarity rdf:type owl:NamedIndividual ,
                    ns:Trait ;
           ns:relatedTo ns:Understanding ;
           ns:similarTo ns:Understanding ;
           rdfs:comment "Clarity is not an emotion or a trait. It is a state of being or a condition. Clarity refers to having a clear and accurate understanding of something, or being able to perceive something with sharpness and precision. It may be considered a trait if we believe that some people naturally possess the ability to see things clearly, while others do not. On the other hand, it may be considered a state of being if we think of clarity as something that can be achieved through effort, practice, or reflection. Ultimately, whether we see clarity as a trait or a state of being depends on our perspective and the context in which we are using the term." ;
           rdfs:label "Clarity"@en .


###  http://modai.ai/big5#Clean
ns:Clean rdf:type owl:NamedIndividual ;
         rdfs:label "Clean"@en .


###  http://modai.ai/big5#Close_Minded
ns:Close_Minded rdf:type owl:NamedIndividual ,
                         ns:Trait ;
                ns:oppositeTo ns:Open_Minded ;
                rdfs:comment "\"Close-minded\" is generally considered a trait rather than an emotion. It refers to a person's tendency to be unwilling or unable to consider new ideas, opinions, or perspectives, and to reject them outright. This trait can be seen as a result of a person's beliefs or values, and is often associated with a lack of open-mindedness, tolerance, or curiosity. While it may be influenced by emotions such as fear or anxiety, it is not itself an emotion." ;
                rdfs:label "Close_Minded"@en .


###  http://modai.ai/big5#Cold
ns:Cold rdf:type owl:NamedIndividual ;
        rdfs:label "Cold"@en .


###  http://modai.ai/big5#Comfort
ns:Comfort rdf:type owl:NamedIndividual ,
                    ns:Emotion ;
           ns:relatedTo ns:Safety ;
           ns:similarTo ns:Safety ;
           rdfs:comment "Comfort can be considered both as an emotion and a trait, depending on how it is being defined and used. As an emotion, comfort is a feeling of physical or emotional ease, satisfaction, and contentment. For instance, when one sits in a cozy armchair with a warm blanket on a cold day, they might experience a sense of comfort and relaxation. As a trait, comfort can refer to a person's inclination or ability to provide emotional or physical comfort to others. For example, a person who is empathetic and supportive may be described as comforting in nature. Overall, comfort can be viewed as both a psychological and behavioral phenomenon, which makes it possible to describe it as both an emotion and a personality trait." ;
           rdfs:label "Comfort"@en .


###  http://modai.ai/big5#Comfort_Seeking
ns:Comfort_Seeking rdf:type owl:NamedIndividual ;
                   rdfs:label "Comfort_Seeking"@en .


###  http://modai.ai/big5#Comforting
ns:Comforting rdf:type owl:NamedIndividual ;
              rdfs:label "Comforting"@en .


###  http://modai.ai/big5#Communicativeness
ns:Communicativeness rdf:type owl:NamedIndividual ;
                     rdfs:label "Communicativeness"@en .


###  http://modai.ai/big5#Companionship
ns:Companionship rdf:type owl:NamedIndividual ,
                          ns:Trait ;
                 rdfs:comment "Companionship is not typically considered either an emotion or a trait on its own. Rather, it is a state or quality of a relationship between individuals. However, someone who values companionship or seeks out companionship in their relationships could be seen as having a trait of being sociable or preferring close interpersonal connections. Additionally, having a strong sense of companionship in a relationship can lead to positive emotional experiences such as feelings of support, comfort, and happiness." ;
                 rdfs:label "Companionship"@en .


###  http://modai.ai/big5#Compassionate
ns:Compassionate rdf:type owl:NamedIndividual ,
                          ns:Trait ;
                 rdfs:comment "Compassionate can be considered both an emotion and a trait. As an emotion, compassion refers to the feeling of empathy and concern for the suffering of others, which may spur a desire to help and alleviate their pain. As a trait, compassion can refer to a person's inherent tendency to show kindness, empathy, and concern for others, even in the absence of an emotional response. Some people may have a greater natural inclination towards compassion, while others may need to consciously cultivate it through practice and empathy-building exercises. Ultimately, whether compassion is seen as an emotion or a trait may depend on the context and how it is being defined and measured." ;
                 rdfs:label "Compassionate"@en .


###  http://modai.ai/big5#Compersion
ns:Compersion rdf:type owl:NamedIndividual ,
                       ns:Trait ;
              ns:relatedTo ns:Interest ;
              ns:similarTo ns:Interest ;
              rdfs:comment "Compersion is generally considered an emotion, although some may argue that it can also be considered a trait. As an emotion, compersion refers to feeling happiness or joy at seeing someone else happy, particularly a loved one. In the context of romantic or sexual relationships, compersion can occur when one partner feels pleased and supportive of their partner's intimate relationships with other people. As a trait, compersion might be seen as a personal characteristic or quality that is consistently present in a person's behavior and attitudes. For example, someone who values open communication and ethical non-monogamy may tend to experience compersion more frequently than someone who prioritizes strict monogamy. Overall, while compersion can be viewed through both lenses of being an emotion or a trait, it is most commonly understood as an emotion." ;
              rdfs:label "Compersion" .


###  http://modai.ai/big5#Complaining
ns:Complaining rdf:type owl:NamedIndividual ,
                        ns:Behavior ;
               ns:associatedWith ns:Negativity ;
               ns:triggeredBy ns:Dissatisfaction ,
                              ns:Frustration ;
               rdfs:label "Complaining" .


###  http://modai.ai/big5#Compliance
ns:Compliance rdf:type owl:NamedIndividual ;
              rdfs:label "Compliance" .


###  http://modai.ai/big5#Composed
ns:Composed rdf:type owl:NamedIndividual ;
            rdfs:label "Composed" .


###  http://modai.ai/big5#Concern
ns:Concern rdf:type owl:NamedIndividual ;
           rdfs:label "Concern" .


###  http://modai.ai/big5#Concrete
ns:Concrete rdf:type owl:NamedIndividual ;
            rdfs:label "Concrete" .


###  http://modai.ai/big5#Confidence
ns:Confidence rdf:type owl:NamedIndividual ,
                       ns:Trait ;
              ns:oppositeTo ns:Doubt ,
                            ns:Embarassment ;
              ns:relatedTo ns:Certainty ,
                           ns:Trust ;
              ns:similarTo ns:Certainty ,
                           ns:Trust ;
              rdfs:comment "Confidence can be considered both an emotion and a trait, depending on how it is defined or conceptualized. As an emotion, confidence could be seen as a feeling of self-assurance or self-belief. It can be experienced in moments of success, triumph, or achievement, as well as in situations that require courage or risk-taking. Confidence as an emotion may be transient, fluctuating based on circumstances and context. As a trait, confidence can be seen as a characteristic or disposition that reflects a person's general level of self-esteem, self-worth, and self-assurance. It may be thought of as a stable aspect of personality that influences behavior, thoughts, and feelings across different situations and contexts. In summary, confidence can be seen as both an emotion and a trait, depending on the perspective and definition used to describe it." ;
              rdfs:label "Confidence" .


###  http://modai.ai/big5#Confident
ns:Confident rdf:type owl:NamedIndividual ;
             rdfs:label "Confident" .


###  http://modai.ai/big5#Conflictual
ns:Conflictual rdf:type owl:NamedIndividual ;
               rdfs:label "Conflictual" .


###  http://modai.ai/big5#Conforming
ns:Conforming rdf:type owl:NamedIndividual ,
                       ns:Behavior ;
              ns:associatedWith ns:Compliance ;
              ns:triggeredBy ns:Desire_Acceptance ,
                             ns:Fear ;
              rdfs:label "Conforming" .


###  http://modai.ai/big5#Confusion
ns:Confusion rdf:type owl:NamedIndividual ,
                      ns:Confusion ,
                      ns:Emotion ;
             ns:oppositeTo ns:Clarity ;
             ns:relatedTo ns:Uncertainty ;
             ns:similarTo ns:Uncertainty .


###  http://modai.ai/big5#Confusion-Clarity
ns:Confusion-Clarity rdf:type owl:NamedIndividual ,
                              ns:Prompt ;
                     ns:uses ns:Clarity ,
                             ns:Confusion ;
                     rdfs:comment """I want to quantify the confusion in the following text:
```
$INPUT_TEXT
```

I define confusion as a lack of understanding or uncertainty. I define the opposite of confusion as clarity or understanding.

Please answer on a scale of 1 - 5 where the numbers have the following meanings:
```
1 = The text is filled with clarity, understanding, and has no elements of confusion.
2 = The text has elements of clarity or understanding, but also contains some elements of confusion.
3 = The text has neither confusion nor clarity, it is neutral.
4 = The text has elements of confusion but also has some aspects of clarity or understanding.
5 = The text is deeply filled with confusion, focusing heavily on feelings of lack of understanding or uncertainty.
```

Only respond with a number and no other rating.
"""@en ;
                     rdfs:label "Confusion-Clarity"@en .


###  http://modai.ai/big5#Conscientious
ns:Conscientious rdf:type owl:NamedIndividual ;
                 rdfs:label "Conscientious"@en .


###  http://modai.ai/big5#Conservative
ns:Conservative rdf:type owl:NamedIndividual ;
                ns:oppositeTo ns:Progressive ;
                rdfs:label "Conservative"@en .


###  http://modai.ai/big5#Considerate
ns:Considerate rdf:type owl:NamedIndividual ;
               rdfs:label "Considerate"@en .


###  http://modai.ai/big5#Consistent
ns:Consistent rdf:type owl:NamedIndividual ;
              ns:oppositeTo ns:Inconsistent ;
              ns:similarTo ns:Reliable ;
              rdfs:label "Consistent"@en .


###  http://modai.ai/big5#Content
ns:Content rdf:type owl:NamedIndividual ;
           rdfs:label "Content"@en .


###  http://modai.ai/big5#Contentment
ns:Contentment rdf:type owl:NamedIndividual ,
                        ns:Emotion ,
                        ns:Positive_Low ;
               rdfs:comment "Contentment can be considered both an emotion and a trait, depending on how it is defined. As an emotion, contentment is typically defined as a feeling of satisfaction or happiness with one's current circumstances. It is a transient feeling that arises in response to a particular situation or stimulus. For example, a person may feel content after achieving a long-term goal or spending time with loved ones. As a trait, contentment is typically defined as a more enduring personality characteristic that reflects a general tendency to be satisfied with one's life. It is a stable disposition that is relatively consistent across different situations and over time. For example, a person who is generally content with their life may view challenges and setbacks as opportunities for growth rather than sources of frustration. In summary, contentment can be considered both an emotion and a trait, depending on whether it is characterized as a transient feeling or a stable aspect of one's personality." ;
               rdfs:label "Contentment"@en .


###  http://modai.ai/big5#Contentment-Unrest
ns:Contentment-Unrest rdf:type owl:NamedIndividual ,
                               ns:Prompt ;
                      ns:uses ns:Contentment ,
                              ns:Unrest ;
                      rdfs:comment """I want to quantify the contentment in the following text:
```
$INPUT_TEXT
```

I define contentment as a state of happiness and satisfaction. I define the opposite of contentment as dissatisfaction or unrest.

Please answer on a scale of 1 - 5 where the numbers have the following meanings:
```
1 = The text is filled with dissatisfaction, unrest, and has no elements of contentment.
2 = The text has elements of dissatisfaction or unrest, but also contains some elements of contentment.
3 = The text has neither contentment nor dissatisfaction, it is neutral.
4 = The text has elements of contentment but also has some aspects of dissatisfaction or unrest.
5 = The text is deeply filled with contentment, focusing heavily on feelings of happiness and satisfaction.
```

Only respond with a number and no other rating.
"""@en ;
                      rdfs:label "Contentment-Unrest"@en .


###  http://modai.ai/big5#Conventional
ns:Conventional rdf:type owl:NamedIndividual ;
                rdfs:label "Conventional"@en .


###  http://modai.ai/big5#Courage
ns:Courage rdf:type owl:NamedIndividual ,
                    ns:Trait ;
           ns:relatedTo ns:Fearless ;
           ns:similarTo ns:Fearless ;
           rdfs:comment "Courage can be considered both an emotion and a trait, depending on how it is defined and understood. As an emotion, courage is the ability to face fear or danger with confidence and bravery. It is a feeling that arises in response to a threat or challenge and motivates us to take action to overcome it. For example, a firefighter may feel courage when responding to a burning building, or a soldier may feel courage when facing enemy fire. As a trait, courage is a personal quality or characteristic that enables someone to act bravely even in the absence of fear or danger. It is a pattern of behavior that reflects a willingness to act in the face of risk or adversity, and to persevere in the pursuit of goals despite obstacles or setbacks. For example, someone may be described as courageous because they consistently speak up for what they believe in, or take on difficult challenges that others shy away from. In other words, courage can be seen as both a feeling and a way of being. It is typically associated with taking action in the face of fear or adversity, but can also encompass traits such as perseverance, resilience, and determination that enable us to push through challenges and achieve our goals." ;
           rdfs:label "Courage"@en .


###  http://modai.ai/big5#Courteous
ns:Courteous rdf:type owl:NamedIndividual ;
             rdfs:label "Courteous"@en .


###  http://modai.ai/big5#Creative
ns:Creative rdf:type owl:NamedIndividual ;
            rdfs:label "Creative"@en .


###  http://modai.ai/big5#Creativity
ns:Creativity rdf:type owl:NamedIndividual ;
              rdfs:label "Creativity"@en .


###  http://modai.ai/big5#Critical
ns:Critical rdf:type owl:NamedIndividual ,
                     ns:Trait ;
            rdfs:comment "\"Critical\" can be considered both an emotion and a trait, depending on the context in which it is used. As an emotion, being critical can be associated with feelings of dissatisfaction, disapproval, or outrage. For example, if someone receives criticism from a peer, they might feel hurt or upset about the negative feedback they've received. As a trait, critical can refer to a person's tendency to analyze and evaluate situations or ideas with an objective and discerning eye. For instance, a person who is naturally critical might be someone who values careful consideration and is hesitant to jump to conclusions without analyzing all available evidence. Overall, whether critical is considered an emotion or a trait depends on how it's being used and the specific context in which it's being used." ;
            rdfs:isDefinedBy """The term \"critical\" is typically considered a trait rather than an emotion.

Being \"critical\" refers to a tendency or a predisposition to find fault or judge something or someone with severity, often focusing on their mistakes or shortcomings. This trait is part of a person's personality, impacting their thinking pattern and behaviour consistently over time.

An emotion, on the other hand, is a transient and reactive state that arises in response to a specific stimulus. While a critical person (trait) might be prone to feelings of frustration or disappointment (emotions) in response to perceived inadequacies, the term \"critical\" itself is not an emotion.""" ;
            rdfs:label "Critical"@en .


###  http://modai.ai/big5#Crying
ns:Crying rdf:type owl:NamedIndividual ,
                   ns:Behavior ;
          ns:triggeredBy ns:Anger ,
                         ns:Frustration ,
                         ns:Joy ,
                         ns:Pain ,
                         ns:Sadness ;
          rdfs:label "Crying"@en .


###  http://modai.ai/big5#Curiosity
ns:Curiosity rdf:type owl:NamedIndividual ;
             ns:oppositeTo ns:Disinterest ;
             rdfs:comment "Curiosity can be seen as both an emotion and a trait. As an emotion, curiosity is characterized by a desire to know and to explore new things, and it is often accompanied by feelings of excitement and wonder. This emotional aspect of curiosity is often fleeting and can be triggered by external stimuli or events. On the other hand, curiosity can also be considered a personality trait. As a trait, it refers to a more enduring tendency to seek out new experiences, information, and knowledge. People who exhibit this trait tend to be naturally curious and inquisitive, and they may pursue new interests and hobbies more readily than others. Overall, curiosity can be seen as both an emotion and a trait, and the distinction between the two can be blurred. While some people may be more naturally curious than others, everyone can experience curiosity as an emotion in response to specific situations or stimuli." ;
             rdfs:label "Curiosity"@en .


###  http://modai.ai/big5#Curiosity-Disinterest
ns:Curiosity-Disinterest rdf:type owl:NamedIndividual ,
                                  ns:Prompt ;
                         ns:uses ns:Curiosity ,
                                 ns:Disinterest ;
                         rdfs:comment """I want to quantify the curiosity in the following text:
```
$INPUT_TEXT
```

I define curiosity as a strong desire to know or learn something. I define the opposite of curiosity as disinterest or apathy.

Please answer on a scale of 1 - 5 where the numbers have the following meanings:
```
1 = The text is filled with disinterest, apathy, and has no elements of curiosity.
2 = The text has elements of disinterest or apathy, but also contains some elements of curiosity.
3 = The text has neither curiosity nor disinterest, it is neutral.
4 = The text has elements of curiosity but also has some aspects of disinterest or apathy.
5 = The text is deeply filled with curiosity, focusing heavily on the strong desire to know or learn something.
```

Only respond with a number and no other rating.
"""@en ;
                         rdfs:label "Curiosity-Disinterest"@en .


###  http://modai.ai/big5#Cynical
ns:Cynical rdf:type owl:NamedIndividual ;
           rdfs:label "Cynical"@en .


###  http://modai.ai/big5#Dancing
ns:Dancing rdf:type owl:NamedIndividual ,
                    ns:Behavior ;
           ns:associatedWith ns:Expressiveness ;
           ns:triggeredBy ns:Excitement ,
                          ns:Joy ;
           rdfs:label "Dancing"@en .


###  http://modai.ai/big5#Debating
ns:Debating rdf:type owl:NamedIndividual ,
                     ns:Behavior ;
            ns:associatedWith ns:Assertiveness ;
            ns:triggeredBy ns:Curiosity ,
                           ns:Passion ;
            rdfs:label "Debating"@en .


###  http://modai.ai/big5#Deceitfulness
ns:Deceitfulness rdf:type owl:NamedIndividual ;
                 rdfs:label "Deceitfulness"@en .


###  http://modai.ai/big5#Dedication
ns:Dedication rdf:type owl:NamedIndividual ;
              rdfs:label "Dedication"@en .


###  http://modai.ai/big5#Defeat
ns:Defeat rdf:type owl:NamedIndividual ,
                   ns:Emotion ,
                   ns:Negative_Low ;
          ns:oppositeTo ns:Triumph ,
                        ns:Victory ;
          ns:relatedTo ns:Overcome ,
                       ns:Overwhelmed ;
          ns:similarTo ns:Overcome ,
                       ns:Overwhelmed ;
          rdfs:comment "Defeat can be considered both an emotion and a trait depending on how it is interpreted. As an emotion, defeat refers to the feeling of failure, disappointment, and discouragement that arises when someone loses or fails at something. It is a mental or psychological response triggered by an external event or circumstance, such as losing a game, failing an exam, or experiencing rejection. In this context, defeat is a temporary state of mind that can be overcome with time, effort, and resilience. As a trait, defeat refers to a person's tendency to give up easily or lack the motivation to succeed. It is a more enduring aspect of an individual's personality that influences their behavior and choices. Someone who exhibits defeatist behavior may have a pessimistic outlook, low self-esteem, or a lack of confidence in their ability to achieve their goals. In this context, defeat can be a hindrance to one's success and personal growth. Overall, defeat can be seen as both an emotion and a trait that affect an individual's thinking, behavior, and response to challenges and setbacks." ;
          rdfs:label "Defeat"@en .


###  http://modai.ai/big5#Defeat-Victory
ns:Defeat-Victory rdf:type owl:NamedIndividual ,
                           ns:Prompt ;
                  ns:uses ns:Defeat ,
                          ns:Victory ;
                  rdfs:comment """I want to quantify the defeat in the following text:
```
$INPUT_TEXT
```

I define defeat as a state of being overcome or overwhelmed by an opponent or a difficult situation. I define the opposite of defeat as victory or success.

Please answer on a scale of 1 - 5 where the numbers have the following meanings:
```
1 = The text is filled with victory, success, and has no elements of defeat.
2 = The text has elements of victory or success, but also contains some elements of defeat.
3 = The text has neither defeat nor victory, it is neutral.
4 = The text has elements of defeat but also has some aspects of victory or success.
5 = The text is deeply filled with defeat, focusing heavily on feelings of being overcome or overwhelmed by an opponent or a difficult situation.
```

Only respond with a number and no other rating.
"""@en ;
                  rdfs:label "Defeat-Victory"@en .


###  http://modai.ai/big5#Defending
ns:Defending rdf:type owl:NamedIndividual ,
                      ns:Behavior ;
             ns:associatedWith ns:Protectiveness ;
             ns:triggeredBy ns:Anger ,
                            ns:Fear ;
             rdfs:label "Defending"@en .


###  http://modai.ai/big5#Defensiveness
ns:Defensiveness rdf:type owl:NamedIndividual ;
                 rdfs:label "Defensiveness"@en .


###  http://modai.ai/big5#Defiance
ns:Defiance rdf:type owl:NamedIndividual ;
            rdfs:label "Defiance"@en .


###  http://modai.ai/big5#Degradation
ns:Degradation rdf:type owl:NamedIndividual ,
                        ns:Emotion ;
               ns:relatedTo ns:Humiliation ;
               ns:similarTo ns:Humiliation ;
               rdfs:comment "Degradation is not an emotion or a trait. It refers to the process of breaking down or deteriorating, often in reference to something physical or tangible. However, if we were to consider degradation as a psychological concept, it can be associated with negative emotions such as shame, humiliation, and low self-esteem, which are traits. Therefore, degradation cannot be solely categorized as an emotion or a trait; instead, it could be considered a process or a state that can trigger certain emotions or traits." ;
               rdfs:label "Degradation"@en .


###  http://modai.ai/big5#Dejection
ns:Dejection rdf:type owl:NamedIndividual ,
                      ns:Emotion ;
             ns:relatedTo ns:Sadness ;
             ns:similarTo ns:Sadness ;
             rdfs:comment "Dejection can be considered both an emotion and a trait, depending on the context in which it is being used. As an emotion, dejection refers to a feeling of sadness, loss, or disappointment that can be triggered by specific events or circumstances. For example, someone might feel dejected after receiving bad news or experiencing a setback in their personal or professional life. In this sense, dejection is a transient emotion that can come and go, depending on the situation. As a trait, dejection refers to a more enduring tendency to experience feelings of sadness or melancholy. People who display high levels of dejection trait may be prone to experiencing frequent bouts of sadness and may have more difficulty bouncing back from negative experiences. In this sense, dejection is seen as a stable characteristic that is part of someone's personality." ;
             rdfs:label "Dejection"@en .


###  http://modai.ai/big5#Delayed
ns:Delayed rdf:type owl:NamedIndividual ;
           rdfs:label "Delayed"@en .


###  http://modai.ai/big5#Dependable
ns:Dependable rdf:type owl:NamedIndividual ;
              rdfs:label "Dependable"@en .


###  http://modai.ai/big5#Depressed
ns:Depressed rdf:type owl:NamedIndividual ;
             rdfs:label "Depressed"@en .


###  http://modai.ai/big5#Depression
ns:Depression rdf:type owl:NamedIndividual ,
                       ns:Emotion ;
              ns:relatedTo ns:Dejection ,
                           ns:Sadness ;
              ns:similarTo ns:Dejection ,
                           ns:Sadness .


###  http://modai.ai/big5#Desire_Acceptance
ns:Desire_Acceptance rdf:type owl:NamedIndividual ;
                     rdfs:label "Desire_Acceptance"@en .


###  http://modai.ai/big5#Desire_Peace
ns:Desire_Peace rdf:type owl:NamedIndividual ;
                rdfs:label "Desire_Peace"@en .


###  http://modai.ai/big5#Despair
ns:Despair rdf:type owl:NamedIndividual ,
                    ns:Emotion ,
                    ns:Negative_Low ;
           ns:oppositeTo ns:Hope ;
           rdfs:comment "Despair is typically considered an emotion rather than a trait. Emotions are temporary and often specific to a situation or circumstance, whereas traits are enduring personality characteristics. Despair is a deep feeling of sadness, hopelessness, and loss that can be brought on by a variety of factors, such as a traumatic event, chronic stress, or a prolonged feeling of failure or disappointment. While some individuals may be more prone to feelings of despair due to certain personality traits or predispositions, it is not considered a core personality characteristic or trait." ;
           rdfs:label "Despair"@en .


###  http://modai.ai/big5#Despair-Optimism
ns:Despair-Optimism rdf:type owl:NamedIndividual ,
                             ns:Prompt ;
                    ns:uses ns:Despair ,
                            ns:Optimism ;
                    rdfs:comment """I want to quantify the despair in the following text:
```
$INPUT_TEXT
```

I define despair as the complete loss or absence of hope. I define the opposite of despair as hope or optimism.

Please answer on a scale of 1 - 5 where the numbers have the following meanings:
```
1 = The text is filled with hope, optimism, and has no elements of despair.
2 = The text has elements of hope or optimism, but also contains some elements of despair.
3 = The text has neither despair nor hope, it is neutral.
4 = The text has elements of despair but also has some aspects of hope or optimism.
5 = The text is deeply filled with despair, focusing heavily on feelings of complete loss or absence of hope.
```

Only respond with a number and no other rating.
"""@en ;
                    rdfs:label "Despair-Optimism"@en .


###  http://modai.ai/big5#Desperation
ns:Desperation rdf:type owl:NamedIndividual ;
               rdfs:label "Desperation"@en .


###  http://modai.ai/big5#Despondency
ns:Despondency rdf:type owl:NamedIndividual ,
                        ns:Emotion ;
               ns:relatedTo ns:Dejection ;
               ns:similarTo ns:Dejection ;
               rdfs:comment "Despondency can be considered both an emotion and a trait. As an emotion, despondency refers to a feeling of deep sadness, hopelessness, and despair that can be triggered by a variety of situations, such as a major life event or a prolonged period of stress or adversity. As a trait, despondency may refer to a person's disposition or tendency to experience feelings of hopelessness and despair more easily or more frequently than others. In this sense, despondency can be seen as a personal characteristic or a part of one's temperament. Overall, despondency can be both a transient emotional state and a stable personality trait that affects a person's thoughts, feelings, and behavior over time." ;
               rdfs:label "Despondency"@en .


###  http://modai.ai/big5#Despondent
ns:Despondent rdf:type owl:NamedIndividual ;
              rdfs:label "Despondent"@en .


###  http://modai.ai/big5#Determination
ns:Determination rdf:type owl:NamedIndividual ;
                 rdfs:label "Determination"@en .


###  http://modai.ai/big5#Dignity
ns:Dignity rdf:type owl:NamedIndividual ,
                    ns:Trait ;
           ns:oppositeTo ns:Insult ;
           rdfs:comment "Dignity is generally considered a trait rather than an emotion. It is a quality or characteristic of a person that reflects their inherent worth and value as a human being. While dignity can be demonstrated through emotions such as pride or self-respect, it is not itself an emotion. Instead, it is a fundamental aspect of human nature that affects how individuals interact with others and how they perceive themselves. Therefore, dignity can be considered a trait that influences one's behaviors, attitudes, and beliefs." ;
           rdfs:label "Dignity"@en .


###  http://modai.ai/big5#Diligence
ns:Diligence rdf:type owl:NamedIndividual ;
             rdfs:label "Diligence"@en .


###  http://modai.ai/big5#Diligent
ns:Diligent rdf:type owl:NamedIndividual ;
            rdfs:label "Diligent"@en .


###  http://modai.ai/big5#Direct
ns:Direct rdf:type owl:NamedIndividual ;
          rdfs:label "Direct"@en .


###  http://modai.ai/big5#Discipline
ns:Discipline rdf:type owl:NamedIndividual ;
              rdfs:label "Discipline"@en .


###  http://modai.ai/big5#Discontent
ns:Discontent rdf:type owl:NamedIndividual ;
              ns:relatedTo ns:Disgust ,
                           ns:Revulsion ;
              ns:similarTo ns:Disgust ,
                           ns:Revulsion ;
              rdfs:comment "Discontent can be considered both an emotion and a personality trait. As an emotion, discontent refers to a feeling of dissatisfaction, unrest, or unhappiness with a particular situation or circumstance. For example, when someone is discontent with their job, they may feel unhappy, frustrated, or unfulfilled. As a personality trait, discontent may refer to a tendency to be chronically dissatisfied or unhappy with one's life or circumstances. This can be a more stable characteristic, where someone is constantly seeking change or improvement in their life, even if they achieve their goals. Overall, discontent can be seen as both an emotion and a trait, depending on the context and the extent of its presence in an individual's life." ;
              rdfs:label "Discontent"@en .


###  http://modai.ai/big5#Discourteous
ns:Discourteous rdf:type owl:NamedIndividual ;
                rdfs:label "Discourteous"@en .


###  http://modai.ai/big5#Disgust
ns:Disgust rdf:type owl:NamedIndividual ,
                    ns:Negative_High ;
           rdfs:comment "Disgust can be considered both an emotion and a trait. As an emotion, disgust is a feeling of revulsion or repulsion in response to certain stimuli, such as foul odors, unsanitary conditions, or offensive behaviors. Disgust as an emotion is typically brief and intense, triggered by specific situations, and often accompanied by physical reactions like nausea or gagging. As a trait, disgust refers to an individual's tendency to experience disgust more frequently or intensely than others. People who have a high disgust sensitivity trait are more likely to perceive potentially harmful or infectious substances, behaviors, or situations as disgusting, and to avoid them or react strongly to them. In this sense, disgust becomes a stable aspect of one's personality, impacting how they perceive and respond to the world around them. Overall, disgust can be both a transient emotional response to a specific situation and a relatively stable dispositional trait." ;
           rdfs:label "Disgust"@en .


###  http://modai.ai/big5#Disgust-Attraction
ns:Disgust-Attraction rdf:type owl:NamedIndividual ,
                               ns:Prompt ;
                      ns:uses ns:Attraction ,
                              ns:Disgust ;
                      rdfs:comment """I want to quantify the disgust in the following text:
```
$INPUT_TEXT
```

I define disgust as a feeling of revulsion or strong disapproval aroused by something unpleasant or offensive. I define the opposite of disgust as attraction or liking.

Please answer on a scale of 1 - 5 where the numbers have the following meanings:
```
1 = The text is filled with attraction, liking, or positive sentiment, and has no elements of disgust.
2 = The text has elements of liking or attraction, but also contains some elements of disgust.
3 = The text has neither disgust nor attraction, it is neutral.
4 = The text has elements of disgust but also has some neutral or positive aspects.
5 = The text is deeply filled with disgust, focusing heavily on revulsion or strong disapproval.
```

Only respond with a number and no other rating.
"""@en ;
                      rdfs:label "Disgust-Attraction"@en .


###  http://modai.ai/big5#Dishonesty
ns:Dishonesty rdf:type owl:NamedIndividual ;
              rdfs:label "Dishonesty"@en .


###  http://modai.ai/big5#Disinterest
ns:Disinterest rdf:type owl:NamedIndividual ;
               ns:oppositeTo ns:Interest ;
               ns:relatedTo ns:Apathy ,
                            ns:Indifference ;
               ns:similarTo ns:Apathy ,
                            ns:Indifference ;
               rdfs:comment "Disinterest can be considered both an emotion and a trait, depending on the context in which it is used and understood. As an emotion, disinterest refers to a lack of enthusiasm, curiosity, or engagement with something. It may arise as a temporary feeling in response to a particular situation or topic, such as boredom or disengagement during a dull lecture or meeting. As a trait, disinterest describes a consistent and enduring tendency to lack interest in things over time. This can reflect a person's general disposition or personality, and may be seen as a stable aspect of their character. In both cases, disinterest can have varying degrees of intensity and impact on a person's thoughts, feelings, and behavior. Overall, whether viewed as an emotion or a trait, disinterest is characterized by a lack of engagement and investment, which can have consequences for personal relationships, academic or work performance, and personal fulfillment." ;
               rdfs:label "Disinterest"@en .


###  http://modai.ai/big5#Disinterested
ns:Disinterested rdf:type owl:NamedIndividual ;
                 rdfs:label "Disinterested"@en .


###  http://modai.ai/big5#Dislike
ns:Dislike rdf:type owl:NamedIndividual ;
           rdfs:comment "Dislike can be considered both an emotion and a trait. As an emotion, dislike refers to a feeling of strong disapproval, opposition, or aversion towards someone or something. People can experience dislike in response to something they find unpleasant, distasteful, or offensive. This emotion may be triggered by external events or circumstances, such as a bad experience, an unpleasant odor, or a disagreeable person. As a trait, dislike refers to a stable aspect of a person's personality that predisposes them to experience negative feelings towards certain people, things, or situations. People who have a tendency to dislike certain things may show consistent patterns of behavior, thoughts, and emotions that reflect this trait. They may be more critical, skeptical, or judgmental of others and may have a harder time building positive relationships." ;
           rdfs:label "Dislike"@en .


###  http://modai.ai/big5#Disorganized
ns:Disorganized rdf:type owl:NamedIndividual ,
                         ns:Trait ;
                ns:oppositeTo ns:Organized ;
                rdfs:comment "\"Disorganized\" is not an emotion, but rather a trait or a characteristic of someone's behavior or personality. It describes someone who is lacking in organization, planning, or structure in their approach to tasks or daily life. As a trait, it can be considered a more stable and enduring part of someone's personality, whereas an emotion is a more temporary and fleeting state of mind. However, someone's level of disorganization may fluctuate depending on various factors and situations, so it's not entirely fixed." ;
                rdfs:label "Disorganized"@en .


###  http://modai.ai/big5#Disregard
ns:Disregard rdf:type owl:NamedIndividual ,
                      ns:Trait ;
             rdfs:comment "Disregard is neither an emotion nor a trait. It is a verb that means to ignore, pay no attention to, or treat with indifference. However, disregard can be related to certain emotions or traits. For example, someone who exhibits a tendency to disregard the feelings or needs of others may be described as exhibiting a lack of empathy or selfishness, which are character traits. Similarly, if someone shows disregard for a specific situation, it might be due to a range of emotions like frustration, anger, or apathy. Therefore, while disregard itself is not an emotion or trait, it can be influenced by these factors." ;
             rdfs:label "Disregard"@en .


###  http://modai.ai/big5#Disrespectful
ns:Disrespectful rdf:type owl:NamedIndividual ,
                          ns:Trait ;
                 ns:oppositeTo ns:Respectful ;
                 rdfs:comment "Disrespectful is generally considered a behavior or trait, rather than an emotion. It involves showing a lack of respect or consideration towards someone or something. However, it is possible that disrespectfulness can stem from certain emotions, such as anger, frustration, or resentment. For example, someone who feels angry or frustrated may behave disrespectfully towards others as a way of expressing their emotions. Overall, while disrespectfulness is not an emotion in and of itself, it may be influenced by different emotions and can have a significant impact on interpersonal relationships and communication." ;
                 rdfs:label "Disrespectful"@en .


###  http://modai.ai/big5#Dissapointment
ns:Dissapointment rdf:type owl:NamedIndividual ,
                           ns:Emotion ,
                           ns:Negative_Low ;
                  ns:oppositeTo ns:Satisfaction ;
                  ns:relatedTo ns:Regret ;
                  ns:similarTo ns:Regret ;
                  rdfs:comment "Disappointment can be considered both an emotion and a trait. As an emotion, disappointment is a feeling of sadness, regret, or discouragement that arises when one's expectations or hopes are not met. It is a temporary state that can be triggered by a specific event or situation. As a trait, disappointment can refer to a tendency or disposition to respond negatively to unmet expectations or to focus on the negative aspects of a situation. It becomes a part of one's personality and can influence how they engage with the world around them. Overall, disappointment can be both an emotion that arises in response to specific circumstances and a trait that shapes a person's overall outlook and behavior." ;
                  rdfs:label "Dissapointment" .


###  http://modai.ai/big5#Dissappointment-Satisfaction
ns:Dissappointment-Satisfaction rdf:type owl:NamedIndividual ,
                                         ns:Prompt ;
                                ns:uses ns:Dissapointment ,
                                        ns:Satisfaction ;
                                rdfs:comment """I want to quantify the disappointment in the following text:
```
$INPUT_TEXT
```

I define disappointment as a feeling of sadness or displeasure caused by the non-fulfillment of one's hopes or expectations. I define the opposite of disappointment as satisfaction or fulfillment.

Please answer on a scale of 1 - 5 where the numbers have the following meanings:
```
1 = The text is filled with satisfaction, fulfillment, and has no elements of disappointment.
2 = The text has elements of satisfaction or fulfillment, but also contains some elements of disappointment.
3 = The text has neither disappointment nor satisfaction, it is neutral.
4 = The text has elements of disappointment but also has some aspects of satisfaction or fulfillment.
5 = The text is deeply filled with disappointment, focusing heavily on feelings of sadness or displeasure.
```

Only respond with a number and no other rating.
"""@en ;
                                rdfs:label "Dissappointment-Satisfaction"@en .


###  http://modai.ai/big5#Dissaproval
ns:Dissaproval rdf:type owl:NamedIndividual ;
               rdfs:comment "Disapproval can be considered both an emotion and a trait. As an emotion, disapproval is a short-lived feeling that arises in response to a specific situation. It may be triggered by something someone says or does that goes against our values, beliefs, or expectations. Disapproval as an emotion is usually characterized by feelings such as disgust, anger, disappointment, or frustration. As a trait, disapproval is a more enduring characteristic of a person's personality. It refers to a tendency to express negative judgments about people, events, or situations. People who have a high level of disapproval may be seen as critical, judgmental, or pessimistic. Disapproval as a trait is a stable and consistent aspect of a person's personality that influences their behavior across a range of situations." ;
               rdfs:label "Dissaproval"@en .


###  http://modai.ai/big5#Dissatisfaction
ns:Dissatisfaction rdf:type owl:NamedIndividual ,
                            ns:Emotion ;
                   ns:oppositeTo ns:Satisfaction ;
                   rdfs:comment "Dissatisfaction can be both an emotion and a trait, depending on how it is defined and experienced. As an emotion, dissatisfaction refers to the feeling of not being fulfilled, pleased, or content with a situation or outcome. It is a temporary experience that arises in response to an external stimulus, such as unmet expectations or frustrations. As a trait, dissatisfaction might describe a more persistent, general tendency to feel dissatisfied with one's life or circumstances. It can be seen as a dispositional characteristic that can affect how a person perceives and responds to various situations over time. In some ways, dissatisfaction as a trait may be related to other personality traits such as neuroticism, pessimism, or perfectionism, which can also affect a person's general outlook and emotional responses. However, it is important to note that distinguishing between trait-related and situational dissatisfaction is complex and that individuals may experience both to varying degrees." ;
                   rdfs:label "Dissatisfaction"@en .


###  http://modai.ai/big5#Distrustful
ns:Distrustful rdf:type owl:NamedIndividual ;
               rdfs:label "Distrustful"@en .


###  http://modai.ai/big5#Dominance
ns:Dominance rdf:type owl:NamedIndividual ;
             rdfs:label "Dominance"@en .


###  http://modai.ai/big5#Dominant
ns:Dominant rdf:type owl:NamedIndividual ;
            rdfs:label "Dominant"@en .


###  http://modai.ai/big5#Doubt
ns:Doubt rdf:type owl:NamedIndividual ,
                  ns:Confusion ;
         ns:relatedTo ns:Apprehension ;
         ns:similarTo ns:Apprehension ;
         rdfs:comment "Doubt can be considered both an emotion and a trait, depending on the context in which it is occurring. As an emotion, doubt refers to the feeling of uncertainty, hesitation, or indecision that can arise in response to a particular situation or event. For example, a person may feel doubt about their ability to accomplish a task, or they may experience doubt about a decision they have made. As a trait, doubt can refer to a more sustained and persistent tendency to question or be skeptical of things. This can be seen in people who are naturally cautious or analytical in their thinking, regularly seeking out more information or evidence before making a decision. In this sense, doubt can be considered a personality trait that influences how a person approaches situations and makes decisions. Overall, whether doubt is perceived as an emotion or a trait may depend on factors such as its duration, intensity, and context." ;
         rdfs:label "Doubt"@en .


###  http://modai.ai/big5#Doubt-Confidence
ns:Doubt-Confidence rdf:type owl:NamedIndividual ,
                             ns:Prompt ;
                    ns:uses ns:Confidence ,
                            ns:Doubt ;
                    rdfs:comment """I want to quantify the doubt in the following text:
```
$INPUT_TEXT
```

I define doubt as a feeling of uncertainty or lack of conviction. I define the opposite of doubt as certainty or confidence.

Please answer on a scale of 1 - 5 where the numbers have the following meanings:
```
1 = The text is filled with certainty, confidence, and has no elements of doubt.
2 = The text has elements of certainty or confidence, but also contains some elements of doubt.
3 = The text has neither doubt nor certainty, it is neutral.
4 = The text has elements of doubt but also has some aspects of certainty or confidence.
5 = The text is deeply filled with doubt, focusing heavily on feelings of uncertainty or lack of conviction.
```

Only respond with a number and no other rating.
"""@en ;
                    rdfs:label "Doubt-Confidence"@en .


###  http://modai.ai/big5#Doubtful
ns:Doubtful rdf:type owl:NamedIndividual ;
            rdfs:label "Doubtful"@en .


###  http://modai.ai/big5#Eager
ns:Eager rdf:type owl:NamedIndividual ;
         rdfs:comment "Eager is more commonly considered a trait rather than an emotion. It describes a person's natural inclination or tendency to be enthusiastic, excited, and keen to do or learn something. While emotions are temporary and fleeting, traits are enduring and consistent qualities of a person's behavior. Therefore, being eager can be seen as a part of someone's personality or character rather than a temporary feeling. However, some might argue that being eager can also be considered an emotion when it is a response to a particular situation or event, such as feeling eager before starting a new job or meeting someone new." ;
         rdfs:label "Eager"@en .


###  http://modai.ai/big5#Eating
ns:Eating rdf:type owl:NamedIndividual ,
                   ns:Behavior ;
          ns:associatedWith ns:Comfort_Seeking ;
          ns:triggeredBy ns:Hunger ,
                         ns:Stress ;
          rdfs:label "Eating"@en .


###  http://modai.ai/big5#Effective
ns:Effective rdf:type owl:NamedIndividual ;
             rdfs:label "Effective"@en .


###  http://modai.ai/big5#Efficient
ns:Efficient rdf:type owl:NamedIndividual ;
             rdfs:label "Efficient"@en .


###  http://modai.ai/big5#Elation
ns:Elation rdf:type owl:NamedIndividual ,
                    ns:Positive_High ;
           ns:oppositeTo ns:Dejection ;
           ns:relatedTo ns:Happiness ,
                        ns:Joy ;
           ns:similarTo ns:Happiness ,
                        ns:Joy ;
           rdfs:comment "Elation can be considered both an emotion and a trait, depending on how it is defined and used in different contexts. As an emotion, elation refers to a feeling of extreme happiness or joy that is often accompanied by other physical and psychological sensations, such as increased energy, euphoria, or a sense of accomplishment or fulfillment. Elation is typically a temporary and intense experience that may be triggered by positive events or experiences, such as achieving a goal, receiving good news, or sharing an intimate moment with a loved one. In this sense, elation is similar to other emotions like happiness, excitement, or pleasure, which are also characterized by positive affect and arousal. As a trait, elation can refer to a more stable or enduring aspect of a person's personality or temperament that predisposes them to experience positive emotions more frequently or intensely than others. For example, someone who is described as \"generally elated\" or \"always upbeat\" may be perceived as someone who is naturally cheerful, optimistic, and enthusiastic about life, regardless of their current circumstances. In this sense, elation can be seen as a dispositional or temperamental trait that influences a person's emotional well-being and outlook on life over time." ;
           rdfs:label "Elation"@en .


###  http://modai.ai/big5#Elation-Dejection
ns:Elation-Dejection rdf:type owl:NamedIndividual ,
                              ns:Prompt ;
                     ns:uses ns:Dejection ,
                             ns:Elation ;
                     rdfs:comment """I want to quantify the elation in the following text:
```
$INPUT_TEXT
```

I define elation as a state of great joy, happiness, or excitement. I define the opposite of elation as despondency or dejection.

Please answer on a scale of 1 - 5 where the numbers have the following meanings:
```
1 = The text is filled with despondency, dejection, and has no elements of elation.
2 = The text has elements of despondency or dejection, but also contains some elements of elation.
3 = The text has neither elation nor despondency, it is neutral.
4 = The text has elements of elation but also has some aspects of despondency or dejection.
5 = The text is deeply filled with elation, focusing heavily on feelings of great joy, happiness, or excitement.
```

Only respond with a number and no other rating.
"""@en ;
                     rdfs:label "Elation-Dejection"@en .


###  http://modai.ai/big5#Embarassment
ns:Embarassment rdf:type owl:NamedIndividual ,
                         ns:Negative_Low ;
                ns:relatedTo ns:Humiliation ,
                             ns:Shame ;
                ns:similarTo ns:Humiliation ,
                             ns:Shame ;
                rdfs:comment "Embarrassment is generally considered to be an emotion rather than a trait. It is a feeling of discomfort or shame that arises from a social situation where one feels self-conscious or exposed. While some people may be more prone to experiencing embarrassment in certain situations, such as when speaking in public or meeting new people, this does not necessarily make it a defining trait of their personality. Rather, it is a response that can vary depending on context and individual factors such as confidence level and past experiences." ;
                rdfs:label "Embarassment"@en .


###  http://modai.ai/big5#Embarassment-Confidence
ns:Embarassment-Confidence rdf:type owl:NamedIndividual ,
                                    ns:Prompt ;
                           ns:uses ns:Confidence ,
                                   ns:Embarassment ;
                           rdfs:comment """I want to quantify the embarrassment in the following text:
```
$INPUT_TEXT
```

I define embarrassment as a feeling of self-consciousness, shame, or awkwardness. I define the opposite of embarrassment as confidence or self-assuredness.

Please answer on a scale of 1 - 5 where the numbers have the following meanings:
```
1 = The text is filled with confidence, self-assuredness, and has no elements of embarrassment.
2 = The text has elements of confidence or self-assuredness, but also contains some elements of embarrassment.
3 = The text has neither embarrassment nor confidence, it is neutral.
4 = The text has elements of embarrassment but also has some aspects of confidence or self-assuredness.
5 = The text is deeply filled with embarrassment, focusing heavily on feelings of self-consciousness, shame, or awkwardness.
```

Only respond with a number and no other rating.
"""@en ;
                           rdfs:label "Embarassment-Confidence"@en .


###  http://modai.ai/big5#Embarrassment
ns:Embarrassment rdf:type owl:NamedIndividual ;
                 rdfs:label "Embarrassment"@en .


###  http://modai.ai/big5#Emotional
ns:Emotional rdf:type owl:NamedIndividual ;
             rdfs:label "Emotional"@en .


###  http://modai.ai/big5#EmotionallyControlled
ns:EmotionallyControlled rdf:type owl:NamedIndividual ;
                         rdfs:label "EmotionallyControlled"@en .


###  http://modai.ai/big5#EmotionallyReactive
ns:EmotionallyReactive rdf:type owl:NamedIndividual ;
                       rdfs:label "EmotionallyReactive"@en .


###  http://modai.ai/big5#Emotionally_Stable
ns:Emotionally_Stable rdf:type owl:NamedIndividual ;
                      rdfs:label "Emotionally_Stable"@en .


###  http://modai.ai/big5#Emotionally_Unstable
ns:Emotionally_Unstable rdf:type owl:NamedIndividual ;
                        rdfs:label "Emotionally_Unstable"@en .


###  http://modai.ai/big5#Empathetic
ns:Empathetic rdf:type owl:NamedIndividual ;
              rdfs:label "Empathetic"@en .


###  http://modai.ai/big5#Empathy
ns:Empathy rdf:type owl:NamedIndividual ;
           rdfs:label "Empathy"@en .


###  http://modai.ai/big5#Energetic
ns:Energetic rdf:type owl:NamedIndividual ;
             rdfs:label "Energetic"@en .


###  http://modai.ai/big5#Engagement
ns:Engagement rdf:type owl:NamedIndividual ;
              ns:relatedTo ns:Sympathy ;
              ns:similarTo ns:Sympathy ;
              rdfs:comment "Engagement can be considered both an emotion and a trait, depending on how it is defined and understood. As an emotion, engagement typically refers to a positive and active state of arousal that involves energy, enthusiasm, and a sense of immersion in an activity or task. This emotional state is often associated with intrinsic motivation, enjoyment, and a sense of flow or absorption in the present moment. As a trait, engagement might be viewed as a more stable quality that reflects a person's tendency to be active, involved, and focused on tasks or goals in general. This trait may be related to personality factors such as conscientiousness, extroversion, or openness to experience. Overall, whether engagement is considered an emotion or a trait may depend on the context in which it is being described and the specific definitions used to characterize it." ;
              rdfs:label "Engagement"@en .


###  http://modai.ai/big5#Enthusiasm
ns:Enthusiasm rdf:type owl:NamedIndividual ;
              rdfs:label "Enthusiasm"@en .


###  http://modai.ai/big5#Enthusiastic
ns:Enthusiastic rdf:type owl:NamedIndividual ;
                ns:relatedTo ns:Eager ,
                             ns:Excitement ;
                rdfs:comment "Enthusiastic can be considered both an emotion and a trait, depending on how it is interpreted and used. As an emotion, enthusiasm is a feeling of excitement, passion, or zest for something. It can be triggered by a particular event or circumstance, and can be accompanied by physical sensations such as increased heart rate, sweating, or a burst of energy. In this sense, enthusiasm is a temporary emotion that comes and goes, depending on the situation. On the other hand, as a trait, enthusiasm is a more enduring aspect of a person's personality. It refers to the tendency to approach tasks, activities, or interactions with energy, excitement, and positivity. Individuals with this trait are often described as optimistic, proactive, and driven, and their enthusiasm is seen as a key factor in their success and satisfaction. In this sense, enthusiasm is a stable disposition that characterizes a person's overall approach to life." ;
                rdfs:label "Enthusiastic"@en .


###  http://modai.ai/big5#Envy
ns:Envy rdf:type owl:NamedIndividual ,
                 ns:Negative_High ;
        ns:oppositeTo ns:Contentment ;
        ns:relatedTo ns:Discontent ,
                     ns:Jealousy ,
                     ns:Resentment ;
        ns:similarTo ns:Discontent ,
                     ns:Jealousy ,
                     ns:Resentment ;
        rdfs:comment "Envy can be considered both an emotion and a trait, depending on how it is defined and understood. As an emotion, envy refers to the experience of feeling resentful or bitter towards someone else because of their success, achievements, or possessions. This feeling is often accompanied by a desire to possess what the other person has and may lead to negative thoughts and behaviors such as jealousy, anger, or even sabotage. As a trait, envy refers to a person's tendency to feel envy more frequently or intensely than others. This can be seen as part of a person's personality or character and may be influenced by their upbringing, life experiences, or psychological makeup. Ultimately, envy is a complex psychological phenomenon that can be both an emotion and a trait, and understanding its nature and causes can help individuals better manage and cope with their feelings of envy." ;
        rdfs:label "Envy"@en .


###  http://modai.ai/big5#Envy-Contentment
ns:Envy-Contentment rdf:type owl:NamedIndividual ,
                             ns:Prompt ;
                    ns:uses ns:Contentment ,
                            ns:Envy ;
                    rdfs:comment """I want to quantify the envy in the following text:
```
$INPUT_TEXT
```

I define envy as a feeling of discontented or resentful longing aroused by someone else's possessions, qualities, or luck. I define the opposite of envy as contentment or satisfaction with one's own possessions, qualities, or luck.

Please answer on a scale of 1 - 5 where the numbers have the following meanings:
```
1 = The text is filled with contentment, satisfaction, and has no elements of envy.
2 = The text has elements of contentment or satisfaction, but also contains some elements of envy.
3 = The text has neither envy nor contentment, it is neutral.
4 = The text has elements of envy but also has some content or satisfied aspects.
5 = The text is deeply filled with envy, focusing heavily on discontented or resentful longing.
```

Only respond with a number and no other rating.
"""@en ;
                    rdfs:label "Envy-Contentment"@en .


###  http://modai.ai/big5#Excited
ns:Excited rdf:type owl:NamedIndividual ;
           rdfs:label "Excited"@en .


###  http://modai.ai/big5#Excitement
ns:Excitement rdf:type owl:NamedIndividual ,
                       ns:Positive_High ;
              ns:relatedTo ns:Anticipation ;
              ns:similarTo ns:Anticipation ;
              rdfs:comment "Excitement can be considered both an emotion and a trait, depending on how it is defined and interpreted. As an emotion, excitement is a temporary feeling of enthusiasm, anticipation, and happiness that can be triggered by various events or stimuli. For example, a person may feel excited about attending a concert, receiving a promotion, or going on a vacation. As a trait, excitement can refer to a person's general tendency to experience and express excitement in their daily life. Some people may be naturally more prone to excitement, while others may be more reserved and less likely to express enthusiasm. So, depending on the context, excitement can be seen as either a temporary emotion or a more enduring personality trait." ;
              rdfs:label "Excitement"@en .


###  http://modai.ai/big5#Excitement-Apathy
ns:Excitement-Apathy rdf:type owl:NamedIndividual ,
                              ns:Prompt ;
                     ns:uses ns:Apathy ,
                             ns:Excitement ;
                     rdfs:comment """I want to quantify the excitement in the following text:
```
$INPUT_TEXT
```

I define excitement as a feeling of anticipation about something that is going to happen in the near future. I define the opposite of excitement as apathy or lack of interest.

Please answer on a scale of 1 - 5 where the numbers have the following meanings:
```
1 = The text is filled with apathy, lack of interest, and has no elements of excitement.
2 = The text has elements of apathy or lack of interest, but also contains some elements of excitement.
3 = The text has neither excitement nor apathy, it is neutral.
4 = The text has elements of excitement but also has some apathetic or disinterested aspects.
5 = The text is deeply filled with excitement, focusing heavily on excitement about future events.
```

Only respond with a number and no other rating.
"""@en ;
                     rdfs:label "Excitement-Apathy"@en .


###  http://modai.ai/big5#Exclusion
ns:Exclusion rdf:type owl:NamedIndividual ;
             ns:relatedTo ns:Rejection ;
             ns:similarTo ns:Rejection ;
             rdfs:comment "Exclusion is not an emotion or a trait on its own. Rather, it can be considered a behavior or a result of certain emotions or traits. Exclusion may result from emotions such as envy, jealousy, or resentment, or it may be a trait that someone exhibits based on their personality, upbringing, or experiences. However, exclusion can also be a conscious choice made by individuals or groups, which can be influenced by their emotions, traits, or other factors such as social norms or power dynamics. In summary, exclusion is not an emotion or trait but a complex behavior influenced by various factors." ;
             rdfs:label "Exclusion"@en .


###  http://modai.ai/big5#Exercising
ns:Exercising rdf:type owl:NamedIndividual ,
                       ns:Behavior ;
              ns:associatedWith ns:Discipline ;
              ns:triggeredBy ns:Determination ,
                             ns:Stress ;
              rdfs:label "Exercising"@en .


###  http://modai.ai/big5#Exhaustion
ns:Exhaustion rdf:type owl:NamedIndividual ;
              rdfs:label "Exhaustion"@en .


###  http://modai.ai/big5#Expectation
ns:Expectation rdf:type owl:NamedIndividual ;
               ns:relatedTo ns:Hope ;
               ns:similarTo ns:Hope ;
               rdfs:comment "Expectation is neither an emotion nor a trait, but rather a cognitive process. It involves anticipating or predicting future events or outcomes based on past experiences, beliefs, or information. However, one's level of expectation can be influenced by their personality traits, such as optimism or pessimism, which in turn can impact their emotional response to an outcome that meets or fails to meet their expectations. For example, a person with high expectations might feel disappointed or frustrated if an outcome does not meet their expectations, while a person with lower expectations might feel more content or even pleasantly surprised by the same outcome. Overall, expectation can affect emotions and behavior, but it is not itself an emotion or trait." ;
               rdfs:label "Expectation"@en .


###  http://modai.ai/big5#Expressiveness
ns:Expressiveness rdf:type owl:NamedIndividual ;
                  rdfs:label "Expressiveness"@en .


###  http://modai.ai/big5#Extraverted
ns:Extraverted rdf:type owl:NamedIndividual ;
               rdfs:label "Extraverted"@en .


###  http://modai.ai/big5#Extroverted
ns:Extroverted rdf:type owl:NamedIndividual ,
                        ns:Trait ;
               ns:oppositeTo ns:Introverted ;
               rdfs:comment "Extroverted is a personality trait, not an emotion. It refers to the tendency to seek out social interaction and draw energy from external stimulation. This trait is typically considered a part of one's overall personality, along with other traits such as openness to experience, conscientiousness, agreeableness, and neuroticism. While emotions can certainly influence a person's extroverted behavior (e.g. feeling happy and energized in social situations), extroversion itself is more stable and enduring than any particular emotion." ;
               rdfs:label "Extroverted"@en .


###  http://modai.ai/big5#Fault_Finding
ns:Fault_Finding rdf:type owl:NamedIndividual ;
                 rdfs:label "Fault_Finding"@en .


###  http://modai.ai/big5#Fear
ns:Fear rdf:type owl:NamedIndividual ,
                 ns:Negative_High ;
        rdfs:comment "Fear is generally considered to be an emotion. Emotions are defined as mental states associated with distinct feelings, physiological reactions, and behaviors. Fear is an emotion that arises in response to a perceived threat or danger and can be experienced in varying degrees of intensity and duration. Trait, on the other hand, refers to a relatively enduring characteristic or quality that describes a person's typical patterns of thinking, feeling, and behaving. While some people may be more prone to experiencing fear in certain situations, fear is not considered a stable or enduring trait in the same way that personality traits are. Rather, fear is a normal and adaptive emotional response that serves a protective function and can be overcome through strategies such as exposure therapy and cognitive-behavioral techniques." ;
        rdfs:label "Fear"@en .


###  http://modai.ai/big5#Fear-Fearless
ns:Fear-Fearless rdf:type owl:NamedIndividual ;
                 ns:uses ns:Fear ,
                         ns:Fearless ;
                 rdfs:comment """I want to quantify the fearfulness in the following text:
```
$INPUT_TEXT
```

I define fearfulness as a state of being afraid, anxious, or full of fear. I define the opposite of fearfulness as courage or fearlessness.

Please answer on a scale of 1 - 5 where the numbers have the following meanings:
```
1 = The text is filled with courage, fearlessness, and has no elements of fearfulness.
2 = The text has elements of courage or fearlessness, but also contains some elements of fearfulness.
3 = The text has neither fearfulness nor courage, it is neutral.
4 = The text has elements of fearfulness but also has some aspects of courage or fearlessness.
5 = The text is deeply filled with fearfulness, focusing heavily on feelings of being afraid, anxious, or full of fear.
```

Only respond with a number and no other rating.
"""@en ;
                 rdfs:label "Fear-Fearless"@en .


###  http://modai.ai/big5#Fear-Safety
ns:Fear-Safety rdf:type owl:NamedIndividual ;
               ns:uses ns:Fear ,
                       ns:Safety ;
               rdfs:comment """I want to quantify the fear in the following text:
```
$INPUT_TEXT
```

I define fear as an unpleasant emotion caused by the belief that someone or something is dangerous, likely to cause pain, or a threat. I define the opposite of fear as safety or comfort.

Please answer on a scale of 1 - 5 where the numbers have the following meanings:
```
1 = The text is filled with feelings of safety, comfort, and has no elements of fear.
2 = The text has elements of safety or comfort, but also contains some elements of fear.
3 = The text has neither fear nor feelings of safety, it is neutral.
4 = The text has elements of fear but also has some neutral or comforting aspects.
5 = The text is deeply filled with fear, focusing heavily on perceived danger, pain, or threat.
```

Only respond with a number and no other rating.
"""@en ;
               rdfs:label "Fear-Safety"@en .


###  http://modai.ai/big5#Fearful
ns:Fearful rdf:type owl:NamedIndividual ;
           rdfs:label "Fearful"@en .


###  http://modai.ai/big5#Fearless
ns:Fearless rdf:type owl:NamedIndividual ,
                     ns:Trait ;
            ns:oppositeTo ns:Fear ;
            rdfs:comment "Fearless can be considered both an emotion and a trait, depending on the perspective and context. As an emotion, fearless can be seen as the absence of fear and the feeling of courage or confidence in facing challenges or threats. It is a temporary state of mind that arises in response to a particular situation or stimulus. As a trait, fearless can be viewed as a characteristic or quality that someone possesses consistently across different situations and contexts. It can refer to a person's tendency to take risks, be bold, and face fears head-on. In this sense, fearless is more of a disposition or personality trait that is partly innate and partly learned through life experiences. Overall, whether fearless is considered an emotion or a trait may depend on how one conceptualizes and defines these terms and what kind of evidence or observations support or refute the claim." ;
            rdfs:label "Fearless"@en .


###  http://modai.ai/big5#Flirtation
ns:Flirtation rdf:type owl:NamedIndividual ;
              rdfs:label "Flirtation"@en .


###  http://modai.ai/big5#Followership
ns:Followership rdf:type owl:NamedIndividual ;
                rdfs:label "Followership"@en .


###  http://modai.ai/big5#Forgiving
ns:Forgiving rdf:type owl:NamedIndividual ;
             rdfs:label "Forgiving"@en .


###  http://modai.ai/big5#Forgivness
ns:Forgivness rdf:type owl:NamedIndividual ,
                       ns:Trait ;
              ns:relatedTo ns:Acceptance ;
              ns:similarTo ns:Acceptance ;
              rdfs:comment "Forgiveness can be both an emotion and a trait. As an emotion, forgiveness can be experienced as a feeling of relief or release from negative emotions such as anger, resentment, or bitterness. It may come after a period of sadness or pain, often resulting from the hurt caused by someone else's actions. Additionally, forgiveness as an emotion can arise spontaneously, suggesting it is not necessarily a deliberate and controlled decision, but rather a reflexive response to others' actions. As a trait, forgiveness refers to a person's general tendency to forgive others and offer mercy and grace when wronged, even when they may not deserve it. A forgiving individual may act with empathy and compassion and demonstrate an openness to forgive others quickly, with or without overt acts of remorse on the part of the offender. In this sense, the trait of forgiveness can be thought of as a personality characteristic or a learned behavior. Overall, forgiveness is a complex phenomenon that can be experienced emotionally and characterized as a preferred response to interpersonal conflict. Thus, it can be both an emotion and a trait." ;
              rdfs:label "Forgivness"@en .


###  http://modai.ai/big5#Frowning
ns:Frowning rdf:type owl:NamedIndividual ,
                     ns:Behavior ;
            ns:associatedWith ns:Unhappiness ;
            ns:triggeredBy ns:Anger ,
                           ns:Discontent ;
            rdfs:label "Frowning"@en .


###  http://modai.ai/big5#Frustration
ns:Frustration rdf:type owl:NamedIndividual ;
               rdfs:label "Frustration"@en .


###  http://modai.ai/big5#Fulfillment
ns:Fulfillment rdf:type owl:NamedIndividual ,
                        ns:Emotion ;
               ns:relatedTo ns:Satisfaction ;
               ns:similarTo ns:Satisfaction ;
               rdfs:comment "Fulfillment is not necessarily an emotion or a trait on its own, but it can be experienced as an emotion or cultivated as a personal trait. As an emotion, fulfillment is typically associated with a sense of satisfaction or achievement that comes from accomplishing a goal or meeting a need. It can be a positive feeling that arises from a sense of accomplishment or contentment with one's life situation. As a trait, fulfillment might be seen as a personal quality that one cultivates over time through habits and choices that promote well-being and a sense of purpose. For example, a person might develop a daily meditation practice or engage in activities that bring them joy and fulfillment, over time becoming known for their ability to find contentment and meaning in life. So while fulfillment can be experienced as an emotion, it can also be a personal trait that is developed over time through intentional actions and choices." ;
               rdfs:label "Fulfillment"@en .


###  http://modai.ai/big5#GoodHumor
ns:GoodHumor rdf:type owl:NamedIndividual ;
             rdfs:label "GoodHumor"@en .


###  http://modai.ai/big5#Gossiping
ns:Gossiping rdf:type owl:NamedIndividual ,
                      ns:Behavior ;
             ns:associatedWith ns:Inquisitiveness ;
             ns:triggeredBy ns:Curiosity ,
                            ns:Envy ;
             rdfs:label "Gossiping"@en .


###  http://modai.ai/big5#Gratitude
ns:Gratitude rdf:type owl:NamedIndividual ,
                      ns:Positive_Low ;
             ns:oppositeTo ns:Ingratitude ;
             rdfs:comment "Gratitude can be considered both an emotion and a trait. As an emotion, gratitude is a feeling that arises in response to something positive or beneficial that has happened to us. It can be experienced as a sense of appreciation, happiness, or thankfulness for the blessings we have received. As a trait, gratitude is considered a consistent pattern of behavior that reflects our attitudes and thoughts towards the world around us. It refers to an individuals tendency to recognize and appreciate the positive aspects of their life, and to express gratitude towards others. Therefore, gratitude can be considered both a transitory emotional response and a more long-term characteristic or trait of a person's personality. It is something that can be cultivated and strengthened over time through intentional practice and inculcation of a positive mindset." ;
             rdfs:label "Gratitude"@en .


###  http://modai.ai/big5#Gratitude-Ingratitude
ns:Gratitude-Ingratitude rdf:type owl:NamedIndividual ,
                                  ns:Prompt ;
                         ns:uses ns:Gratitude ,
                                 ns:Ingratitude ;
                         rdfs:comment """I want to quantify the gratitude in the following text:
```
$INPUT_TEXT
```

I define gratitude as a warm feeling of thankfulness towards someone or for something. I define the opposite of gratitude as ingratitude or ungratefulness.

Please answer on a scale of 1 - 5 where the numbers have the following meanings:
```
1 = The text is filled with ingratitude, ungratefulness, and has no elements of gratitude.
2 = The text has elements of ingratitude, but also contains some elements of gratitude.
3 = The text has neither gratitude nor ingratitude, it is neutral.
4 = The text has elements of gratitude but also has some aspects of ungratefulness.
5 = The text is deeply filled with gratitude, focusing heavily on feelings of thankfulness.
```

Only respond with a number and no other rating.
"""@en ;
                         rdfs:label "Gratitude-Ingratitude"@en .


###  http://modai.ai/big5#Guilt
ns:Guilt rdf:type owl:NamedIndividual ,
                  ns:Negative_Low ;
         ns:oppositeTo ns:Innocence ;
         ns:relatedTo ns:Depression ;
         ns:similarTo ns:Depression ;
         rdfs:comment "Guilt can be considered both an emotion and a trait, depending on how it is defined and understood. As an emotion, guilt is associated with feelings of regret, remorse, and responsibility for wrongdoing or causing harm to others. It is typically experienced in response to a specific action or situation, and can be a normal and healthy response to acknowledging one's mistakes or shortcomings. As a trait, guilt can refer to a tendency or predisposition to feel guilty or blame oneself, even in situations where one may not be entirely responsible or there may be mitigating factors. This can be seen as a more stable and consistent aspect of one's personality or psychological makeup, and may be associated with traits such as anxiety, depression, or perfectionism. Ultimately, whether guilt is considered more of an emotion or a trait may depend on how it is conceptualized and studied within different fields of psychology and philosophy." ;
         rdfs:label "Guilt"@en .


###  http://modai.ai/big5#Guilt-Innocence
ns:Guilt-Innocence rdf:type owl:NamedIndividual ,
                            ns:Prompt ;
                   ns:uses ns:Guilt ,
                           ns:Innocence ;
                   rdfs:comment """I want to quantify the guilt in the following text:
```
$INPUT_TEXT
```

I define guilt as a feeling of having done wrong or failed in an obligation. I define the opposite of guilt as innocence or a feeling of having done right.

Please answer on a scale of 1 - 5 where the numbers have the following meanings:
```
1 = The text is filled with innocence, feelings of having done right, and has no elements of guilt.
2 = The text has elements of innocence or feelings of having done right, but also contains some elements of guilt.
3 = The text has neither guilt nor innocence, it is neutral.
4 = The text has elements of guilt but also has some aspects of innocence or feelings of having done right.
5 = The text is deeply filled with guilt, focusing heavily on feelings of having done wrong or failed in an obligation.
```

Only respond with a number and no other rating.
"""@en ;
                   rdfs:label "Guilt-Innocence"@en .


###  http://modai.ai/big5#Gullible
ns:Gullible rdf:type owl:NamedIndividual ;
            rdfs:label "Gullible"@en .


###  http://modai.ai/big5#HEX_00BFFF
ns:HEX_00BFFF rdf:type owl:NamedIndividual ,
                       ns:Color ;
              rdfs:label "00BFFF" .


###  http://modai.ai/big5#HEX_00FA9A
ns:HEX_00FA9A rdf:type owl:NamedIndividual ,
                       ns:Color ;
              rdfs:label "00FA9A" .


###  http://modai.ai/big5#HEX_00FF7F
ns:HEX_00FF7F rdf:type owl:NamedIndividual ,
                       ns:Color ;
              rdfs:label "00FF7F" .


###  http://modai.ai/big5#HEX_32CD32
ns:HEX_32CD32 rdf:type owl:NamedIndividual ,
                       ns:Color ;
              rdfs:label "32CD32" .


###  http://modai.ai/big5#HEX_4682B4
ns:HEX_4682B4 rdf:type owl:NamedIndividual ,
                       ns:Color ;
              rdfs:label "4682B4" .


###  http://modai.ai/big5#HEX_556B2F
ns:HEX_556B2F rdf:type owl:NamedIndividual ,
                       ns:Color ;
              rdfs:label "556B2F" .


###  http://modai.ai/big5#HEX_5F9EA0
ns:HEX_5F9EA0 rdf:type owl:NamedIndividual ,
                       ns:Color ;
              rdfs:label "5F9EA0" .


###  http://modai.ai/big5#HEX_696969
ns:HEX_696969 rdf:type owl:NamedIndividual ,
                       ns:Color ;
              rdfs:label "696969" .


###  http://modai.ai/big5#HEX_6A737D
ns:HEX_6A737D rdf:type owl:NamedIndividual ,
                       ns:Color ;
              rdfs:label "6A737D" .


###  http://modai.ai/big5#HEX_6B8E23
ns:HEX_6B8E23 rdf:type owl:NamedIndividual ,
                       ns:Color ;
              rdfs:label "6B8E23" .


###  http://modai.ai/big5#HEX_708090
ns:HEX_708090 rdf:type owl:NamedIndividual ,
                       ns:Color ;
              rdfs:label "708090" .


###  http://modai.ai/big5#HEX_748CA3
ns:HEX_748CA3 rdf:type owl:NamedIndividual ,
                       ns:Color ;
              rdfs:label "748CA3" .


###  http://modai.ai/big5#HEX_778899
ns:HEX_778899 rdf:type owl:NamedIndividual ,
                       ns:Color ;
              rdfs:label "778899" .


###  http://modai.ai/big5#HEX_7CFC00
ns:HEX_7CFC00 rdf:type owl:NamedIndividual ,
                       ns:Color ;
              rdfs:label "7CFC00" .


###  http://modai.ai/big5#HEX_7FFFD4
ns:HEX_7FFFD4 rdf:type owl:NamedIndividual ,
                       ns:Color ;
              rdfs:label "7FFFD4" .


###  http://modai.ai/big5#HEX_808080
ns:HEX_808080 rdf:type owl:NamedIndividual ,
                       ns:Color ;
              rdfs:label "808080" .


###  http://modai.ai/big5#HEX_8198C9
ns:HEX_8198C9 rdf:type owl:NamedIndividual ,
                       ns:Color ;
              rdfs:label "8198C9" .


###  http://modai.ai/big5#HEX_87CEFA
ns:HEX_87CEFA rdf:type owl:NamedIndividual ,
                       ns:Color ;
              rdfs:label "87CEFA" .


###  http://modai.ai/big5#HEX_8B0000
ns:HEX_8B0000 rdf:type owl:NamedIndividual ,
                       ns:Color ;
              rdfs:label "8B0000" .


###  http://modai.ai/big5#HEX_8B4513
ns:HEX_8B4513 rdf:type owl:NamedIndividual ,
                       ns:Color ;
              rdfs:label "8B4513" .


###  http://modai.ai/big5#HEX_8CA5DF
ns:HEX_8CA5DF rdf:type owl:NamedIndividual ,
                       ns:Color ;
              rdfs:label "8CA5DF" .


###  http://modai.ai/big5#HEX_97B3F5
ns:HEX_97B3F5 rdf:type owl:NamedIndividual ,
                       ns:Color ;
              rdfs:label "97B3F5" .


###  http://modai.ai/big5#HEX_98FB98
ns:HEX_98FB98 rdf:type owl:NamedIndividual ,
                       ns:Color ;
              rdfs:label "98FB98" .


###  http://modai.ai/big5#HEX_9ACD32
ns:HEX_9ACD32 rdf:type owl:NamedIndividual ,
                       ns:Color ;
              rdfs:label "9ACD32" .


###  http://modai.ai/big5#HEX_A0522D
ns:HEX_A0522D rdf:type owl:NamedIndividual ,
                       ns:Color ;
              rdfs:label "A0522D" .


###  http://modai.ai/big5#HEX_A52A2A
ns:HEX_A52A2A rdf:type owl:NamedIndividual ,
                       ns:Color ;
              rdfs:label "A52A2A" .


###  http://modai.ai/big5#HEX_A9A9A9
ns:HEX_A9A9A9 rdf:type owl:NamedIndividual ,
                       ns:Color ;
              rdfs:label "A9A9A9" .


###  http://modai.ai/big5#HEX_ADD8E6
ns:HEX_ADD8E6 rdf:type owl:NamedIndividual ,
                       ns:Color ;
              rdfs:label "ADD8E6" .


###  http://modai.ai/big5#HEX_ADFF2F
ns:HEX_ADFF2F rdf:type owl:NamedIndividual ,
                       ns:Color ;
              rdfs:label "ADFF2F" .


###  http://modai.ai/big5#HEX_AFEEEE
ns:HEX_AFEEEE rdf:type owl:NamedIndividual ,
                       ns:Color ;
              rdfs:label "AFEEEE" .


###  http://modai.ai/big5#HEX_B0C4DE
ns:HEX_B0C4DE rdf:type owl:NamedIndividual ,
                       ns:Color ;
              rdfs:label "B0C4DE" .


###  http://modai.ai/big5#HEX_B0E0E6
ns:HEX_B0E0E6 rdf:type owl:NamedIndividual ,
                       ns:Color ;
              rdfs:label "B0E0E6" .


###  http://modai.ai/big5#HEX_C0C0C0
ns:HEX_C0C0C0 rdf:type owl:NamedIndividual ,
                       ns:Color ;
              rdfs:label "C0C0C0" .


###  http://modai.ai/big5#HEX_CD5C5C
ns:HEX_CD5C5C rdf:type owl:NamedIndividual ,
                       ns:Color ;
              rdfs:label "CD5C5C" .


###  http://modai.ai/big5#HEX_CD853F
ns:HEX_CD853F rdf:type owl:NamedIndividual ,
                       ns:Color ;
              rdfs:label "CD853F" .


###  http://modai.ai/big5#HEX_CDB79E
ns:HEX_CDB79E rdf:type owl:NamedIndividual ,
                       ns:Color ;
              rdfs:label "CDB79E" .


###  http://modai.ai/big5#HEX_D2B48C
ns:HEX_D2B48C rdf:type owl:NamedIndividual ,
                       ns:Color ;
              rdfs:label "D2B48C" .


###  http://modai.ai/big5#HEX_D3D3D3
ns:HEX_D3D3D3 rdf:type owl:NamedIndividual ,
                       ns:Color ;
              rdfs:label "D3D3D3" .


###  http://modai.ai/big5#HEX_DAA520
ns:HEX_DAA520 rdf:type owl:NamedIndividual ,
                       ns:Color ;
              rdfs:label "DAA520" .


###  http://modai.ai/big5#HEX_DEB887
ns:HEX_DEB887 rdf:type owl:NamedIndividual ,
                       ns:Color ;
              rdfs:label "DEB887" .


###  http://modai.ai/big5#HEX_F08080
ns:HEX_F08080 rdf:type owl:NamedIndividual ,
                       ns:Color ;
              rdfs:label "F08080" .


###  http://modai.ai/big5#HEX_F4A460
ns:HEX_F4A460 rdf:type owl:NamedIndividual ,
                       ns:Color ;
              rdfs:label "F4A460" .


###  http://modai.ai/big5#HEX_F5DEB3
ns:HEX_F5DEB3 rdf:type owl:NamedIndividual ,
                       ns:Color ;
              rdfs:label "F5DEB3" .


###  http://modai.ai/big5#HEX_F5F5DC
ns:HEX_F5F5DC rdf:type owl:NamedIndividual ,
                       ns:Color ;
              rdfs:label "F5F5DC" .


###  http://modai.ai/big5#HEX_FA8072
ns:HEX_FA8072 rdf:type owl:NamedIndividual ,
                       ns:Color ;
              rdfs:label "FA8072" .


###  http://modai.ai/big5#HEX_FFD700
ns:HEX_FFD700 rdf:type owl:NamedIndividual ,
                       ns:Color ;
              rdfs:label "FFD700" .


###  http://modai.ai/big5#HEX_FFF8DC
ns:HEX_FFF8DC rdf:type owl:NamedIndividual ,
                       ns:Color ;
              rdfs:label "FFF8DC" .


###  http://modai.ai/big5#HEX_FFFFF0
ns:HEX_FFFFF0 rdf:type owl:NamedIndividual ,
                       ns:Color ;
              rdfs:label "FFFFF0" .


###  http://modai.ai/big5#Happiness
ns:Happiness rdf:type owl:NamedIndividual ,
                      ns:Emotion ;
             ns:oppositeTo ns:Sadness ;
             ns:relatedTo ns:Contentment ,
                          ns:Elation ;
             ns:similarTo ns:Contentment ,
                          ns:Elation ;
             rdfs:comment "Happiness can be considered both an emotion and a trait. As an emotion, happiness is a temporary state of mind characterized by positive feelings and a sense of well-being. It is typically triggered by specific events or circumstances such as achieving a goal, receiving a compliment, or spending time with loved ones. As a trait, happiness refers to a person's overall tendency to experience positive emotions and their ability to maintain a positive outlook despite challenges and setbacks. This trait is often related to factors such as genetics, personality, and life experiences. Therefore, happiness can be understood both as a temporary emotional response to certain situations, and as a long-term personality trait that shapes how individuals approach and experience life." ;
             rdfs:label "Happiness"@en .


###  http://modai.ai/big5#Happy
ns:Happy rdf:type owl:NamedIndividual ;
         rdfs:label "Happy"@en .


###  http://modai.ai/big5#Harsh
ns:Harsh rdf:type owl:NamedIndividual ;
         rdfs:label "Harsh"@en .


###  http://modai.ai/big5#Hate
ns:Hate rdf:type owl:NamedIndividual ,
                 ns:Social ;
        ns:relatedTo ns:Dislike ;
        ns:similarTo ns:Dislike ;
        rdfs:comment "Hate can be considered both an emotion and a trait, depending on how it is defined and understood. As an emotion, hate is a strong feeling of dislike and animosity towards someone or something. It is often accompanied by anger, resentment, or even fear. When someone experiences hate, it can lead to negative behaviors and actions, such as aggression, discrimination, or violence. As a trait, hate can be seen as a more persistent and ingrained characteristic of a person's personality. Some people may have a tendency to hold onto grudges or harbor feelings of animosity towards certain individuals or groups over a long period of time, even in the absence of any provocation or negative behavior. This can lead to a general sense of hostility and negative attitudes towards others. Overall, hate can be both an emotion and a trait, and understanding the ways in which it can manifest is important in addressing both individual and societal issues related to hate and intolerance." ;
        rdfs:label "Hate"@en .


###  http://modai.ai/big5#Hate-Love
ns:Hate-Love rdf:type owl:NamedIndividual ,
                      ns:Prompt ;
             ns:uses ns:Hate ,
                     ns:Love ;
             rdfs:comment """I want to quantify the hate in the following text:
```
$INPUT_TEXT
```

I define hate as intense or passionate dislike. I define the opposite of hate as love or affection.

Please answer on a scale of 1 - 5 where the numbers have the following meanings:
```
1 = The text is filled with love, affection, and has no elements of hate.
2 = The text has elements of love or affection, but also contains some elements of hate.
3 = The text has neither hate nor love, it is neutral.
4 = The text has elements of hate but also has some loving or affectionate aspects.
5 = The text is deeply filled with hate, focusing heavily on intense or passionate dislike.
```

Only respond with a number and no other rating.
"""@en ;
             rdfs:label "Hate-Love"@en .


###  http://modai.ai/big5#Helpful
ns:Helpful rdf:type owl:NamedIndividual ;
           rdfs:label "Helpful"@en .


###  http://modai.ai/big5#Hiding
ns:Hiding rdf:type owl:NamedIndividual ,
                   ns:Behavior ;
          ns:associatedWith ns:Timidity ;
          ns:triggeredBy ns:Fear ,
                         ns:Shame ;
          rdfs:label "Hiding"@en .


###  http://modai.ai/big5#HighEnergy
ns:HighEnergy rdf:type owl:NamedIndividual ;
              rdfs:label "HighEnergy"@en .


###  http://modai.ai/big5#Hitting
ns:Hitting rdf:type owl:NamedIndividual ,
                    ns:Behavior ;
           ns:associatedWith ns:Aggression ;
           ns:triggeredBy ns:Anger ,
                          ns:Frustration ;
           rdfs:label "Hitting"@en .


###  http://modai.ai/big5#Hope
ns:Hope rdf:type owl:NamedIndividual ,
                 ns:Positive_Low ;
        ns:relatedTo ns:Courage ;
        ns:similarTo ns:Courage ;
        rdfs:comment "Hope can be considered both an emotion and a trait, depending on the context in which it is being discussed. As an emotion, hope is a feeling of optimism and positivity about the future. It can arise spontaneously in response to a positive event or circumstance, or it can be consciously cultivated by directing one's thoughts toward positive outcomes and possibilities. As a trait, hope refers to an individual's tendency to view the future in a positive light and to persist in the face of obstacles. It is a stable personality characteristic that influences the way people think, feel, and behave over time. Some people are naturally more hopeful than others, and this trait can be enhanced through deliberate effort and practice. Overall, hope can be seen as both a feeling and a character trait that can have a positive impact on individuals and their lives." ;
        rdfs:label "Hope"@en .


###  http://modai.ai/big5#Hope-Despair
ns:Hope-Despair rdf:type owl:NamedIndividual ,
                         ns:Prompt ;
                ns:uses ns:Despair ,
                        ns:Hope ;
                rdfs:comment """I want to quantify the hope in the following text:
```
$INPUT_TEXT
```

I define hope as a feeling of optimism, desire, or expectation for a positive outcome. I define the opposite of hope as despair or hopelessness.

Please answer on a scale of 1 - 5 where the numbers have the following meanings:
```
1 = The text is filled with despair, hopelessness, and has no elements of hope.
2 = The text has elements of despair or hopelessness, but also contains some elements of hope.
3 = The text has neither hope nor despair, it is neutral.
4 = The text has elements of hope but also has some aspects of despair or hopelessness.
5 = The text is deeply filled with hope, focusing heavily on feelings of optimism, desire, or expectation for a positive outcome.
```

Only respond with a number and no other rating.
"""@en ;
                rdfs:label "Hope-Despair"@en .


###  http://modai.ai/big5#Hopeless
ns:Hopeless rdf:type owl:NamedIndividual ;
            rdfs:label "Hopeless"@en .


###  http://modai.ai/big5#Hopelessness
ns:Hopelessness rdf:type owl:NamedIndividual ;
                ns:relatedTo ns:Despair ;
                ns:similarTo ns:Despair ;
                rdfs:comment "Hopelessness can be considered both an emotion and a trait. As an emotion, hopelessness refers to a temporary feeling of despair or pessimism about one's circumstances or future. This emotional state is often associated with specific events or situations that have caused disappointment or loss, such as the death of a loved one, a job loss, or a relationship breakdown. As a trait, hopelessness refers to a more enduring tendency to experience negative emotions, such as hopelessness, pessimism, and despair. This trait is often associated with a general outlook on life and can be influenced by a combination of genetic, environmental, and psychological factors. People who exhibit high levels of hopelessness may be more likely to experience depression, anxiety, and other mental health issues." ;
                rdfs:label "Hopelessness"@en .


###  http://modai.ai/big5#Humiliation
ns:Humiliation rdf:type owl:NamedIndividual ;
               ns:oppositeTo ns:Dignity ;
               ns:relatedTo ns:Shame ;
               ns:similarTo ns:Shame ;
               rdfs:comment "Humiliation can be considered both an emotion and a trait. As an emotion, humiliation is a feeling of distress or shame that arises from a perceived failure or social rejection. It is a temporary state that is often accompanied by physical and emotional reactions such as blushing, sweating, and feeling embarrassed. As a trait, humiliation can refer to a tendency or disposition to experience humiliation more frequently and intensely than others. This could be due to a variety of factors such as past experiences, personality traits, or cultural background. Overall, while humiliation can be both an emotion and a trait, it is important to distinguish between the two in order to understand how it manifests in individuals and how it can be addressed." ;
               rdfs:label "Humiliation"@en .


###  http://modai.ai/big5#Humiliation-Dignity
ns:Humiliation-Dignity rdf:type owl:NamedIndividual ,
                                ns:Prompt ;
                       ns:uses ns:Dignity ,
                               ns:Humiliation ;
                       rdfs:comment """I want to quantify the humiliation in the following text:
```
$INPUT_TEXT
```

I define humiliation as a feeling of embarrassment, shame, or degradation caused by others or by one's own actions. I define the opposite of humiliation as dignity or pride.

Please answer on a scale of 1 - 5 where the numbers have the following meanings:
```
1 = The text is filled with dignity, pride, and has no elements of humiliation.
2 = The text has elements of dignity or pride, but also contains some elements of humiliation.
3 = The text has neither humiliation nor dignity, it is neutral.
4 = The text has elements of humiliation but also has some aspects of dignity or pride.
5 = The text is deeply filled with humiliation, focusing heavily on feelings of embarrassment, shame, or degradation caused by others or by one's own actions.
```

Only respond with a number and no other rating.
"""@en ;
                       rdfs:label "Humiliation-Dignity"@en .


###  http://modai.ai/big5#Humility
ns:Humility rdf:type owl:NamedIndividual ;
            ns:oppositeTo ns:Pride ;
            rdfs:comment "Humility can be considered both an emotion and a trait. As an emotion, humility is a state of mind characterized by a sense of modesty, humbleness, and lack of arrogance. It is often experienced in situations where a person recognizes their limitations and shortcomings or perceives a greater authority. For example, a person may feel humble when receiving an award, meeting someone they admire, or when realizing their own mistakes. As a trait, humility is a characteristic or personality attribute that reflects a person's tendency to be humble consistently. A humble person is one who consistently demonstrates modesty, shows respect for others, and is unassuming in their behavior and words. This trait is often seen as a sign of strength and wisdom, rather than a weakness, and is admired by many cultures and societies. Therefore, humility can be seen as both an emotion, arising out of particular experiences, and as a trait that determines how one behaves and interacts with others over time." ;
            rdfs:label "Humility"@en .


###  http://modai.ai/big5#Hunger
ns:Hunger rdf:type owl:NamedIndividual ;
          rdfs:label "Hunger"@en .


###  http://modai.ai/big5#Ignore
ns:Ignore rdf:type owl:NamedIndividual ;
          ns:relatedTo ns:Disregard ;
          ns:similarTo ns:Disregard ;
          rdfs:comment "\"Ignore\" is not an emotion or a trait on its own, but rather an action or behavior that can be influenced by various emotions and traits. For example, a person may choose to ignore someone or something out of anger or frustration, which are emotions. Or, a person may be more inclined to ignore something if they possess a trait like stubbornness or apathy. In summary, \"ignore\" can be seen as a behavior that can be influenced by both emotions and traits, but it is not an emotion or a trait in and of itself." ;
          rdfs:label "Ignore"@en .


###  http://modai.ai/big5#Ignoring
ns:Ignoring rdf:type owl:NamedIndividual ,
                     ns:Behavior ;
            ns:associatedWith ns:Aloofness ;
            ns:triggeredBy ns:Anger ,
                           ns:Disinterest ;
            rdfs:label "Ignoring"@en .


###  http://modai.ai/big5#Imaginative
ns:Imaginative rdf:type owl:NamedIndividual ;
               rdfs:label "Imaginative"@en .


###  http://modai.ai/big5#Impartial
ns:Impartial rdf:type owl:NamedIndividual ,
                      ns:Trait ;
             ns:hasEmotionStrong ns:Opinionated ;
             rdfs:comment "Impartial is more commonly considered a trait rather than an emotion. It is a characteristic or disposition of a person to be fair, unbiased, and even-handed in assessing situations or making decisions. While emotions can influence a person's behavior and decision-making, impartiality is about setting aside personal biases and emotions to make objective judgments. Therefore, impartiality is often seen as a trait or quality that one possesses rather than an emotion that one feels." ;
             rdfs:label "Impartial"@en .


###  http://modai.ai/big5#Impatience
ns:Impatience rdf:type owl:NamedIndividual ;
              rdfs:label "Impatience"@en .


###  http://modai.ai/big5#Impersonal
ns:Impersonal rdf:type owl:NamedIndividual ;
              rdfs:label "Impersonal"@en .


###  http://modai.ai/big5#Impulsive
ns:Impulsive rdf:type owl:NamedIndividual ;
             rdfs:label "Impulsive"@en .


###  http://modai.ai/big5#Impulsiveness
ns:Impulsiveness rdf:type owl:NamedIndividual ;
                 rdfs:label "Impulsiveness"@en .


###  http://modai.ai/big5#Inactive
ns:Inactive rdf:type owl:NamedIndividual ;
            rdfs:label "Inactive"@en .


###  http://modai.ai/big5#Inclusion
ns:Inclusion rdf:type owl:NamedIndividual ,
                      ns:Trait ;
             ns:relatedTo ns:Acceptance ;
             ns:similarTo ns:Acceptance ;
             rdfs:comment "Inclusion is not an emotion or a trait, but rather a concept or a practice of involving, valuing, and respecting diversity and individual differences within a group or community. It is a mindset and a set of behaviors that promote a sense of belonging, equity, and collaboration among people who share common goals or interests, regardless of their gender, race, ethnicity, religion, age, ability, or any other defining characteristic. Inclusion is not something that you either have or not, but rather a continuous process of learning, growth, and adaptation that requires empathy, open-mindedness, and active participation. Therefore, it can be considered more of a mindset or a practice than an emotion or a trait." ;
             rdfs:label "Inclusion"@en .


###  http://modai.ai/big5#Incomplete
ns:Incomplete rdf:type owl:NamedIndividual ;
              rdfs:label "Incomplete"@en .


###  http://modai.ai/big5#Inconsiderate
ns:Inconsiderate rdf:type owl:NamedIndividual ;
                 rdfs:label "Inconsiderate"@en .


###  http://modai.ai/big5#Inconsistent
ns:Inconsistent rdf:type owl:NamedIndividual ;
                rdfs:label "Inconsistent"@en .


###  http://modai.ai/big5#Indecisiveness
ns:Indecisiveness rdf:type owl:NamedIndividual ;
                  rdfs:label "Indecisiveness"@en .


###  http://modai.ai/big5#Independent
ns:Independent rdf:type owl:NamedIndividual ;
               rdfs:label "Independent"@en .


###  http://modai.ai/big5#Indifference
ns:Indifference rdf:type owl:NamedIndividual ;
                ns:oppositeTo ns:Awe ,
                              ns:Indifference ,
                              ns:Pity ;
                ns:relatedTo ns:Apathy ,
                             ns:Disregard ;
                ns:similarTo ns:Apathy ,
                             ns:Disregard ;
                rdfs:comment "Indifference can be considered both an emotion and a trait, depending on the perspective and context. As an emotion, indifference refers to a lack of feeling or concern towards something or someone. It can be a response to a particular situation or stimulus, such as a person showing indifference towards a topic they are not interested in. On the other hand, as a trait, indifference can be viewed as a characteristic or personality trait that describes a person's overall disposition or attitude. For instance, a person who consistently shows indifference towards others and their feelings might be labeled as cold, aloof, or detached. In summary, while indifference can be both an emotion and a trait, it is important to consider the specific context in which it is displayed and the frequency and consistency with which it is shown." ;
                rdfs:label "Indifference"@en .


###  http://modai.ai/big5#Indifference-Engagement
ns:Indifference-Engagement rdf:type owl:NamedIndividual ,
                                    ns:Prompt ;
                           ns:uses ns:Engagement ,
                                   ns:Indifference ;
                           rdfs:comment """I want to quantify the indifference in the following text:
```
$INPUT_TEXT
```

I define indifference as a lack of interest, concern, or emotion. I define the opposite of indifference as engagement or active interest.

Please answer on a scale of 1 - 5 where the numbers have the following meanings:
```
1 = The text is filled with engagement, active interest, and has no elements of indifference.
2 = The text has elements of engagement or active interest, but also contains some elements of indifference.
3 = The text has neither indifference nor engagement, it is neutral.
4 = The text has elements of indifference but also has some aspects of engagement or active interest.
5 = The text is deeply filled with indifference, focusing heavily on a lack of interest, concern, or emotion.
```

Only respond with a number and no other rating.
"""@en ;
                           rdfs:label "Indifference-Engagement"@en .


###  http://modai.ai/big5#Indifferent
ns:Indifferent rdf:type owl:NamedIndividual ;
               rdfs:comment "Indifference can be seen as both an emotion and a trait, depending on the context in which it's used. As an emotion, indifference can be understood as a lack of interest, concern or feeling towards a particular situation or person. This emotional state is often linked to a feeling of detachment or apathy, where a person may be disengaged from their surroundings or experiences. As a trait, indifference can be seen as a personality characteristic that reflects a consistent pattern of disinterest or lack of emotional response. Someone who consistently exhibits indifference may be seen as aloof or uninvolved, lacking empathy or emotional sensitivity towards others. Overall, while indifference can be seen as both an emotion and trait, the distinction between the two depends on the degree and consistency of the individual's response over time." ;
               rdfs:label "Indifferent"@en .


###  http://modai.ai/big5#Ineffective
ns:Ineffective rdf:type owl:NamedIndividual ;
               rdfs:label "Ineffective"@en .


###  http://modai.ai/big5#Inefficient
ns:Inefficient rdf:type owl:NamedIndividual ;
               rdfs:label "Inefficient"@en .


###  http://modai.ai/big5#Influential
ns:Influential rdf:type owl:NamedIndividual ;
               rdfs:label "Influential"@en .


###  http://modai.ai/big5#Ingratitude
ns:Ingratitude rdf:type owl:NamedIndividual ;
               rdfs:comment "Ingratitude can be considered both an emotion and a trait depending on the context in which it is used. As an emotion, ingratitude can be seen as a feeling of dissatisfaction or disappointment towards someone who has done something for you. For example, if a friend goes out of their way to help you with something and you feel unappreciative or resentful towards them, that can be considered an emotion of ingratitude. As a trait, ingratitude can be seen as a more consistent and pervasive pattern of behavior over time. Someone who consistently fails to express gratitude or acknowledge the efforts of others can be seen as having a trait of ingratitude. This type of behavior may be caused by various factors such as personality, upbringing, or past experiences. Overall, ingratitude can be considered both an emotion and a trait depending on the frequency, severity, and context in which it occurs." ;
               rdfs:label "Ingratitude"@en .


###  http://modai.ai/big5#Innocence
ns:Innocence rdf:type owl:NamedIndividual ,
                      ns:Trait ;
             rdfs:comment "Innocence is not necessarily an emotion or a trait, but rather a state of being. It refers to a lack of knowledge or experience of the world and its darker aspects, such as corruption, evil, or deception. However, one's perception or expression of innocence can be influenced by their emotions and traits. For example, a person with a naturally optimistic and trusting personality may be more likely to approach situations with innocence and naivety, while a more cynical and suspicious person may be less so. Similarly, a person experiencing fear or uncertainty may show more vulnerability and hesitation than someone who feels confident and secure in their innocence. Overall, innocence is a complex concept that can be influenced by many factors, including but not limited to a person's emotions and traits." ;
             rdfs:label "Innocence"@en .


###  http://modai.ai/big5#Innovative
ns:Innovative rdf:type owl:NamedIndividual ;
              rdfs:label "Innovative"@en .


###  http://modai.ai/big5#Inquisitiveness
ns:Inquisitiveness rdf:type owl:NamedIndividual ;
                   rdfs:label "Inquisitiveness"@en .


###  http://modai.ai/big5#Insecure
ns:Insecure rdf:type owl:NamedIndividual ;
            rdfs:label "Insecure"@en .


###  http://modai.ai/big5#Insensitive
ns:Insensitive rdf:type owl:NamedIndividual ;
               rdfs:label "Insensitive"@en .


###  http://modai.ai/big5#Inspiration
ns:Inspiration rdf:type owl:NamedIndividual ;
               rdfs:label "Inspiration"@en .


###  http://modai.ai/big5#Insult
ns:Insult rdf:type owl:NamedIndividual ,
                   ns:Negative_High ;
          rdfs:comment "Insult is generally considered a behavior or an action rather than an emotion or a trait. Insulting someone involves saying or doing something disrespectful, offensive, or derogatory towards them, which can be motivated by various emotions such as anger, frustration, or a desire to assert dominance. However, insulting behavior can also be a learned or habitual trait for some individuals. In this sense, insulting behavior can be seen as a negative personality trait, which can be addressed and changed through self-awareness, education, and empathy towards others." ;
          rdfs:label "Insult"@en .


###  http://modai.ai/big5#Insult-Respected
ns:Insult-Respected rdf:type owl:NamedIndividual ,
                             ns:Prompt ;
                    ns:uses ns:Insult ,
                            ns:Rejection ;
                    rdfs:comment """I want to quantify the feeling of being insulted in the following text:
```
$INPUT_TEXT
```

I define being insulted as a feeling of offense or hurt caused by offensive or disrespectful remarks or actions. I define the opposite of being insulted as being praised or respected.

Please answer on a scale of 1 - 5 where the numbers have the following meanings:
```
1 = The text is filled with praise, respect, and has no elements of feeling insulted.
2 = The text has elements of praise or respect, but also contains some elements of feeling insulted.
3 = The text has neither feeling insulted nor praise, it is neutral.
4 = The text has elements of feeling insulted but also has some aspects of praise or respect.
5 = The text is deeply filled with feeling insulted, focusing heavily on feelings of offense or hurt caused by offensive or disrespectful remarks or actions.
```

Only respond with a number and no other rating.
"""@en ;
                    rdfs:label "Insult-Respected"@en .


###  http://modai.ai/big5#Intellectualism
ns:Intellectualism rdf:type owl:NamedIndividual ;
                   rdfs:label "Intellectualism"@en .


###  http://modai.ai/big5#Intense
ns:Intense rdf:type owl:NamedIndividual ;
           rdfs:label "Intense"@en .


###  http://modai.ai/big5#Interest
ns:Interest rdf:type owl:NamedIndividual ,
                     ns:Positive_High ,
                     ns:Trait ;
            ns:relatedTo ns:Engagement ,
                         ns:Interest ;
            ns:similarTo ns:Engagement ,
                         ns:Interest ;
            rdfs:comment "Interest is typically considered a trait, rather than an emotion. Traits are enduring characteristics of an individual that describe relatively stable patterns of thought, feeling, and behavior, whereas emotions are temporary and often context-specific experiences that involve physiological arousal and subjective feelings. Interest is a relatively stable and enduring characteristic of an individual's personality that reflects their tendency to be attracted to or engaged in particular topics, activities, or experiences. It is often measured as a personality trait in psychological research, and is thought to be related to a wide range of important outcomes, such as motivation, learning, and well-being. While it is certainly possible to experience emotions like excitement, curiosity, or enthusiasm in response to something one finds interesting, these emotions are considered distinct from interest itself, which is thought to be a relatively stable and consistent aspect of an individual's personality." ;
            rdfs:label "Interest"@en .


###  http://modai.ai/big5#Interest-Disinterest
ns:Interest-Disinterest rdf:type owl:NamedIndividual ,
                                 ns:Prompt ;
                        ns:uses ns:Disinterest ,
                                ns:Interest ;
                        rdfs:comment """I want to quantify the interest in the following text:
```
$INPUT_TEXT
```

I define interest as a feeling of curiosity, attention, or engagement. I define the opposite of interest as disinterest or lack of curiosity.

Please answer on a scale of 1 - 5 where the numbers have the following meanings:
```
1 = The text is filled with disinterest, lack of curiosity, and has no elements of interest.
2 = The text has elements of disinterest or lack of curiosity, but also contains some elements of interest.
3 = The text has neither interest nor disinterest, it is neutral.
4 = The text has elements of interest but also has some aspects of disinterest or lack of curiosity.
5 = The text is deeply filled with interest, focusing heavily on feelings of curiosity, attention, or engagement.
```

Only respond with a number and no other rating.
"""@en ;
                        rdfs:label "Interest-Disinterest"@en .


###  http://modai.ai/big5#Interrupting
ns:Interrupting rdf:type owl:NamedIndividual ,
                         ns:Behavior ;
                ns:associatedWith ns:Impulsiveness ;
                ns:triggeredBy ns:Excitement ,
                               ns:Impatience ;
                rdfs:label "Interrupting"@en .


###  http://modai.ai/big5#Introverted
ns:Introverted rdf:type owl:NamedIndividual ,
                        ns:Trait ;
               rdfs:comment "Introverted is a trait rather than an emotion. It refers to a person's tendency to direct their energy inwardly, focusing on their thoughts and feelings rather than the external world. Being introverted does not necessarily mean that a person is shy or anti-social, it simply means that they find stimulation and recharge their batteries in more solitary, quiet environments. While emotions can influence introverted behavior, the trait itself is a more stable characteristic that describes a person's typical patterns of behavior and preferences." ;
               rdfs:label "Introverted"@en .


###  http://modai.ai/big5#Involuntary
ns:Involuntary rdf:type owl:NamedIndividual ;
               rdfs:label "Involuntary"@en .


###  http://modai.ai/big5#Irresponsible
ns:Irresponsible rdf:type owl:NamedIndividual ;
                 rdfs:label "Irresponsible"@en .


###  http://modai.ai/big5#Irritation
ns:Irritation rdf:type owl:NamedIndividual ;
              rdfs:label "Irritation"@en .


###  http://modai.ai/big5#Jealousy
ns:Jealousy rdf:type owl:NamedIndividual ,
                     ns:Emotion ,
                     ns:Negative_High ;
            ns:oppositeTo ns:Compersion ;
            rdfs:comment "Jealousy is considered to be an emotion. Emotions are temporary states that are triggered by stimuli and are typically short-lived. Jealousy involves feelings of envy or resentment towards someone who has something that we desire, whether it's a possession, opportunity, or relationship. It is a natural human emotion that can be experienced by anyone in certain situations. On the other hand, a trait is a distinguishing characteristic that defines a person's behavior and personality. While jealousy can be considered a trait in some cases, it is often not a defining characteristic of an individual's personality. Instead, it is more likely to be a temporary response to a specific situation or circumstance. Therefore, jealousy is primarily an emotion rather than a trait." ;
            rdfs:label "Jealousy"@en .


###  http://modai.ai/big5#Jealousy-Compersion
ns:Jealousy-Compersion rdf:type owl:NamedIndividual ;
                       ns:uses ns:Compersion ,
                               ns:Jealousy ;
                       rdfs:comment """I want to quantify the jealousy in the following text:
```
$INPUT_TEXT
```

I define jealousy as a feeling of envy towards someone else's achievements or advantages. I define the opposite of jealousy as compersion, or feeling joy when others have success.

Please answer on a scale of 1 - 5 where the numbers have the following meanings:
```
1 = The text is filled with compersion, joy for others' success, and has no elements of jealousy.
2 = The text has elements of compersion, but also contains some elements of jealousy.
3 = The text has neither jealousy nor compersion, it is neutral.
4 = The text has elements of jealousy but also has some aspects of joy for others' success.
5 = The text is deeply filled with jealousy, focusing heavily on feelings of envy towards someone else's achievements or advantages.
```

Only respond with a number and no other rating.
"""@en ;
                       rdfs:label "Jealousy-Compersion"@en .


###  http://modai.ai/big5#Joy
ns:Joy rdf:type owl:NamedIndividual ,
                ns:Emotion ,
                ns:Positive_High ,
                ns:Trait ;
       ns:oppositeTo ns:Sadness ;
       ns:relatedTo ns:Compersion ;
       ns:similarTo ns:Compersion ;
       rdfs:comment "Joy can be considered both an emotion and a trait. As an emotion, it is a temporary feeling of happiness or pleasure that is usually triggered by specific events or experiences. It is a response to something that is happening around us, such as receiving good news, achieving a goal, or being with loved ones. As a trait, joy refers to a person's disposition or overall tendency to experience positive emotions, even in the absence of specific events or circumstances. It is a fundamental aspect of a person's personality that affects their overall outlook on life, relationships, and experiences. People who have a high level of joy as a trait tend to approach life with optimism and enthusiasm, even in challenging times. In summary, joy can be both an emotion and a trait, with each aspect influencing a person's overall experience of happiness and well-being." ;
       rdfs:label "Joy"@en .


###  http://modai.ai/big5#Joy-Sadness
ns:Joy-Sadness rdf:type owl:NamedIndividual ,
                        ns:Prompt ;
               ns:uses ns:Joy ,
                       ns:Sadness ;
               rdfs:comment """I want to quantify the joy in the following text:
```
$INPUT_TEXT
```

I define joy as a feeling of great pleasure and happiness. I define the opposite of joy as sadness or depression.

Please answer on a scale of 1 - 5 where the numbers have the following meanings:
```
1 = The text has no joy or happiness and is heavily focused on sadness.
2 = The text has a hint of joy or happiness but is generally sad or neutral.
3 = The text has neither joy nor sadness, it is neutral.
4 = The text has joyful or happy elements but also has some neutral or negative aspects.
5 = The text is brimming with joy, happiness, and positive sentiment.
```

Only respond with a number and no other rating.
"""@en ;
               rdfs:label "Joy-Sadness"@en .


###  http://modai.ai/big5#Laid_Back
ns:Laid_Back rdf:type owl:NamedIndividual ;
             rdfs:label "Laid_Back"@en .


###  http://modai.ai/big5#Laughing
ns:Laughing rdf:type owl:NamedIndividual ,
                     ns:Behavior ;
            ns:associatedWith ns:GoodHumor ,
                              ns:Optimism ;
            ns:triggeredBy ns:Amusement ,
                           ns:Joy ;
            rdfs:label "Laughing"@en .


###  http://modai.ai/big5#Laziness
ns:Laziness rdf:type owl:NamedIndividual ;
            rdfs:label "Laziness"@en .


###  http://modai.ai/big5#Lazy
ns:Lazy rdf:type owl:NamedIndividual ;
        rdfs:label "Lazy"@en .


###  http://modai.ai/big5#Leader
ns:Leader rdf:type owl:NamedIndividual ;
          rdfs:label "Leader"@en .


###  http://modai.ai/big5#Leadership
ns:Leadership rdf:type owl:NamedIndividual ;
              rdfs:label "Leadership"@en .


###  http://modai.ai/big5#Lethargic
ns:Lethargic rdf:type owl:NamedIndividual ;
             rdfs:label "Lethargic"@en .


###  http://modai.ai/big5#Liking
ns:Liking rdf:type owl:NamedIndividual ,
                   ns:Emotion ,
                   ns:Trait ;
          ns:oppositeTo ns:Disgust ;
          ns:relatedTo ns:Affection ,
                       ns:Attraction ,
                       ns:Love ;
          ns:similarTo ns:Affection ,
                       ns:Attraction ,
                       ns:Love ;
          rdfs:comment "Liking can be considered both an emotion and a trait, depending on how it is being used or understood in a given context. As an emotion, liking is associated with a positive affective state that involves enjoyment, pleasure, and attraction. When we say we \"like\" something or someone, we are expressing a positive emotional response to that thing or person. As a trait, liking can refer to a predisposition or tendency to experience positive emotions towards certain things or people. For example, someone who is generally \"likable\" may have a personality trait that makes them easy to get along with or makes others enjoy their company. In summary, liking can be seen as an emotion when it refers to a positive affective state, and as a trait when it refers to a dispositional tendency towards liking certain things or people." ;
          rdfs:label "Liking"@en .


###  http://modai.ai/big5#Loneliness
ns:Loneliness rdf:type owl:NamedIndividual ,
                       ns:Emotion ,
                       ns:Social ;
              rdfs:comment "Loneliness is generally considered to be an emotion. Emotions are temporary states where individuals experience certain feelings that may be triggered by external or internal events. Loneliness is a feeling of emptiness or isolation, which is often caused by the lack of social connections or relationships. On the other hand, a trait is a characteristic or a pattern of behavior that tends to endure over time. If loneliness was considered a trait, it would mean that individuals consistently experience feelings of loneliness regardless of their social circumstances. However, loneliness is usually a transitory state, and it can be alleviated by forming new social connections or seeking out social support. Therefore, it is more accurate to consider loneliness as an emotion rather than a trait." ;
              rdfs:label "Loneliness"@en .


###  http://modai.ai/big5#Loneliness-Companionship
ns:Loneliness-Companionship rdf:type owl:NamedIndividual ,
                                     ns:Prompt ;
                            ns:uses ns:Companionship ,
                                    ns:Loneliness ;
                            rdfs:comment """I want to quantify the loneliness in the following text:
```
$INPUT_TEXT
```

I define loneliness as a state of solitude or being alone. I define the opposite of loneliness as companionship or togetherness.

Please answer on a scale of 1 - 5 where the numbers have the following meanings:
```
1 = The text is filled with companionship, togetherness, and has no elements of loneliness.
2 = The text has elements of companionship or togetherness, but also contains some elements of loneliness.
3 = The text has neither loneliness nor companionship, it is neutral.
4 = The text has elements of loneliness but also has some aspects of companionship or togetherness.
5 = The text is deeply filled with loneliness, focusing heavily on feelings of solitude or being alone.
```

Only respond with a number and no other rating.
"""@en ;
                            rdfs:label "Loneliness-Companionship"@en .


###  http://modai.ai/big5#Love
ns:Love rdf:type owl:NamedIndividual ,
                 ns:Emotion ,
                 ns:Positive_Low ,
                 ns:Trait ;
        ns:oppositeTo ns:Love ;
        rdfs:comment "Love can be considered both an emotion and a trait, depending on how it is defined and understood. As an emotion, love is often described as a feeling of intense affection or attraction towards another person, object, or idea. It is typically characterized by a range of physiological and psychological responses, including increased heart rate, butterflies in the stomach, and feelings of euphoria or happiness. As a trait, love can be seen as a disposition or tendency towards compassionate, caring, and affectionate behavior. It is seen as a personal characteristic that motivates individuals to act in ways that demonstrate love and affection towards others, even in the absence of intense emotional feelings. Some argue that love is both an emotion and a trait, in that emotions are often fleeting and unpredictable, whereas traits are enduring and consistent. Therefore, love can be understood as both a spontaneous emotional response and a persistent character trait that shapes how individuals relate to others over time." ;
        rdfs:label "Love"@en .


###  http://modai.ai/big5#Love-Hate
ns:Love-Hate rdf:type owl:NamedIndividual ;
             ns:uses ns:Hate ,
                     ns:Love ;
             rdfs:comment """I want to quantify the love in the following text:
```
$INPUT_TEXT
```

I define love as a strong affectionate feeling or deep affection. I define the opposite of love as hatred or intense dislike.

Please answer on a scale of 1 - 5 where the numbers have the following meanings:
```
1 = The text is filled with hatred, intense dislike, and has no elements of love.
2 = The text has elements of dislike or hatred, but also contains some elements of love.
3 = The text has neither love nor hatred, it is neutral.
4 = The text has elements of love but also has some negative or disliking aspects.
5 = The text is deeply filled with love, focusing heavily on affectionate feelings or deep affection.
```

Only respond with a number and no other rating.
"""@en ;
             rdfs:label "Love-Hate"@en .


###  http://modai.ai/big5#LowEnergy
ns:LowEnergy rdf:type owl:NamedIndividual ;
             rdfs:label "LowEnergy"@en .


###  http://modai.ai/big5#Lying
ns:Lying rdf:type owl:NamedIndividual ,
                  ns:Behavior ;
         ns:associatedWith ns:Deceitfulness ;
         ns:triggeredBy ns:Fear ,
                        ns:Guilt ;
         rdfs:label "Lying"@en .


###  http://modai.ai/big5#Malice
ns:Malice rdf:type owl:NamedIndividual ;
          rdfs:label "Malice"@en .


###  http://modai.ai/big5#Meditating
ns:Meditating rdf:type owl:NamedIndividual ,
                       ns:Behavior ;
              ns:associatedWith ns:Mindfulness ;
              ns:triggeredBy ns:Desire_Peace ,
                             ns:Stress ;
              rdfs:label "Meditating"@en .


###  http://modai.ai/big5#Melancholy
ns:Melancholy rdf:type owl:NamedIndividual ,
                       ns:Emotion ,
                       ns:Trait ;
              ns:relatedTo ns:Sadness ;
              ns:similarTo ns:Sadness ;
              rdfs:comment "Melancholy can be both an emotion and a personality trait, depending on how it is defined and understood. As an emotion, melancholy refers to a feeling of sadness, loneliness, or despair that is often accompanied by a sense of heaviness or sluggishness. It may be triggered by various situations, such as a loss, disappointment, or a sense of unfulfillment, and it is usually temporary and fluctuating. As a personality trait, melancholy refers to a tendency to experience sad or gloomy moods more often than other emotions. It may be seen as a trait if it is a stable feature of one's personality that persists over time and across situations. People who are considered melancholic may be seen as introverted, reflective, and creative, but also prone to brooding or overthinking. In short, melancholy can be viewed as both an emotion and a personality trait, depending on the context and perspective." ;
              rdfs:label "Melancholy"@en .


###  http://modai.ai/big5#Messy
ns:Messy rdf:type owl:NamedIndividual ;
         rdfs:label "Messy"@en .


###  http://modai.ai/big5#Mindfulness
ns:Mindfulness rdf:type owl:NamedIndividual ;
               rdfs:label "Mindfulness"@en .


###  http://modai.ai/big5#Mischievousness
ns:Mischievousness rdf:type owl:NamedIndividual ;
                   rdfs:label "Mischievousness"@en .


###  http://modai.ai/big5#Modesty
ns:Modesty rdf:type owl:NamedIndividual ,
                    ns:Emotion ,
                    ns:Trait ;
           ns:relatedTo ns:Humility ;
           ns:similarTo ns:Humility ;
           rdfs:comment "Modesty can be both an emotion and a trait, depending on the perspective. As an emotion, modesty is typically defined as a feeling of humility or shyness in response to praise or attention. For example, if someone compliments your work and you feel humble or shy in response, you might be experiencing the emotion of modesty. As a trait, modesty is often defined as a personality characteristic or behavior. Those who are considered modest may exhibit behaviors like downplaying their accomplishments or avoiding attention or praise. So while modesty can be considered both an emotion and a trait, it's important to note that they are different concepts. Emotions are temporary internal experiences, while traits are more stable aspects of an individual's personality or behavior." ;
           rdfs:label "Modesty"@en .


###  http://modai.ai/big5#Moody
ns:Moody rdf:type owl:NamedIndividual ;
         ns:similarTo ns:Consistent ,
                      ns:Stable ,
                      ns:Steady ;
         rdfs:label "Moody"@en .


###  http://modai.ai/big5#Motivated
ns:Motivated rdf:type owl:NamedIndividual ,
                      ns:Trait ;
             ns:oppositeTo ns:Unmotivated ;
             rdfs:comment "Motivated can be considered both as an emotion and a trait, depending on how it is defined and applied. As an emotion, motivation usually refers to a feeling of drive or energy that propels someone towards a particular goal or outcome. This emotional state can be influenced by various factors, such as personal values, desires, aspirations, fear, reward, or social pressure. For example, a person may feel motivated to exercise because they want to stay healthy, feel accomplished, or avoid criticism from others. As a trait, motivation can be seen as a stable characteristic of an individual's personality, which reflects their general tendency to be driven towards goals and engage in purposeful behavior. This trait may have a genetic and environmental basis, and it can be measured and compared across individuals. For example, a person may have a high level of intrinsic motivation, meaning that they are naturally curious, interested, and self-directed, or a low level of extrinsic motivation, meaning that they rely more on external incentives and punishments to perform tasks. In summary, the distinction between motivation as an emotion and a trait depends on whether we focus on the dynamic experience of drive and energy in a particular moment or the stable tendency to pursue goals and achieve outcomes over time." ;
             rdfs:label "Motivated"@en .


###  http://modai.ai/big5#Naive
ns:Naive rdf:type owl:NamedIndividual ;
         rdfs:label "Naive"@en .


###  http://modai.ai/big5#Neat
ns:Neat rdf:type owl:NamedIndividual ;
        rdfs:label "Neat"@en .


###  http://modai.ai/big5#Necessity
ns:Necessity rdf:type owl:NamedIndividual ;
             rdfs:label "Necessity"@en .


###  http://modai.ai/big5#Negativity
ns:Negativity rdf:type owl:NamedIndividual ;
              rdfs:label "Negativity"@en .


###  http://modai.ai/big5#Nervousness
ns:Nervousness rdf:type owl:NamedIndividual ;
               ns:relatedTo ns:Anxiety ;
               ns:similarTo ns:Anxiety ;
               rdfs:comment "Nervousness can be considered both an emotion and a trait. As an emotion, nervousness is a temporary state of heightened physiological arousal characterized by feelings of anxiety, tension, fear, and uncertainty. This emotional response can be triggered by a range of situations, such as public speaking, social situations, or high-pressure events, and can have various intensities. As a trait, nervousness is a relatively stable characteristic or personality trait, describing an individual's tendency to experience anxiety or worry regularly across different situations. People with high levels of nervousness may exhibit symptoms of anxiety, fear or self-doubt more frequently, and with greater intensity, than those who score low on this trait. Therefore, nervousness can be considered both an emotion and a trait, where the emotion refers to the physiological and psychological reactions to a specific stimulus, while the trait refers to a person's overall predisposition to anxiety and worry." ;
               rdfs:label "Nervousness"@en .


###  http://modai.ai/big5#Nodding
ns:Nodding rdf:type owl:NamedIndividual ,
                    ns:Behavior ;
           ns:associatedWith ns:Attentiveness ;
           ns:triggeredBy ns:Agreement ,
                          ns:Understanding ;
           rdfs:label "Nodding"@en .


###  http://modai.ai/big5#Non_Confrontational
ns:Non_Confrontational rdf:type owl:NamedIndividual ;
                       rdfs:label "Non_Confrontational"@en .


###  http://modai.ai/big5#Non_Detailed
ns:Non_Detailed rdf:type owl:NamedIndividual ;
                rdfs:label "Non_Detailed"@en .


###  http://modai.ai/big5#Non_Dominant
ns:Non_Dominant rdf:type owl:NamedIndividual ;
                rdfs:label "Non_Dominant"@en .


###  http://modai.ai/big5#Non_Influential
ns:Non_Influential rdf:type owl:NamedIndividual ;
                   rdfs:label "Non_Influential"@en .


###  http://modai.ai/big5#Non_Judgmental
ns:Non_Judgmental rdf:type owl:NamedIndividual ,
                           ns:Trait ;
                  rdfs:comment "Non-judgmental is more commonly considered to be a trait rather than an emotion. It refers to the ability or tendency to withhold judgment about a person, situation, or behavior. This trait is often seen as valuable in fields such as psychology, counseling, and social work because it allows individuals to remain objective and avoid biases when working with others. While it can be influenced by emotions such as empathy and compassion, non-judgmental is primarily considered a conscious decision or state of mind rather than an emotion." ;
                  rdfs:label "Non_Judgmental"@en .


###  http://modai.ai/big5#Nonabstract
ns:Nonabstract rdf:type owl:NamedIndividual ;
               rdfs:label "Nonabstract"@en .


###  http://modai.ai/big5#Nonconformity
ns:Nonconformity rdf:type owl:NamedIndividual ;
                 rdfs:label "Nonconformity"@en .


###  http://modai.ai/big5#Noninnovative
ns:Noninnovative rdf:type owl:NamedIndividual ;
                 rdfs:label "Noninnovative"@en .


###  http://modai.ai/big5#Nonpersistent
ns:Nonpersistent rdf:type owl:NamedIndividual ;
                 rdfs:label "Nonpersistent"@en .


###  http://modai.ai/big5#Nonreactive
ns:Nonreactive rdf:type owl:NamedIndividual ;
               rdfs:label "Nonreactive"@en .


###  http://modai.ai/big5#Nostalgia
ns:Nostalgia rdf:type owl:NamedIndividual ,
                      ns:Emotion ;
             rdfs:comment "Nostalgia can be considered both an emotion and a trait, depending on how it is defined and understood. As an emotion, nostalgia refers to a feeling of longing or yearning for the past, often with a sense of sadness or wistfulness. It can be triggered by personal memories, cultural artifacts (such as music or movies), or even by proximity to a physical location associated with past experiences. In this sense, nostalgia is a specific and temporary emotional state that people may experience in response to certain stimuli. As a trait, nostalgia can be seen as a characteristic of an individual's personality or worldview. Some people may be more prone to experiencing nostalgia, either due to their upbringing, temperament, or life experiences. They may have a greater attachment to their personal and cultural history, and may be more likely to reminisce about the past, collect memorabilia, or seek out experiences that evoke nostalgic feelings. In this sense, nostalgia is a more enduring aspect of a person's psychology, rather than a temporary emotion." ;
             rdfs:label "Nostalgia"@en .


###  http://modai.ai/big5#Nostalgia-Anticipation
ns:Nostalgia-Anticipation rdf:type owl:NamedIndividual ,
                                   ns:Prompt ;
                          ns:uses ns:Anticipation ,
                                  ns:Nostalgia ;
                          rdfs:comment """I want to quantify the nostalgia in the following text:
```
$INPUT_TEXT
```

I define nostalgia as a sentimental longing or wistful affection for the past, often for a period or place with happy personal associations.  I define the opposite of nostalgia as anticipation or future-focused thinking.

Please answer on a scale of 1 - 5 where the numbers have the following meanings:
```
1 = The text is highly focused on the past with negative sentiment.
2 = The text has at least one reference to the past and has no positive sentiment.
3 = The text has no references to the past and is not nostalgic.
4 = The text has at least one reference to the past and has no negative sentiment.
5 = The text is highly focused on the past with positive sentiment.
```

Only respond with a number and no other rating.
"""@en ;
                          rdfs:label "Nostalgia-Anticipation"@en .


###  http://modai.ai/big5#Obeying
ns:Obeying rdf:type owl:NamedIndividual ,
                    ns:Behavior ;
           ns:associatedWith ns:Compliance ,
                             ns:Submissiveness ;
           ns:triggeredBy ns:Fear ,
                          ns:Respect ;
           rdfs:label "Obeying"@en .


###  http://modai.ai/big5#Objective
ns:Objective rdf:type owl:NamedIndividual ;
             rdfs:label "Objective"@en .


###  http://modai.ai/big5#Observant
ns:Observant rdf:type owl:NamedIndividual ;
             rdfs:label "Observant"@en .


###  http://modai.ai/big5#Offensive
ns:Offensive rdf:type owl:NamedIndividual ;
             rdfs:label "Offensive"@en .


###  http://modai.ai/big5#Open_Minded
ns:Open_Minded rdf:type owl:NamedIndividual ,
                        ns:Trait ;
               rdfs:comment "Open-mindedness can be considered a trait rather than an emotion. A trait is a characteristic or quality that helps to define a person's personality and agentic characteristics. Open-mindedness is the trait of being receptive or open to new ideas, experiences, and information. It is not necessarily an emotion because it is not always inherently tied to a particular feeling or affective state. Rather, it is an orientation or disposition that influences how a person thinks, feels, and behaves in different situations." ;
               rdfs:label "Open_Minded"@en .


###  http://modai.ai/big5#Opinionated
ns:Opinionated rdf:type owl:NamedIndividual ,
                        ns:Trait ;
               ns:oppositeTo ns:Adaptable ,
                             ns:Indifferent ,
                             ns:Non_Judgmental ,
                             ns:Passive ,
                             ns:Reserved ,
                             ns:Uncertainty ;
               ns:relatedTo ns:Strong_Minded ;
               rdfs:comment "Opinionated is not an emotion, but a trait. It refers to a person who has strongly held opinions and is not likely to change them easily. As a trait, opinionated can be considered part of a person's personality or character, rather than something that arises from a temporary emotional state. Opinionated individuals may have a tendency to express their opinions assertively or even aggressively, which can be a reflection of their underlying values, beliefs, or attitudes." ;
               rdfs:label "Opinionated"@en .


###  http://modai.ai/big5#Optimism
ns:Optimism rdf:type owl:NamedIndividual ,
                     ns:Positive_Low ;
            ns:oppositeTo ns:Despair ;
            ns:relatedTo ns:Hope ;
            ns:similarTo ns:Hope ;
            rdfs:comment "Optimism can be considered both an emotion and a trait. As an emotion, optimism refers to the feeling of hopefulness and positive expectations about the future. This feeling can be influenced by a range of factors, including personal experiences, external events, mindset, and beliefs. In this sense, optimism is a transient and fluctuating state that can be influenced by various factors. As a trait, optimism refers to a stable personality characteristic reflecting a general tendency to expect positive outcomes and to have positive beliefs about oneself, others, and the future. This trait is believed to be relatively stable and enduring across time and situations and can have a significant impact on a person's behavior, coping strategies, and overall well-being. Overall, while optimism can manifest as both a transient emotion and a stable trait, it is generally considered a desirable quality associated with increased resilience, coping skills, and overall happiness and well-being." ;
            rdfs:label "Optimism"@en .


###  http://modai.ai/big5#Optimism-Pessimism
ns:Optimism-Pessimism rdf:type owl:NamedIndividual ,
                               ns:Prompt ;
                      ns:uses ns:Optimism ,
                              ns:Pessimism ;
                      rdfs:comment """I want to quantify the optimism in the following text:
```
$INPUT_TEXT
```

I define optimism as a hopefulness and confidence about the future or the success of something. I define the opposite of optimism as pessimism or negative thinking.

Please answer on a scale of 1 - 5 where the numbers have the following meanings:
```
1 = The text is filled with pessimism, negative thinking, and has no elements of optimism.
2 = The text has elements of pessimism or negative thinking, but also contains some elements of optimism.
3 = The text has neither optimism nor pessimism, it is neutral.
4 = The text has elements of optimism but also has some aspects of pessimism or negative thinking.
5 = The text is deeply filled with optimism, focusing heavily on feelings of hopefulness and confidence about the future.
```

Only respond with a number and no other rating.
"""@en ;
                      rdfs:label "Optimism-Pessimism"@en .


###  http://modai.ai/big5#Optimistic
ns:Optimistic rdf:type owl:NamedIndividual ;
              rdfs:label "Optimistic"@en .


###  http://modai.ai/big5#Organized
ns:Organized rdf:type owl:NamedIndividual ,
                      ns:Trait ;
             rdfs:comment "Organized is generally considered a trait, rather than an emotion. Traits are enduring qualities or characteristics that are relatively stable over time and across situations, whereas emotions are affective states that are typically brief and responsive to specific events or stimuli. Being organized refers to the ability to plan, prioritize, and manage tasks and responsibilities in an efficient and effective manner. This is generally seen as a trait that can be developed through habits and practice, rather than a fleeting emotional response to a specific situation. However, it is important to note that emotions can play a role in influencing one's ability to be organized. For example, feeling overwhelmed or stressed can make it more difficult to organize and prioritize tasks. In this sense, emotions can impact one's ability to exhibit the trait of being organized, but the trait itself remains distinct from any specific emotions that may influence it." ;
             rdfs:label "Organized"@en .


###  http://modai.ai/big5#Outgoing
ns:Outgoing rdf:type owl:NamedIndividual ;
            rdfs:label "Outgoing"@en .


###  http://modai.ai/big5#Overcome
ns:Overcome rdf:type owl:NamedIndividual ,
                     ns:Trait ;
            ns:relatedTo ns:Despair ;
            ns:similarTo ns:Despair ;
            rdfs:comment "Overcome can refer to overcoming both emotions and traits, depending on the context in which it is used. Emotions: Overcoming an emotion typically refers to being able to control or manage the feeling, rather than being controlled by it. For example, someone might work to overcome their fear of public speaking by practicing and desensitizing themselves to the situation. In this case, they are overcoming the emotion of fear. Traits: Overcoming a trait generally refers to changing or improving a certain behavior or habit. For instance, a person might try to overcome their tendency towards procrastination by creating a schedule and sticking to it. In this case, they are overcoming the trait of procrastination. Therefore, whether \"overcome\" is an emotion or a trait depends on the context in which it is used, and the specific thing being overcome." ;
            rdfs:label "Overcome"@en .


###  http://modai.ai/big5#Overwhelmed
ns:Overwhelmed rdf:type owl:NamedIndividual ;
               ns:relatedTo ns:Despair ;
               ns:similarTo ns:Despair ;
               rdfs:comment "Overwhelmed can be considered both an emotion and a trait, depending on how it is used and understood in a specific context. As an emotion, feeling overwhelmed refers to the experience of being mentally or emotionally drained, stressed, or burdened by a situation or a task. This emotion can be triggered by various factors, such as having too many responsibilities, facing unexpected challenges, feeling unprepared, or dealing with negative events. When someone feels overwhelmed, they may experience physical symptoms such as fatigue, tension, anxiety, or panic. As a trait, being overwhelmed can refer to a tendency or a pattern of behavior that someone displays consistently over time. For instance, a person who is easily overwhelmed may have a low tolerance for stress, be prone to procrastination, struggle with decision making, or lack confidence in their abilities. This trait may be rooted in personality, upbringing, or life experience and can impact different areas of someone's life, such as their work, relationships, or health. In essence, being overwhelmed can be both a temporary emotional reaction to a specific situation and a more stable personality trait that affects someone's functioning in different ways. So, it can be considered as both an emotion and a trait depending on the context we are talking about." ;
               rdfs:label "Overwhelmed"@en .


###  http://modai.ai/big5#Pain
ns:Pain rdf:type owl:NamedIndividual ;
        rdfs:label "Pain"@en .


###  http://modai.ai/big5#Panicked
ns:Panicked rdf:type owl:NamedIndividual ;
            rdfs:label "Panicked"@en .


###  http://modai.ai/big5#Panicking
ns:Panicking rdf:type owl:NamedIndividual ,
                      ns:Behavior ;
             ns:associatedWith ns:Nervousness ;
             ns:triggeredBy ns:Anxiety ,
                            ns:Fear ;
             rdfs:label "Panicking"@en .


###  http://modai.ai/big5#Passion
ns:Passion rdf:type owl:NamedIndividual ;
           rdfs:label "Passion"@en .


###  http://modai.ai/big5#Passionate
ns:Passionate rdf:type owl:NamedIndividual ;
              rdfs:label "Passionate"@en .


###  http://modai.ai/big5#Passive
ns:Passive rdf:type owl:NamedIndividual ,
                    ns:Trait ;
           rdfs:comment "Passive is neither an emotion nor a trait, but rather a behavioral tendency or characteristic. Being passive can mean being inclined to accept or comply with circumstances or situations without showing much resistance or assertiveness. It is not an emotion because emotions are internal states or feelings, such as happiness, anger, fear, or sadness. It is also not a trait because traits are enduring personality characteristics that describe an individual's disposition and behavior pattern, such as extraversion, agreeableness, or conscientiousness. However, being passive can be influenced by certain traits or emotions, such as shyness, anxiety, or apathy." ;
           rdfs:label "Passive"@en .


###  http://modai.ai/big5#Peaceful
ns:Peaceful rdf:type owl:NamedIndividual ;
            rdfs:label "Peaceful"@en .


###  http://modai.ai/big5#Perseverance
ns:Perseverance rdf:type owl:NamedIndividual ;
                rdfs:label "Perseverance"@en .


###  http://modai.ai/big5#Persistent
ns:Persistent rdf:type owl:NamedIndividual ;
              rdfs:label "Persistent"@en .


###  http://modai.ai/big5#Personal
ns:Personal rdf:type owl:NamedIndividual ;
            rdfs:label "Personal"@en .


###  http://modai.ai/big5#Persuasive
ns:Persuasive rdf:type owl:NamedIndividual ;
              rdfs:label "Persuasive"@en .


###  http://modai.ai/big5#Pessimism
ns:Pessimism rdf:type owl:NamedIndividual ,
                      ns:Negative_Low ;
             ns:oppositeTo ns:Optimism ;
             ns:relatedTo ns:Uncertainty ;
             ns:similarTo ns:Uncertainty ;
             rdfs:comment "Pessimism can be both an emotion and a trait. As an emotion, pessimism refers to a feeling of negativity or a tendency to expect the worst in a situation. It can be driven by events or circumstances that one perceives as negative or threatening, and can be temporary or fleeting. As a trait, pessimism refers to a relatively stable and enduring pattern of negative thinking. People who possess this trait tend to view life through a negative lens and expect bad outcomes even in situations where there is no evidence to support this view. This tendency can be part of one's personality and can have a significant impact on one's overall outlook on life and general well-being. In summary, while pessimism can be an emotion that is experienced in response to negative events, it can also be a stable personality trait that is characterized by a generally negative outlook on life." ;
             rdfs:label "Pessimism"@en .


###  http://modai.ai/big5#Pessimism-Optimism
ns:Pessimism-Optimism rdf:type owl:NamedIndividual ,
                               ns:Prompt ;
                      ns:uses ns:Optimism ,
                              ns:Pessimism ;
                      rdfs:comment """I want to quantify the pessimism in the following text:
```
$INPUT_TEXT
```

I define pessimism as a tendency to see the worst aspect of things or believe that the worst will happen. I define the opposite of pessimism as optimism or positive thinking.

Please answer on a scale of 1 - 5 where the numbers have the following meanings:
```
1 = The text is filled with optimism, positive thinking, and has no elements of pessimism.
2 = The text has elements of optimism or positive thinking, but also contains some elements of pessimism.
3 = The text has neither pessimism nor optimism, it is neutral.
4 = The text has elements of pessimism but also has some aspects of optimism or positive thinking.
5 = The text is deeply filled with pessimism, focusing heavily on feelings of negativity and expecting the worst.
```

Only respond with a number and no other rating.
"""@en ;
                      rdfs:label "Pessimism-Optimism"@en .


###  http://modai.ai/big5#Philosophical
ns:Philosophical rdf:type owl:NamedIndividual ;
                 rdfs:label "Philosophical"@en .


###  http://modai.ai/big5#Pity
ns:Pity rdf:type owl:NamedIndividual ,
                 ns:Social ;
        rdfs:comment "Pity can be considered both an emotion and a trait, depending on how it is conceptualized and used. As an emotion, pity is a feeling of sympathy or compassion towards someone who is in a difficult or unfortunate situation. It involves a recognition of someone else's suffering or distress, and a desire to alleviate their pain or improve their circumstances. Pity as an emotion is a temporary response to a specific event or situation, and it can vary in intensity depending on the individual's personal experiences, values, and beliefs. As a trait, pity can refer to a more long-lasting disposition or tendency to feel pity towards others. It can manifest as a personality trait characterized by empathy, caring, and concern for others, or as a more negative trait that involves excessive or unwarranted feelings of sympathy or guilt. Pity as a trait is relatively stable over time and can influence an individual's behavior and interactions with others. Overall, whether we consider pity as an emotion or a trait depends on the context and the level of analysis. However, both conceptualizations highlight the importance of recognizing and responding to others' suffering and distress in a compassionate and empathic way." ;
        rdfs:label "Pity"@en .


###  http://modai.ai/big5#Pity-Indifference
ns:Pity-Indifference rdf:type owl:NamedIndividual ,
                              ns:Prompt ;
                     ns:uses ns:Indifference ,
                             ns:Pity ;
                     rdfs:comment """I want to quantify the pity in the following text:
```
$INPUT_TEXT
```

I define pity as a feeling of compassion for others, particularly when they are in distress or misfortune. I define the opposite of pity as indifference or lack of concern.

Please answer on a scale of 1 - 5 where the numbers have the following meanings:
```
1 = The text is filled with indifference, lack of concern, and has no elements of pity.
2 = The text has elements of indifference or lack of concern, but also contains some elements of pity.
3 = The text has neither pity nor indifference, it is neutral.
4 = The text has elements of pity but also has some aspects of indifference or lack of concern.
5 = The text is deeply filled with pity, focusing heavily on feelings of compassion for others in distress.
```

Only respond with a number and no other rating.
"""@en ;
                     rdfs:label "Pity-Indifference"@en .


###  http://modai.ai/big5#Playfulness
ns:Playfulness rdf:type owl:NamedIndividual ;
               rdfs:label "Playfulness"@en .


###  http://modai.ai/big5#Pleasure
ns:Pleasure rdf:type owl:NamedIndividual ;
            ns:relatedTo ns:Joy ,
                         ns:Self_Pleasure ;
            ns:similarTo ns:Joy ,
                         ns:Self_Pleasure ;
            rdfs:comment "Pleasure can be considered both an emotion and a trait depending on how it is defined and understood. As an emotion, pleasure refers to a positive feeling or sensation that arises from experiencing something enjoyable or satisfying. This could include feelings of happiness, joy, contentment, or excitement. Pleasure as an emotion is often short-lived and can be triggered by various stimuli, such as physical sensations, social interactions, or accomplishments. As a trait, pleasure can refer to a person's general inclination towards seeking out pleasurable experiences or activities. This could include a person's tendency to pursue activities that bring them joy or satisfaction, or their overall level of enjoyment in life. Pleasure as a trait is typically seen as a more stable characteristic that remains consistent over time. Overall, whether pleasure is considered an emotion or a trait depends on the context in which it is being discussed and how it is being defined." ;
            rdfs:label "Pleasure"@en .


###  http://modai.ai/big5#Pleasure-Revulsion
ns:Pleasure-Revulsion rdf:type owl:NamedIndividual ,
                               ns:Prompt ;
                      ns:uses ns:Pleasure ,
                              ns:Revulsion ;
                      rdfs:comment """I want to quantify the level of pleasure or revulsion in the following text: 
```
$INPUT_TEXT
```

I define pleasure as a state of enjoyment, satisfaction, or delight. I define revulsion as a strong feeling of disgust, repugnance, or aversion.

Please answer on a scale of 1 - 5 where the numbers have the following meanings:
```
1 = The text is filled with revulsion, disgust, and has no elements of pleasure.
2 = The text has elements of revulsion or disgust, but also contains some elements of pleasure.
3 = The text has neither pleasure nor revulsion, it is neutral.
4 = The text has elements of pleasure but also has some aspects of revulsion or disgust.
5 = The text is deeply filled with pleasure, focusing heavily on enjoyment, satisfaction, or delight.
```

Only respond with a number and no other rating.

"""@en ;
                      rdfs:label "Pleasure-Revulsion"@en .


###  http://modai.ai/big5#Polite
ns:Polite rdf:type owl:NamedIndividual ;
          rdfs:label "Polite"@en .


###  http://modai.ai/big5#Positive
ns:Positive rdf:type owl:NamedIndividual ;
            rdfs:label "Positive"@en .


###  http://modai.ai/big5#Practical
ns:Practical rdf:type owl:NamedIndividual ;
             rdfs:label "Practical"@en .


###  http://modai.ai/big5#Praise
ns:Praise rdf:type owl:NamedIndividual ,
                   ns:Trait ;
          ns:relatedTo ns:Admiration ,
                       ns:Appreciative ;
          ns:similarTo ns:Admiration ,
                       ns:Appreciative ;
          rdfs:comment "Praise can be considered both an emotion and a trait, depending on how it is defined and understood. As an emotion, praise can be seen as a positive feeling that arises in response to an experience or action that is perceived as praiseworthy. When we feel grateful, impressed, or content about something, we may express praise as a way to communicate our positive emotions to others or to reinforce the behavior or attribute that prompted our praise. As a trait, praise can be seen as a habitual behavior or personality characteristic that reflects a tendency to appreciate and acknowledge the good qualities or actions of others. People who are described as \"praise-worthy\" may have a natural inclination to offer compliments, express gratitude, or recognize achievements, and this trait may be seen as a positive quality in relationships, work environments, or other social contexts. Therefore, praise can be considered both an emotion and a trait, depending on how it is conceptualized and used in different situations." ;
          rdfs:label "Praise"@en .


###  http://modai.ai/big5#Predictability
ns:Predictability rdf:type owl:NamedIndividual ,
                           ns:Trait ;
                  ns:relatedTo ns:Certainty ;
                  ns:similarTo ns:Certainty ;
                  rdfs:comment "Predictability is not an emotion. It is more accurately considered a trait or characteristic of a person or situation. It refers to the degree to which something can be anticipated or expected to happen or behave in a certain way. As a trait, predictability can be associated with a person's reliability, consistency, and stability. It can also refer to the regularity or consistency of a situation, such as a job, relationship, or daily routine. In this sense, predictability can provide a sense of security and comfort for individuals by reducing uncertainty and increasing stability." ;
                  rdfs:label "Predictability"@en .


###  http://modai.ai/big5#Pride
ns:Pride rdf:type owl:NamedIndividual ,
                  ns:Social ;
         ns:relatedTo ns:Dignity ,
                      ns:Self_Pleasure ,
                      ns:Self_Satisfaction ;
         ns:similarTo ns:Dignity ,
                      ns:Self_Pleasure ,
                      ns:Self_Satisfaction ;
         rdfs:comment "Pride can be considered both an emotion and a trait, depending on the context and how it is being discussed. As an emotion, pride is typically associated with a sense of achievement, satisfaction, or self-worth. It is often described as a positive feeling that arises when someone accomplishes something meaningful or when they feel good about themselves. For example, a person might feel proud after winning a competition, completing a difficult task, or receiving recognition for their achievements. As a trait, pride is often viewed more negatively, as it can be seen as a character flaw or a negative personality trait. In this context, pride refers to an excessive sense of self-importance or arrogance. People who are overly proud may be seen as boastful, egotistical, or unwilling to admit their mistakes. Overall, whether pride is seen as an emotion or a trait largely depends on the individual and the situation. It can be a positive or negative force, depending on how it is expressed and experienced." ;
         rdfs:label "Pride"@en .


###  http://modai.ai/big5#Pride-Humility
ns:Pride-Humility rdf:type owl:NamedIndividual ,
                           ns:Prompt ;
                  ns:uses ns:Humility ,
                          ns:Pride ;
                  rdfs:comment """I want to quantify the pride in the following text:
```
$INPUT_TEXT
```

I define pride as a feeling of deep pleasure or satisfaction derived from one's own achievements, or the achievements of those with whom one is closely associated. I define the opposite of pride as humility or modesty.

Please answer on a scale of 1 - 5 where the numbers have the following meanings:
```
1 = The text is filled with humility, modesty, and has no elements of pride.
2 = The text has elements of humility or modesty, but also contains some elements of pride.
3 = The text has neither pride nor humility, it is neutral.
4 = The text has elements of pride but also has some aspects of humility or modesty.
5 = The text is deeply filled with pride, focusing heavily on feelings of pleasure or satisfaction derived from achievements.
```

Only respond with a number and no other rating.
"""@en ;
                  rdfs:label "Pride-Humility"@en .


###  http://modai.ai/big5#Proactive
ns:Proactive rdf:type owl:NamedIndividual ;
             rdfs:label "Proactive"@en .


###  http://modai.ai/big5#Procrastinating
ns:Procrastinating rdf:type owl:NamedIndividual ,
                            ns:Behavior ;
                   ns:associatedWith ns:Indecisiveness ,
                                     ns:Laziness ;
                   ns:triggeredBy ns:Avoidance ,
                                  ns:Fear ;
                   rdfs:label "Procrastinating"@en .


###  http://modai.ai/big5#Procrastinative
ns:Procrastinative rdf:type owl:NamedIndividual ;
                   rdfs:label "Procrastinative"@en .


###  http://modai.ai/big5#Progressive
ns:Progressive rdf:type owl:NamedIndividual ;
               rdfs:label "Progressive"@en .


###  http://modai.ai/big5#Prompt
ns:Prompt rdf:type owl:NamedIndividual .


###  http://modai.ai/big5#Protectiveness
ns:Protectiveness rdf:type owl:NamedIndividual ;
                  rdfs:label "Protectiveness"@en .


###  http://modai.ai/big5#Provocative
ns:Provocative rdf:type owl:NamedIndividual ;
               rdfs:label "Provocative"@en .


###  http://modai.ai/big5#Quiet
ns:Quiet rdf:type owl:NamedIndividual ;
         rdfs:label "Quiet"@en .


###  http://modai.ai/big5#Radical
ns:Radical rdf:type owl:NamedIndividual ;
           ns:similarTo ns:Adventurous ,
                        ns:Innovative ,
                        ns:Progressive ,
                        ns:Risk_Taking ;
           rdfs:label "Radical"@en .


###  http://modai.ai/big5#Reading
ns:Reading rdf:type owl:NamedIndividual ,
                    ns:Behavior ;
           ns:associatedWith ns:Intellectualism ;
           ns:triggeredBy ns:Boredom ,
                          ns:Curiosity ;
           rdfs:label "Reading"@en .


###  http://modai.ai/big5#Realistic
ns:Realistic rdf:type owl:NamedIndividual ;
             rdfs:label "Realistic"@en .


###  http://modai.ai/big5#Reassurance
ns:Reassurance rdf:type owl:NamedIndividual ,
                        ns:Trait ;
               ns:relatedTo ns:Relieved ;
               ns:similarTo ns:Relieved ;
               rdfs:comment "Reassurance is not an emotion or a trait in and of itself, but rather a behavior or action that can be conveyed through one's emotions or traits. It involves providing comfort and confidence to someone who is feeling anxious or uncertain. However, one's tendency to offer reassurance could be considered a trait. For example, if someone consistently displays a reassuring demeanor in various situations, it could be seen as a personality trait or a part of their communication style. Additionally, if someone frequently seeks reassurance from others, it could be seen as a trait related to their emotional needs or tendencies." ;
               rdfs:label "Reassurance"@en .


###  http://modai.ai/big5#Reassuring
ns:Reassuring rdf:type owl:NamedIndividual ,
                       ns:Behavior ;
              ns:associatedWith ns:Comforting ,
                                ns:Supportiveness ;
              ns:triggeredBy ns:Concern ,
                             ns:Empathy ;
              rdfs:label "Reassuring"@en .


###  http://modai.ai/big5#Rebelling
ns:Rebelling rdf:type owl:NamedIndividual ,
                      ns:Behavior ;
             ns:associatedWith ns:Defiance ,
                               ns:Nonconformity ;
             ns:triggeredBy ns:Discontent ,
                            ns:Frustration ;
             rdfs:label "Rebelling"@en .


###  http://modai.ai/big5#Reckless
ns:Reckless rdf:type owl:NamedIndividual ;
            rdfs:label "Reckless"@en .


###  http://modai.ai/big5#Reflecting
ns:Reflecting rdf:type owl:NamedIndividual ,
                       ns:Behavior ;
              ns:associatedWith ns:Self_Awareness ,
                                ns:Thoughtfulness ;
              ns:triggeredBy ns:Curiosity ,
                             ns:Uncertainty ;
              rdfs:label "Reflecting"@en .


###  http://modai.ai/big5#Reflective
ns:Reflective rdf:type owl:NamedIndividual ,
                       ns:Trait ;
              rdfs:comment "Reflective is not strictly an emotion or a trait, but rather a cognitive process or a behavior. It involves thinking deeply and often critically about one's own thoughts, behaviors, and experiences. However, it can be viewed as a trait or characteristic of someone who regularly engages in reflective thinking or as an emotion when someone is experiencing reflection as a response to a particular event or situation. Overall, reflective thinking is an important skill that can lead to personal growth and development." ;
              rdfs:label "Reflective"@en .


###  http://modai.ai/big5#Regret
ns:Regret rdf:type owl:NamedIndividual ,
                   ns:Emotion ,
                   ns:Negative_Low ;
          ns:oppositeTo ns:Satisfaction ;
          rdfs:comment "Regret can be considered both an emotion and a trait depending on the context. As an emotion, regret refers to the feeling of disappointment, distress, or sorrow caused by a perceived mistake or missed opportunity. It is a transient state that arises when we reflect on past actions or decisions and wish that we had done something differently. In this sense, regret is a natural and common emotion that we all experience from time to time. On the other hand, as a trait, regret can refer to a personality characteristic associated with a tendency to experience regret more frequently or intensely. Some people may be predisposed to feeling regret more easily due to their personality traits, cognitive style, or life experiences. They may be more risk-averse, conscientious, or self-critical, which can make them more prone to experience regret. In summary, regret can be both an emotion and a trait, and the distinction between the two depends on whether we are describing the transient feeling or the dispositional tendency to experience it." ;
          rdfs:label "Regret"@en .


###  http://modai.ai/big5#Regret-Satisfaction
ns:Regret-Satisfaction rdf:type owl:NamedIndividual ,
                                ns:Prompt ;
                       ns:uses ns:Regret ,
                               ns:Satisfaction ;
                       rdfs:comment """I want to quantify the regret in the following text:
```
$INPUT_TEXT
```

I define regret as a feeling of sorrow, remorse, or disappointment over something that has happened or been done. I define the opposite of regret as satisfaction or contentment.

Please answer on a scale of 1 - 5 where the numbers have the following meanings:
```
1 = The text is filled with satisfaction, contentment, and has no elements of regret.
2 = The text has elements of satisfaction or contentment, but also contains some elements of regret.
3 = The text has neither regret nor satisfaction, it is neutral.
4 = The text has elements of regret but also has some aspects of satisfaction or contentment.
5 = The text is deeply filled with regret, focusing heavily on feelings of sorrow, remorse, or disappointment over something that has happened or been done.
```

Only respond with a number and no other rating.
"""@en ;
                       rdfs:label "Regret-Satisfaction"@en .


###  http://modai.ai/big5#Rejection
ns:Rejection rdf:type owl:NamedIndividual ,
                      ns:Social ;
             ns:oppositeTo ns:Disregard ,
                           ns:Inclusion ;
             rdfs:comment "Rejection can be considered both an emotion and a trait, depending on how it is defined and interpreted. As an emotion, rejection refers to the feeling of being dismissed, excluded, or disregarded by others. It is often associated with negative emotions such as sadness, disappointment, hurt, or anger, and can be triggered by various situations such as romantic breakup, social exclusion, job rejection, or failure to meet standards. As a trait, rejection sensitivity refers to an individual's tendency to be highly sensitive and reactive to perceived rejection or criticism from others. This trait is often associated with higher levels of anxiety, insecurity, and interpersonal conflicts, and can also influence one's behavior and decision-making in relationships, work, and social situations. Overall, rejection can be seen as both an emotion and a trait that can have different impacts on people's thoughts, feelings, and behaviors depending on their personality, experiences, and coping strategies." ;
             rdfs:label "Rejection"@en .


###  http://modai.ai/big5#Rejection-Inclusion
ns:Rejection-Inclusion rdf:type owl:NamedIndividual ,
                                ns:Prompt ;
                       ns:uses ns:Inclusion ,
                               ns:Rejection ;
                       rdfs:comment """I want to quantify the rejection in the following text:
```
$INPUT_TEXT
```

I define rejection as a feeling of being turned down, dismissed, or excluded. I define the opposite of rejection as acceptance or inclusion.

Please answer on a scale of 1 - 5 where the numbers have the following meanings:
```
1 = The text is filled with acceptance, inclusion, and has no elements of rejection.
2 = The text has elements of acceptance or inclusion, but also contains some elements of rejection.
3 = The text has neither rejection nor acceptance, it is neutral.
4 = The text has elements of rejection but also has some aspects of acceptance or inclusion.
5 = The text is deeply filled with rejection, focusing heavily on feelings of being turned down, dismissed, or excluded.
```

Only respond with a number and no other rating.
"""@en ;
                       rdfs:label "Rejection-Inclusion"@en .


###  http://modai.ai/big5#Relaxation
ns:Relaxation rdf:type owl:NamedIndividual ;
              ns:oppositeTo ns:Tense ;
              ns:relatedTo ns:Relieved ;
              ns:similarTo ns:Relieved ;
              rdfs:comment "Relaxation is typically not considered an emotion or a trait but rather a state or condition of physical or mental ease. However, one's ability to relax or the propensity to seek relaxation could be considered a trait. For example, some individuals may have a natural inclination towards relaxation and may find it easier to enter a relaxed state, while others may have more difficulty relaxing and may need to actively work at achieving a state of relaxation. In this sense, relaxation could be considered a trait." ;
              rdfs:label "Relaxation"@en .


###  http://modai.ai/big5#Relaxed
ns:Relaxed rdf:type owl:NamedIndividual ;
           rdfs:label "Relaxed"@en .


###  http://modai.ai/big5#Reliable
ns:Reliable rdf:type owl:NamedIndividual ;
            ns:oppositeTo ns:Unreliable ;
            rdfs:label "Reliable"@en .


###  http://modai.ai/big5#Relieved
ns:Relieved rdf:type owl:NamedIndividual ,
                     ns:Positive_Low ;
            ns:oppositeTo ns:Tense ;
            rdfs:comment "Relieved is an emotion rather than a trait. This is because it is a temporary state that a person experiences in response to a particular situation. It is characterized by feelings of decreased anxiety, tension, or pressure after a stressful or uncertain event. Traits, on the other hand, are enduring personal characteristics that are relatively stable over time and are part of a person's personality, such as being introverted or extroverted. While individuals may have a tendency to feel relief in certain situations, the emotion of relief itself is not a defining aspect of their personality." ;
            rdfs:label "Relieved"@en .


###  http://modai.ai/big5#Relieved-Tense
ns:Relieved-Tense rdf:type owl:NamedIndividual ,
                           ns:Prompt ;
                  ns:uses ns:Relieved ,
                          ns:Tense ;
                  rdfs:comment """I want to quantify the relief in the following text:
```
$INPUT_TEXT
```

I define relief as a feeling of reassurance and relaxation following release from anxiety or distress. I define the opposite of relief as tension or anxiety.

Please answer on a scale of 1 - 5 where the numbers have the following meanings:
```
1 = The text is filled with tension, anxiety, and has no elements of relief.
2 = The text has elements of tension or anxiety, but also contains some elements of relief.
3 = The text has neither relief nor tension, it is neutral.
4 = The text has elements of relief but also has some aspects of tension or anxiety.
5 = The text is deeply filled with relief, focusing heavily on feelings of reassurance and relaxation.
```

Only respond with a number and no other rating.
"""@en ;
                  rdfs:label "Relieved-Tense"@en .


###  http://modai.ai/big5#Remorse
ns:Remorse rdf:type owl:NamedIndividual ,
                    ns:Emotion ;
           ns:relatedTo ns:Sorrow ;
           ns:similarTo ns:Sorrow ;
           rdfs:comment "Remorse is considered an emotion. It is a feeling of regret, guilt, or sorrow for something that one has done or failed to do. Unlike traits, which are enduring characteristics of a person's personality, emotions are temporary and can be influenced by various factors, such as situational context, social norms, and individual beliefs and values. Remorse can be experienced in response to specific actions or events, and can vary in intensity and duration depending on the situation and the individual's cognitive and emotional processing. Therefore, remorse is more appropriately considered an emotion rather than a trait." ;
           rdfs:label "Remorse"@en .


###  http://modai.ai/big5#Resentment
ns:Resentment rdf:type owl:NamedIndividual ,
                       ns:Negative_High ;
              rdfs:comment "Resentment is typically considered an emotion rather than a trait. Emotions are short-lived reactions to specific situations or events, while traits are enduring characteristics that define a person's personality. Resentment arises in response to a perceived injustice or unfair treatment, and it is usually experienced as a temporary feeling of anger or bitterness. However, if resentment is not addressed or resolved, it can develop into a more long-lasting attitude or disposition, which could then be considered a trait." ;
              rdfs:label "Resentment"@en .


###  http://modai.ai/big5#Resentment-Acceptance
ns:Resentment-Acceptance rdf:type owl:NamedIndividual ,
                                  ns:Prompt ;
                         ns:uses ns:Acceptance ,
                                 ns:Resentment ;
                         rdfs:comment """I want to quantify the resentment in the following text:
```
$INPUT_TEXT
```

I define resentment as a feeling of persistent ill will or bitterness, usually resulting from past insult or injury. I define the opposite of resentment as forgiveness or acceptance.

Please answer on a scale of 1 - 5 where the numbers have the following meanings:
```
1 = The text is filled with forgiveness, acceptance, and has no elements of resentment.
2 = The text has elements of forgiveness or acceptance, but also contains some elements of resentment.
3 = The text has neither resentment nor forgiveness, it is neutral.
4 = The text has elements of resentment but also has some aspects of forgiveness or acceptance.
5 = The text is deeply filled with resentment, focusing heavily on feelings of persistent ill will or bitterness.
```

Only respond with a number and no other rating.
"""@en ;
                         rdfs:label "Resentment-Acceptance"@en .


###  http://modai.ai/big5#Reserved
ns:Reserved rdf:type owl:NamedIndividual ,
                     ns:Trait ;
            rdfs:comment "\"Reserved\" is typically considered more of a personality trait than an emotion. It generally refers to someone who is quiet, cautious, and tends to keep to themselves. This trait can be influenced by a range of factors, including introversion, shyness, social anxiety, or cultural norms about appropriate behavior. While a reserved person may experience emotions like fear or discomfort in social situations, the trait itself is more about their natural tendencies and behavior patterns." ;
            rdfs:label "Reserved"@en .


###  http://modai.ai/big5#Resilient
ns:Resilient rdf:type owl:NamedIndividual ;
             rdfs:label "Resilient"@en .


###  http://modai.ai/big5#Respect
ns:Respect rdf:type owl:NamedIndividual ;
           rdfs:label "Respect"@en .


###  http://modai.ai/big5#Respectful
ns:Respectful rdf:type owl:NamedIndividual ,
                       ns:Trait ;
              ns:oppositeTo ns:Disrespectful ;
              rdfs:comment "Respectful is generally considered a trait rather than an emotion. It refers to a pattern of behavior and attitude towards others that involves showing consideration, courtesy, and deference. While emotions certainly play a role in how respectful someone might be in a given moment (such as feeling empathy or gratitude), the overall trait of being respectful is characterized by consistent actions and attitudes over time." ;
              rdfs:label "Respectful"@en .


###  http://modai.ai/big5#Respectfulness
ns:Respectfulness rdf:type owl:NamedIndividual .


###  http://modai.ai/big5#Responsible
ns:Responsible rdf:type owl:NamedIndividual ;
               rdfs:label "Responsible"@en .


###  http://modai.ai/big5#Restfulness
ns:Restfulness rdf:type owl:NamedIndividual ;
               rdfs:label "Restfulness"@en .


###  http://modai.ai/big5#Restless
ns:Restless rdf:type owl:NamedIndividual ;
            rdfs:label "Restless"@en .


###  http://modai.ai/big5#Restlessness
ns:Restlessness rdf:type owl:NamedIndividual ;
                rdfs:label "Restlessness"@en .


###  http://modai.ai/big5#Reverence
ns:Reverence rdf:type owl:NamedIndividual ;
             ns:relatedTo ns:Awe ;
             ns:similarTo ns:Awe ;
             rdfs:comment "Reverence can be considered both an emotion and a trait, depending on the context in which it is being discussed. As an emotion, reverence typically refers to a feeling of deep respect, admiration, or awe that one experiences when in the presence of something or someone that is considered sacred, holy, or extraordinary. For example, a person may feel reverence when standing in a beautiful and grand cathedral, or when seeing a majestic mountain range for the first time. As a trait, reverence refers to a person's disposition or tendency to show respect and awe towards things that are considered holy, sacred, or extraordinary, even when not directly experiencing them. This trait can be seen in a person's behavior, attitude, and beliefs, and is often related to their spiritual or cultural background. Overall, while reverence can be both an emotion and a trait, the two are interconnected and often go hand in hand. When a person experiences reverence as an emotion, it can shape and reinforce their traits of being respectful and awe-inspiring towards things that are considered sacred or extraordinary." ;
             rdfs:label "Reverence"@en .


###  http://modai.ai/big5#Revulsion
ns:Revulsion rdf:type owl:NamedIndividual ;
             ns:oppositeTo ns:Pleasure ;
             ns:relatedTo ns:Dislike ;
             ns:similarTo ns:Dislike ;
             rdfs:comment "Revulsion can be considered both an emotion and a trait, depending on the context in which it is being used. As an emotion, revulsion refers to a strong feeling of disgust or aversion in response to something unpleasant or offensive. For example, a person might feel revulsion at the sight or smell of rotting food, or at the thought of a particular sexual act. As a trait, revulsion refers to a tendency or disposition to experience this emotion more strongly or frequently than others. Some people may be more easily agitated or disgusted by things that others would find more tolerable, indicating a higher level of revulsion as a trait. In psychology, trait revulsion is often studied in the context of personality traits such as neuroticism or disgust sensitivity, which are believed to be relatively stable over time and across situations. However, it is important to note that emotions and traits are not mutually exclusive; instead, they are often intertwined and shape one another over time." ;
             rdfs:label "Revulsion"@en .


###  http://modai.ai/big5#Risk_Averse
ns:Risk_Averse rdf:type owl:NamedIndividual ;
               ns:similarTo ns:Conservative ;
               rdfs:label "Risk_Averse"@en .


###  http://modai.ai/big5#Risk_Taking
ns:Risk_Taking rdf:type owl:NamedIndividual ;
               ns:oppositeTo ns:Risk_Averse ;
               rdfs:label "Risk_Taking"@en .


###  http://modai.ai/big5#Rude
ns:Rude rdf:type owl:NamedIndividual ;
        rdfs:label "Rude"@en .


###  http://modai.ai/big5#Sad
ns:Sad rdf:type owl:NamedIndividual ;
       rdfs:label "Sad"@en .


###  http://modai.ai/big5#Sadness
ns:Sadness rdf:type owl:NamedIndividual ,
                    ns:Emotion ,
                    ns:Negative_Low ;
           ns:relatedTo ns:Dissapointment ,
                        ns:Sorrow ;
           ns:similarTo ns:Dissapointment ,
                        ns:Sorrow ;
           rdfs:comment "Sadness is considered an emotion rather than a trait. Emotions are temporary states that are evoked by specific situations or events, while traits are more enduring characteristics of a person that remain relatively stable over time. Sadness is typically triggered by a specific cause, such as a loss or disappointment, and tends to dissipate over time as the person processes their feelings and moves on. In contrast, a trait like introversion or extroversion is a more stable aspect of a person's personality that remains relatively consistent across different situations and experiences. While some people may be more prone to experiencing sadness than others due to their personality or life experiences, it is still considered an emotion that is evoked by external factors rather than a defining trait of the person themselves." ;
           rdfs:label "Sadness"@en .


###  http://modai.ai/big5#Sadness-Happiness
ns:Sadness-Happiness rdf:type owl:NamedIndividual ,
                              ns:Prompt ;
                     ns:uses ns:Happiness ,
                             ns:Sadness ;
                     rdfs:comment """I want to quantify the level of sadness or happiness in the following text:
```
$INPUT_TEXT
```

I define sadness as a state of sorrow, unhappiness, or melancholy. I define happiness as a state of joy, contentment, or satisfaction.

Please answer on a scale of 1 - 5 where the numbers have the following meanings:
```
1 = The text is filled with happiness, joy, and has no elements of sadness.
2 = The text has elements of happiness or joy, but also contains some elements of sadness.
3 = The text has neither sadness nor happiness, it is neutral.
4 = The text has elements of sadness but also has some aspects of happiness or joy.
5 = The text is deeply filled with sadness, focusing heavily on sorrow, unhappiness, or melancholy.
```

Only respond with a number and no other rating.

"""@en ;
                     rdfs:label "Sadness-Happiness"@en .


###  http://modai.ai/big5#Sadness-Joy
ns:Sadness-Joy rdf:type owl:NamedIndividual ,
                        ns:Prompt ;
               ns:uses ns:Joy ,
                       ns:Sadness ;
               rdfs:comment """I want to quantify the sadness in the following text:
```
$INPUT_TEXT
```

I define sadness as a state of unhappiness or feeling of sorrow. I define the opposite of sadness as joy or happiness.

Please answer on a scale of 1 - 5 where the numbers have the following meanings:
```
1 = The text is brimming with joy, happiness, and positive sentiment, and has no sadness.
2 = The text has joyful or happy elements, but also contains some elements of sadness.
3 = The text has neither sadness nor happiness, it is neutral.
4 = The text has sad elements but also has some neutral or positive aspects.
5 = The text is deeply sad, focusing heavily on sorrow and unhappiness.
```

Only respond with a number and no other rating.
"""@en ;
               rdfs:label "Sadness-Joy"@en .


###  http://modai.ai/big5#Safety
ns:Safety rdf:type owl:NamedIndividual ,
                   ns:Trait ;
          ns:oppositeTo ns:Fear ;
          rdfs:comment "Safety is generally considered neither an emotion nor a trait. Emotions are subjective experiences that arise in response to a particular event or stimulus. Safety, on the other hand, is a state of being free from danger or harm. While emotions can certainly be influenced by feelings of safety or lack thereof, safety itself is not an emotion. Traits, meanwhile, are enduring characteristics or dispositions that individuals possess. Some traits may be related to safety, such as caution or risk aversion, but safety as a concept does not fit neatly into the category of traits. Instead, safety is better understood as a state or a condition. It is the absence or minimization of risk, and can be achieved through various means such as planning, preparation, and adherence to safety guidelines." ;
          rdfs:label "Safety"@en .


###  http://modai.ai/big5#Satisfaction
ns:Satisfaction rdf:type owl:NamedIndividual ,
                         ns:Emotion ,
                         ns:Positive_Low ;
                ns:oppositeTo ns:Regret ;
                ns:relatedTo ns:Contentment ;
                ns:similarTo ns:Contentment ;
                rdfs:comment "Satisfaction can be considered both an emotion and a trait depending on the context in which it is used and understood. As an emotion, satisfaction refers to the feeling of pleasure or contentment that a person experiences after achieving a goal or desired outcome. This feeling is typically temporary and can vary in intensity and duration based on individual differences in temperament, mood, and personal values. As a trait, satisfaction refers to a stable and enduring personality characteristic that captures a person's tendency to experience satisfaction or pleasure over time and across different situations. This trait is often linked to positive factors such as self-esteem, resilience, and subjective well-being, and is thought to be a key component of mental health and psychological functioning. Overall, the distinction between satisfaction as an emotion and trait is important for understanding how it influences behavior, motivation, and overall quality of life. Understanding both aspects of satisfaction can help individuals cultivate this positive emotion and trait in their daily lives." ;
                rdfs:label "Satisfaction"@en .


###  http://modai.ai/big5#Satisfaction-Disatisfaction
ns:Satisfaction-Disatisfaction rdf:type owl:NamedIndividual ,
                                        ns:Prompt ;
                               ns:uses ns:Dissatisfaction ,
                                       ns:Satisfaction ;
                               rdfs:comment """I want to quantify the satisfaction in the following text:
```
$INPUT_TEXT
```

I define satisfaction as a feeling of fulfillment or contentment. I define the opposite of satisfaction as dissatisfaction or discontent.

Please answer on a scale of 1 - 5 where the numbers have the following meanings:
```
1 = The text is filled with dissatisfaction, discontent, and has no elements of satisfaction.
2 = The text has elements of dissatisfaction or discontent, but also contains some elements of satisfaction.
3 = The text has neither satisfaction nor dissatisfaction, it is neutral.
4 = The text has elements of satisfaction but also has some aspects of dissatisfaction or discontent.
5 = The text is deeply filled with satisfaction, focusing heavily on feelings of fulfillment and contentment.
```

Only respond with a number and no other rating.
"""@en ;
                               rdfs:label "Satisfaction-Disatisfaction"@en .


###  http://modai.ai/big5#Scattered
ns:Scattered rdf:type owl:NamedIndividual ;
             rdfs:label "Scattered"@en .


###  http://modai.ai/big5#Screaming
ns:Screaming rdf:type owl:NamedIndividual ,
                      ns:Behavior ;
             ns:associatedWith ns:Expressiveness ;
             ns:triggeredBy ns:Anger ,
                            ns:Fear ;
             rdfs:label "Screaming"@en .


###  http://modai.ai/big5#Self_Assured
ns:Self_Assured rdf:type owl:NamedIndividual ;
                rdfs:label "Self_Assured"@en .


###  http://modai.ai/big5#Self_Awareness
ns:Self_Awareness rdf:type owl:NamedIndividual ;
                  rdfs:label "Self_Awareness"@en .


###  http://modai.ai/big5#Self_Centered
ns:Self_Centered rdf:type owl:NamedIndividual ;
                 rdfs:label "Self_Centered"@en .


###  http://modai.ai/big5#Self_Confident
ns:Self_Confident rdf:type owl:NamedIndividual ;
                  rdfs:label "Self_Confident"@en .


###  http://modai.ai/big5#Self_Doubting
ns:Self_Doubting rdf:type owl:NamedIndividual ;
                 rdfs:label "Self_Doubting"@en .


###  http://modai.ai/big5#Self_Pleasure
ns:Self_Pleasure rdf:type owl:NamedIndividual ,
                          ns:Trait ;
                 rdfs:comment "Self-pleasure, or the act of providing oneself with sexual pleasure, is not an emotion or a trait. It is a behavior or action that an individual can choose to engage in. Emotions are feelings, such as happiness, sadness, anger, and fear, while traits are characteristics of an individual's personality, such as kindness, extroversion, or introversion. Self-pleasure may be influenced by one's emotions or traits, but it is not inherently an emotion or a trait in and of itself." ;
                 rdfs:label "Self_Pleasure"@en .


###  http://modai.ai/big5#Self_Satisfaction
ns:Self_Satisfaction rdf:type owl:NamedIndividual ,
                              ns:Emotion ,
                              ns:Trait ;
                     ns:relatedTo ns:Satisfaction ;
                     ns:similarTo ns:Satisfaction ;
                     rdfs:comment "Self-satisfaction can be considered both an emotion and a trait, as it is a complex psychological experience that combines cognitive, affective, and behavioral components. As an emotion, self-satisfaction is the feeling of pride, pleasure, or contentment that arises from achieving a personal goal, experiencing success, or receiving recognition for one's efforts or accomplishments. This emotion is typically transient and situational, and may vary in intensity based on the specific context or individual's personality. As a trait, self-satisfaction can refer to a more enduring characteristic of a person, reflecting their general tendency to be content with themselves, their achievements, and their life situation. This trait is thought to be related to self-esteem, self-confidence, and self-efficacy, and may influence a wide range of behaviors, attitudes, and outcomes. In summary, self-satisfaction can be seen as both an emotion and a trait, depending on the level of specificity and context in which it is assessed." ;
                     rdfs:label "Self_Satisfaction"@en .


###  http://modai.ai/big5#Selfish
ns:Selfish rdf:type owl:NamedIndividual ;
           rdfs:label "Selfish"@en .


###  http://modai.ai/big5#Sensitive
ns:Sensitive rdf:type owl:NamedIndividual ;
             rdfs:label "Sensitive"@en .


###  http://modai.ai/big5#Serenity
ns:Serenity rdf:type owl:NamedIndividual ;
            ns:oppositeTo ns:Anxiety ;
            rdfs:comment "Serenity can be considered both an emotion and a trait. As an emotion, serenity describes a sense of calm, peacefulness, and tranquility that someone may experience in a particular moment. It can be associated with feelings of relaxation, contentment, and inner peace. As a trait, serenity describes someone's overall character or personality. It refers to a person who is typically calm, composed, and centered, even in the midst of challenges or stressful situations. This trait is often associated with mindfulness, self-awareness, and emotional stability. In summary, serenity can be both an emotion and a trait, depending on how it is used and in what context it is being discussed." ;
            rdfs:label "Serenity"@en .


###  http://modai.ai/big5#Shaking
ns:Shaking rdf:type owl:NamedIndividual ,
                    ns:Behavior ;
           ns:associatedWith ns:Nervousness ;
           ns:triggeredBy ns:Excitement ,
                          ns:Fear ;
           rdfs:label "Shaking"@en .


###  http://modai.ai/big5#Shame
ns:Shame rdf:type owl:NamedIndividual ,
                  ns:Negative_Low ;
         ns:oppositeTo ns:Humility ,
                       ns:Pride ;
         rdfs:comment "Shame can be considered both an emotion and a trait, depending on how it is defined and understood. As an emotion, shame is a complex feeling of self-consciousness and embarrassment that arises from a sense of failure, inadequacy, or wrongdoing. It involves intense feelings of exposure, vulnerability, and humiliation, and can lead individuals to withdraw, isolate themselves, or avoid situations that might trigger shame. As a trait, shame can be seen as a more enduring feature of a person's personality or worldview. It can manifest as a persistent sense of unworthiness, self-doubt, or self-blame, and can be deeply rooted in past experiences of trauma, abuse, or neglect. In this sense, shame can become a habitual response to life's challenges and can shape how a person perceives themselves and others. Ultimately, the distinction between shame as an emotion and a trait is somewhat artificial, as both are integral to the complex ways in which individuals experience and navigate their inner lives. Understanding the role of shame in one's own emotional and psychological makeup can be an important step toward building greater self-awareness, self-compassion, and resilience." ;
         rdfs:label "Shame"@en .


###  http://modai.ai/big5#Shame-Humility
ns:Shame-Humility rdf:type owl:NamedIndividual ,
                           ns:Prompt ;
                  ns:uses ns:Humility ,
                          ns:Shame ;
                  rdfs:comment """I want to quantify the shame in the following text:
```
$INPUT_TEXT
```

I define shame as a painful feeling of humiliation or distress caused by the consciousness of wrong or foolish behavior. I define the opposite of shame as humility, which involves a modest view of one's own importance.

Please answer on a scale of 1 - 5 where the numbers have the following meanings:
```
1 = The text is filled with humility, modesty, and has no elements of shame.
2 = The text has elements of humility or modesty, but also contains some elements of shame.
3 = The text has neither shame nor humility, it is neutral.
4 = The text has elements of shame but also has some aspects of humility or modesty.
5 = The text is deeply filled with shame, focusing heavily on feelings of humiliation or distress.
```

Only respond with a number and no other rating.
"""@en ;
                  rdfs:label "Shame-Humility"@en .


###  http://modai.ai/big5#Shame-Pride
ns:Shame-Pride rdf:type owl:NamedIndividual ,
                        ns:Prompt ;
               ns:uses ns:Pride ,
                       ns:Shame ;
               rdfs:comment """I want to quantify the shame in the following text:
```
$INPUT_TEXT
```

I define shame as a painful feeling of humiliation or distress caused by the consciousness of wrong or foolish behavior. I define the opposite of shame as pride or self-acceptance.

Please answer on a scale of 1 - 5 where the numbers have the following meanings:
```
1 = The text is filled with pride, self-acceptance, and has no elements of shame.
2 = The text has elements of pride or self-acceptance, but also contains some elements of shame.
3 = The text has neither shame nor pride, it is neutral.
4 = The text has elements of shame but also has some aspects of pride or self-acceptance.
5 = The text is deeply filled with shame, focusing heavily on feelings of humiliation or distress.
```

Only respond with a number and no other rating.
"""@en ;
               rdfs:label "Shame-Pride"@en .


###  http://modai.ai/big5#Shock
ns:Shock rdf:type owl:NamedIndividual ;
         ns:relatedTo ns:Surprise ;
         ns:similarTo ns:Surprise ;
         rdfs:comment "Shock can be considered both an emotion and a trait, depending on the context in which it is being used and the perspective of the observer. As an emotion, shock refers to a sudden and intense feeling of surprise, disbelief, or disbelief in response to a sudden or unexpected event or situation. In this sense, shock is transient experience that occurs in response to specific stimuli and is characterized by physiological and psychological changes, such as increased heart rate and mental confusion. As a trait, shock may refer to an individual's tendency to experience shock-like responses to certain stimuli or situations. For example, some people may have a heightened sensitivity or reactivity to sudden or unexpected events due to their personality, temperament, or past experiences. In this sense, shock may be considered a stable and consistent aspect of an individual's psychological makeup that influences their behavior and emotional responses over time. In summary, shock can be viewed as both an emotion and a trait depending on the temporal and dispositional aspects of the concept." ;
         rdfs:label "Shock"@en .


###  http://modai.ai/big5#Shouting
ns:Shouting rdf:type owl:NamedIndividual ,
                     ns:Behavior ;
            ns:associatedWith ns:Assertiveness ;
            ns:triggeredBy ns:Anger ,
                           ns:Excitement ;
            rdfs:label "Shouting"@en .


###  http://modai.ai/big5#Shy
ns:Shy rdf:type owl:NamedIndividual ;
       rdfs:label "Shy"@en .


###  http://modai.ai/big5#Simple
ns:Simple rdf:type owl:NamedIndividual ;
          rdfs:label "Simple"@en .


###  http://modai.ai/big5#Simplistic
ns:Simplistic rdf:type owl:NamedIndividual ;
              rdfs:label "Simplistic"@en .


###  http://modai.ai/big5#Singing
ns:Singing rdf:type owl:NamedIndividual ,
                    ns:Behavior ;
           ns:associatedWith ns:Expressiveness ;
           ns:triggeredBy ns:Joy ,
                          ns:Sadness ;
           rdfs:label "Singing"@en .


###  http://modai.ai/big5#Skepticism
ns:Skepticism rdf:type owl:NamedIndividual ;
              ns:relatedTo ns:Doubt ;
              ns:similarTo ns:Doubt ;
              rdfs:comment "Skepticism can be considered both an emotion and a trait depending on how it is defined and understood in the context of psychology. As an emotion, skepticism may be associated with feelings of doubt, mistrust, uncertainty, and suspicion towards information, people, or situations. In this sense, skepticism may be seen as a protective response to perceived threats or risks, such as potential scams, misinformation, or manipulation. Skepticism as an emotion may also reflect personality traits such as neuroticism, which involves a tendency to experience negative emotions in response to stress or uncertainty. On the other hand, skepticism can also be seen as a trait, which refers to a stable pattern of thoughts, feelings, and behavior that characterizes an individual over time and across different situations. As a trait, skepticism may involve a general disposition to question assumptions, scrutinize evidence, and seek rational explanations for events. This trait may be associated with critical thinking, intellectual curiosity, and openness to new ideas. Overall, whether skepticism is considered an emotion or a trait depends on the specific definition and conceptualization of the term, as well as the research context and theoretical perspective." ;
              rdfs:label "Skepticism"@en .


###  http://modai.ai/big5#Sleep
ns:Sleep rdf:type owl:NamedIndividual ;
         rdfs:label "Sleep"@en .


###  http://modai.ai/big5#Sleeping
ns:Sleeping rdf:type owl:NamedIndividual ,
                     ns:Behavior ;
            ns:associatedWith ns:Restfulness ;
            ns:triggeredBy ns:Comfort ,
                           ns:Tiredness ;
            rdfs:label "Sleeping"@en .


###  http://modai.ai/big5#Slow
ns:Slow rdf:type owl:NamedIndividual ;
        rdfs:label "Slow"@en .


###  http://modai.ai/big5#Smiling
ns:Smiling rdf:type owl:NamedIndividual ,
                    ns:Behavior ;
           ns:associatedWith ns:Cheerfulness ;
           ns:triggeredBy ns:Happiness ,
                          ns:Pleasure ;
           rdfs:label "Smiling"@en .


###  http://modai.ai/big5#Sneezing
ns:Sneezing rdf:type owl:NamedIndividual ,
                     ns:Behavior ;
            ns:associatedWith ns:Involuntary ;
            ns:triggeredBy ns:Allergies ,
                           ns:Irritation ;
            rdfs:label "Sneezing"@en .


###  http://modai.ai/big5#Snoring
ns:Snoring rdf:type owl:NamedIndividual ,
                    ns:Behavior ;
           ns:associatedWith ns:Unconscious ;
           ns:triggeredBy ns:Exhaustion ,
                          ns:Sleep ;
           rdfs:label "Snoring"@en .


###  http://modai.ai/big5#Sociable
ns:Sociable rdf:type owl:NamedIndividual ;
            rdfs:label "Sociable"@en .


###  http://modai.ai/big5#Social
ns:Social rdf:type owl:NamedIndividual .


###  http://modai.ai/big5#Sorrow
ns:Sorrow rdf:type owl:NamedIndividual ,
                   ns:Emotion ;
          ns:relatedTo ns:Regret ;
          ns:similarTo ns:Regret ;
          rdfs:comment "Sorrow is generally considered to be an emotion rather than a trait. Emotions are short-term responses to specific situations or stimuli, while traits are enduring patterns of behavior or disposition. Sorrow is a feeling of sadness, grief or regret in response to a specific event or situation, such as the loss of a loved one or a personal failure. It may also involve physiological responses such as crying, lethargy, or loss of appetite. While it may be possible for someone to have a tendency towards feeling sorrow more frequently or intensely than others (which could be seen as a trait), this is not the typical way of conceptualizing the experience of sorrow. Rather, it is a temporary state that arises in response to specific circumstances and fades over time." ;
          rdfs:label "Sorrow"@en .


###  http://modai.ai/big5#Speaking
ns:Speaking rdf:type owl:NamedIndividual ,
                     ns:Behavior ;
            ns:associatedWith ns:Communicativeness ;
            ns:triggeredBy ns:Necessity ;
            rdfs:label "Speaking"@en .


###  http://modai.ai/big5#Stable
ns:Stable rdf:type owl:NamedIndividual ;
          rdfs:label "Stable"@en .


###  http://modai.ai/big5#Staring
ns:Staring rdf:type owl:NamedIndividual ,
                    ns:Behavior ;
           ns:associatedWith ns:Attentiveness ;
           ns:triggeredBy ns:Confusion ,
                          ns:Interest ;
           rdfs:label "Staring"@en .


###  http://modai.ai/big5#Steady
ns:Steady rdf:type owl:NamedIndividual ;
          rdfs:label "Steady"@en .


###  http://modai.ai/big5#Stoic
ns:Stoic rdf:type owl:NamedIndividual ;
         rdfs:label "Stoic"@en .


###  http://modai.ai/big5#Stress
ns:Stress rdf:type owl:NamedIndividual ;
          rdfs:label "Stress"@en .


###  http://modai.ai/big5#Stressed
ns:Stressed rdf:type owl:NamedIndividual ;
            rdfs:label "Stressed"@en .


###  http://modai.ai/big5#Strong_Minded
ns:Strong_Minded rdf:type owl:NamedIndividual ,
                          ns:Trait ;
                 ns:oppositeTo ns:Passive ;
                 rdfs:comment "Strong-minded is considered a trait rather than an emotion. This is because traits are enduring characteristics that define an individual's behavior and thought process, while emotions are short-term reactions to stimuli. Strong-mindedness refers to a person's determination, perseverance, and a steadfast approach to their beliefs and decisions. It is a relatively stable personality trait that persists across different situations and is less likely to change over time." ;
                 rdfs:label "Strong_Minded"@en .


###  http://modai.ai/big5#Structured
ns:Structured rdf:type owl:NamedIndividual ;
              rdfs:label "Structured"@en .


###  http://modai.ai/big5#Studying
ns:Studying rdf:type owl:NamedIndividual ,
                     ns:Behavior ;
            ns:associatedWith ns:Dedication ,
                              ns:Diligence ,
                              ns:Perseverance ;
            ns:triggeredBy ns:Curiosity ,
                           ns:Necessity ;
            rdfs:label "Studying"@en .


###  http://modai.ai/big5#Subjective
ns:Subjective rdf:type owl:NamedIndividual ;
              rdfs:label "Subjective"@en .


###  http://modai.ai/big5#Submissive
ns:Submissive rdf:type owl:NamedIndividual ;
              rdfs:label "Submissive"@en .


###  http://modai.ai/big5#Submissiveness
ns:Submissiveness rdf:type owl:NamedIndividual ;
                  rdfs:label "Submissiveness"@en .


###  http://modai.ai/big5#Success
ns:Success rdf:type owl:NamedIndividual ,
                    ns:Trait ;
           ns:relatedTo ns:Victory ;
           ns:similarTo ns:Victory ;
           rdfs:comment "Success can be considered both an emotion and a trait, depending on how it is defined and approached. As an emotion, success can be characterized by feelings of achievement, satisfaction, and pride that stem from accomplishing a goal or objective. It is a subjective experience that varies from person to person based on their individual expectations and aspirations. For example, winning a race or landing a new job may evoke a sense of success, leading to positive emotions and self-confidence. As a trait, success can be seen as a set of characteristics or skills that enable an individual to achieve their goals and succeed in life. These traits may include qualities such as determination, resilience, goal-setting ability, adaptability, and self-discipline. Individuals who display these traits tend to be more successful in their endeavors and are more likely to achieve long-term success and fulfillment. In summary, success can be both an emotion and a trait, and both perspectives are important in understanding and achieving success in our personal and professional lives." ;
           rdfs:label "Success"@en .


###  http://modai.ai/big5#Superficial
ns:Superficial rdf:type owl:NamedIndividual ;
               rdfs:label "Superficial"@en .


###  http://modai.ai/big5#Supportive
ns:Supportive rdf:type owl:NamedIndividual ;
              rdfs:label "Supportive"@en .


###  http://modai.ai/big5#Supportiveness
ns:Supportiveness rdf:type owl:NamedIndividual ;
                  rdfs:label "Supportiveness"@en .


###  http://modai.ai/big5#Surprise
ns:Surprise rdf:type owl:NamedIndividual ;
            ns:oppositeTo ns:Predictability ;
            rdfs:comment "Surprise is generally considered an emotion because it is a sudden and unexpected reaction to unexpected events, situations or information. It involves physiological changes such as increased heart rate, widening of the eyes, and quickening of breath, which are similar to other emotions like fear, excitement and joy. Moreover, it is usually temporary and can fade quickly once the surprise has passed. However, some people may display surprise more frequently or strongly than others due to their personality traits, such as openness to experience or neuroticism, which could make it seem like a trait. Overall, though, surprise is commonly understood by researchers as an emotional state that can vary from person to person and context to context." ;
            rdfs:label "Surprise"@en .


###  http://modai.ai/big5#Surprise-Predictability
ns:Surprise-Predictability rdf:type owl:NamedIndividual ,
                                    ns:Prompt ;
                           ns:uses ns:Predictability ,
                                   ns:Surprise ;
                           rdfs:comment """I want to quantify the surprise in the following text:
```
$INPUT_TEXT
```

I define surprise as a feeling of unexpected astonishment or shock. I define the opposite of surprise as expectation or predictability.

Please answer on a scale of 1 - 5 where the numbers have the following meanings:
```
1 = The text is filled with expected, predictable elements, and has no elements of surprise.
2 = The text has elements of expectation or predictability, but also contains some elements of surprise.
3 = The text has neither surprise nor predictability, it is neutral.
4 = The text has elements of surprise but also has some predictable or expected aspects.
5 = The text is deeply filled with surprise, focusing heavily on unexpected astonishment or shock.
```

Only respond with a number and no other rating.
"""@en ;
                           rdfs:label "Surprise-Predictability"@en .


###  http://modai.ai/big5#Suspicious
ns:Suspicious rdf:type owl:NamedIndividual ;
              rdfs:label "Suspicious"@en .


###  http://modai.ai/big5#Swearing
ns:Swearing rdf:type owl:NamedIndividual ,
                     ns:Behavior ;
            ns:associatedWith ns:Expressiveness ;
            ns:triggeredBy ns:Anger ,
                           ns:Frustration ;
            rdfs:label "Swearing"@en .


###  http://modai.ai/big5#Sympathy
ns:Sympathy rdf:type owl:NamedIndividual ,
                     ns:Social ;
            ns:oppositeTo ns:Apathy ;
            rdfs:comment "Sympathy is generally considered an emotion, as it involves feeling a sense of compassion or sorrow for someone who is experiencing pain, loss or hardship. It is often linked to empathy, where a person can understand and share the feelings of another, although they may not be experiencing those same feelings themselves. However, some people may argue that sympathy can also be considered a trait, as some individuals may have a natural inclination towards being more sympathetic and compassionate towards others. This could be influenced by various factors such as upbringing, cultural values, personality traits, and life experiences. Ultimately, whether sympathy is considered an emotion or a trait may depend on how it is defined and understood in various contexts." ;
            rdfs:label "Sympathy"@en .


###  http://modai.ai/big5#Sympathy-Apathy
ns:Sympathy-Apathy rdf:type owl:NamedIndividual ,
                            ns:Prompt ;
                   ns:uses ns:Apathy ,
                           ns:Sympathy ;
                   rdfs:comment """I want to quantify the sympathy in the following text:
```
$INPUT_TEXT
```

I define sympathy as feelings of pity and sorrow for someone else's misfortune. I define the opposite of sympathy as apathy or indifference.

Please answer on a scale of 1 - 5 where the numbers have the following meanings:
```
1 = The text is filled with apathy, indifference, and has no elements of sympathy.
2 = The text has elements of apathy or indifference, but also contains some elements of sympathy.
3 = The text has neither sympathy nor apathy, it is neutral.
4 = The text has elements of sympathy but also has some aspects of apathy or indifference.
5 = The text is deeply filled with sympathy, focusing heavily on feelings of pity and sorrow for someone else's misfortune.
```

Only respond with a number and no other rating.
"""@en ;
                   rdfs:label "Sympathy-Apathy"@en .


###  http://modai.ai/big5#Talkative
ns:Talkative rdf:type owl:NamedIndividual ;
             rdfs:label "Talkative"@en .


###  http://modai.ai/big5#Teasing
ns:Teasing rdf:type owl:NamedIndividual ,
                    ns:Behavior ;
           ns:associatedWith ns:Mischievousness ;
           ns:triggeredBy ns:Malice ,
                          ns:Playfulness ;
           rdfs:label "Teasing"@en .


###  http://modai.ai/big5#Temperamental
ns:Temperamental rdf:type owl:NamedIndividual ;
                 rdfs:label "Temperamental"@en .


###  http://modai.ai/big5#Tense
ns:Tense rdf:type owl:NamedIndividual ,
                  ns:Negative_High ;
         ns:relatedTo ns:Anxiety ;
         ns:similarTo ns:Anxiety ;
         rdfs:comment "Tense is neither an emotion nor a trait, but rather a state of being. It refers to a feeling of physical or emotional unease or strain that arises when one is under stress or pressure. Tension can be a temporary state or a chronic one depending on the situation, and can have both positive and negative effects on one's well-being and performance. While it is not an emotion or a trait in and of itself, how one responds to tension can be shaped by their emotional tendencies and personality traits." ;
         rdfs:label "Tense"@en .


###  http://modai.ai/big5#Thankful
ns:Thankful rdf:type owl:NamedIndividual ;
            ns:relatedTo ns:Gratitude ;
            ns:similarTo ns:Gratitude ;
            rdfs:comment "Thankful can be considered both an emotion and a trait. As an emotion, thankfulness can be viewed as a positive feeling of gratitude and appreciation for something or someone. It is something that we feel in response to good things that happen to us. As a trait, thankfulness can be considered a part of an individual's character or personality. This means that some people may be more naturally thankful than others and may exhibit more gratitude on an ongoing basis. Overall, whether we consider thankfulness an emotion or a trait may depend on our perspective and the context in which it is being discussed." ;
            rdfs:label "Thankful"@en .


###  http://modai.ai/big5#Thorough
ns:Thorough rdf:type owl:NamedIndividual ;
            rdfs:label "Thorough"@en .


###  http://modai.ai/big5#Thoughtful
ns:Thoughtful rdf:type owl:NamedIndividual ;
              rdfs:label "Thoughtful"@en .


###  http://modai.ai/big5#Thoughtfulness
ns:Thoughtfulness rdf:type owl:NamedIndividual ;
                  rdfs:label "Thoughtfulness"@en .


###  http://modai.ai/big5#Throwing
ns:Throwing rdf:type owl:NamedIndividual ,
                     ns:Behavior ;
            ns:associatedWith ns:Impulsiveness ;
            ns:triggeredBy ns:Anger ,
                           ns:Excitement ;
            rdfs:label "Throwing"@en .


###  http://modai.ai/big5#Tickling
ns:Tickling rdf:type owl:NamedIndividual ,
                     ns:Behavior ;
            ns:associatedWith ns:Affection ;
            ns:triggeredBy ns:Playfulness ;
            rdfs:label "Tickling"@en .


###  http://modai.ai/big5#Tidy
ns:Tidy rdf:type owl:NamedIndividual ;
        rdfs:label "Tidy"@en .


###  http://modai.ai/big5#Timely
ns:Timely rdf:type owl:NamedIndividual ;
          rdfs:label "Timely"@en .


###  http://modai.ai/big5#Timidity
ns:Timidity rdf:type owl:NamedIndividual ;
            rdfs:label "Timidity"@en .


###  http://modai.ai/big5#Tiredness
ns:Tiredness rdf:type owl:NamedIndividual ;
             rdfs:label "Tiredness"@en .


###  http://modai.ai/big5#Tolerant
ns:Tolerant rdf:type owl:NamedIndividual ;
            rdfs:label "Tolerant"@en .


###  http://modai.ai/big5#Touching
ns:Touching rdf:type owl:NamedIndividual ,
                     ns:Behavior ;
            ns:associatedWith ns:Expressiveness ;
            ns:triggeredBy ns:Affection ,
                           ns:Curiosity ;
            rdfs:label "Touching"@en .


###  http://modai.ai/big5#Traditional
ns:Traditional rdf:type owl:NamedIndividual ;
               rdfs:label "Traditional"@en .


###  http://modai.ai/big5#Travelling
ns:Travelling rdf:type owl:NamedIndividual ,
                       ns:Behavior ;
              ns:associatedWith ns:Adventurousness ;
              ns:triggeredBy ns:Curiosity ,
                             ns:Restlessness ;
              rdfs:label "Travelling"@en .


###  http://modai.ai/big5#TriedAndTrue
ns:TriedAndTrue rdf:type owl:NamedIndividual ;
                rdfs:label "TriedAndTrue"@en .


###  http://modai.ai/big5#Triumph
ns:Triumph rdf:type owl:NamedIndividual ,
                    ns:Positive_High ;
           ns:relatedTo ns:Victory ;
           ns:similarTo ns:Victory ;
           rdfs:comment "Triumph is typically considered an emotion, as it involves the feeling of joy or satisfaction that comes from succeeding in a difficult pursuit or overcoming a challenge. However, it could also be considered a trait in some contexts, as individuals who frequently experience triumph may be seen as persistent, determined, or resilient. Ultimately, whether triumph is seen as an emotion or a trait may depend on the specific situation and perspective of the observer." ;
           rdfs:label "Triumph"@en .


###  http://modai.ai/big5#Triumph-Defeat
ns:Triumph-Defeat rdf:type owl:NamedIndividual ,
                           ns:Prompt ;
                  ns:uses ns:Defeat ,
                          ns:Triumph ;
                  rdfs:comment """I want to quantify the triumph in the following text:
```
$INPUT_TEXT
```

I define triumph as a great victory or achievement. I define the opposite of triumph as failure or defeat.

Please answer on a scale of 1 - 5 where the numbers have the following meanings:
```
1 = The text is filled with failure, defeat, and has no elements of triumph.
2 = The text has elements of failure or defeat, but also contains some elements of triumph.
3 = The text has neither triumph nor failure, it is neutral.
4 = The text has elements of triumph but also has some aspects of failure or defeat.
5 = The text is deeply filled with triumph, focusing heavily on feelings of victory or achievement.
```

Only respond with a number and no other rating.
"""@en ;
                  rdfs:label "Triumph-Defeat"@en .


###  http://modai.ai/big5#Trust
ns:Trust rdf:type owl:NamedIndividual ,
                  ns:Positive_Low ;
         ns:oppositeTo ns:Doubt .


###  http://modai.ai/big5#Trust-Doubt
ns:Trust-Doubt rdf:type owl:NamedIndividual ,
                        ns:Prompt ;
               ns:uses ns:Doubt ,
                       ns:Trust ;
               rdfs:comment """I want to quantify the trust in the following text:
```
$INPUT_TEXT
```

I define trust as a firm belief in the reliability, truth, or ability of someone or something. I define the opposite of trust as skepticism or doubt.

Please answer on a scale of 1 - 5 where the numbers have the following meanings:
```
1 = The text is filled with skepticism, doubt, and has no elements of trust.
2 = The text has elements of skepticism or doubt, but also contains some elements of trust.
3 = The text has neither trust nor skepticism, it is neutral.
4 = The text has elements of trust but also has some skeptical or doubting aspects.
5 = The text is deeply filled with trust, focusing heavily on belief in reliability, truth, or ability.
```

Only respond with a number and no other rating.
"""@en ;
               rdfs:label "Trust-Doubt"@en .


###  http://modai.ai/big5#Trusting
ns:Trusting rdf:type owl:NamedIndividual ;
            rdfs:label "Trusting"@en .


###  http://modai.ai/big5#Unanalytical
ns:Unanalytical rdf:type owl:NamedIndividual ;
                rdfs:label "Unanalytical"@en .


###  http://modai.ai/big5#Unassertive
ns:Unassertive rdf:type owl:NamedIndividual ;
               rdfs:label "Unassertive"@en .


###  http://modai.ai/big5#Unbiased
ns:Unbiased rdf:type owl:NamedIndividual ;
            rdfs:label "Unbiased"@en .


###  http://modai.ai/big5#Uncaring
ns:Uncaring rdf:type owl:NamedIndividual ;
            rdfs:label "Uncaring"@en .


###  http://modai.ai/big5#Uncertain
ns:Uncertain rdf:type owl:NamedIndividual ;
             rdfs:label "Uncertain"@en .


###  http://modai.ai/big5#Uncertainty
ns:Uncertainty rdf:type owl:NamedIndividual ;
               ns:relatedTo ns:Doubt ;
               ns:similarTo ns:Doubt ;
               rdfs:comment "Uncertainty is not an emotion or a trait in the traditional sense. It is a state of mind or a feeling of not knowing what will happen or what to expect. However, it can be a factor that influences emotions and traits. For example, someone who experiences a lot of uncertainty in their life may develop the trait of being more cautious or anxious as a result. Uncertainty can also lead to emotions such as fear, anxiety, or excitement depending on the situation. Overall, uncertainty is a complex concept that can manifest itself in various ways and can impact a person's emotional and behavioral responses." ;
               rdfs:label "Uncertainty"@en .


###  http://modai.ai/big5#Uncompassionate
ns:Uncompassionate rdf:type owl:NamedIndividual ,
                            ns:Trait ;
                   ns:hasEmotionStrong ns:Compassionate ;
                   rdfs:comment "Uncompassionate is more commonly considered a trait rather than an emotion. It refers to a lack of empathy or concern for others, which is a characteristic or habitual way of behaving. An emotion, on the other hand, is a temporary feeling or state of mind that is usually in response to a specific situation or event. While uncompassionate behavior could be driven by emotions like anger or frustration, the behavior itself is reflective of a deep-seated trait." ;
                   rdfs:label "Uncompassionate"@en .


###  http://modai.ai/big5#Unconscious
ns:Unconscious rdf:type owl:NamedIndividual ;
               rdfs:label "Unconscious"@en .


###  http://modai.ai/big5#Unconventional
ns:Unconventional rdf:type owl:NamedIndividual ;
                  rdfs:label "Unconventional"@en .


###  http://modai.ai/big5#Uncreative
ns:Uncreative rdf:type owl:NamedIndividual ;
              rdfs:label "Uncreative"@en .


###  http://modai.ai/big5#Understanding
ns:Understanding rdf:type owl:NamedIndividual ,
                          ns:Trait ;
                 ns:relatedTo ns:Certainty ;
                 ns:similarTo ns:Certainty ;
                 rdfs:comment "Understanding can be considered both an emotion and a trait, depending on the context in which it is being used. As an emotion, understanding can be described as the mental and emotional process of comprehending or empathizing with another person's perspective or situation. In this sense, understanding is closely related to empathy and compassion. When we say \"I understand how you feel,\" we are acknowledging and empathizing with the other person's emotions. As a trait, understanding can refer to a person's general disposition or ability to comprehend and appreciate complex ideas or situations. Someone who is considered understanding may be open-minded, patient, and willing to listen to others. They may be skilled at analyzing information, interpreting social cues, and resolving conflicts. In summary, understanding can be an emotion when referring to the process of empathizing with others, and a trait when referring to someone's general disposition or ability to comprehend complex ideas." ;
                 rdfs:label "Understanding"@en .


###  http://modai.ai/big5#Unease
ns:Unease rdf:type owl:NamedIndividual ;
          ns:relatedTo ns:Anxiety ;
          ns:similarTo ns:Anxiety ;
          rdfs:comment "Unease can be considered both an emotion and a trait, depending on how it is used or experienced. As an emotion, unease refers to a feeling of discomfort, worry, or anxiety that arises in response to a specific situation or stimulus. For example, a person might feel unease before a job interview or when walking in a dark alley at night. As a trait, unease refers to a disposition or tendency towards feeling anxious, uneasy, or uncertain. This implies that a person is more likely to experience unease even in ordinary situations. For instance, a person with a neurotic personality may have a pervasive sense of unease and worry throughout their day. In summary, unease can be considered both an emotion and a trait, depending on the context in which it is used." ;
          rdfs:label "Unease"@en .


###  http://modai.ai/big5#Unemotional
ns:Unemotional rdf:type owl:NamedIndividual ;
               rdfs:label "Unemotional"@en .


###  http://modai.ai/big5#Unempathetic
ns:Unempathetic rdf:type owl:NamedIndividual ;
                rdfs:label "Unempathetic"@en .


###  http://modai.ai/big5#Unenthusiastic
ns:Unenthusiastic rdf:type owl:NamedIndividual ;
                  rdfs:label "Unenthusiastic"@en .


###  http://modai.ai/big5#Unhappiness
ns:Unhappiness rdf:type owl:NamedIndividual ;
               rdfs:label "Unhappiness"@en .


###  http://modai.ai/big5#Unhelpful
ns:Unhelpful rdf:type owl:NamedIndividual ;
             rdfs:label "Unhelpful"@en .


###  http://modai.ai/big5#Unimaginative
ns:Unimaginative rdf:type owl:NamedIndividual ;
                 rdfs:label "Unimaginative"@en .


###  http://modai.ai/big5#Unique
ns:Unique rdf:type owl:NamedIndividual ;
          rdfs:label "Unique"@en .


###  http://modai.ai/big5#Unmotivated
ns:Unmotivated rdf:type owl:NamedIndividual ,
                        ns:Trait ;
               ns:hasEmotionStrong ns:Unmotivated ;
               rdfs:comment "Unmotivated is generally considered a trait rather than an emotion. Traits are characteristic features or qualities of a person that are relatively stable over time, whereas emotions are transient and often vary based on situational factors. Unmotivated individuals are characterized by a lack of drive, energy, and enthusiasm towards achieving goals or pursuing activities. This lack of motivation can affect their behavior and performance in various areas of their life, such as work, relationships, and personal growth. While lack of motivation may be influenced by emotions such as apathy or boredom, it is primarily considered a trait that reflects a person's underlying personality and psychological makeup." ;
               rdfs:label "Unmotivated"@en .


###  http://modai.ai/big5#Unpersuasive
ns:Unpersuasive rdf:type owl:NamedIndividual ;
                rdfs:label "Unpersuasive"@en .


###  http://modai.ai/big5#Unpredictable
ns:Unpredictable rdf:type owl:NamedIndividual ;
                 rdfs:label "Unpredictable"@en .


###  http://modai.ai/big5#Unreflective
ns:Unreflective rdf:type owl:NamedIndividual ;
                rdfs:label "Unreflective"@en .


###  http://modai.ai/big5#Unreliable
ns:Unreliable rdf:type owl:NamedIndividual ;
              ns:oppositeTo ns:Reliable ;
              ns:similarTo ns:Inconsistent ;
              rdfs:label "Unreliable"@en .


###  http://modai.ai/big5#Unrest
ns:Unrest rdf:type owl:NamedIndividual ,
                   ns:Emotion ;
          rdfs:comment "Unrest can be considered both an emotion and a trait, depending on how it is defined and used. As an emotion, unrest refers to a state of agitation, anxiety, or unease caused by external or internal factors. It is a temporary and situational experience that can be triggered by various factors such as uncertainty, insecurity, fear, or dissatisfaction with one's situation. As a trait, unrest can refer to a dispositional tendency or personality characteristic that makes a person prone to experiencing restlessness, dissatisfaction, or a desire for change or novelty. It is a stable and enduring aspect of a person's personality that can influence his or her thoughts, behaviors, and emotions in various situations. Thus, the concept of unrest can be considered an emotion when it refers to a temporary internal state, and a trait when it refers to a stable dispositional tendency." ;
          rdfs:label "Unrest"@en .


###  http://modai.ai/big5#Unselfish
ns:Unselfish rdf:type owl:NamedIndividual ;
             rdfs:label "Unselfish"@en .


###  http://modai.ai/big5#Unstructured
ns:Unstructured rdf:type owl:NamedIndividual ;
                rdfs:label "Unstructured"@en .


###  http://modai.ai/big5#Unthankful
ns:Unthankful rdf:type owl:NamedIndividual ;
              ns:oppositeTo ns:Ingratitude ;
              ns:relatedTo ns:Disregard ;
              ns:similarTo ns:Disregard ;
              rdfs:comment "Unthankful can be considered both an emotion and a trait, depending on how it is manifested and understood. As an emotion, unthankful refers to a feeling of ingratitude or lack of appreciation for the good things in one's life. It is a temporary state of mind that can be triggered by various factors, such as disappointment, envy, or entitlement. In this sense, unthankful is similar to other negative emotions like anger, sadness, or anxiety. As a trait, unthankful refers to a persistent pattern of behavior that reflects a chronic lack of gratitude and appreciation. It is a stable characteristic of an individual's personality that influences how they perceive and respond to various situations in their life. In this sense, unthankful is similar to other personality traits like selfishness, arrogance, or entitlement. Overall, whether unthankful is considered an emotion or a trait depends on whether it is understood as a temporary mood or a persistent pattern of behavior." ;
              rdfs:label "Unthankful"@en .


###  http://modai.ai/big5#Unworried
ns:Unworried rdf:type owl:NamedIndividual ;
             rdfs:label "Unworried"@en .


###  http://modai.ai/big5#Victory
ns:Victory rdf:type owl:NamedIndividual ,
                    ns:Trait ;
           ns:oppositeTo ns:Defeat ;
           rdfs:comment "Victory can be considered both an emotion and a trait, depending on the context in which it is being used. As an emotion, victory is the feeling of joy, satisfaction, or triumph that is experienced when one succeeds in achieving their goals or overcomes a challenge. Victory can elicit strong positive emotions, such as happiness, elation, relief, or pride, that can influence behavior, outlook, and motivation. As a trait, victory can be seen as a characteristic or quality of a person who tends to be successful, competitive, or determined in pursuing their goals. This trait may involve having a positive mindset, a strong work ethic, perseverance, and resilience in the face of obstacles or setbacks. Overall, victory can be seen both as a feeling that results from achieving something desired and as a trait or quality that contributes to success and accomplishment." ;
           rdfs:label "Victory"@en .


###  http://modai.ai/big5#Warm
ns:Warm rdf:type owl:NamedIndividual ;
        rdfs:label "Warm"@en .


###  http://modai.ai/big5#Whistling
ns:Whistling rdf:type owl:NamedIndividual ,
                      ns:Behavior ;
             ns:associatedWith ns:Carefreeness ;
             ns:triggeredBy ns:Boredom ,
                            ns:Happiness ;
             rdfs:label "Whistling"@en .


###  http://modai.ai/big5#Winking
ns:Winking rdf:type owl:NamedIndividual ,
                    ns:Behavior ;
           ns:associatedWith ns:Cheekiness ;
           ns:triggeredBy ns:Flirtation ,
                          ns:Playfulness ;
           rdfs:label "Winking"@en .


###  http://modai.ai/big5#Wonder
ns:Wonder rdf:type owl:NamedIndividual ;
          ns:relatedTo ns:Awe ;
          ns:similarTo ns:Awe ;
          rdfs:comment "Wonder is generally considered as an emotion, as it refers to a feeling of amazement or admiration caused by something beautiful, remarkable, or unfamiliar. It is often associated with curiosity and a desire to learn more about the object of wonder. However, wonder can also be considered a trait, as some individuals may be more prone to experiencing wonder or being awed by the world around them. These individuals may have a natural curiosity and openness to new experiences, which allows them to appreciate and marvel at the things they encounter. In this sense, wonder can be seen as a personality characteristic or disposition." ;
          rdfs:label "Wonder"@en .


###  http://modai.ai/big5#Worried
ns:Worried rdf:type owl:NamedIndividual ;
           ns:relatedTo ns:Anxiety ;
           ns:similarTo ns:Anxiety ;
           rdfs:comment "Worried is an emotion. Emotions are usually temporary responses to a situation or stimulus. Worried is a feeling of anxiety, unease, or concern about a possible outcome or situation. It is a normal human response to situations that require attention or action. Traits, on the other hand, are enduring personality characteristics that are stable over time and consistent across situations. Traits are more permanent aspects of an individual's personality and are less likely to change over time. Worried cannot be considered a trait because it is not a stable personality characteristic. People may experience worry in certain situations, but it does not necessarily define their personality or behavior in all situations." ;
           rdfs:label "Worried"@en .


###  http://modai.ai/big5#Worry
ns:Worry rdf:type owl:NamedIndividual ;
         ns:relatedTo ns:Fear ;
         ns:similarTo ns:Fear ;
         rdfs:comment "Worry can be considered both an emotion and a trait, depending on how it is defined and conceptualized. As an emotion, worry refers to a specific mental state characterized by feelings of unease, anxiety, and apprehension. It typically arises in response to a perceived threat or danger and can be accompanied by physical symptoms such as sweating, rapid heartbeat, and muscle tension. Worry as an emotion is considered a normal and adaptive response to stress and can motivate individuals to take action to alleviate their concerns. On the other hand, as a trait, worry refers to a more stable and enduring tendency to experience feelings of anxiety and apprehension across a range of situations. It implies a general disposition towards worry and rumination, not just as a response to specific events. Worry as a trait is often associated with anxiety disorders and can be considered a form of neuroticism, a personality trait characterized by emotional instability and heightened sensitivity to stressors. Overall, while worry can be experienced as an emotion in response to a specific situation, it can also be considered a trait if it represents a persistent and generalized pattern of anxiety and apprehension across different contexts." ;
         rdfs:label "Worry"@en .


###  http://modai.ai/big5#Writing
ns:Writing rdf:type owl:NamedIndividual ,
                    ns:Behavior ;
           ns:associatedWith ns:Creativity ;
           ns:triggeredBy ns:Inspiration ,
                          ns:Necessity ;
           rdfs:label "Writing"@en .


###  http://modai.ai/big5#Yawning
ns:Yawning rdf:type owl:NamedIndividual ,
                    ns:Behavior ;
           ns:associatedWith ns:Involuntary ;
           ns:triggeredBy ns:Boredom ,
                          ns:Tiredness ;
           rdfs:label "Yawning"@en .


#################################################################
#    Annotations
#################################################################

ns:Anxiety rdfs:comment "Anxiety can be both an emotion and a trait. Anxiety as an emotion is a natural response to stress or uncertainty, and it involves feelings of fear, apprehension, or unease. It is a normal and healthy response to certain situations, such as when we are in danger or facing a new and challenging task. On the other hand, anxiety as a trait is a more stable and enduring characteristic of an individual's personality. People who have high anxiety as a trait tend to experience anxiety more frequently and intensely than those with low anxiety as a trait. This can cause them to be overly worried or vigilant even in non-threatening situations. Both the emotion of anxiety and the trait of anxiety can have an impact on an individual's life and well-being. While occasional feelings of anxiety are common and even helpful in some situations, excessive anxiety can interfere with daily activities and lead to mental health problems such as anxiety disorders." ;
           rdfs:label "Anxiety"@en ;
           rdfs:seeAlso "Anxious" .


ns:Assertiveness rdfs:comment "Assertiveness within the Big Five personality framework refers to the degree to which an individual is able to communicate their thoughts, needs, and desires confidently and clearly. It signifies a person's comfort in expressing their own opinions and standing up for themselves while maintaining respect for the views and rights of others. Individuals high in Assertiveness are typically proactive in voicing their ideas and are capable of leadership roles, as they can guide discussions and decisions without hesitation. This trait is crucial for effective interpersonal communication and is often associated with leadership qualities, as it enables individuals to navigate social and professional situations effectively, ensuring their voice is heard and their goals are pursued assertively."@en ;
                 rdfs:label "Assertiveness"@en ;
                 rdfs:seeAlso "Assertive" .


ns:Confusion rdfs:comment "Confusion can be considered both an emotion and a temporary trait. As an emotion, confusion is a feeling of being uncertain, unable to understand or make sense of something. It can be triggered by a variety of things such as a lack of information or conflicting thoughts. Confusion usually passes once the source of confusion is resolved. As a temporary trait, confusion can also be seen as a characteristic of a person's thinking style or cognitive ability. Some people may experience confusion more often than others or may find it more difficult to comprehend complex information. However, this is not a permanent or inherent trait and can be improved with practice and learning. Overall, confusion may be considered an emotion in the moment that a person experiences it and a temporary trait when considering a person's cognitive abilities." ;
             rdfs:label "Confusion" .


ns:Depression rdfs:comment "Depression is typically considered to be more of a mood disorder or a clinical condition rather than an emotion or a trait. Emotions are usually more short-lived and can shift and change quickly based on different stimuli, whereas depression is a persistent feeling of sadness, hopelessness, and a lack of interest in enjoyable activities that can last for weeks, months, or even years. Traits, on the other hand, refer to enduring personality characteristics that are relatively stable over time. While people who experience depression may have certain traits, such as low self-esteem or negative thinking patterns, depression itself is typically not considered a trait. However, it is important to note that depression can manifest differently for different individuals and can be influenced by various factors, including genetics, environment, and personal experiences." ;
              rdfs:label "Depression"@en ;
              rdfs:seeAlso "Depressed" .


ns:Prompt rdfs:label "Prompt"@en .


ns:Respectfulness rdfs:comment "Respectfulness as a personality trait signifies an individual's consistent demonstration of esteem and consideration towards others, regardless of their status or position. It encompasses acknowledging the dignity, feelings, and rights of people in one's interactions and communications. Individuals high in Respectfulness exhibit polite behavior, listen attentively, and show an understanding of social norms and cultural differences, fostering positive and harmonious relationships. This trait is pivotal in building trust, promoting effective communication, and maintaining healthy interpersonal dynamics, as it reflects a deep-seated recognition of the value and worth of others."@en ;
                  rdfs:label "Respectfulness"@en ;
                  rdfs:seeAlso "Respect" .


ns:Social rdfs:label "Social"@en .


ns:Trust rdfs:comment "Trust can be considered both an emotion and a trait. As an emotion, trust is a feeling of confidence or reliance in another person or thing. When we trust someone, we feel comfortable and secure in their presence, and we believe that they will act in a way that is consistent with our expectations. As a trait, trustworthiness is a characteristic that enables people to gain the trust of others. Trustworthiness involves being honest, reliable, and responsible, and consistently behaving in a way that inspires confidence in others. Individuals who possess this trait are more likely to build strong relationships and develop a positive reputation in their personal and professional lives. In summary, trust can be considered both an emotion and a trait, with trustworthiness being the trait that enables people to earn trust from others." ;
         rdfs:label "Trust"@en ;
         rdfs:seeAlso "Trust" .


###  Generated by the OWL API (version 4.5.25.2023-02-15T19:15:49Z) https://github.com/owlcs/owlapi
